<?xml version="1.0"?>


<!DOCTYPE rdf:RDF [
    <!ENTITY owl "http://www.w3.org/2002/07/owl#" >
    <!ENTITY xsd "http://www.w3.org/2001/XMLSchema#" >
    <!ENTITY xml "http://www.w3.org/XML/1998/namespace" >
    <!ENTITY rdfs "http://www.w3.org/2000/01/rdf-schema#" >
    <!ENTITY Governance "http://www.semanticweb.org/IG/Governance#" >
    <!ENTITY rdf "http://www.w3.org/1999/02/22-rdf-syntax-ns#" >
]>


<rdf:RDF xmlns="http://www.semanticweb.org/IG/Governance/"
     xml:base="http://www.semanticweb.org/IG/Governance/"
     xmlns:rdfs="http://www.w3.org/2000/01/rdf-schema#"
     xmlns:owl="http://www.w3.org/2002/07/owl#"
     xmlns:xsd="http://www.w3.org/2001/XMLSchema#"
     xmlns:rdf="http://www.w3.org/1999/02/22-rdf-syntax-ns#"
     xmlns:xml="http://www.w3.org/XML/1998/namespace"
     xmlns:Governance="http://www.semanticweb.org/IG/Governance#">
    


    <!-- 
    ///////////////////////////////////////////////////////////////////////////////////////
    //
    // Object Properties
    //
    ///////////////////////////////////////////////////////////////////////////////////////
     -->

    


    <!-- http://www.semanticweb.org/IG/Governance#accountableForStrageticPlan -->

    <owl:ObjectProperty rdf:about="&Governance;accountableForStrageticPlan">
        <rdfs:domain rdf:resource="&Governance;Executive_Sponsor"/>
        <rdfs:range rdf:resource="&Governance;IG_Strategic_Plan"/>
        <rdfs:subPropertyOf rdf:resource="&owl;topObjectProperty"/>
    </owl:ObjectProperty>
    


    <!-- http://www.semanticweb.org/IG/Governance#articleInvolvedIn -->

    <owl:ObjectProperty rdf:about="&Governance;articleInvolvedIn">
        <rdfs:range rdf:resource="&Governance;Capability"/>
        <rdfs:range rdf:resource="&Governance;Data_Retention_Policy"/>
        <rdfs:domain rdf:resource="&Governance;GDPR"/>
        <owl:inverseOf rdf:resource="&Governance;involvesArticle"/>
        <rdfs:subPropertyOf rdf:resource="&owl;topObjectProperty"/>
    </owl:ObjectProperty>
    


    <!-- http://www.semanticweb.org/IG/Governance#canBeInvolvedWith -->

    <owl:ObjectProperty rdf:about="&Governance;canBeInvolvedWith"/>
    


    <!-- http://www.semanticweb.org/IG/Governance#clearsObstaclesFor -->

    <owl:ObjectProperty rdf:about="&Governance;clearsObstaclesFor">
        <rdfs:domain rdf:resource="&Governance;Executive_Sponsor"/>
        <rdfs:range rdf:resource="&Governance;IG_Chief_Officer"/>
        <rdfs:range rdf:resource="&Governance;Steering_Commitee"/>
        <rdfs:subPropertyOf rdf:resource="&owl;topObjectProperty"/>
    </owl:ObjectProperty>
    


    <!-- http://www.semanticweb.org/IG/Governance#collaboratesInLTDP -->

    <owl:ObjectProperty rdf:about="&Governance;collaboratesInLTDP">
        <rdfs:range rdf:resource="&Governance;Long_Term_Digital_Preservation"/>
        <rdfs:domain rdf:resource="&Governance;Stakeholder"/>
        <rdfs:subPropertyOf rdf:resource="&owl;topObjectProperty"/>
    </owl:ObjectProperty>
    


    <!-- http://www.semanticweb.org/IG/Governance#collaboratesWithOrganization -->

    <owl:ObjectProperty rdf:about="&Governance;collaboratesWithOrganization">
        <rdfs:range rdf:resource="&Governance;Organization"/>
        <rdfs:domain rdf:resource="&Governance;Steering_Commitee"/>
        <rdfs:subPropertyOf rdf:resource="&owl;topObjectProperty"/>
    </owl:ObjectProperty>
    


    <!-- http://www.semanticweb.org/IG/Governance#consultaionNeededForMetrics -->

    <owl:ObjectProperty rdf:about="&Governance;consultaionNeededForMetrics">
        <rdfs:range rdf:resource="&Governance;Metrics"/>
        <rdfs:domain rdf:resource="&Governance;Stakeholder"/>
        <rdfs:subPropertyOf rdf:resource="&owl;topObjectProperty"/>
    </owl:ObjectProperty>
    


    <!-- http://www.semanticweb.org/IG/Governance#contactPersonForSupervisor -->

    <owl:ObjectProperty rdf:about="&Governance;contactPersonForSupervisor">
        <rdfs:domain rdf:resource="&Governance;DPO"/>
        <rdfs:range rdf:resource="&Governance;Supervisor_Authority"/>
        <rdfs:subPropertyOf rdf:resource="&owl;topObjectProperty"/>
    </owl:ObjectProperty>
    


    <!-- http://www.semanticweb.org/IG/Governance#createsRiskPlan -->

    <owl:ObjectProperty rdf:about="&Governance;createsRiskPlan">
        <rdfs:range rdf:resource="&Governance;Information_Asset_Risk_Mitigation_Plan"/>
        <rdfs:domain rdf:resource="&Governance;Steering_Commitee"/>
        <rdfs:subPropertyOf rdf:resource="&owl;topObjectProperty"/>
    </owl:ObjectProperty>
    


    <!-- http://www.semanticweb.org/IG/Governance#defines -->

    <owl:ObjectProperty rdf:about="&Governance;defines">
        <owl:inverseOf rdf:resource="&Governance;isDefinedBy"/>
        <rdfs:subPropertyOf rdf:resource="&owl;topObjectProperty"/>
    </owl:ObjectProperty>
    


    <!-- http://www.semanticweb.org/IG/Governance#definesPracticesFor -->

    <owl:ObjectProperty rdf:about="&Governance;definesPracticesFor">
        <rdfs:range rdf:resource="&Governance;Capability"/>
        <rdfs:range rdf:resource="&Governance;Data_Retention_Policy"/>
        <rdfs:domain rdf:resource="&Governance;ISO"/>
        <owl:inverseOf rdf:resource="&Governance;practicesDefinedInIso"/>
        <rdfs:subPropertyOf rdf:resource="&owl;topObjectProperty"/>
    </owl:ObjectProperty>
    


    <!-- http://www.semanticweb.org/IG/Governance#drivenByExcutiveSponsor -->

    <owl:ObjectProperty rdf:about="&Governance;drivenByExcutiveSponsor">
        <rdfs:range rdf:resource="&Governance;Executive_Sponsor"/>
        <rdfs:domain rdf:resource="&Governance;IG_Policy"/>
        <rdfs:subPropertyOf rdf:resource="&owl;topObjectProperty"/>
    </owl:ObjectProperty>
    


    <!-- http://www.semanticweb.org/IG/Governance#ensures -->

    <owl:ObjectProperty rdf:about="&Governance;ensures">
        <rdfs:range rdf:resource="&Governance;Goal"/>
        <rdfs:domain rdf:resource="&Governance;Organization"/>
        <rdfs:subPropertyOf rdf:resource="&owl;topObjectProperty"/>
    </owl:ObjectProperty>
    


    <!-- http://www.semanticweb.org/IG/Governance#ensuresGDPRComplianceForDataController -->

    <owl:ObjectProperty rdf:about="&Governance;ensuresGDPRComplianceForDataController">
        <rdfs:range rdf:resource="&Governance;Data"/>
        <rdfs:domain rdf:resource="&Governance;Data_Controller"/>
        <rdfs:subPropertyOf rdf:resource="&owl;topObjectProperty"/>
    </owl:ObjectProperty>
    


    <!-- http://www.semanticweb.org/IG/Governance#givesInputToLHNRequirements -->

    <owl:ObjectProperty rdf:about="&Governance;givesInputToLHNRequirements">
        <rdfs:range rdf:resource="&Governance;LHN_Requirements"/>
        <rdfs:domain rdf:resource="&Governance;Stakeholder"/>
        <rdfs:subPropertyOf rdf:resource="&owl;topObjectProperty"/>
    </owl:ObjectProperty>
    


    <!-- http://www.semanticweb.org/IG/Governance#givesInstructionsToDataProcessor -->

    <owl:ObjectProperty rdf:about="&Governance;givesInstructionsToDataProcessor">
        <rdfs:domain rdf:resource="&Governance;Data_Controller"/>
        <rdfs:range rdf:resource="&Governance;Data_Processor"/>
        <rdfs:subPropertyOf rdf:resource="&owl;topObjectProperty"/>
    </owl:ObjectProperty>
    


    <!-- http://www.semanticweb.org/IG/Governance#hasData -->

    <owl:ObjectProperty rdf:about="&Governance;hasData">
        <rdfs:range rdf:resource="&Governance;Data"/>
        <rdfs:domain rdf:resource="&Governance;Data_Subject"/>
        <rdfs:subPropertyOf rdf:resource="&owl;topObjectProperty"/>
    </owl:ObjectProperty>
    


    <!-- http://www.semanticweb.org/IG/Governance#hasGoal -->

    <owl:ObjectProperty rdf:about="&Governance;hasGoal">
        <rdfs:subPropertyOf rdf:resource="&owl;topObjectProperty"/>
    </owl:ObjectProperty>
    


    <!-- http://www.semanticweb.org/IG/Governance#hasInputOnRiskProfile -->

    <owl:ObjectProperty rdf:about="&Governance;hasInputOnRiskProfile">
        <rdfs:range rdf:resource="&Governance;Risk_Profile"/>
        <rdfs:domain rdf:resource="&Governance;Stakeholder"/>
        <rdfs:subPropertyOf rdf:resource="&owl;topObjectProperty"/>
    </owl:ObjectProperty>
    


    <!-- http://www.semanticweb.org/IG/Governance#hasLHNRequirements -->

    <owl:ObjectProperty rdf:about="&Governance;hasLHNRequirements">
        <rdfs:range rdf:resource="&Governance;LHN_Requirements"/>
        <rdfs:domain rdf:resource="&Governance;Legal_Hold_Notification"/>
        <rdfs:subPropertyOf rdf:resource="&owl;topObjectProperty"/>
    </owl:ObjectProperty>
    


    <!-- http://www.semanticweb.org/IG/Governance#hasTechnicalNeedsDesription -->

    <owl:ObjectProperty rdf:about="&Governance;hasTechnicalNeedsDesription">
        <rdfs:subPropertyOf rdf:resource="&owl;topObjectProperty"/>
    </owl:ObjectProperty>
    


    <!-- http://www.semanticweb.org/IG/Governance#inMaturityLevel -->

    <owl:ObjectProperty rdf:about="&Governance;inMaturityLevel">
        <rdfs:domain rdf:resource="&Governance;Capability"/>
        <rdfs:range rdf:resource="&Governance;Maturity"/>
        <owl:inverseOf rdf:resource="&Governance;maturityLevelDefinedFor"/>
        <rdfs:subPropertyOf rdf:resource="&owl;topObjectProperty"/>
    </owl:ObjectProperty>
    


    <!-- http://www.semanticweb.org/IG/Governance#involvedInRiskAndCompliance -->

    <owl:ObjectProperty rdf:about="&Governance;involvedInRiskAndCompliance">
        <rdfs:domain rdf:resource="&Governance;CCO"/>
        <rdfs:range rdf:resource="&Governance;Risk_And_Compliance"/>
        <rdfs:subPropertyOf rdf:resource="&owl;topObjectProperty"/>
    </owl:ObjectProperty>
    


    <!-- http://www.semanticweb.org/IG/Governance#involvesArticle -->

    <owl:ObjectProperty rdf:about="&Governance;involvesArticle">
        <rdfs:domain rdf:resource="&Governance;Capability"/>
        <rdfs:domain rdf:resource="&Governance;Data_Retention_Policy"/>
        <rdfs:range rdf:resource="&Governance;GDPR"/>
        <rdfs:subPropertyOf rdf:resource="&owl;topObjectProperty"/>
    </owl:ObjectProperty>
    


    <!-- http://www.semanticweb.org/IG/Governance#isDefinedBy -->

    <owl:ObjectProperty rdf:about="&Governance;isDefinedBy">
        <rdfs:subPropertyOf rdf:resource="&owl;topObjectProperty"/>
    </owl:ObjectProperty>
    


    <!-- http://www.semanticweb.org/IG/Governance#leadsRIM -->

    <owl:ObjectProperty rdf:about="&Governance;leadsRIM">
        <rdfs:range rdf:resource="&Governance;Records_And_Information_Management"/>
        <rdfs:domain rdf:resource="&Governance;Senior_Records_Officer"/>
        <rdfs:subPropertyOf rdf:resource="&owl;topObjectProperty"/>
    </owl:ObjectProperty>
    


    <!-- http://www.semanticweb.org/IG/Governance#leadsSecurity -->

    <owl:ObjectProperty rdf:about="&Governance;leadsSecurity">
        <rdfs:domain rdf:resource="&Governance;CSO"/>
        <rdfs:range rdf:resource="&Governance;Security"/>
        <rdfs:subPropertyOf rdf:resource="&owl;topObjectProperty"/>
    </owl:ObjectProperty>
    


    <!-- http://www.semanticweb.org/IG/Governance#linkedToBusinessUnit -->

    <owl:ObjectProperty rdf:about="&Governance;linkedToBusinessUnit"/>
    


    <!-- http://www.semanticweb.org/IG/Governance#linkedToFramework -->

    <owl:ObjectProperty rdf:about="&Governance;linkedToFramework"/>
    


    <!-- http://www.semanticweb.org/IG/Governance#linkedToProcess -->

    <owl:ObjectProperty rdf:about="&Governance;linkedToProcess"/>
    


    <!-- http://www.semanticweb.org/IG/Governance#managesIGProgramm -->

    <owl:ObjectProperty rdf:about="&Governance;managesIGProgramm">
        <rdfs:domain rdf:resource="&Governance;IG_Chief_Officer"/>
        <rdfs:range rdf:resource="&Governance;IG_Programm"/>
        <rdfs:subPropertyOf rdf:resource="&owl;topObjectProperty"/>
    </owl:ObjectProperty>
    


    <!-- http://www.semanticweb.org/IG/Governance#maturityLevelDefinedFor -->

    <owl:ObjectProperty rdf:about="&Governance;maturityLevelDefinedFor">
        <rdfs:range rdf:resource="&Governance;Capability"/>
        <rdfs:domain rdf:resource="&Governance;Maturity"/>
        <rdfs:subPropertyOf rdf:resource="&owl;topObjectProperty"/>
    </owl:ObjectProperty>
    


    <!-- http://www.semanticweb.org/IG/Governance#memberOfOrganization -->

    <owl:ObjectProperty rdf:about="&Governance;memberOfOrganization">
        <rdfs:range rdf:resource="&Governance;Organization"/>
        <rdfs:domain rdf:resource="&Governance;Role"/>
        <rdfs:subPropertyOf rdf:resource="&owl;topObjectProperty"/>
    </owl:ObjectProperty>
    


    <!-- http://www.semanticweb.org/IG/Governance#needsTechnicalRequirement -->

    <owl:ObjectProperty rdf:about="&Governance;needsTechnicalRequirement">
        <rdfs:domain rdf:resource="&Governance;Capability"/>
        <rdfs:range rdf:resource="&Governance;Data_Retention_Policy"/>
        <rdfs:range rdf:resource="&Governance;Electronic_Records_Management"/>
        <owl:inverseOf rdf:resource="&Governance;technicalRequirementFor"/>
        <rdfs:subPropertyOf rdf:resource="&owl;topObjectProperty"/>
    </owl:ObjectProperty>
    


    <!-- http://www.semanticweb.org/IG/Governance#organizesTeam -->

    <owl:ObjectProperty rdf:about="&Governance;organizesTeam">
        <rdfs:domain rdf:resource="&Governance;Executive_Sponsor"/>
        <rdfs:range rdf:resource="&Governance;IG_Team"/>
        <rdfs:subPropertyOf rdf:resource="&owl;topObjectProperty"/>
    </owl:ObjectProperty>
    


    <!-- http://www.semanticweb.org/IG/Governance#participateInIGProgramm -->

    <owl:ObjectProperty rdf:about="&Governance;participateInIGProgramm">
        <rdfs:range rdf:resource="&Governance;IG_Programm"/>
        <rdfs:domain rdf:resource="&Governance;Stakeholder"/>
        <rdfs:subPropertyOf rdf:resource="&owl;topObjectProperty"/>
    </owl:ObjectProperty>
    


    <!-- http://www.semanticweb.org/IG/Governance#paysPeriodicAttentionToIGProgramm -->

    <owl:ObjectProperty rdf:about="&Governance;paysPeriodicAttentionToIGProgramm">
        <rdfs:domain rdf:resource="&Governance;Executive_Sponsor"/>
        <rdfs:range rdf:resource="&Governance;IG_Programm"/>
        <rdfs:subPropertyOf rdf:resource="&owl;topObjectProperty"/>
    </owl:ObjectProperty>
    


    <!-- http://www.semanticweb.org/IG/Governance#practicesDefinedInIso -->

    <owl:ObjectProperty rdf:about="&Governance;practicesDefinedInIso">
        <rdfs:domain rdf:resource="&Governance;Capability"/>
        <rdfs:domain rdf:resource="&Governance;Data_Retention_Policy"/>
        <rdfs:range rdf:resource="&Governance;ISO"/>
        <rdfs:subPropertyOf rdf:resource="&owl;topObjectProperty"/>
    </owl:ObjectProperty>
    


    <!-- http://www.semanticweb.org/IG/Governance#responsibleFor -->

    <owl:ObjectProperty rdf:about="&Governance;responsibleFor"/>
    


    <!-- http://www.semanticweb.org/IG/Governance#responsibleForCapability -->

    <owl:ObjectProperty rdf:about="&Governance;responsibleForCapability">
        <rdfs:range rdf:resource="&Governance;Capability"/>
        <rdfs:domain rdf:resource="&Governance;Role"/>
        <rdfs:subPropertyOf rdf:resource="&owl;topObjectProperty"/>
    </owl:ObjectProperty>
    


    <!-- http://www.semanticweb.org/IG/Governance#sellsChangesToStakeholder -->

    <owl:ObjectProperty rdf:about="&Governance;sellsChangesToStakeholder">
        <rdfs:domain rdf:resource="&Governance;Change_Management"/>
        <rdfs:range rdf:resource="&Governance;Stakeholder"/>
        <rdfs:subPropertyOf rdf:resource="&owl;topObjectProperty"/>
    </owl:ObjectProperty>
    


    <!-- http://www.semanticweb.org/IG/Governance#setsRulesForDataController -->

    <owl:ObjectProperty rdf:about="&Governance;setsRulesForDataController">
        <rdfs:range rdf:resource="&Governance;Data_Controller"/>
        <rdfs:domain rdf:resource="&Governance;GDPR"/>
        <rdfs:subPropertyOf rdf:resource="&owl;topObjectProperty"/>
    </owl:ObjectProperty>
    


    <!-- http://www.semanticweb.org/IG/Governance#technicalRequirementFor -->

    <owl:ObjectProperty rdf:about="&Governance;technicalRequirementFor">
        <rdfs:subPropertyOf rdf:resource="&owl;topObjectProperty"/>
    </owl:ObjectProperty>
    


    <!-- http://www.semanticweb.org/IG/Governance#uses -->

    <owl:ObjectProperty rdf:about="&Governance;uses">
        <rdfs:subPropertyOf rdf:resource="&owl;topObjectProperty"/>
    </owl:ObjectProperty>
    


    <!-- 
    ///////////////////////////////////////////////////////////////////////////////////////
    //
    // Data properties
    //
    ///////////////////////////////////////////////////////////////////////////////////////
     -->

    


    <!-- http://www.semanticweb.org/IG/Governance#capabilityDescription -->

    <owl:DatatypeProperty rdf:about="&Governance;capabilityDescription">
        <rdfs:subPropertyOf rdf:resource="&owl;topDataProperty"/>
    </owl:DatatypeProperty>
    


    <!-- http://www.semanticweb.org/IG/Governance#processDescription -->

    <owl:DatatypeProperty rdf:about="&Governance;processDescription"/>
    


    <!-- 
    ///////////////////////////////////////////////////////////////////////////////////////
    //
    // Classes
    //
    ///////////////////////////////////////////////////////////////////////////////////////
     -->

    


    <!-- http://www.semanticweb.org/IG/Governance#AccessControl -->

    <owl:Class rdf:about="&Governance;AccessControl">
        <rdfs:subClassOf rdf:resource="&Governance;Security"/>
    </owl:Class>
    


    <!-- http://www.semanticweb.org/IG/Governance#Analytics -->

    <owl:Class rdf:about="&Governance;Analytics">
        <rdfs:subClassOf rdf:resource="&Governance;Risk_Assessment_And_Compliance_Tools"/>
    </owl:Class>
    


    <!-- http://www.semanticweb.org/IG/Governance#Archieving -->

    <owl:Class rdf:about="&Governance;Archieving">
        <rdfs:subClassOf rdf:resource="&Governance;Data_Management_And_Governance_Tools"/>
    </owl:Class>
    


    <!-- http://www.semanticweb.org/IG/Governance#Asset_Database -->

    <owl:Class rdf:about="&Governance;Asset_Database">
        <rdfs:subClassOf rdf:resource="&Governance;Data_Management_And_Governance_Tools"/>
    </owl:Class>
    


    <!-- http://www.semanticweb.org/IG/Governance#Audit -->

    <owl:Class rdf:about="&Governance;Audit">
        <rdfs:subClassOf rdf:resource="&Governance;Security"/>
    </owl:Class>
    


    <!-- http://www.semanticweb.org/IG/Governance#Authentication -->

    <owl:Class rdf:about="&Governance;Authentication">
        <rdfs:subClassOf rdf:resource="&Governance;Security_Tools"/>
    </owl:Class>
    


    <!-- http://www.semanticweb.org/IG/Governance#Automated_Chain_Of_Custody_Logging -->

    <owl:Class rdf:about="&Governance;Automated_Chain_Of_Custody_Logging">
        <rdfs:subClassOf rdf:resource="&Governance;Evidence_And_Data_Logging_Tools"/>
    </owl:Class>
    


    <!-- http://www.semanticweb.org/IG/Governance#Automated_Data_Collection -->

    <owl:Class rdf:about="&Governance;Automated_Data_Collection">
        <rdfs:subClassOf rdf:resource="&Governance;Evidence_And_Data_Logging_Tools"/>
    </owl:Class>
    


    <!-- http://www.semanticweb.org/IG/Governance#Automated_Data_Culling_And_Scoping -->

    <owl:Class rdf:about="&Governance;Automated_Data_Culling_And_Scoping">
        <rdfs:subClassOf rdf:resource="&Governance;Data_Management_And_Governance_Tools"/>
    </owl:Class>
    


    <!-- http://www.semanticweb.org/IG/Governance#Automated_Data_Retention_And_Disposal -->

    <owl:Class rdf:about="&Governance;Automated_Data_Retention_And_Disposal">
        <rdfs:subClassOf rdf:resource="&Governance;Data_Management_And_Governance_Tools"/>
    </owl:Class>
    


    <!-- http://www.semanticweb.org/IG/Governance#Automated_Notification_System -->

    <owl:Class rdf:about="&Governance;Automated_Notification_System">
        <rdfs:subClassOf rdf:resource="&Governance;Communication_And_Collaboration_Tools"/>
    </owl:Class>
    


    <!-- http://www.semanticweb.org/IG/Governance#Automated_Record_Flagging_System -->

    <owl:Class rdf:about="&Governance;Automated_Record_Flagging_System">
        <rdfs:subClassOf rdf:resource="&Governance;Evidence_And_Data_Logging_Tools"/>
    </owl:Class>
    


    <!-- http://www.semanticweb.org/IG/Governance#Automated_Retention_Execution -->

    <owl:Class rdf:about="&Governance;Automated_Retention_Execution">
        <rdfs:subClassOf rdf:resource="&Governance;Data_Management_And_Governance_Tools"/>
    </owl:Class>
    


    <!-- http://www.semanticweb.org/IG/Governance#Automated_Risk_Assessment_System -->

    <owl:Class rdf:about="&Governance;Automated_Risk_Assessment_System">
        <rdfs:subClassOf rdf:resource="&Governance;Risk_Assessment_And_Compliance_Tools"/>
    </owl:Class>
    


    <!-- http://www.semanticweb.org/IG/Governance#Automated_Storage_Utilization_Reporting -->

    <owl:Class rdf:about="&Governance;Automated_Storage_Utilization_Reporting">
        <rdfs:subClassOf rdf:resource="&Governance;Monitoring_And_Visibility_Tools"/>
    </owl:Class>
    


    <!-- http://www.semanticweb.org/IG/Governance#Automted_Integration -->

    <owl:Class rdf:about="&Governance;Automted_Integration">
        <rdfs:subClassOf rdf:resource="&Governance;Data_Management_And_Governance_Tools"/>
    </owl:Class>
    


    <!-- http://www.semanticweb.org/IG/Governance#Backup -->

    <owl:Class rdf:about="&Governance;Backup">
        <rdfs:subClassOf rdf:resource="&Governance;Backup_And_Recovery_Tools"/>
    </owl:Class>
    


    <!-- http://www.semanticweb.org/IG/Governance#Backup_And_Recovery_Tools -->

    <owl:Class rdf:about="&Governance;Backup_And_Recovery_Tools">
        <rdfs:subClassOf rdf:resource="&Governance;Tools"/>
    </owl:Class>
    


    <!-- http://www.semanticweb.org/IG/Governance#Business_Unit -->

    <owl:Class rdf:about="&Governance;Business_Unit">
        <rdfs:subClassOf rdf:resource="&Governance;Organization"/>
    </owl:Class>
    


    <!-- http://www.semanticweb.org/IG/Governance#CCO -->

    <owl:Class rdf:about="&Governance;CCO">
        <rdfs:subClassOf rdf:resource="&Governance;Role"/>
    </owl:Class>
    


    <!-- http://www.semanticweb.org/IG/Governance#CIGO -->

    <owl:Class rdf:about="&Governance;CIGO">
        <rdfs:subClassOf rdf:resource="&Governance;Role"/>
    </owl:Class>
    


    <!-- http://www.semanticweb.org/IG/Governance#CSO -->

    <owl:Class rdf:about="&Governance;CSO">
        <rdfs:subClassOf rdf:resource="&Governance;Role"/>
    </owl:Class>
    


    <!-- http://www.semanticweb.org/IG/Governance#Capability -->

    <owl:Class rdf:about="&Governance;Capability"/>
    


    <!-- http://www.semanticweb.org/IG/Governance#Centralized_Data_Repository -->

    <owl:Class rdf:about="&Governance;Centralized_Data_Repository">
        <rdfs:subClassOf rdf:resource="&Governance;Data_Management_And_Governance_Tools"/>
    </owl:Class>
    


    <!-- http://www.semanticweb.org/IG/Governance#Centralized_Data_Source_Catalog -->

    <owl:Class rdf:about="&Governance;Centralized_Data_Source_Catalog">
        <rdfs:subClassOf rdf:resource="&Governance;Data_Management_And_Governance_Tools"/>
    </owl:Class>
    


    <!-- http://www.semanticweb.org/IG/Governance#Centralized_Instructions_Repository -->

    <owl:Class rdf:about="&Governance;Centralized_Instructions_Repository">
        <rdfs:subClassOf rdf:resource="&Governance;Document_And_Records_Management_Tools"/>
    </owl:Class>
    


    <!-- http://www.semanticweb.org/IG/Governance#Chain_Of_Custody_Tracking -->

    <owl:Class rdf:about="&Governance;Chain_Of_Custody_Tracking">
        <rdfs:subClassOf rdf:resource="&Governance;Monitoring_And_Visibility_Tools"/>
    </owl:Class>
    


    <!-- http://www.semanticweb.org/IG/Governance#Change_Management -->

    <owl:Class rdf:about="&Governance;Change_Management">
        <rdfs:subClassOf rdf:resource="&Governance;Organization"/>
    </owl:Class>
    


    <!-- http://www.semanticweb.org/IG/Governance#Collaboration_Tools -->

    <owl:Class rdf:about="&Governance;Collaboration_Tools">
        <rdfs:subClassOf rdf:resource="&Governance;Communication_And_Collaboration_Tools"/>
    </owl:Class>
    


    <!-- http://www.semanticweb.org/IG/Governance#Communication_And_Collaboration_Tools -->

    <owl:Class rdf:about="&Governance;Communication_And_Collaboration_Tools">
        <rdfs:subClassOf rdf:resource="&Governance;Tools"/>
    </owl:Class>
    


    <!-- http://www.semanticweb.org/IG/Governance#Communication_Platforms -->

    <owl:Class rdf:about="&Governance;Communication_Platforms">
        <rdfs:subClassOf rdf:resource="&Governance;Communication_And_Collaboration_Tools"/>
    </owl:Class>
    


    <!-- http://www.semanticweb.org/IG/Governance#Confirmation_Tracking_Mechanism -->

    <owl:Class rdf:about="&Governance;Confirmation_Tracking_Mechanism">
        <rdfs:subClassOf rdf:resource="&Governance;Risk_Assessment_And_Compliance_Tools"/>
    </owl:Class>
    


    <!-- http://www.semanticweb.org/IG/Governance#Continous_Visibility_And_Monitoring_System -->

    <owl:Class rdf:about="&Governance;Continous_Visibility_And_Monitoring_System">
        <rdfs:subClassOf rdf:resource="&Governance;Monitoring_And_Visibility_Tools"/>
    </owl:Class>
    


    <!-- http://www.semanticweb.org/IG/Governance#Cost_Calculations -->

    <owl:Class rdf:about="&Governance;Cost_Calculations">
        <rdfs:subClassOf rdf:resource="&Governance;Workflow_And_Process_Management_Tools"/>
    </owl:Class>
    


    <!-- http://www.semanticweb.org/IG/Governance#DPO -->

    <owl:Class rdf:about="&Governance;DPO">
        <rdfs:subClassOf rdf:resource="&Governance;Role"/>
    </owl:Class>
    


    <!-- http://www.semanticweb.org/IG/Governance#Data -->

    <owl:Class rdf:about="&Governance;Data"/>
    


    <!-- http://www.semanticweb.org/IG/Governance#Data_Controller -->

    <owl:Class rdf:about="&Governance;Data_Controller">
        <rdfs:subClassOf rdf:resource="&Governance;Role"/>
    </owl:Class>
    


    <!-- http://www.semanticweb.org/IG/Governance#Data_Management_And_Governance_Tools -->

    <owl:Class rdf:about="&Governance;Data_Management_And_Governance_Tools">
        <rdfs:subClassOf rdf:resource="&Governance;Tools"/>
    </owl:Class>
    


    <!-- http://www.semanticweb.org/IG/Governance#Data_Mapping_And_Classification_System -->

    <owl:Class rdf:about="&Governance;Data_Mapping_And_Classification_System">
        <rdfs:subClassOf rdf:resource="&Governance;Data_Management_And_Governance_Tools"/>
    </owl:Class>
    


    <!-- http://www.semanticweb.org/IG/Governance#Data_Privacy_Masking -->

    <owl:Class rdf:about="&Governance;Data_Privacy_Masking">
        <rdfs:subClassOf rdf:resource="&Governance;Data_Management_And_Governance_Tools"/>
    </owl:Class>
    


    <!-- http://www.semanticweb.org/IG/Governance#Data_Processor -->

    <owl:Class rdf:about="&Governance;Data_Processor">
        <rdfs:subClassOf rdf:resource="&Governance;Role"/>
    </owl:Class>
    


    <!-- http://www.semanticweb.org/IG/Governance#Data_Quality_Assurance_Framework -->

    <owl:Class rdf:about="&Governance;Data_Quality_Assurance_Framework">
        <rdfs:subClassOf rdf:resource="&Governance;Data_Management_And_Governance_Tools"/>
    </owl:Class>
    


    <!-- http://www.semanticweb.org/IG/Governance#Data_Quality_Management -->

    <owl:Class rdf:about="&Governance;Data_Quality_Management">
        <rdfs:subClassOf rdf:resource="&Governance;Data_Management_And_Governance_Tools"/>
    </owl:Class>
    


    <!-- http://www.semanticweb.org/IG/Governance#Data_Retention_Policy -->

    <owl:Class rdf:about="&Governance;Data_Retention_Policy">
        <rdfs:subClassOf rdf:resource="&Governance;Data_Management_And_Governance_Tools"/>
    </owl:Class>
    


    <!-- http://www.semanticweb.org/IG/Governance#Data_Sharing_Protocols -->

    <owl:Class rdf:about="&Governance;Data_Sharing_Protocols">
        <rdfs:subClassOf rdf:resource="&Governance;Data_Management_And_Governance_Tools"/>
    </owl:Class>
    


    <!-- http://www.semanticweb.org/IG/Governance#Data_Storage -->

    <owl:Class rdf:about="&Governance;Data_Storage">
        <rdfs:subClassOf rdf:resource="&Governance;Data_Management_And_Governance_Tools"/>
    </owl:Class>
    


    <!-- http://www.semanticweb.org/IG/Governance#Data_Subject -->

    <owl:Class rdf:about="&Governance;Data_Subject">
        <rdfs:subClassOf rdf:resource="&Governance;Role"/>
    </owl:Class>
    


    <!-- http://www.semanticweb.org/IG/Governance#Data_Testing_And_Validation_Tools -->

    <owl:Class rdf:about="&Governance;Data_Testing_And_Validation_Tools">
        <rdfs:subClassOf rdf:resource="&Governance;Tools"/>
    </owl:Class>
    


    <!-- http://www.semanticweb.org/IG/Governance#Database_Management_System -->

    <owl:Class rdf:about="&Governance;Database_Management_System">
        <rdfs:subClassOf rdf:resource="&Governance;Records_Management"/>
    </owl:Class>
    


    <!-- http://www.semanticweb.org/IG/Governance#Deadline_Tracking -->

    <owl:Class rdf:about="&Governance;Deadline_Tracking">
        <rdfs:subClassOf rdf:resource="&Governance;Workflow_And_Process_Management_Tools"/>
    </owl:Class>
    


    <!-- http://www.semanticweb.org/IG/Governance#Designation_Interface -->

    <owl:Class rdf:about="&Governance;Designation_Interface">
        <rdfs:subClassOf rdf:resource="&Governance;Data_Management_And_Governance_Tools"/>
    </owl:Class>
    


    <!-- http://www.semanticweb.org/IG/Governance#Development -->

    <owl:Class rdf:about="&Governance;Development">
        <rdfs:subClassOf rdf:resource="&Governance;Organization"/>
    </owl:Class>
    


    <!-- http://www.semanticweb.org/IG/Governance#Digital_Signatures_And_Timestamps -->

    <owl:Class rdf:about="&Governance;Digital_Signatures_And_Timestamps">
        <rdfs:subClassOf rdf:resource="&Governance;Data_Management_And_Governance_Tools"/>
    </owl:Class>
    


    <!-- http://www.semanticweb.org/IG/Governance#Disposition_Policies_And_Procedures -->

    <owl:Class rdf:about="&Governance;Disposition_Policies_And_Procedures">
        <rdfs:subClassOf rdf:resource="&Governance;Data_Management_And_Governance_Tools"/>
    </owl:Class>
    


    <!-- http://www.semanticweb.org/IG/Governance#Document_And_Records_Management_Tools -->

    <owl:Class rdf:about="&Governance;Document_And_Records_Management_Tools">
        <rdfs:subClassOf rdf:resource="&Governance;Tools"/>
    </owl:Class>
    


    <!-- http://www.semanticweb.org/IG/Governance#Document_Management_System -->

    <owl:Class rdf:about="&Governance;Document_Management_System">
        <rdfs:subClassOf rdf:resource="&Governance;Document_And_Records_Management_Tools"/>
    </owl:Class>
    


    <!-- http://www.semanticweb.org/IG/Governance#Early_Case_Assessment -->

    <owl:Class rdf:about="&Governance;Early_Case_Assessment">
        <rdfs:subClassOf rdf:resource="&Governance;Workflow_And_Process_Management_Tools"/>
    </owl:Class>
    


    <!-- http://www.semanticweb.org/IG/Governance#Electronic_Records_Management -->

    <owl:Class rdf:about="&Governance;Electronic_Records_Management">
        <rdfs:subClassOf rdf:resource="&Governance;Records_Management"/>
        <owl:disjointWith rdf:resource="&Governance;Records_And_Information_Management"/>
    </owl:Class>
    


    <!-- http://www.semanticweb.org/IG/Governance#Employee_Engagement_Platforms -->

    <owl:Class rdf:about="&Governance;Employee_Engagement_Platforms">
        <rdfs:subClassOf rdf:resource="&Governance;Communication_And_Collaboration_Tools"/>
    </owl:Class>
    


    <!-- http://www.semanticweb.org/IG/Governance#Employee_Interviews -->

    <owl:Class rdf:about="&Governance;Employee_Interviews">
        <rdfs:subClassOf rdf:resource="&Governance;Knowledge_And_resource_Repository_Tools"/>
    </owl:Class>
    


    <!-- http://www.semanticweb.org/IG/Governance#Employee_Self_Service_Portal -->

    <owl:Class rdf:about="&Governance;Employee_Self_Service_Portal">
        <rdfs:subClassOf rdf:resource="&Governance;Communication_And_Collaboration_Tools"/>
    </owl:Class>
    


    <!-- http://www.semanticweb.org/IG/Governance#Encryption -->

    <owl:Class rdf:about="&Governance;Encryption">
        <rdfs:subClassOf rdf:resource="&Governance;Security_Tools"/>
    </owl:Class>
    


    <!-- http://www.semanticweb.org/IG/Governance#Enterprise_Risk_Management -->

    <owl:Class rdf:about="&Governance;Enterprise_Risk_Management">
        <rdfs:subClassOf rdf:resource="&Governance;Risk_And_Compliance"/>
        <owl:disjointWith rdf:resource="&Governance;Information_Risk_Management"/>
    </owl:Class>
    


    <!-- http://www.semanticweb.org/IG/Governance#Evidence_And_Data_Logging_Tools -->

    <owl:Class rdf:about="&Governance;Evidence_And_Data_Logging_Tools">
        <rdfs:subClassOf rdf:resource="&Governance;Tools"/>
    </owl:Class>
    


    <!-- http://www.semanticweb.org/IG/Governance#Exception_Handling_System -->

    <owl:Class rdf:about="&Governance;Exception_Handling_System">
        <rdfs:subClassOf rdf:resource="&Governance;Risk_Assessment_And_Compliance_Tools"/>
    </owl:Class>
    


    <!-- http://www.semanticweb.org/IG/Governance#Executive_Sponsor -->

    <owl:Class rdf:about="&Governance;Executive_Sponsor">
        <rdfs:subClassOf rdf:resource="&Governance;Role"/>
    </owl:Class>
    


    <!-- http://www.semanticweb.org/IG/Governance#Framework -->

    <owl:Class rdf:about="&Governance;Framework"/>
    


    <!-- http://www.semanticweb.org/IG/Governance#GDPR -->

    <owl:Class rdf:about="&Governance;GDPR"/>
    


    <!-- http://www.semanticweb.org/IG/Governance#Goal -->

    <owl:Class rdf:about="&Governance;Goal"/>
    


    <!-- http://www.semanticweb.org/IG/Governance#Hold_Enforcement_Automation_System -->

    <owl:Class rdf:about="&Governance;Hold_Enforcement_Automation_System">
        <rdfs:subClassOf rdf:resource="&Governance;Workflow_And_Process_Management_Tools"/>
    </owl:Class>
    


    <!-- http://www.semanticweb.org/IG/Governance#IG_Capability -->

    <owl:Class rdf:about="&Governance;IG_Capability">
        <rdfs:subClassOf rdf:resource="&Governance;Capability"/>
    </owl:Class>
    


    <!-- http://www.semanticweb.org/IG/Governance#IG_Chief_Officer -->

    <owl:Class rdf:about="&Governance;IG_Chief_Officer">
        <rdfs:subClassOf rdf:resource="&Governance;Role"/>
    </owl:Class>
    


    <!-- http://www.semanticweb.org/IG/Governance#IG_Leadership -->

    <owl:Class rdf:about="&Governance;IG_Leadership">
        <rdfs:subClassOf rdf:resource="&Governance;Role"/>
    </owl:Class>
    


    <!-- http://www.semanticweb.org/IG/Governance#IG_Policy -->

    <owl:Class rdf:about="&Governance;IG_Policy"/>
    


    <!-- http://www.semanticweb.org/IG/Governance#IG_Programm -->

    <owl:Class rdf:about="&Governance;IG_Programm"/>
    


    <!-- http://www.semanticweb.org/IG/Governance#IG_Strategic_Plan -->

    <owl:Class rdf:about="&Governance;IG_Strategic_Plan"/>
    


    <!-- http://www.semanticweb.org/IG/Governance#IG_Team -->

    <owl:Class rdf:about="&Governance;IG_Team"/>
    


    <!-- http://www.semanticweb.org/IG/Governance#ISO -->

    <owl:Class rdf:about="&Governance;ISO"/>
    


    <!-- http://www.semanticweb.org/IG/Governance#IT_Planning_And_Strategy_Framework -->

    <owl:Class rdf:about="&Governance;IT_Planning_And_Strategy_Framework">
        <rdfs:subClassOf rdf:resource="&Governance;Workflow_And_Process_Management_Tools"/>
    </owl:Class>
    


    <!-- http://www.semanticweb.org/IG/Governance#Incident_Response_And_Remediation_Protocol -->

    <owl:Class rdf:about="&Governance;Incident_Response_And_Remediation_Protocol">
        <rdfs:subClassOf rdf:resource="&Governance;Risk_Assessment_And_Compliance_Tools"/>
    </owl:Class>
    


    <!-- http://www.semanticweb.org/IG/Governance#Information_Asset_Risk_Mitigation_Plan -->

    <owl:Class rdf:about="&Governance;Information_Asset_Risk_Mitigation_Plan"/>
    


    <!-- http://www.semanticweb.org/IG/Governance#Information_Risk_Management -->

    <owl:Class rdf:about="&Governance;Information_Risk_Management">
        <rdfs:subClassOf rdf:resource="&Governance;Risk_And_Compliance"/>
    </owl:Class>
    


    <!-- http://www.semanticweb.org/IG/Governance#Inventory_Of_Evidence -->

    <owl:Class rdf:about="&Governance;Inventory_Of_Evidence">
        <rdfs:subClassOf rdf:resource="&Governance;Monitoring_And_Visibility_Tools"/>
    </owl:Class>
    


    <!-- http://www.semanticweb.org/IG/Governance#Knowledge_And_resource_Repository_Tools -->

    <owl:Class rdf:about="&Governance;Knowledge_And_resource_Repository_Tools">
        <rdfs:subClassOf rdf:resource="&Governance;Tools"/>
    </owl:Class>
    


    <!-- http://www.semanticweb.org/IG/Governance#LHN_Requirements -->

    <owl:Class rdf:about="&Governance;LHN_Requirements"/>
    


    <!-- http://www.semanticweb.org/IG/Governance#Laws_Mapping_And_Compliance_Tracking -->

    <owl:Class rdf:about="&Governance;Laws_Mapping_And_Compliance_Tracking">
        <rdfs:subClassOf rdf:resource="&Governance;Legal_And_Compliance_Tools"/>
    </owl:Class>
    


    <!-- http://www.semanticweb.org/IG/Governance#Legal -->

    <owl:Class rdf:about="&Governance;Legal">
        <rdfs:subClassOf rdf:resource="&Governance;Organization"/>
    </owl:Class>
    


    <!-- http://www.semanticweb.org/IG/Governance#Legal_And_Compliance_Tools -->

    <owl:Class rdf:about="&Governance;Legal_And_Compliance_Tools">
        <rdfs:subClassOf rdf:resource="&Governance;Tools"/>
    </owl:Class>
    


    <!-- http://www.semanticweb.org/IG/Governance#Legal_Hold_Inventory -->

    <owl:Class rdf:about="&Governance;Legal_Hold_Inventory">
        <rdfs:subClassOf rdf:resource="&Governance;Legal_And_Compliance_Tools"/>
    </owl:Class>
    


    <!-- http://www.semanticweb.org/IG/Governance#Legal_Hold_Management -->

    <owl:Class rdf:about="&Governance;Legal_Hold_Management">
        <rdfs:subClassOf rdf:resource="&Governance;Legal_And_Compliance_Tools"/>
    </owl:Class>
    


    <!-- http://www.semanticweb.org/IG/Governance#Legal_Hold_Notification -->

    <owl:Class rdf:about="&Governance;Legal_Hold_Notification"/>
    


    <!-- http://www.semanticweb.org/IG/Governance#Legal_Matters_Testing -->

    <owl:Class rdf:about="&Governance;Legal_Matters_Testing">
        <rdfs:subClassOf rdf:resource="&Governance;Data_Testing_And_Validation_Tools"/>
    </owl:Class>
    


    <!-- http://www.semanticweb.org/IG/Governance#Long_Term_Digital_Preservation -->

    <owl:Class rdf:about="&Governance;Long_Term_Digital_Preservation">
        <rdfs:subClassOf rdf:resource="&Governance;Organization"/>
    </owl:Class>
    


    <!-- http://www.semanticweb.org/IG/Governance#Maturity -->

    <owl:Class rdf:about="&Governance;Maturity"/>
    


    <!-- http://www.semanticweb.org/IG/Governance#Metadata -->

    <owl:Class rdf:about="&Governance;Metadata"/>
    


    <!-- http://www.semanticweb.org/IG/Governance#Metadata_Framework -->

    <owl:Class rdf:about="&Governance;Metadata_Framework">
        <rdfs:subClassOf rdf:resource="&Governance;Document_And_Records_Management_Tools"/>
    </owl:Class>
    


    <!-- http://www.semanticweb.org/IG/Governance#Metrics -->

    <owl:Class rdf:about="&Governance;Metrics"/>
    


    <!-- http://www.semanticweb.org/IG/Governance#Monitoring -->

    <owl:Class rdf:about="&Governance;Monitoring">
        <rdfs:subClassOf rdf:resource="&Governance;Security"/>
    </owl:Class>
    


    <!-- http://www.semanticweb.org/IG/Governance#Monitoring_And_Visibility_Tools -->

    <owl:Class rdf:about="&Governance;Monitoring_And_Visibility_Tools">
        <rdfs:subClassOf rdf:resource="&Governance;Tools"/>
    </owl:Class>
    


    <!-- http://www.semanticweb.org/IG/Governance#Organization -->

    <owl:Class rdf:about="&Governance;Organization"/>
    


    <!-- http://www.semanticweb.org/IG/Governance#Privacy -->

    <owl:Class rdf:about="&Governance;Privacy">
        <rdfs:subClassOf rdf:resource="&Governance;Organization"/>
    </owl:Class>
    


    <!-- http://www.semanticweb.org/IG/Governance#Privacy_Impact_Assessment_Tools -->

    <owl:Class rdf:about="&Governance;Privacy_Impact_Assessment_Tools">
        <rdfs:subClassOf rdf:resource="&Governance;Risk_Assessment_And_Compliance_Tools"/>
    </owl:Class>
    


    <!-- http://www.semanticweb.org/IG/Governance#Privacy_Laws_And_Policies_Repository -->

    <owl:Class rdf:about="&Governance;Privacy_Laws_And_Policies_Repository">
        <rdfs:subClassOf rdf:resource="&Governance;Legal_And_Compliance_Tools"/>
    </owl:Class>
    


    <!-- http://www.semanticweb.org/IG/Governance#Process -->

    <owl:Class rdf:about="&Governance;Process"/>
    


    <!-- http://www.semanticweb.org/IG/Governance#Project_Manager -->

    <owl:Class rdf:about="&Governance;Project_Manager">
        <rdfs:subClassOf rdf:resource="&Governance;Role"/>
    </owl:Class>
    


    <!-- http://www.semanticweb.org/IG/Governance#Query -->

    <owl:Class rdf:about="&Governance;Query"/>
    


    <!-- http://www.semanticweb.org/IG/Governance#Records_And_Information_Management -->

    <owl:Class rdf:about="&Governance;Records_And_Information_Management">
        <rdfs:subClassOf rdf:resource="&Governance;Records_Management"/>
    </owl:Class>
    


    <!-- http://www.semanticweb.org/IG/Governance#Records_Management -->

    <owl:Class rdf:about="&Governance;Records_Management">
        <rdfs:subClassOf rdf:resource="&Governance;Organization"/>
    </owl:Class>
    


    <!-- http://www.semanticweb.org/IG/Governance#Records_Retention_Schedule -->

    <owl:Class rdf:about="&Governance;Records_Retention_Schedule">
        <rdfs:subClassOf rdf:resource="&Governance;Data_Management_And_Governance_Tools"/>
    </owl:Class>
    


    <!-- http://www.semanticweb.org/IG/Governance#Remote_Wiping -->

    <owl:Class rdf:about="&Governance;Remote_Wiping">
        <rdfs:subClassOf rdf:resource="&Governance;Backup_And_Recovery_Tools"/>
    </owl:Class>
    


    <!-- http://www.semanticweb.org/IG/Governance#Reporting_And_Analysis_System -->

    <owl:Class rdf:about="&Governance;Reporting_And_Analysis_System">
        <rdfs:subClassOf rdf:resource="&Governance;Communication_And_Collaboration_Tools"/>
    </owl:Class>
    


    <!-- http://www.semanticweb.org/IG/Governance#Request_Management_System -->

    <owl:Class rdf:about="&Governance;Request_Management_System">
        <rdfs:subClassOf rdf:resource="&Governance;Legal_And_Compliance_Tools"/>
    </owl:Class>
    


    <!-- http://www.semanticweb.org/IG/Governance#Retention_Rule_Management_System -->

    <owl:Class rdf:about="&Governance;Retention_Rule_Management_System">
        <rdfs:subClassOf rdf:resource="&Governance;Data_Management_And_Governance_Tools"/>
    </owl:Class>
    


    <!-- http://www.semanticweb.org/IG/Governance#Review_Cycles -->

    <owl:Class rdf:about="&Governance;Review_Cycles">
        <rdfs:subClassOf rdf:resource="&Governance;Workflow_And_Process_Management_Tools"/>
    </owl:Class>
    


    <!-- http://www.semanticweb.org/IG/Governance#Revisitation_And_Refinement -->

    <owl:Class rdf:about="&Governance;Revisitation_And_Refinement">
        <rdfs:subClassOf rdf:resource="&Governance;Workflow_And_Process_Management_Tools"/>
    </owl:Class>
    


    <!-- http://www.semanticweb.org/IG/Governance#Risk_And_Compliance -->

    <owl:Class rdf:about="&Governance;Risk_And_Compliance">
        <rdfs:subClassOf rdf:resource="&Governance;Organization"/>
    </owl:Class>
    


    <!-- http://www.semanticweb.org/IG/Governance#Risk_Assessment_And_Compliance_Tools -->

    <owl:Class rdf:about="&Governance;Risk_Assessment_And_Compliance_Tools">
        <rdfs:subClassOf rdf:resource="&Governance;Tools"/>
    </owl:Class>
    


    <!-- http://www.semanticweb.org/IG/Governance#Risk_Profile -->

    <owl:Class rdf:about="&Governance;Risk_Profile"/>
    


    <!-- http://www.semanticweb.org/IG/Governance#Role -->

    <owl:Class rdf:about="&Governance;Role"/>
    


    <!-- http://www.semanticweb.org/IG/Governance#SLA -->

    <owl:Class rdf:about="&Governance;SLA">
        <rdfs:subClassOf rdf:resource="&Governance;Monitoring_And_Visibility_Tools"/>
    </owl:Class>
    


    <!-- http://www.semanticweb.org/IG/Governance#Search_And_Retrieval_System -->

    <owl:Class rdf:about="&Governance;Search_And_Retrieval_System">
        <rdfs:subClassOf rdf:resource="&Governance;Evidence_And_Data_Logging_Tools"/>
    </owl:Class>
    


    <!-- http://www.semanticweb.org/IG/Governance#Security -->

    <owl:Class rdf:about="&Governance;Security">
        <rdfs:subClassOf rdf:resource="&Governance;Organization"/>
    </owl:Class>
    


    <!-- http://www.semanticweb.org/IG/Governance#Security_Assessment_Framework -->

    <owl:Class rdf:about="&Governance;Security_Assessment_Framework">
        <rdfs:subClassOf rdf:resource="&Governance;Security_Tools"/>
    </owl:Class>
    


    <!-- http://www.semanticweb.org/IG/Governance#Security_Tools -->

    <owl:Class rdf:about="&Governance;Security_Tools">
        <rdfs:subClassOf rdf:resource="&Governance;Tools"/>
    </owl:Class>
    


    <!-- http://www.semanticweb.org/IG/Governance#Senior_Records_Officer -->

    <owl:Class rdf:about="&Governance;Senior_Records_Officer">
        <rdfs:subClassOf rdf:resource="&Governance;Role"/>
    </owl:Class>
    


    <!-- http://www.semanticweb.org/IG/Governance#Shared_Library_Of_Country_Protocols -->

    <owl:Class rdf:about="&Governance;Shared_Library_Of_Country_Protocols">
        <rdfs:subClassOf rdf:resource="&Governance;Knowledge_And_resource_Repository_Tools"/>
    </owl:Class>
    


    <!-- http://www.semanticweb.org/IG/Governance#Stakeholder -->

    <owl:Class rdf:about="&Governance;Stakeholder">
        <rdfs:subClassOf rdf:resource="&Governance;Role"/>
    </owl:Class>
    


    <!-- http://www.semanticweb.org/IG/Governance#Steering_Commitee -->

    <owl:Class rdf:about="&Governance;Steering_Commitee">
        <rdfs:subClassOf rdf:resource="&Governance;Role"/>
    </owl:Class>
    


    <!-- http://www.semanticweb.org/IG/Governance#Supervisor_Authority -->

    <owl:Class rdf:about="&Governance;Supervisor_Authority"/>
    


    <!-- http://www.semanticweb.org/IG/Governance#Syndication_System_For_Hold_Release -->

    <owl:Class rdf:about="&Governance;Syndication_System_For_Hold_Release">
        <rdfs:subClassOf rdf:resource="&Governance;Legal_And_Compliance_Tools"/>
    </owl:Class>
    


    <!-- http://www.semanticweb.org/IG/Governance#System_Log -->

    <owl:Class rdf:about="&Governance;System_Log">
        <rdfs:subClassOf rdf:resource="&Governance;Monitoring_And_Visibility_Tools"/>
    </owl:Class>
    


    <!-- http://www.semanticweb.org/IG/Governance#TOSCA_Capability -->

    <owl:Class rdf:about="&Governance;TOSCA_Capability">
        <rdfs:subClassOf rdf:resource="&Governance;Capability"/>
    </owl:Class>
    


    <!-- http://www.semanticweb.org/IG/Governance#Testing -->

    <owl:Class rdf:about="&Governance;Testing">
        <rdfs:subClassOf rdf:resource="&Governance;Data_Testing_And_Validation_Tools"/>
    </owl:Class>
    


    <!-- http://www.semanticweb.org/IG/Governance#Tools -->

    <owl:Class rdf:about="&Governance;Tools"/>
    


    <!-- http://www.semanticweb.org/IG/Governance#Training -->

    <owl:Class rdf:about="&Governance;Training">
        <rdfs:subClassOf rdf:resource="&Governance;Communication_And_Collaboration_Tools"/>
    </owl:Class>
    


    <!-- http://www.semanticweb.org/IG/Governance#Workflow_And_Process_Management_Tools -->

    <owl:Class rdf:about="&Governance;Workflow_And_Process_Management_Tools">
        <rdfs:subClassOf rdf:resource="&Governance;Tools"/>
    </owl:Class>
    


    <!-- http://www.semanticweb.org/IG/Governance#Workflow_Tools -->

    <owl:Class rdf:about="&Governance;Workflow_Tools">
        <rdfs:subClassOf rdf:resource="&Governance;Data_Management_And_Governance_Tools"/>
    </owl:Class>
    


    <!-- http://www.semanticweb.org/IG/Governance#eDiscovery_Integration -->

    <owl:Class rdf:about="&Governance;eDiscovery_Integration">
        <rdfs:subClassOf rdf:resource="&Governance;Legal_And_Compliance_Tools"/>
    </owl:Class>
    


    <!-- 
    ///////////////////////////////////////////////////////////////////////////////////////
    //
    // Individuals
    //
    ///////////////////////////////////////////////////////////////////////////////////////
     -->

    


    <!-- http://www.semanticweb.org/IG/Governance#1_SubStandard -->

    <owl:NamedIndividual rdf:about="&Governance;1_SubStandard">
        <rdf:type rdf:resource="&Governance;Maturity"/>
    </owl:NamedIndividual>
    


    <!-- http://www.semanticweb.org/IG/Governance#2_InDevelopment -->

    <owl:NamedIndividual rdf:about="&Governance;2_InDevelopment">
        <rdf:type rdf:resource="&Governance;Maturity"/>
    </owl:NamedIndividual>
    


    <!-- http://www.semanticweb.org/IG/Governance#3_Essential -->

    <owl:NamedIndividual rdf:about="&Governance;3_Essential">
        <rdf:type rdf:resource="&Governance;Maturity"/>
    </owl:NamedIndividual>
    


    <!-- http://www.semanticweb.org/IG/Governance#4_Proactive -->

    <owl:NamedIndividual rdf:about="&Governance;4_Proactive">
        <rdf:type rdf:resource="&Governance;Maturity"/>
    </owl:NamedIndividual>
    


    <!-- http://www.semanticweb.org/IG/Governance#5_Transformational -->

    <owl:NamedIndividual rdf:about="&Governance;5_Transformational">
        <rdf:type rdf:resource="&Governance;Maturity"/>
    </owl:NamedIndividual>
    


    <!-- http://www.semanticweb.org/IG/Governance#AC_1_1_3 -->

    <owl:NamedIndividual rdf:about="&Governance;AC_1_1_3">
        <rdf:type rdf:resource="&Governance;IG_Capability"/>
        <Governance:capabilityDescription>A records management program (RMP)  is established.</Governance:capabilityDescription>
        <Governance:inMaturityLevel rdf:resource="&Governance;3_Essential"/>
        <Governance:linkedToFramework rdf:resource="&Governance;ARMA_00"/>
        <Governance:hasGoal rdf:resource="&Governance;Accountability"/>
        <Governance:involvesArticle rdf:resource="&Governance;Article_30"/>
        <Governance:involvesArticle rdf:resource="&Governance;Article_5"/>
        <Governance:needsTechnicalRequirement rdf:resource="&Governance;Document_Management_System_1"/>
        <Governance:practicesDefinedInIso rdf:resource="&Governance;ISO_15489"/>
        <Governance:practicesDefinedInIso rdf:resource="&Governance;ISO_23081"/>
        <Governance:needsTechnicalRequirement rdf:resource="&Governance;Metadata_Framework_1"/>
        <Governance:needsTechnicalRequirement rdf:resource="&Governance;Records_Retention_Schedule_1"/>
    </owl:NamedIndividual>
    <owl:Axiom>
        <rdfs:comment>A robust DMS provides a centralized platform for creating, storing, managing, and retrieving records. It ensures proper organization, version control, and accessibility of records within the RMP.</rdfs:comment>
        <owl:annotatedSource rdf:resource="&Governance;AC_1_1_3"/>
        <owl:annotatedTarget rdf:resource="&Governance;Document_Management_System_1"/>
        <owl:annotatedProperty rdf:resource="&Governance;needsTechnicalRequirement"/>
    </owl:Axiom>
    <owl:Axiom>
        <rdfs:comment>A metadata framework allows consistent and structured metadata assignment to records, facilitating their identification, classification, and retrieval, which is essential for effective records management.</rdfs:comment>
        <owl:annotatedSource rdf:resource="&Governance;AC_1_1_3"/>
        <owl:annotatedTarget rdf:resource="&Governance;Metadata_Framework_1"/>
        <owl:annotatedProperty rdf:resource="&Governance;needsTechnicalRequirement"/>
    </owl:Axiom>
    <owl:Axiom>
        <rdfs:comment>Establishing a records retention schedule ensures that records are retained for the appropriate duration, in alignment with legal, regulatory, and business requirements.</rdfs:comment>
        <owl:annotatedSource rdf:resource="&Governance;AC_1_1_3"/>
        <owl:annotatedTarget rdf:resource="&Governance;Records_Retention_Schedule_1"/>
        <owl:annotatedProperty rdf:resource="&Governance;needsTechnicalRequirement"/>
    </owl:Axiom>
    


    <!-- http://www.semanticweb.org/IG/Governance#AC_1_1_4 -->

    <owl:NamedIndividual rdf:about="&Governance;AC_1_1_4">
        <rdf:type rdf:resource="&Governance;IG_Capability"/>
        <Governance:capabilityDescription>IG professional supervises IG program.</Governance:capabilityDescription>
        <Governance:linkedToFramework rdf:resource="&Governance;ARMA_00"/>
        <Governance:needsTechnicalRequirement rdf:resource="&Governance;AccessControl_1"/>
        <Governance:hasGoal rdf:resource="&Governance;Accountability"/>
        <Governance:involvesArticle rdf:resource="&Governance;Article_24"/>
        <Governance:involvesArticle rdf:resource="&Governance;Article_32"/>
        <Governance:involvesArticle rdf:resource="&Governance;Article_37"/>
        <Governance:involvesArticle rdf:resource="&Governance;Article_38"/>
        <Governance:involvesArticle rdf:resource="&Governance;Article_39"/>
        <Governance:involvesArticle rdf:resource="&Governance;Article_5"/>
        <Governance:needsTechnicalRequirement rdf:resource="&Governance;DPO_1"/>
        <Governance:needsTechnicalRequirement rdf:resource="&Governance;IG_Programm_1"/>
        <Governance:practicesDefinedInIso rdf:resource="&Governance;ISO_15489"/>
        <Governance:practicesDefinedInIso rdf:resource="&Governance;ISO_15939"/>
        <Governance:practicesDefinedInIso rdf:resource="&Governance;ISO_27000"/>
        <Governance:needsTechnicalRequirement rdf:resource="&Governance;Stakeholder_1"/>
    </owl:NamedIndividual>
    <owl:Axiom>
        <rdfs:comment> Clear role definitions and well-defined responsibilities for IG professionals within the organization are essential. This involves outlining their authority, tasks, and accountability to ensure effective oversight of the IG program.</rdfs:comment>
        <owl:annotatedSource rdf:resource="&Governance;AC_1_1_4"/>
        <owl:annotatedTarget rdf:resource="&Governance;IG_Programm_1"/>
        <owl:annotatedProperty rdf:resource="&Governance;needsTechnicalRequirement"/>
    </owl:Axiom>
    <owl:Axiom>
        <rdfs:comment>It is crucial to have skilled and knowledgeable Information Governance (IG) professionals who possess expertise in various aspects of IG, including data protection, privacy, records management, and compliance. These professionals play a pivotal role in overseeing and managing the IG program.</rdfs:comment>
        <owl:annotatedSource rdf:resource="&Governance;AC_1_1_4"/>
        <owl:annotatedTarget rdf:resource="&Governance;DPO_1"/>
        <owl:annotatedProperty rdf:resource="&Governance;needsTechnicalRequirement"/>
    </owl:Axiom>
    <owl:Axiom>
        <rdfs:comment>IG professionals must collaborate with various stakeholders, including legal, compliance, IT, and business units, to ensure that the IG program is well-integrated and aligned with organizational goals.</rdfs:comment>
        <owl:annotatedSource rdf:resource="&Governance;AC_1_1_4"/>
        <owl:annotatedTarget rdf:resource="&Governance;Stakeholder_1"/>
        <owl:annotatedProperty rdf:resource="&Governance;needsTechnicalRequirement"/>
    </owl:Axiom>
    <owl:Axiom>
        <rdfs:comment> IG professionals require access to appropriate tools, technologies, and resources to manage and supervise the IG program efficiently. This includes access to data management software, analytics tools, compliance monitoring systems, and relevant documentation.</rdfs:comment>
        <owl:annotatedSource rdf:resource="&Governance;AC_1_1_4"/>
        <owl:annotatedTarget rdf:resource="&Governance;AccessControl_1"/>
        <owl:annotatedProperty rdf:resource="&Governance;needsTechnicalRequirement"/>
    </owl:Axiom>
    


    <!-- http://www.semanticweb.org/IG/Governance#AC_1_1_5 -->

    <owl:NamedIndividual rdf:about="&Governance;AC_1_1_5">
        <rdf:type rdf:resource="&Governance;IG_Capability"/>
        <Governance:capabilityDescription>SMgmnt and Governing Board place great emphasis on IG.</Governance:capabilityDescription>
        <Governance:inMaturityLevel rdf:resource="&Governance;5_Transformational"/>
        <Governance:linkedToFramework rdf:resource="&Governance;ARMA_00"/>
        <Governance:hasGoal rdf:resource="&Governance;Accountability"/>
        <Governance:involvesArticle rdf:resource="&Governance;Article_24"/>
        <Governance:involvesArticle rdf:resource="&Governance;Article_35"/>
        <Governance:involvesArticle rdf:resource="&Governance;Article_5"/>
        <Governance:needsTechnicalRequirement rdf:resource="&Governance;IG_Leadership_1"/>
        <Governance:needsTechnicalRequirement rdf:resource="&Governance;IG_Strategic_Plan_1"/>
        <Governance:practicesDefinedInIso rdf:resource="&Governance;ISO_15489"/>
        <Governance:practicesDefinedInIso rdf:resource="&Governance;ISO_23081"/>
        <Governance:practicesDefinedInIso rdf:resource="&Governance;ISO_27000"/>
        <Governance:needsTechnicalRequirement rdf:resource="&Governance;Steering_Commitee_1"/>
    </owl:NamedIndividual>
    <owl:Axiom>
        <rdfs:comment>Active involvement and support from senior management and the Governing Board demonstrate the organization&apos;s commitment to IG. Their engagement helps allocate resources, make strategic decisions, and prioritize IG initiatives.</rdfs:comment>
        <owl:annotatedSource rdf:resource="&Governance;AC_1_1_5"/>
        <owl:annotatedTarget rdf:resource="&Governance;IG_Leadership_1"/>
        <owl:annotatedProperty rdf:resource="&Governance;needsTechnicalRequirement"/>
    </owl:Axiom>
    <owl:Axiom>
        <rdfs:comment>An IG Steering Committee, composed of representatives from different departments, ensures cross-functional collaboration and coordination in IG efforts. It provides oversight, direction, and decision-making for IG initiatives.</rdfs:comment>
        <owl:annotatedSource rdf:resource="&Governance;AC_1_1_5"/>
        <owl:annotatedTarget rdf:resource="&Governance;Steering_Commitee_1"/>
        <owl:annotatedProperty rdf:resource="&Governance;needsTechnicalRequirement"/>
    </owl:Axiom>
    <owl:Axiom>
        <rdfs:comment> A well-defined and comprehensive Information Governance (IG) strategic plan and policy framework outlines the principles, objectives, and guidelines for IG initiatives within the organization. It ensures a structured approach to IG implementation and decision-making.</rdfs:comment>
        <owl:annotatedSource rdf:resource="&Governance;AC_1_1_5"/>
        <owl:annotatedTarget rdf:resource="&Governance;IG_Strategic_Plan_1"/>
        <owl:annotatedProperty rdf:resource="&Governance;needsTechnicalRequirement"/>
    </owl:Axiom>
    


    <!-- http://www.semanticweb.org/IG/Governance#AC_1_2_3 -->

    <owl:NamedIndividual rdf:about="&Governance;AC_1_2_3">
        <rdf:type rdf:resource="&Governance;IG_Capability"/>
        <Governance:capabilityDescription>The RIM role is assigned</Governance:capabilityDescription>
        <Governance:inMaturityLevel rdf:resource="&Governance;3_Essential"/>
        <Governance:linkedToFramework rdf:resource="&Governance;ARMA_00"/>
        <Governance:needsTechnicalRequirement rdf:resource="&Governance;AccessControl_1"/>
        <Governance:hasGoal rdf:resource="&Governance;Accountability"/>
        <Governance:involvesArticle rdf:resource="&Governance;Article_24"/>
        <Governance:involvesArticle rdf:resource="&Governance;Article_32"/>
        <Governance:involvesArticle rdf:resource="&Governance;Article_39"/>
        <Governance:practicesDefinedInIso rdf:resource="&Governance;ISO_15489"/>
        <Governance:practicesDefinedInIso rdf:resource="&Governance;ISO_27000"/>
        <Governance:needsTechnicalRequirement rdf:resource="&Governance;Training_1"/>
    </owl:NamedIndividual>
    <owl:Axiom>
        <rdfs:comment>RIM personnel should receive proper training and have the necessary knowledge to fulfill their role effectively. This includes training on records management principles, legal requirements, privacy considerations, and technology usage.</rdfs:comment>
        <owl:annotatedSource rdf:resource="&Governance;AC_1_2_3"/>
        <owl:annotatedTarget rdf:resource="&Governance;Training_1"/>
        <owl:annotatedProperty rdf:resource="&Governance;needsTechnicalRequirement"/>
    </owl:Axiom>
    <owl:Axiom>
        <rdfs:comment>The individuals in the RIM role need access to the necessary tools and systems to carry out their responsibilities effectively. This includes access to records management software, document repositories, and other technology platforms that support RIM activities.</rdfs:comment>
        <owl:annotatedSource rdf:resource="&Governance;AC_1_2_3"/>
        <owl:annotatedTarget rdf:resource="&Governance;AccessControl_1"/>
        <owl:annotatedProperty rdf:resource="&Governance;needsTechnicalRequirement"/>
    </owl:Axiom>
    


    <!-- http://www.semanticweb.org/IG/Governance#AC_1_2_4 -->

    <owl:NamedIndividual rdf:about="&Governance;AC_1_2_4">
        <rdf:type rdf:resource="&Governance;IG_Capability"/>
        <Governance:capabilityDescription> A senior officer is appointed RM and responsible for the RMP.</Governance:capabilityDescription>
        <Governance:inMaturityLevel rdf:resource="&Governance;4_Proactive"/>
        <Governance:linkedToFramework rdf:resource="&Governance;ARMA_00"/>
        <Governance:needsTechnicalRequirement rdf:resource="&Governance;AccessControl_1"/>
        <Governance:hasGoal rdf:resource="&Governance;Accountability"/>
        <Governance:involvesArticle rdf:resource="&Governance;Article_32"/>
        <Governance:involvesArticle rdf:resource="&Governance;Article_5"/>
        <Governance:needsTechnicalRequirement rdf:resource="&Governance;Data_Retention_Policy_Dummy"/>
        <Governance:practicesDefinedInIso rdf:resource="&Governance;ISO_15489"/>
        <Governance:practicesDefinedInIso rdf:resource="&Governance;ISO_15939"/>
        <Governance:practicesDefinedInIso rdf:resource="&Governance;ISO_27001"/>
        <Governance:needsTechnicalRequirement rdf:resource="&Governance;Records_Information_Management_1"/>
    </owl:NamedIndividual>
    <owl:Axiom>
        <rdfs:comment> A systematic metadata management system enables accurate identification and management of records in accordance with RMP requirements.</rdfs:comment>
        <owl:annotatedSource rdf:resource="&Governance;AC_1_2_4"/>
        <owl:annotatedTarget rdf:resource="&Governance;Records_Information_Management_1"/>
        <owl:annotatedProperty rdf:resource="&Governance;needsTechnicalRequirement"/>
    </owl:Axiom>
    <owl:Axiom>
        <rdfs:comment>Implementing automated retention and disposition processes ensures that records are managed and disposed of in compliance with RMP requirements and legal obligations.</rdfs:comment>
        <owl:annotatedSource rdf:resource="&Governance;AC_1_2_4"/>
        <owl:annotatedTarget rdf:resource="&Governance;Data_Retention_Policy_Dummy"/>
        <owl:annotatedProperty rdf:resource="&Governance;needsTechnicalRequirement"/>
    </owl:Axiom>
    <owl:Axiom>
        <rdfs:comment>An effective Access Control system ensures that the senior officer appointed as the Records Manager (RM) has appropriate access rights and responsibilities for the Records Management Program (RMP), ensuring the integrity and security of recorded information.</rdfs:comment>
        <owl:annotatedSource rdf:resource="&Governance;AC_1_2_4"/>
        <owl:annotatedTarget rdf:resource="&Governance;AccessControl_1"/>
        <owl:annotatedProperty rdf:resource="&Governance;needsTechnicalRequirement"/>
    </owl:Axiom>
    


    <!-- http://www.semanticweb.org/IG/Governance#AC_1_2_5 -->

    <owl:NamedIndividual rdf:about="&Governance;AC_1_2_5">
        <rdf:type rdf:resource="&Governance;IG_Capability"/>
        <Governance:capabilityDescription>There is a Chief Information Governance Officer (CIGO) appointed.</Governance:capabilityDescription>
        <Governance:needsTechnicalRequirement rdf:resource="&Governance;AC_1_2_5"/>
        <Governance:linkedToFramework rdf:resource="&Governance;ARMA_00"/>
        <Governance:hasGoal rdf:resource="&Governance;Accountability"/>
        <Governance:involvesArticle rdf:resource="&Governance;Article_35"/>
        <Governance:involvesArticle rdf:resource="&Governance;Article_39"/>
        <Governance:involvesArticle rdf:resource="&Governance;Article_5"/>
        <Governance:needsTechnicalRequirement rdf:resource="&Governance;CIGO_1"/>
        <Governance:needsTechnicalRequirement rdf:resource="&Governance;DPO_1"/>
        <Governance:practicesDefinedInIso rdf:resource="&Governance;ISO_15489"/>
        <Governance:practicesDefinedInIso rdf:resource="&Governance;ISO_23081"/>
        <Governance:practicesDefinedInIso rdf:resource="&Governance;ISO_27001"/>
        <Governance:needsTechnicalRequirement rdf:resource="&Governance;Supervisor_Authority_1"/>
    </owl:NamedIndividual>
    <owl:Axiom>
        <rdfs:comment> GDPR Article 35 emphasizes the importance of consulting with data protection authorities when conducting data protection impact assessments, which may require collaboration led by the CIGO.</rdfs:comment>
        <owl:annotatedSource rdf:resource="&Governance;AC_1_2_5"/>
        <owl:annotatedTarget rdf:resource="&Governance;Supervisor_Authority_1"/>
        <owl:annotatedProperty rdf:resource="&Governance;needsTechnicalRequirement"/>
    </owl:Axiom>
    <owl:Axiom>
        <rdfs:comment>Clearly defining the role and responsibilities of the Chief Information Governance Officer (CIGO) is essential for effective leadership and management of information governance initiatives. The CIGO plays a central role in developing and implementing IG strategies, policies, and processes.

Effective communication and collaboration skills are vital for the CIGO to engage with senior leadership, departments, and external stakeholders. Collaboration ensures that IG goals align with organizational objectives and that IG initiatives are integrated into business processes.</rdfs:comment>
        <owl:annotatedSource rdf:resource="&Governance;AC_1_2_5"/>
        <owl:annotatedTarget rdf:resource="&Governance;CIGO_1"/>
        <owl:annotatedProperty rdf:resource="&Governance;needsTechnicalRequirement"/>
    </owl:Axiom>
    <owl:Axiom>
        <rdfs:comment>GDPR Article 39 emphasizes the role of the Data Protection Officer (DPO) in an organization. While the CIGO is not explicitly mentioned in GDPR, the DPO&apos;s responsibilities and expertise are relevant to the CIGO&apos;s role in overseeing data protection and privacy aspects.</rdfs:comment>
        <owl:annotatedSource rdf:resource="&Governance;AC_1_2_5"/>
        <owl:annotatedTarget rdf:resource="&Governance;DPO_1"/>
        <owl:annotatedProperty rdf:resource="&Governance;needsTechnicalRequirement"/>
    </owl:Axiom>
    


    <!-- http://www.semanticweb.org/IG/Governance#AC_1_3_3 -->

    <owl:NamedIndividual rdf:about="&Governance;AC_1_3_3">
        <rdf:type rdf:resource="&Governance;IG_Capability"/>
        <Governance:capabilityDescription>Electronic records are part of  The RMP.</Governance:capabilityDescription>
        <Governance:inMaturityLevel rdf:resource="&Governance;3_Essential"/>
        <Governance:linkedToFramework rdf:resource="&Governance;ARMA_00"/>
        <Governance:needsTechnicalRequirement rdf:resource="&Governance;AccessControl_1"/>
        <Governance:hasGoal rdf:resource="&Governance;Accountability"/>
        <Governance:involvesArticle rdf:resource="&Governance;Article_30"/>
        <Governance:involvesArticle rdf:resource="&Governance;Article_32"/>
        <Governance:involvesArticle rdf:resource="&Governance;Article_5"/>
        <Governance:needsTechnicalRequirement rdf:resource="&Governance;Audit_1"/>
        <Governance:needsTechnicalRequirement rdf:resource="&Governance;Data_Retention_Policy_Dummy"/>
        <Governance:needsTechnicalRequirement rdf:resource="&Governance;ERM_1"/>
        <Governance:practicesDefinedInIso rdf:resource="&Governance;ISO_15489"/>
        <Governance:practicesDefinedInIso rdf:resource="&Governance;ISO_17000"/>
    </owl:NamedIndividual>
    <owl:Axiom>
        <rdfs:comment>An ERM (Electronic Records Management) enables efficient management of electronic records by facilitating the capture, storage, processing, and access to these records. Also the metadata defining and capturing is done by the Records Management</rdfs:comment>
        <owl:annotatedSource rdf:resource="&Governance;AC_1_3_3"/>
        <owl:annotatedTarget rdf:resource="&Governance;ERM_1"/>
        <owl:annotatedProperty rdf:resource="&Governance;needsTechnicalRequirement"/>
    </owl:Axiom>
    <owl:Axiom>
        <rdfs:comment>Access control and audit trails ensure the security and traceability of electronic records, preventing unauthorized access and monitoring processing activities.</rdfs:comment>
        <owl:annotatedSource rdf:resource="&Governance;AC_1_3_3"/>
        <owl:annotatedTarget rdf:resource="&Governance;AccessControl_1"/>
        <owl:annotatedProperty rdf:resource="&Governance;needsTechnicalRequirement"/>
    </owl:Axiom>
    <owl:Axiom>
        <rdfs:comment>Clear and actionable guidelines for the retention of electronic records ensure compliance with retention periods and processing purposes.</rdfs:comment>
        <owl:annotatedSource rdf:resource="&Governance;AC_1_3_3"/>
        <owl:annotatedTarget rdf:resource="&Governance;Data_Retention_Policy_Dummy"/>
        <owl:annotatedProperty rdf:resource="&Governance;needsTechnicalRequirement"/>
    </owl:Axiom>
    <owl:Axiom>
        <rdfs:comment>Access control and audit trails ensure the security and traceability of electronic records, preventing unauthorized access and monitoring processing activities.</rdfs:comment>
        <owl:annotatedSource rdf:resource="&Governance;AC_1_3_3"/>
        <owl:annotatedTarget rdf:resource="&Governance;Audit_1"/>
        <owl:annotatedProperty rdf:resource="&Governance;needsTechnicalRequirement"/>
    </owl:Axiom>
    


    <!-- http://www.semanticweb.org/IG/Governance#AC_1_3_4 -->

    <owl:NamedIndividual rdf:about="&Governance;AC_1_3_4">
        <rdf:type rdf:resource="&Governance;IG_Capability"/>
        <Governance:capabilityDescription>RMP is an element of the IGP.</Governance:capabilityDescription>
        <Governance:inMaturityLevel rdf:resource="&Governance;4_Proactive"/>
        <Governance:linkedToFramework rdf:resource="&Governance;ARMA_00"/>
        <Governance:hasGoal rdf:resource="&Governance;Accountability"/>
        <Governance:involvesArticle rdf:resource="&Governance;Article_24"/>
        <Governance:involvesArticle rdf:resource="&Governance;Article_32"/>
        <Governance:involvesArticle rdf:resource="&Governance;Article_5"/>
        <Governance:needsTechnicalRequirement rdf:resource="&Governance;IG_Programm_1"/>
        <Governance:practicesDefinedInIso rdf:resource="&Governance;ISO_15489"/>
        <Governance:practicesDefinedInIso rdf:resource="&Governance;ISO_23081"/>
        <Governance:needsTechnicalRequirement rdf:resource="&Governance;Stakeholder_1"/>
    </owl:NamedIndividual>
    <owl:Axiom>
        <rdfs:comment>The Information Governance Program should be well-documented, outlining its objectives, scope, policies, procedures, and key components such as the Records Management Program (RMP). This documentation provides a clear roadmap for the implementation and management of the IGP.</rdfs:comment>
        <owl:annotatedSource rdf:resource="&Governance;AC_1_3_4"/>
        <owl:annotatedTarget rdf:resource="&Governance;IG_Programm_1"/>
        <owl:annotatedProperty rdf:resource="&Governance;needsTechnicalRequirement"/>
    </owl:Axiom>
    <owl:Axiom>
        <rdfs:comment>Collaboration among various stakeholders, including legal, compliance, IT, and business units, is essential for the successful integration of the RMP within the IGP. This collaboration ensures that records management practices align with organizational goals and regulatory requirements.</rdfs:comment>
        <owl:annotatedSource rdf:resource="&Governance;AC_1_3_4"/>
        <owl:annotatedTarget rdf:resource="&Governance;Stakeholder_1"/>
        <owl:annotatedProperty rdf:resource="&Governance;needsTechnicalRequirement"/>
    </owl:Axiom>
    


    <!-- http://www.semanticweb.org/IG/Governance#AC_1_3_5 -->

    <owl:NamedIndividual rdf:about="&Governance;AC_1_3_5">
        <rdf:type rdf:resource="&Governance;IG_Capability"/>
        <Governance:capabilityDescription>CIGO and RM are member of the governing body.</Governance:capabilityDescription>
        <Governance:inMaturityLevel rdf:resource="&Governance;5_Transformational"/>
        <Governance:linkedToFramework rdf:resource="&Governance;ARMA_00"/>
        <Governance:hasGoal rdf:resource="&Governance;Accountability"/>
        <Governance:involvesArticle rdf:resource="&Governance;Article_38"/>
        <Governance:involvesArticle rdf:resource="&Governance;Article_39"/>
        <Governance:involvesArticle rdf:resource="&Governance;Article_5"/>
        <Governance:needsTechnicalRequirement rdf:resource="&Governance;CIGO_1"/>
        <Governance:practicesDefinedInIso rdf:resource="&Governance;ISO_15489"/>
        <Governance:needsTechnicalRequirement rdf:resource="&Governance;Reporting_And_Analysis_System_1"/>
        <Governance:needsTechnicalRequirement rdf:resource="&Governance;Senior_Records_Officer_1"/>
    </owl:NamedIndividual>
    <owl:Axiom>
        <rdfs:comment>The reporting structure within the organization must clearly establish the link between the CIGO, RM, and the governing body. This ensures that information governance issues are properly communicated, managed, and escalated as needed.</rdfs:comment>
        <owl:annotatedSource rdf:resource="&Governance;AC_1_3_5"/>
        <owl:annotatedTarget rdf:resource="&Governance;Reporting_And_Analysis_System_1"/>
        <owl:annotatedProperty rdf:resource="&Governance;needsTechnicalRequirement"/>
    </owl:Axiom>
    <owl:Axiom>
        <rdfs:comment> The governing body of the organization, such as a board of directors or executive management, must have a structure that includes roles for the Chief Information Governance Officer (CIGO) and the Records Manager (RM). This ensures that these key positions are formally integrated into the leadership and decision-making processes of the organization.</rdfs:comment>
        <owl:annotatedSource rdf:resource="&Governance;AC_1_3_5"/>
        <owl:annotatedTarget rdf:resource="&Governance;Senior_Records_Officer_1"/>
        <owl:annotatedProperty rdf:resource="&Governance;needsTechnicalRequirement"/>
    </owl:Axiom>
    <owl:Axiom>
        <rdfs:comment> The governing body of the organization, such as a board of directors or executive management, must have a structure that includes roles for the Chief Information Governance Officer (CIGO) and the Records Manager (RM). This ensures that these key positions are formally integrated into the leadership and decision-making processes of the organization.</rdfs:comment>
        <owl:annotatedSource rdf:resource="&Governance;AC_1_3_5"/>
        <owl:annotatedTarget rdf:resource="&Governance;CIGO_1"/>
        <owl:annotatedProperty rdf:resource="&Governance;needsTechnicalRequirement"/>
    </owl:Axiom>
    


    <!-- http://www.semanticweb.org/IG/Governance#AC_1_4_3 -->

    <owl:NamedIndividual rdf:about="&Governance;AC_1_4_3">
        <rdf:type rdf:resource="&Governance;IG_Capability"/>
        <Governance:capabilityDescription> RIM is engaged with other officers.   </Governance:capabilityDescription>
        <Governance:inMaturityLevel rdf:resource="&Governance;3_Essential"/>
        <Governance:linkedToFramework rdf:resource="&Governance;ARMA_00"/>
        <Governance:hasGoal rdf:resource="&Governance;Accountability"/>
        <Governance:involvesArticle rdf:resource="&Governance;Article_24"/>
        <Governance:involvesArticle rdf:resource="&Governance;Article_32"/>
        <Governance:involvesArticle rdf:resource="&Governance;Article_5"/>
        <Governance:needsTechnicalRequirement rdf:resource="&Governance;Collaboration_Tools_1"/>
        <Governance:needsTechnicalRequirement rdf:resource="&Governance;Data_Sharing_Protocols_1"/>
        <Governance:practicesDefinedInIso rdf:resource="&Governance;ISO_15489"/>
        <Governance:needsTechnicalRequirement rdf:resource="&Governance;Workflow_Tools_1"/>
    </owl:NamedIndividual>
    <owl:Axiom>
        <rdfs:comment>Implement collaboration tools and platforms that enable seamless communication and interaction between Records and Information Management (RIM) officers and other key officers across various departments. These tools facilitate the exchange of information, decision-making, and collaboration on records management initiatives.</rdfs:comment>
        <owl:annotatedSource rdf:resource="&Governance;AC_1_4_3"/>
        <owl:annotatedTarget rdf:resource="&Governance;Collaboration_Tools_1"/>
        <owl:annotatedProperty rdf:resource="&Governance;needsTechnicalRequirement"/>
    </owl:Axiom>
    <owl:Axiom>
        <rdfs:comment>Establish clear protocols and guidelines for sharing records and information between different departments or officers. These protocols should address data formats, access controls, security measures, and privacy considerations to ensure proper handling and sharing of information.</rdfs:comment>
        <owl:annotatedSource rdf:resource="&Governance;AC_1_4_3"/>
        <owl:annotatedTarget rdf:resource="&Governance;Data_Sharing_Protocols_1"/>
        <owl:annotatedProperty rdf:resource="&Governance;needsTechnicalRequirement"/>
    </owl:Axiom>
    <owl:Axiom>
        <rdfs:comment>Integrating RIM officers into cross-functional workflows helps ensure that records management requirements are met throughout the information lifecycle, enhancing compliance, transparency, and accountability.</rdfs:comment>
        <owl:annotatedSource rdf:resource="&Governance;AC_1_4_3"/>
        <owl:annotatedTarget rdf:resource="&Governance;Workflow_Tools_1"/>
        <owl:annotatedProperty rdf:resource="&Governance;needsTechnicalRequirement"/>
    </owl:Axiom>
    


    <!-- http://www.semanticweb.org/IG/Governance#AC_1_4_4 -->

    <owl:NamedIndividual rdf:about="&Governance;AC_1_4_4">
        <rdf:type rdf:resource="&Governance;IG_Capability"/>
        <Governance:capabilityDescription> Disposition policies and RM-related issues are reviewed periodically.</Governance:capabilityDescription>
        <Governance:inMaturityLevel rdf:resource="&Governance;4_Proactive"/>
        <Governance:linkedToFramework rdf:resource="&Governance;ARMA_00"/>
        <Governance:hasGoal rdf:resource="&Governance;Accountability"/>
        <Governance:involvesArticle rdf:resource="&Governance;Article_24"/>
        <Governance:involvesArticle rdf:resource="&Governance;Article_32"/>
        <Governance:involvesArticle rdf:resource="&Governance;Article_5"/>
        <Governance:needsTechnicalRequirement rdf:resource="&Governance;Disposition_Policies_And_Procedures_1"/>
        <Governance:practicesDefinedInIso rdf:resource="&Governance;ISO_15489"/>
        <Governance:practicesDefinedInIso rdf:resource="&Governance;ISO_23081"/>
        <Governance:needsTechnicalRequirement rdf:resource="&Governance;Review_Cyles_1"/>
        <Governance:needsTechnicalRequirement rdf:resource="&Governance;Stakeholder_1"/>
        <Governance:needsTechnicalRequirement rdf:resource="&Governance;Workflow_Tools_1"/>
    </owl:NamedIndividual>
    <owl:Axiom>
        <rdfs:comment>Utilizing technology solutions, such as records management software and workflow tools, can streamline the review process for disposition policies and RM-related issues. These tools facilitate document tracking, collaboration, and reporting.</rdfs:comment>
        <owl:annotatedSource rdf:resource="&Governance;AC_1_4_4"/>
        <owl:annotatedTarget rdf:resource="&Governance;Workflow_Tools_1"/>
        <owl:annotatedProperty rdf:resource="&Governance;needsTechnicalRequirement"/>
    </owl:Axiom>
    <owl:Axiom>
        <rdfs:comment>Well-documented disposition policies and procedures should be established to guide the periodic review of records management (RM)-related issues and disposition practices. These documents outline the criteria and processes for reviewing records and making decisions about their retention or disposal.</rdfs:comment>
        <owl:annotatedSource rdf:resource="&Governance;AC_1_4_4"/>
        <owl:annotatedTarget rdf:resource="&Governance;Disposition_Policies_And_Procedures_1"/>
        <owl:annotatedProperty rdf:resource="&Governance;needsTechnicalRequirement"/>
    </owl:Axiom>
    <owl:Axiom>
        <rdfs:comment>Collaboration among stakeholders, including legal, compliance, business units, and records management professionals, is essential for the meaningful review of disposition policies and RM-related issues. Stakeholders should actively participate in the review process.</rdfs:comment>
        <owl:annotatedSource rdf:resource="&Governance;AC_1_4_4"/>
        <owl:annotatedTarget rdf:resource="&Governance;Stakeholder_1"/>
        <owl:annotatedProperty rdf:resource="&Governance;needsTechnicalRequirement"/>
    </owl:Axiom>
    <owl:Axiom>
        <rdfs:comment>Establishing regular review cycles is essential to ensure that disposition policies and RM-related issues are systematically assessed and updated. This involves defining the frequency of reviews and establishing a clear schedule for periodic evaluations.</rdfs:comment>
        <owl:annotatedSource rdf:resource="&Governance;AC_1_4_4"/>
        <owl:annotatedTarget rdf:resource="&Governance;Review_Cyles_1"/>
        <owl:annotatedProperty rdf:resource="&Governance;needsTechnicalRequirement"/>
    </owl:Axiom>
    


    <!-- http://www.semanticweb.org/IG/Governance#AC_1_4_5 -->

    <owl:NamedIndividual rdf:about="&Governance;AC_1_4_5">
        <rdf:type rdf:resource="&Governance;IG_Capability"/>
        <Governance:capabilityDescription>The accountability goals are met.</Governance:capabilityDescription>
        <Governance:inMaturityLevel rdf:resource="&Governance;5_Transformational"/>
        <Governance:linkedToFramework rdf:resource="&Governance;ARMA_00"/>
        <Governance:needsTechnicalRequirement rdf:resource="&Governance;AccessControl_1"/>
        <Governance:hasGoal rdf:resource="&Governance;Accountability"/>
        <Governance:involvesArticle rdf:resource="&Governance;Article_30"/>
        <Governance:involvesArticle rdf:resource="&Governance;Article_32"/>
        <Governance:involvesArticle rdf:resource="&Governance;Article_5"/>
        <Governance:needsTechnicalRequirement rdf:resource="&Governance;Audit_1"/>
        <Governance:needsTechnicalRequirement rdf:resource="&Governance;Data_Mapping_And_Classification_System_1"/>
        <Governance:practicesDefinedInIso rdf:resource="&Governance;ISO_27001"/>
    </owl:NamedIndividual>
    <owl:Axiom>
        <rdfs:comment>Implementing strong access controls and authentication mechanisms ensures that only authorized personnel can access and manipulate data, contributing to accountability and data protection.</rdfs:comment>
        <owl:annotatedSource rdf:resource="&Governance;AC_1_4_5"/>
        <owl:annotatedTarget rdf:resource="&Governance;AccessControl_1"/>
        <owl:annotatedProperty rdf:resource="&Governance;needsTechnicalRequirement"/>
    </owl:Axiom>
    <owl:Axiom>
        <rdfs:comment>An audit trail provides a transparent record of data processing activities and helps in meeting accountability requirements.</rdfs:comment>
        <owl:annotatedSource rdf:resource="&Governance;AC_1_4_5"/>
        <owl:annotatedTarget rdf:resource="&Governance;Audit_1"/>
        <owl:annotatedProperty rdf:resource="&Governance;needsTechnicalRequirement"/>
    </owl:Axiom>
    <owl:Axiom>
        <rdfs:comment>A robust data mapping and classification system is crucial for identifying, categorizing, and labeling data according to its sensitivity and importance, which is essential for meeting accountability goals.</rdfs:comment>
        <owl:annotatedSource rdf:resource="&Governance;AC_1_4_5"/>
        <owl:annotatedTarget rdf:resource="&Governance;Data_Mapping_And_Classification_System_1"/>
        <owl:annotatedProperty rdf:resource="&Governance;needsTechnicalRequirement"/>
    </owl:Axiom>
    


    <!-- http://www.semanticweb.org/IG/Governance#AC_1_5_3 -->

    <owl:NamedIndividual rdf:about="&Governance;AC_1_5_3">
        <rdf:type rdf:resource="&Governance;IG_Capability"/>
        <Governance:capabilityDescription>IG drives information-driven processes.</Governance:capabilityDescription>
        <Governance:inMaturityLevel rdf:resource="&Governance;3_Essential"/>
        <Governance:linkedToFramework rdf:resource="&Governance;ARMA_00"/>
        <Governance:hasGoal rdf:resource="&Governance;Accountability"/>
        <Governance:involvesArticle rdf:resource="&Governance;Article_24"/>
        <Governance:involvesArticle rdf:resource="&Governance;Article_30"/>
        <Governance:involvesArticle rdf:resource="&Governance;Article_32"/>
        <Governance:involvesArticle rdf:resource="&Governance;Article_5"/>
        <Governance:involvesArticle rdf:resource="&Governance;Article_6"/>
        <Governance:needsTechnicalRequirement rdf:resource="&Governance;Database_Management_System_1"/>
        <Governance:practicesDefinedInIso rdf:resource="&Governance;ISO_14271"/>
        <Governance:practicesDefinedInIso rdf:resource="&Governance;ISO_15489"/>
        <Governance:practicesDefinedInIso rdf:resource="&Governance;ISO_15939"/>
        <Governance:practicesDefinedInIso rdf:resource="&Governance;ISO_23081"/>
        <Governance:needsTechnicalRequirement rdf:resource="&Governance;Records_Information_Management_1"/>
        <Governance:needsTechnicalRequirement rdf:resource="&Governance;Reporting_And_Analysis_System_1"/>
        <Governance:needsTechnicalRequirement rdf:resource="&Governance;Workflow_Tools_1"/>
    </owl:NamedIndividual>
    <owl:Axiom>
        <rdfs:comment>Workflow tools enable the automation and control of information-driven processes, enhancing efficiency and consistency.</rdfs:comment>
        <owl:annotatedSource rdf:resource="&Governance;AC_1_5_3"/>
        <owl:annotatedTarget rdf:resource="&Governance;Workflow_Tools_1"/>
        <owl:annotatedProperty rdf:resource="&Governance;needsTechnicalRequirement"/>
    </owl:Axiom>
    <owl:Axiom>
        <rdfs:comment>An integrated reporting and analytics system enables monitoring and assessment of information-driven processes for continuous improvement.</rdfs:comment>
        <owl:annotatedSource rdf:resource="&Governance;AC_1_5_3"/>
        <owl:annotatedTarget rdf:resource="&Governance;Reporting_And_Analysis_System_1"/>
        <owl:annotatedProperty rdf:resource="&Governance;needsTechnicalRequirement"/>
    </owl:Axiom>
    <owl:Axiom>
        <rdfs:comment>RIM is responsible for the management and maintenance of metadata associated with records. Metadata allows for the identification, classification, and retrieval of documents and data, enhancing the efficiency of information-driven processes.</rdfs:comment>
        <owl:annotatedSource rdf:resource="&Governance;AC_1_5_3"/>
        <owl:annotatedTarget rdf:resource="&Governance;Records_Information_Management_1"/>
        <owl:annotatedProperty rdf:resource="&Governance;needsTechnicalRequirement"/>
    </owl:Axiom>
    <owl:Axiom>
        <rdfs:comment>A DMS enables efficient management, storage, retrieval, and sharing of documents and data, which is essential for information-driven processes.</rdfs:comment>
        <owl:annotatedSource rdf:resource="&Governance;AC_1_5_3"/>
        <owl:annotatedTarget rdf:resource="&Governance;Database_Management_System_1"/>
        <owl:annotatedProperty rdf:resource="&Governance;needsTechnicalRequirement"/>
    </owl:Axiom>
    


    <!-- http://www.semanticweb.org/IG/Governance#AC_1_5_5 -->

    <owl:NamedIndividual rdf:about="&Governance;AC_1_5_5">
        <rdf:type rdf:resource="&Governance;IG_Capability"/>
        <Governance:capabilityDescription>The accountability goals are periodically reviewed and revised.</Governance:capabilityDescription>
        <Governance:inMaturityLevel rdf:resource="&Governance;5_Transformational"/>
        <Governance:linkedToFramework rdf:resource="&Governance;ARMA_00"/>
        <Governance:hasGoal rdf:resource="&Governance;Accountability"/>
        <Governance:involvesArticle rdf:resource="&Governance;Article_24"/>
        <Governance:involvesArticle rdf:resource="&Governance;Article_39"/>
        <Governance:involvesArticle rdf:resource="&Governance;Article_5"/>
        <Governance:needsTechnicalRequirement rdf:resource="&Governance;IG_Programm_1"/>
        <Governance:practicesDefinedInIso rdf:resource="&Governance;ISO_15489"/>
        <Governance:practicesDefinedInIso rdf:resource="&Governance;ISO_27000"/>
        <Governance:needsTechnicalRequirement rdf:resource="&Governance;Review_Cyles_1"/>
        <Governance:needsTechnicalRequirement rdf:resource="&Governance;Stakeholder_1"/>
    </owl:NamedIndividual>
    <owl:Axiom>
        <rdfs:comment>A formal process for regular review and revision of accountability goals should be in place. This includes predefined intervals for assessing the effectiveness and relevance of established goals and making updates as necessary.</rdfs:comment>
        <owl:annotatedSource rdf:resource="&Governance;AC_1_5_5"/>
        <owl:annotatedTarget rdf:resource="&Governance;Review_Cyles_1"/>
        <owl:annotatedProperty rdf:resource="&Governance;needsTechnicalRequirement"/>
    </owl:Axiom>
    <owl:Axiom>
        <rdfs:comment>Clear and well-documented accountability goals must be established within the organization&apos;s Information Governance framework. These goals define the organization&apos;s commitments to accountability, data protection, and compliance.</rdfs:comment>
        <owl:annotatedSource rdf:resource="&Governance;AC_1_5_5"/>
        <owl:annotatedTarget rdf:resource="&Governance;IG_Programm_1"/>
        <owl:annotatedProperty rdf:resource="&Governance;needsTechnicalRequirement"/>
    </owl:Axiom>
    <owl:Axiom>
        <rdfs:comment>Engaging relevant stakeholders, including senior management, legal, and data protection officers, in the review and revision process is crucial. Their input ensures that accountability goals reflect the organization&apos;s strategic direction and compliance requirements.</rdfs:comment>
        <owl:annotatedSource rdf:resource="&Governance;AC_1_5_5"/>
        <owl:annotatedTarget rdf:resource="&Governance;Stakeholder_1"/>
        <owl:annotatedProperty rdf:resource="&Governance;needsTechnicalRequirement"/>
    </owl:Axiom>
    


    <!-- http://www.semanticweb.org/IG/Governance#AC_1_6_3 -->

    <owl:NamedIndividual rdf:about="&Governance;AC_1_6_3">
        <rdf:type rdf:resource="&Governance;IG_Capability"/>
        <Governance:capabilityDescription> Accountabiliy goals are defined.</Governance:capabilityDescription>
        <Governance:inMaturityLevel rdf:resource="&Governance;3_Essential"/>
        <Governance:linkedToFramework rdf:resource="&Governance;ARMA_00"/>
        <Governance:hasGoal rdf:resource="&Governance;Accountability"/>
        <Governance:involvesArticle rdf:resource="&Governance;Article_24"/>
        <Governance:involvesArticle rdf:resource="&Governance;Article_30"/>
        <Governance:involvesArticle rdf:resource="&Governance;Article_32"/>
        <Governance:needsTechnicalRequirement rdf:resource="&Governance;Data_Mapping_And_Classification_System_1"/>
        <Governance:needsTechnicalRequirement rdf:resource="&Governance;IG_Policy_1"/>
        <Governance:practicesDefinedInIso rdf:resource="&Governance;ISO_14271"/>
        <Governance:practicesDefinedInIso rdf:resource="&Governance;ISO_15939"/>
        <Governance:practicesDefinedInIso rdf:resource="&Governance;ISO_23081"/>
        <Governance:practicesDefinedInIso rdf:resource="&Governance;ISO_27000"/>
    </owl:NamedIndividual>
    <owl:Axiom>
        <rdfs:comment>Understanding what data is processed, where it&apos;s stored, and who accesses it is essential for setting effective accountability goals. Data mapping helps identify risks and assess compliance.</rdfs:comment>
        <owl:annotatedSource rdf:resource="&Governance;AC_1_6_3"/>
        <owl:annotatedTarget rdf:resource="&Governance;Data_Mapping_And_Classification_System_1"/>
        <owl:annotatedProperty rdf:resource="&Governance;needsTechnicalRequirement"/>
    </owl:Axiom>
    <owl:Axiom>
        <rdfs:comment>Well-documented policies and procedures define the specific accountability goals, set expectations, and provide a reference for implementation and monitoring. These documents ensure a consistent understanding and execution of accountability across the organization.</rdfs:comment>
        <owl:annotatedSource rdf:resource="&Governance;AC_1_6_3"/>
        <owl:annotatedTarget rdf:resource="&Governance;IG_Policy_1"/>
        <owl:annotatedProperty rdf:resource="&Governance;needsTechnicalRequirement"/>
    </owl:Axiom>
    


    <!-- http://www.semanticweb.org/IG/Governance#ARMA_00 -->

    <owl:NamedIndividual rdf:about="&Governance;ARMA_00">
        <rdf:type rdf:resource="&Governance;Framework"/>
    </owl:NamedIndividual>
    


    <!-- http://www.semanticweb.org/IG/Governance#AccessControl_1 -->

    <owl:NamedIndividual rdf:about="&Governance;AccessControl_1">
        <rdf:type rdf:resource="&Governance;AccessControl"/>
        <Governance:involvesArticle rdf:resource="&Governance;Article_24"/>
        <Governance:involvesArticle rdf:resource="&Governance;Article_30"/>
        <Governance:involvesArticle rdf:resource="&Governance;Article_32"/>
        <Governance:involvesArticle rdf:resource="&Governance;Article_35"/>
        <Governance:involvesArticle rdf:resource="&Governance;Article_5"/>
        <Governance:involvesArticle rdf:resource="&Governance;Article_6"/>
        <Governance:uses rdf:resource="&Governance;Digital_Signatures_And_Timestamps_1"/>
        <Governance:canBeInvolvedWith rdf:resource="&Governance;Disposition_Policies_And_Procedures_1"/>
        <Governance:canBeInvolvedWith rdf:resource="&Governance;Document_Management_System_1"/>
        <Governance:practicesDefinedInIso rdf:resource="&Governance;ISO_14271"/>
        <Governance:practicesDefinedInIso rdf:resource="&Governance;ISO_15489"/>
        <Governance:practicesDefinedInIso rdf:resource="&Governance;ISO_27000"/>
        <Governance:practicesDefinedInIso rdf:resource="&Governance;ISO_27001"/>
    </owl:NamedIndividual>
    <owl:Axiom>
        <rdfs:comment>The Access Control subcategory within the Security department ensures that data is accessible only to authorized personnel. Disposition policies and procedures play a role in access control by ensuring that data is appropriately retained and deleted, preventing unauthorized access to outdated or unnecessary information.</rdfs:comment>
        <owl:annotatedSource rdf:resource="&Governance;AccessControl_1"/>
        <owl:annotatedTarget rdf:resource="&Governance;Disposition_Policies_And_Procedures_1"/>
        <owl:annotatedProperty rdf:resource="&Governance;canBeInvolvedWith"/>
    </owl:Axiom>
    <owl:Axiom>
        <rdfs:comment>The Access Control subcategory could use the system to control access to sensitive documents, ensuring that only authorized personnel can view, edit, or modify certain documents.</rdfs:comment>
        <owl:annotatedSource rdf:resource="&Governance;AccessControl_1"/>
        <owl:annotatedTarget rdf:resource="&Governance;Document_Management_System_1"/>
        <owl:annotatedProperty rdf:resource="&Governance;canBeInvolvedWith"/>
    </owl:Axiom>
    <owl:Axiom>
        <rdfs:comment>The Access Control subcategory within the Security department uses &quot;Digital Signatures &amp; Timestamps&quot; as part of its security measures. Digital signatures and timestamps are employed to ensure the integrity of access control mechanisms and authentication processes. They help validate the legitimacy of access requests and actions taken, providing an added layer of security and accountability in controlling data and system access.</rdfs:comment>
        <owl:annotatedSource rdf:resource="&Governance;AccessControl_1"/>
        <owl:annotatedTarget rdf:resource="&Governance;Digital_Signatures_And_Timestamps_1"/>
        <owl:annotatedProperty rdf:resource="&Governance;uses"/>
    </owl:Axiom>
    


    <!-- http://www.semanticweb.org/IG/Governance#Accountability -->

    <owl:NamedIndividual rdf:about="&Governance;Accountability">
        <rdf:type rdf:resource="&Governance;Goal"/>
    </owl:NamedIndividual>
    


    <!-- http://www.semanticweb.org/IG/Governance#Analytics_1 -->

    <owl:NamedIndividual rdf:about="&Governance;Analytics_1">
        <rdf:type rdf:resource="&Governance;Analytics"/>
        <Governance:involvesArticle rdf:resource="&Governance;Article_32"/>
        <Governance:involvesArticle rdf:resource="&Governance;Article_5"/>
        <Governance:practicesDefinedInIso rdf:resource="&Governance;ISO_15939"/>
        <Governance:practicesDefinedInIso rdf:resource="&Governance;ISO_17000"/>
        <Governance:practicesDefinedInIso rdf:resource="&Governance;ISO_27000"/>
        <Governance:practicesDefinedInIso rdf:resource="&Governance;ISO_27001"/>
        <Governance:practicesDefinedInIso rdf:resource="&Governance;ISO_27002"/>
    </owl:NamedIndividual>
    


    <!-- http://www.semanticweb.org/IG/Governance#Archieving_1 -->

    <owl:NamedIndividual rdf:about="&Governance;Archieving_1">
        <rdf:type rdf:resource="&Governance;Archieving"/>
        <Governance:involvesArticle rdf:resource="&Governance;Article_17"/>
        <Governance:involvesArticle rdf:resource="&Governance;Article_5"/>
        <Governance:practicesDefinedInIso rdf:resource="&Governance;ISO_15489"/>
        <Governance:practicesDefinedInIso rdf:resource="&Governance;ISO_27001"/>
    </owl:NamedIndividual>
    


    <!-- http://www.semanticweb.org/IG/Governance#Article_12 -->

    <owl:NamedIndividual rdf:about="&Governance;Article_12">
        <rdf:type rdf:resource="&Governance;GDPR"/>
    </owl:NamedIndividual>
    


    <!-- http://www.semanticweb.org/IG/Governance#Article_15 -->

    <owl:NamedIndividual rdf:about="&Governance;Article_15">
        <rdf:type rdf:resource="&Governance;GDPR"/>
    </owl:NamedIndividual>
    


    <!-- http://www.semanticweb.org/IG/Governance#Article_17 -->

    <owl:NamedIndividual rdf:about="&Governance;Article_17">
        <rdf:type rdf:resource="&Governance;GDPR"/>
    </owl:NamedIndividual>
    


    <!-- http://www.semanticweb.org/IG/Governance#Article_20 -->

    <owl:NamedIndividual rdf:about="&Governance;Article_20">
        <rdf:type rdf:resource="&Governance;GDPR"/>
    </owl:NamedIndividual>
    


    <!-- http://www.semanticweb.org/IG/Governance#Article_24 -->

    <owl:NamedIndividual rdf:about="&Governance;Article_24">
        <rdf:type rdf:resource="&Governance;GDPR"/>
    </owl:NamedIndividual>
    


    <!-- http://www.semanticweb.org/IG/Governance#Article_25 -->

    <owl:NamedIndividual rdf:about="&Governance;Article_25">
        <rdf:type rdf:resource="&Governance;GDPR"/>
    </owl:NamedIndividual>
    


    <!-- http://www.semanticweb.org/IG/Governance#Article_28 -->

    <owl:NamedIndividual rdf:about="&Governance;Article_28">
        <rdf:type rdf:resource="&Governance;GDPR"/>
    </owl:NamedIndividual>
    


    <!-- http://www.semanticweb.org/IG/Governance#Article_30 -->

    <owl:NamedIndividual rdf:about="&Governance;Article_30">
        <rdf:type rdf:resource="&Governance;GDPR"/>
    </owl:NamedIndividual>
    


    <!-- http://www.semanticweb.org/IG/Governance#Article_32 -->

    <owl:NamedIndividual rdf:about="&Governance;Article_32">
        <rdf:type rdf:resource="&Governance;GDPR"/>
    </owl:NamedIndividual>
    


    <!-- http://www.semanticweb.org/IG/Governance#Article_33 -->

    <owl:NamedIndividual rdf:about="&Governance;Article_33">
        <rdf:type rdf:resource="&Governance;GDPR"/>
    </owl:NamedIndividual>
    


    <!-- http://www.semanticweb.org/IG/Governance#Article_34 -->

    <owl:NamedIndividual rdf:about="&Governance;Article_34">
        <rdf:type rdf:resource="&Governance;GDPR"/>
    </owl:NamedIndividual>
    


    <!-- http://www.semanticweb.org/IG/Governance#Article_35 -->

    <owl:NamedIndividual rdf:about="&Governance;Article_35">
        <rdf:type rdf:resource="&Governance;GDPR"/>
    </owl:NamedIndividual>
    


    <!-- http://www.semanticweb.org/IG/Governance#Article_37 -->

    <owl:NamedIndividual rdf:about="&Governance;Article_37">
        <rdf:type rdf:resource="&Governance;GDPR"/>
    </owl:NamedIndividual>
    


    <!-- http://www.semanticweb.org/IG/Governance#Article_38 -->

    <owl:NamedIndividual rdf:about="&Governance;Article_38">
        <rdf:type rdf:resource="&Governance;GDPR"/>
    </owl:NamedIndividual>
    


    <!-- http://www.semanticweb.org/IG/Governance#Article_39 -->

    <owl:NamedIndividual rdf:about="&Governance;Article_39">
        <rdf:type rdf:resource="&Governance;GDPR"/>
    </owl:NamedIndividual>
    


    <!-- http://www.semanticweb.org/IG/Governance#Article_5 -->

    <owl:NamedIndividual rdf:about="&Governance;Article_5">
        <rdf:type rdf:resource="&Governance;GDPR"/>
    </owl:NamedIndividual>
    


    <!-- http://www.semanticweb.org/IG/Governance#Article_50 -->

    <owl:NamedIndividual rdf:about="&Governance;Article_50">
        <rdf:type rdf:resource="&Governance;GDPR"/>
    </owl:NamedIndividual>
    


    <!-- http://www.semanticweb.org/IG/Governance#Article_6 -->

    <owl:NamedIndividual rdf:about="&Governance;Article_6">
        <rdf:type rdf:resource="&Governance;GDPR"/>
    </owl:NamedIndividual>
    


    <!-- http://www.semanticweb.org/IG/Governance#Article_9 -->

    <owl:NamedIndividual rdf:about="&Governance;Article_9">
        <rdf:type rdf:resource="&Governance;GDPR"/>
    </owl:NamedIndividual>
    


    <!-- http://www.semanticweb.org/IG/Governance#Asset_Database_1 -->

    <owl:NamedIndividual rdf:about="&Governance;Asset_Database_1">
        <rdf:type rdf:resource="&Governance;Asset_Database"/>
        <Governance:involvesArticle rdf:resource="&Governance;Article_30"/>
        <Governance:practicesDefinedInIso rdf:resource="&Governance;ISO_15926"/>
    </owl:NamedIndividual>
    


    <!-- http://www.semanticweb.org/IG/Governance#Audit_1 -->

    <owl:NamedIndividual rdf:about="&Governance;Audit_1">
        <rdf:type rdf:resource="&Governance;Audit"/>
        <Governance:involvesArticle rdf:resource="&Governance;Article_24"/>
        <Governance:involvesArticle rdf:resource="&Governance;Article_30"/>
        <Governance:involvesArticle rdf:resource="&Governance;Article_32"/>
        <Governance:involvesArticle rdf:resource="&Governance;Article_5"/>
        <Governance:canBeInvolvedWith rdf:resource="&Governance;Disposition_Policies_And_Procedures_1"/>
        <Governance:practicesDefinedInIso rdf:resource="&Governance;ISO_15489"/>
        <Governance:practicesDefinedInIso rdf:resource="&Governance;ISO_15939"/>
        <Governance:practicesDefinedInIso rdf:resource="&Governance;ISO_17000"/>
        <Governance:practicesDefinedInIso rdf:resource="&Governance;ISO_27000"/>
        <Governance:practicesDefinedInIso rdf:resource="&Governance;ISO_27001"/>
        <Governance:practicesDefinedInIso rdf:resource="&Governance;ISO_27017"/>
    </owl:NamedIndividual>
    <owl:Axiom>
        <rdfs:comment>The Audit subcategory within the Security department is concerned with monitoring and assessing compliance with policies. Disposition policies and procedures are relevant for audit purposes, as they define how data is managed and disposed of. Auditing the adherence to these policies helps maintain transparency and accountability in data handling.</rdfs:comment>
        <owl:annotatedSource rdf:resource="&Governance;Audit_1"/>
        <owl:annotatedTarget rdf:resource="&Governance;Disposition_Policies_And_Procedures_1"/>
        <owl:annotatedProperty rdf:resource="&Governance;canBeInvolvedWith"/>
    </owl:Axiom>
    


    <!-- http://www.semanticweb.org/IG/Governance#Auditing_And_Monitoring -->

    <owl:NamedIndividual rdf:about="&Governance;Auditing_And_Monitoring">
        <rdf:type rdf:resource="&Governance;IG_Capability"/>
    </owl:NamedIndividual>
    


    <!-- http://www.semanticweb.org/IG/Governance#Authentication_1 -->

    <owl:NamedIndividual rdf:about="&Governance;Authentication_1">
        <rdf:type rdf:resource="&Governance;Authentication"/>
        <Governance:involvesArticle rdf:resource="&Governance;Article_32"/>
        <Governance:practicesDefinedInIso rdf:resource="&Governance;ISO_27001"/>
    </owl:NamedIndividual>
    


    <!-- http://www.semanticweb.org/IG/Governance#Automated_Chain_Of_Custody_Logging_1 -->

    <owl:NamedIndividual rdf:about="&Governance;Automated_Chain_Of_Custody_Logging_1">
        <rdf:type rdf:resource="&Governance;Automated_Chain_Of_Custody_Logging"/>
        <Governance:involvesArticle rdf:resource="&Governance;Article_5"/>
        <Governance:practicesDefinedInIso rdf:resource="&Governance;ISO_14271"/>
    </owl:NamedIndividual>
    


    <!-- http://www.semanticweb.org/IG/Governance#Automated_Data_Collection -->

    <owl:NamedIndividual rdf:about="&Governance;Automated_Data_Collection">
        <rdf:type rdf:resource="&Governance;Automated_Data_Collection"/>
        <Governance:involvesArticle rdf:resource="&Governance;Article_32"/>
        <Governance:involvesArticle rdf:resource="&Governance;Article_5"/>
        <Governance:practicesDefinedInIso rdf:resource="&Governance;ISO_15939"/>
        <Governance:practicesDefinedInIso rdf:resource="&Governance;ISO_27000"/>
    </owl:NamedIndividual>
    


    <!-- http://www.semanticweb.org/IG/Governance#Automated_Data_Culling_And_Scoping_1 -->

    <owl:NamedIndividual rdf:about="&Governance;Automated_Data_Culling_And_Scoping_1">
        <rdf:type rdf:resource="&Governance;Automated_Data_Culling_And_Scoping"/>
        <Governance:involvesArticle rdf:resource="&Governance;Article_25"/>
        <Governance:involvesArticle rdf:resource="&Governance;Article_5"/>
        <Governance:practicesDefinedInIso rdf:resource="&Governance;ISO_15489"/>
        <Governance:practicesDefinedInIso rdf:resource="&Governance;ISO_27000"/>
    </owl:NamedIndividual>
    


    <!-- http://www.semanticweb.org/IG/Governance#Automated_Data_Retention_And_Disposa_1 -->

    <owl:NamedIndividual rdf:about="&Governance;Automated_Data_Retention_And_Disposa_1">
        <rdf:type rdf:resource="&Governance;Automated_Data_Retention_And_Disposal"/>
        <Governance:involvesArticle rdf:resource="&Governance;Article_25"/>
        <Governance:involvesArticle rdf:resource="&Governance;Article_5"/>
        <Governance:practicesDefinedInIso rdf:resource="&Governance;ISO_15489"/>
        <Governance:practicesDefinedInIso rdf:resource="&Governance;ISO_27001"/>
    </owl:NamedIndividual>
    


    <!-- http://www.semanticweb.org/IG/Governance#Automated_Integration -->

    <owl:NamedIndividual rdf:about="&Governance;Automated_Integration">
        <rdf:type rdf:resource="&Governance;Automted_Integration"/>
        <Governance:involvesArticle rdf:resource="&Governance;Article_25"/>
        <Governance:involvesArticle rdf:resource="&Governance;Article_32"/>
        <Governance:involvesArticle rdf:resource="&Governance;Article_5"/>
        <Governance:practicesDefinedInIso rdf:resource="&Governance;ISO_15000"/>
        <Governance:practicesDefinedInIso rdf:resource="&Governance;ISO_15489"/>
        <Governance:practicesDefinedInIso rdf:resource="&Governance;ISO_23081"/>
        <Governance:practicesDefinedInIso rdf:resource="&Governance;ISO_27000"/>
        <Governance:practicesDefinedInIso rdf:resource="&Governance;ISO_27001"/>
    </owl:NamedIndividual>
    


    <!-- http://www.semanticweb.org/IG/Governance#Automated_Notification_System_1 -->

    <owl:NamedIndividual rdf:about="&Governance;Automated_Notification_System_1">
        <rdf:type rdf:resource="&Governance;Automated_Notification_System"/>
        <Governance:involvesArticle rdf:resource="&Governance;Article_33"/>
        <Governance:involvesArticle rdf:resource="&Governance;Article_34"/>
        <Governance:involvesArticle rdf:resource="&Governance;Article_5"/>
        <Governance:practicesDefinedInIso rdf:resource="&Governance;ISO_17000"/>
        <Governance:practicesDefinedInIso rdf:resource="&Governance;ISO_27001"/>
    </owl:NamedIndividual>
    


    <!-- http://www.semanticweb.org/IG/Governance#Automated_Record_Flagging_System_1 -->

    <owl:NamedIndividual rdf:about="&Governance;Automated_Record_Flagging_System_1">
        <rdf:type rdf:resource="&Governance;Automated_Record_Flagging_System"/>
        <Governance:involvesArticle rdf:resource="&Governance;Article_25"/>
        <Governance:practicesDefinedInIso rdf:resource="&Governance;ISO_15939"/>
    </owl:NamedIndividual>
    


    <!-- http://www.semanticweb.org/IG/Governance#Automated_Retention_Execution_1 -->

    <owl:NamedIndividual rdf:about="&Governance;Automated_Retention_Execution_1">
        <rdf:type rdf:resource="&Governance;Automated_Retention_Execution"/>
        <Governance:involvesArticle rdf:resource="&Governance;Article_17"/>
        <Governance:involvesArticle rdf:resource="&Governance;Article_25"/>
        <Governance:involvesArticle rdf:resource="&Governance;Article_5"/>
        <Governance:involvesArticle rdf:resource="&Governance;Article_6"/>
        <Governance:practicesDefinedInIso rdf:resource="&Governance;ISO_15489"/>
    </owl:NamedIndividual>
    


    <!-- http://www.semanticweb.org/IG/Governance#Automated_Risk_Assessment_System_1 -->

    <owl:NamedIndividual rdf:about="&Governance;Automated_Risk_Assessment_System_1">
        <rdf:type rdf:resource="&Governance;Automated_Risk_Assessment_System"/>
        <Governance:involvesArticle rdf:resource="&Governance;Article_32"/>
        <Governance:practicesDefinedInIso rdf:resource="&Governance;ISO_27001"/>
    </owl:NamedIndividual>
    


    <!-- http://www.semanticweb.org/IG/Governance#Automated_Storage_Utilization_Reporting_1 -->

    <owl:NamedIndividual rdf:about="&Governance;Automated_Storage_Utilization_Reporting_1">
        <rdf:type rdf:resource="&Governance;Automated_Storage_Utilization_Reporting"/>
        <Governance:involvesArticle rdf:resource="&Governance;Article_25"/>
        <Governance:involvesArticle rdf:resource="&Governance;Article_32"/>
        <Governance:involvesArticle rdf:resource="&Governance;Article_5"/>
        <Governance:practicesDefinedInIso rdf:resource="&Governance;ISO_15489"/>
    </owl:NamedIndividual>
    


    <!-- http://www.semanticweb.org/IG/Governance#Backup_1 -->

    <owl:NamedIndividual rdf:about="&Governance;Backup_1">
        <rdf:type rdf:resource="&Governance;Backup"/>
        <Governance:involvesArticle rdf:resource="&Governance;Article_32"/>
        <Governance:involvesArticle rdf:resource="&Governance;Article_5"/>
        <Governance:practicesDefinedInIso rdf:resource="&Governance;ISO_15489"/>
        <Governance:practicesDefinedInIso rdf:resource="&Governance;ISO_22301"/>
        <Governance:practicesDefinedInIso rdf:resource="&Governance;ISO_27001"/>
    </owl:NamedIndividual>
    


    <!-- http://www.semanticweb.org/IG/Governance#Business_Unit_1 -->

    <owl:NamedIndividual rdf:about="&Governance;Business_Unit_1">
        <rdf:type rdf:resource="&Governance;Business_Unit"/>
        <Governance:uses rdf:resource="&Governance;Collaboration_Tools_1"/>
        <Governance:uses rdf:resource="&Governance;Data_Sharing_Protocols_1"/>
        <Governance:canBeInvolvedWith rdf:resource="&Governance;Document_Management_System_1"/>
        <Governance:responsibleFor rdf:resource="&Governance;Employee_Engagement_Platforms_1"/>
        <Governance:uses rdf:resource="&Governance;Reporting_And_Analysis_System_1"/>
        <Governance:uses rdf:resource="&Governance;Search_And_Retrieval_System_1"/>
        <Governance:uses rdf:resource="&Governance;Training_1"/>
        <Governance:uses rdf:resource="&Governance;Workflow_Tools_1"/>
    </owl:NamedIndividual>
    <owl:Axiom>
        <rdfs:comment>The Business Unit primarily uses &quot;Training&quot; programs to ensure that its employees are equipped with the knowledge and skills needed to adapt to changes, new systems, or updated procedures. Training enhances employee proficiency and performance in their roles.</rdfs:comment>
        <owl:annotatedSource rdf:resource="&Governance;Business_Unit_1"/>
        <owl:annotatedTarget rdf:resource="&Governance;Training_1"/>
        <owl:annotatedProperty rdf:resource="&Governance;uses"/>
    </owl:Axiom>
    <owl:Axiom>
        <rdfs:comment>The Business Unit primarily uses the &quot;Reporting and Analysis System&quot; to access, analyze, and generate reports related to their specific business operations. This system enables them to make informed decisions, track key performance indicators (KPIs), and gain insights into business trends and opportunities.</rdfs:comment>
        <owl:annotatedSource rdf:resource="&Governance;Business_Unit_1"/>
        <owl:annotatedTarget rdf:resource="&Governance;Reporting_And_Analysis_System_1"/>
        <owl:annotatedProperty rdf:resource="&Governance;uses"/>
    </owl:Axiom>
    <owl:Axiom>
        <rdfs:comment>The Business Unit primarily uses the &quot;Search and Retrieval System&quot; to quickly access relevant information, documents, or data required for their specific operations. The system enhances their productivity by providing efficient and accurate retrieval capabilities.</rdfs:comment>
        <owl:annotatedSource rdf:resource="&Governance;Business_Unit_1"/>
        <owl:annotatedTarget rdf:resource="&Governance;Search_And_Retrieval_System_1"/>
        <owl:annotatedProperty rdf:resource="&Governance;uses"/>
    </owl:Axiom>
    <owl:Axiom>
        <rdfs:comment>The Business Unit primarily uses &quot;Workflow Tools&quot; to manage and execute its specific operational workflows and processes. These tools help streamline tasks, improve efficiency, and ensure consistent processes within the business operations.</rdfs:comment>
        <owl:annotatedSource rdf:resource="&Governance;Business_Unit_1"/>
        <owl:annotatedTarget rdf:resource="&Governance;Workflow_Tools_1"/>
        <owl:annotatedProperty rdf:resource="&Governance;uses"/>
    </owl:Axiom>
    <owl:Axiom>
        <rdfs:comment>The Business Unit is responsible for implementing and utilizing &quot;Employee Engagement Platforms.&quot; These platforms are designed to improve employee communication, collaboration, and engagement within the business unit. The Business Unit ensures that the chosen platforms align with their specific goals and enhance employee interactions and productivity.</rdfs:comment>
        <owl:annotatedSource rdf:resource="&Governance;Business_Unit_1"/>
        <owl:annotatedTarget rdf:resource="&Governance;Employee_Engagement_Platforms_1"/>
        <owl:annotatedProperty rdf:resource="&Governance;responsibleFor"/>
    </owl:Axiom>
    <owl:Axiom>
        <rdfs:comment>Business units across the organization may use the &quot;Document Management System&quot; to centralize and organize their documents, collaborate on projects, and streamline document-related processes. This helps improve team efficiency, document accessibility, and version control.</rdfs:comment>
        <owl:annotatedSource rdf:resource="&Governance;Business_Unit_1"/>
        <owl:annotatedTarget rdf:resource="&Governance;Document_Management_System_1"/>
        <owl:annotatedProperty rdf:resource="&Governance;canBeInvolvedWith"/>
    </owl:Axiom>
    <owl:Axiom>
        <rdfs:comment>The Business Unit utilizes &quot;Data Sharing Protocols&quot; to facilitate the secure and compliant sharing of data for business purposes. These protocols outline the steps, permissions, and safeguards necessary to share data while safeguarding its confidentiality and complying with legal and privacy obligations. The Business Unit follows these protocols to ensure responsible and transparent data sharing practices.</rdfs:comment>
        <owl:annotatedSource rdf:resource="&Governance;Business_Unit_1"/>
        <owl:annotatedTarget rdf:resource="&Governance;Data_Sharing_Protocols_1"/>
        <owl:annotatedProperty rdf:resource="&Governance;uses"/>
    </owl:Axiom>
    <owl:Axiom>
        <rdfs:comment>The business unit uses &quot;collaboration tools&quot; to support collaboration and communication within its area. These tools are used to increase the efficiency of teamwork, exchange information and work on projects together. Development:</rdfs:comment>
        <owl:annotatedSource rdf:resource="&Governance;Business_Unit_1"/>
        <owl:annotatedTarget rdf:resource="&Governance;Collaboration_Tools_1"/>
        <owl:annotatedProperty rdf:resource="&Governance;uses"/>
    </owl:Axiom>
    


    <!-- http://www.semanticweb.org/IG/Governance#CGOC_02 -->

    <owl:NamedIndividual rdf:about="&Governance;CGOC_02">
        <rdf:type rdf:resource="&Governance;Framework"/>
    </owl:NamedIndividual>
    


    <!-- http://www.semanticweb.org/IG/Governance#CIGO_1 -->

    <owl:NamedIndividual rdf:about="&Governance;CIGO_1">
        <rdf:type rdf:resource="&Governance;CIGO"/>
        <Governance:involvesArticle rdf:resource="&Governance;Article_35"/>
        <Governance:involvesArticle rdf:resource="&Governance;Article_39"/>
        <Governance:involvesArticle rdf:resource="&Governance;Article_5"/>
        <Governance:practicesDefinedInIso rdf:resource="&Governance;ISO_15489"/>
        <Governance:practicesDefinedInIso rdf:resource="&Governance;ISO_23081"/>
        <Governance:practicesDefinedInIso rdf:resource="&Governance;ISO_27001"/>
    </owl:NamedIndividual>
    


    <!-- http://www.semanticweb.org/IG/Governance#Centralized_Data_Repository_1 -->

    <owl:NamedIndividual rdf:about="&Governance;Centralized_Data_Repository_1">
        <rdf:type rdf:resource="&Governance;Centralized_Data_Repository"/>
        <Governance:involvesArticle rdf:resource="&Governance;Article_32"/>
        <Governance:involvesArticle rdf:resource="&Governance;Article_5"/>
        <Governance:involvesArticle rdf:resource="&Governance;Article_6"/>
        <Governance:practicesDefinedInIso rdf:resource="&Governance;ISO_15489"/>
        <Governance:practicesDefinedInIso rdf:resource="&Governance;ISO_27001"/>
    </owl:NamedIndividual>
    


    <!-- http://www.semanticweb.org/IG/Governance#Centralized_Data_Source_Catalog_1 -->

    <owl:NamedIndividual rdf:about="&Governance;Centralized_Data_Source_Catalog_1">
        <rdf:type rdf:resource="&Governance;Centralized_Data_Source_Catalog"/>
        <Governance:involvesArticle rdf:resource="&Governance;Article_30"/>
        <Governance:involvesArticle rdf:resource="&Governance;Article_32"/>
        <Governance:involvesArticle rdf:resource="&Governance;Article_5"/>
        <Governance:practicesDefinedInIso rdf:resource="&Governance;ISO_15489"/>
        <Governance:practicesDefinedInIso rdf:resource="&Governance;ISO_8000"/>
    </owl:NamedIndividual>
    


    <!-- http://www.semanticweb.org/IG/Governance#Centralized_Instructions_Repository_1 -->

    <owl:NamedIndividual rdf:about="&Governance;Centralized_Instructions_Repository_1">
        <rdf:type rdf:resource="&Governance;Centralized_Instructions_Repository"/>
        <Governance:involvesArticle rdf:resource="&Governance;Article_5"/>
        <Governance:practicesDefinedInIso rdf:resource="&Governance;ISO_15489"/>
        <Governance:practicesDefinedInIso rdf:resource="&Governance;ISO_23081"/>
    </owl:NamedIndividual>
    


    <!-- http://www.semanticweb.org/IG/Governance#Chain_Of_Custody_Tracking_1 -->

    <owl:NamedIndividual rdf:about="&Governance;Chain_Of_Custody_Tracking_1">
        <rdf:type rdf:resource="&Governance;Chain_Of_Custody_Tracking"/>
        <Governance:involvesArticle rdf:resource="&Governance;Article_30"/>
        <Governance:involvesArticle rdf:resource="&Governance;Article_32"/>
        <Governance:involvesArticle rdf:resource="&Governance;Article_5"/>
        <Governance:practicesDefinedInIso rdf:resource="&Governance;ISO_15489"/>
        <Governance:practicesDefinedInIso rdf:resource="&Governance;ISO_15939"/>
        <Governance:practicesDefinedInIso rdf:resource="&Governance;ISO_17000"/>
        <Governance:practicesDefinedInIso rdf:resource="&Governance;ISO_27001"/>
    </owl:NamedIndividual>
    


    <!-- http://www.semanticweb.org/IG/Governance#Change_Management_1 -->

    <owl:NamedIndividual rdf:about="&Governance;Change_Management_1">
        <rdf:type rdf:resource="&Governance;Change_Management"/>
        <Governance:involvesArticle rdf:resource="&Governance;Article_32"/>
        <Governance:involvesArticle rdf:resource="&Governance;Article_5"/>
        <Governance:canBeInvolvedWith rdf:resource="&Governance;Document_Management_System_1"/>
        <Governance:uses rdf:resource="&Governance;Employee_Engagement_Platforms_1"/>
        <Governance:practicesDefinedInIso rdf:resource="&Governance;ISO_15000"/>
        <Governance:practicesDefinedInIso rdf:resource="&Governance;ISO_15939"/>
        <Governance:practicesDefinedInIso rdf:resource="&Governance;ISO_17000"/>
        <Governance:responsibleFor rdf:resource="&Governance;Training_1"/>
    </owl:NamedIndividual>
    <owl:Axiom>
        <rdfs:comment>The Change Management department could use the system to store change-related documents, communication plans, and project documentation. This aids in tracking and managing changes, ensuring that stakeholders have access to accurate and consistent information.</rdfs:comment>
        <owl:annotatedSource rdf:resource="&Governance;Change_Management_1"/>
        <owl:annotatedTarget rdf:resource="&Governance;Document_Management_System_1"/>
        <owl:annotatedProperty rdf:resource="&Governance;canBeInvolvedWith"/>
    </owl:Axiom>
    <owl:Axiom>
        <rdfs:comment>The Change Management department exclusively uses &quot;Employee Engagement Platforms&quot; to facilitate effective communication and engagement during organizational changes. These platforms provide channels for sharing updates, addressing concerns, and involving employees in change initiatives, promoting a smooth transition and buy-in from staff.</rdfs:comment>
        <owl:annotatedSource rdf:resource="&Governance;Change_Management_1"/>
        <owl:annotatedTarget rdf:resource="&Governance;Employee_Engagement_Platforms_1"/>
        <owl:annotatedProperty rdf:resource="&Governance;uses"/>
    </owl:Axiom>
    <owl:Axiom>
        <rdfs:comment>The Change Management department is responsible for designing and implementing &quot;Training&quot; programs. These programs aim to educate employees and stakeholders about changes in processes, technologies, or procedures within the organization. Change Management ensures that training materials are developed, delivered, and assessed effectively to support smooth transitions.</rdfs:comment>
        <owl:annotatedSource rdf:resource="&Governance;Change_Management_1"/>
        <owl:annotatedTarget rdf:resource="&Governance;Training_1"/>
        <owl:annotatedProperty rdf:resource="&Governance;responsibleFor"/>
    </owl:Axiom>
    


    <!-- http://www.semanticweb.org/IG/Governance#Collaboration_Tools_1 -->

    <owl:NamedIndividual rdf:about="&Governance;Collaboration_Tools_1">
        <rdf:type rdf:resource="&Governance;Collaboration_Tools"/>
        <Governance:involvesArticle rdf:resource="&Governance;Article_30"/>
        <Governance:involvesArticle rdf:resource="&Governance;Article_32"/>
        <Governance:involvesArticle rdf:resource="&Governance;Article_5"/>
        <Governance:involvesArticle rdf:resource="&Governance;Article_6"/>
        <Governance:involvesArticle rdf:resource="&Governance;Article_9"/>
        <Governance:practicesDefinedInIso rdf:resource="&Governance;ISO_14271"/>
        <Governance:practicesDefinedInIso rdf:resource="&Governance;ISO_15000"/>
        <Governance:practicesDefinedInIso rdf:resource="&Governance;ISO_15489"/>
        <Governance:practicesDefinedInIso rdf:resource="&Governance;ISO_15939"/>
        <Governance:practicesDefinedInIso rdf:resource="&Governance;ISO_23081"/>
        <Governance:practicesDefinedInIso rdf:resource="&Governance;ISO_27010"/>
    </owl:NamedIndividual>
    


    <!-- http://www.semanticweb.org/IG/Governance#Communication_Platforms_1 -->

    <owl:NamedIndividual rdf:about="&Governance;Communication_Platforms_1">
        <rdf:type rdf:resource="&Governance;Communication_Platforms"/>
        <Governance:involvesArticle rdf:resource="&Governance;Article_12"/>
        <Governance:involvesArticle rdf:resource="&Governance;Article_24"/>
        <Governance:practicesDefinedInIso rdf:resource="&Governance;ISO_15000"/>
        <Governance:practicesDefinedInIso rdf:resource="&Governance;ISO_23081"/>
        <Governance:practicesDefinedInIso rdf:resource="&Governance;ISO_27000"/>
    </owl:NamedIndividual>
    


    <!-- http://www.semanticweb.org/IG/Governance#Compliance -->

    <owl:NamedIndividual rdf:about="&Governance;Compliance">
        <rdf:type rdf:resource="&Governance;Goal"/>
    </owl:NamedIndividual>
    


    <!-- http://www.semanticweb.org/IG/Governance#Confirmation_Tracking_Mechanism_1 -->

    <owl:NamedIndividual rdf:about="&Governance;Confirmation_Tracking_Mechanism_1">
        <rdf:type rdf:resource="&Governance;Confirmation_Tracking_Mechanism"/>
        <Governance:involvesArticle rdf:resource="&Governance;Article_30"/>
        <Governance:practicesDefinedInIso rdf:resource="&Governance;ISO_14271"/>
    </owl:NamedIndividual>
    


    <!-- http://www.semanticweb.org/IG/Governance#Continous_Visibility_And_Monitoring_System_1 -->

    <owl:NamedIndividual rdf:about="&Governance;Continous_Visibility_And_Monitoring_System_1">
        <rdf:type rdf:resource="&Governance;Continous_Visibility_And_Monitoring_System"/>
        <Governance:involvesArticle rdf:resource="&Governance;Article_5"/>
        <Governance:practicesDefinedInIso rdf:resource="&Governance;ISO_15489"/>
    </owl:NamedIndividual>
    


    <!-- http://www.semanticweb.org/IG/Governance#Cost_Calculations_1 -->

    <owl:NamedIndividual rdf:about="&Governance;Cost_Calculations_1">
        <rdf:type rdf:resource="&Governance;Cost_Calculations"/>
        <Governance:involvesArticle rdf:resource="&Governance;Article_25"/>
        <Governance:involvesArticle rdf:resource="&Governance;Article_5"/>
        <Governance:practicesDefinedInIso rdf:resource="&Governance;ISO_15000"/>
        <Governance:practicesDefinedInIso rdf:resource="&Governance;ISO_15939"/>
    </owl:NamedIndividual>
    


    <!-- http://www.semanticweb.org/IG/Governance#DAM -->

    <owl:NamedIndividual rdf:about="&Governance;DAM">
        <rdf:type rdf:resource="&Governance;Framework"/>
    </owl:NamedIndividual>
    


    <!-- http://www.semanticweb.org/IG/Governance#DPO_1 -->

    <owl:NamedIndividual rdf:about="&Governance;DPO_1">
        <rdf:type rdf:resource="&Governance;DPO"/>
        <Governance:involvesArticle rdf:resource="&Governance;Article_39"/>
        <Governance:involvesArticle rdf:resource="&Governance;Article_5"/>
        <Governance:practicesDefinedInIso rdf:resource="&Governance;ISO_15489"/>
        <Governance:practicesDefinedInIso rdf:resource="&Governance;ISO_27001"/>
    </owl:NamedIndividual>
    


    <!-- http://www.semanticweb.org/IG/Governance#DataController1 -->

    <owl:NamedIndividual rdf:about="&Governance;DataController1">
        <rdf:type rdf:resource="&Governance;Data_Controller"/>
        <Governance:responsibleForCapability rdf:resource="&Governance;AC_1_3_3"/>
    </owl:NamedIndividual>
    


    <!-- http://www.semanticweb.org/IG/Governance#Data_Breach_Management -->

    <owl:NamedIndividual rdf:about="&Governance;Data_Breach_Management">
        <rdf:type rdf:resource="&Governance;IG_Capability"/>
    </owl:NamedIndividual>
    


    <!-- http://www.semanticweb.org/IG/Governance#Data_Inventory_And_Mapping -->

    <owl:NamedIndividual rdf:about="&Governance;Data_Inventory_And_Mapping">
        <rdf:type rdf:resource="&Governance;IG_Capability"/>
    </owl:NamedIndividual>
    


    <!-- http://www.semanticweb.org/IG/Governance#Data_Mapping_And_Classification_System_1 -->

    <owl:NamedIndividual rdf:about="&Governance;Data_Mapping_And_Classification_System_1">
        <rdf:type rdf:resource="&Governance;Data_Mapping_And_Classification_System"/>
        <Governance:involvesArticle rdf:resource="&Governance;Article_24"/>
        <Governance:involvesArticle rdf:resource="&Governance;Article_25"/>
        <Governance:involvesArticle rdf:resource="&Governance;Article_30"/>
        <Governance:involvesArticle rdf:resource="&Governance;Article_32"/>
        <Governance:involvesArticle rdf:resource="&Governance;Article_5"/>
        <Governance:practicesDefinedInIso rdf:resource="&Governance;ISO_14271"/>
        <Governance:practicesDefinedInIso rdf:resource="&Governance;ISO_15489"/>
        <Governance:practicesDefinedInIso rdf:resource="&Governance;ISO_15939"/>
        <Governance:practicesDefinedInIso rdf:resource="&Governance;ISO_23081"/>
        <Governance:practicesDefinedInIso rdf:resource="&Governance;ISO_27001"/>
    </owl:NamedIndividual>
    


    <!-- http://www.semanticweb.org/IG/Governance#Data_Privacy_Masking_1 -->

    <owl:NamedIndividual rdf:about="&Governance;Data_Privacy_Masking_1">
        <rdf:type rdf:resource="&Governance;Data_Privacy_Masking"/>
        <Governance:involvesArticle rdf:resource="&Governance;Article_32"/>
        <Governance:involvesArticle rdf:resource="&Governance;Article_5"/>
        <Governance:practicesDefinedInIso rdf:resource="&Governance;ISO_27001"/>
    </owl:NamedIndividual>
    


    <!-- http://www.semanticweb.org/IG/Governance#Data_Quality_Assurance_Framework_1 -->

    <owl:NamedIndividual rdf:about="&Governance;Data_Quality_Assurance_Framework_1">
        <rdf:type rdf:resource="&Governance;Data_Quality_Assurance_Framework"/>
        <Governance:involvesArticle rdf:resource="&Governance;Article_30"/>
        <Governance:involvesArticle rdf:resource="&Governance;Article_32"/>
        <Governance:involvesArticle rdf:resource="&Governance;Article_5"/>
        <Governance:involvesArticle rdf:resource="&Governance;Article_6"/>
        <Governance:practicesDefinedInIso rdf:resource="&Governance;ISO_14271"/>
        <Governance:practicesDefinedInIso rdf:resource="&Governance;ISO_15000"/>
        <Governance:practicesDefinedInIso rdf:resource="&Governance;ISO_15489"/>
        <Governance:practicesDefinedInIso rdf:resource="&Governance;ISO_15939"/>
        <Governance:practicesDefinedInIso rdf:resource="&Governance;ISO_23081"/>
        <Governance:practicesDefinedInIso rdf:resource="&Governance;ISO_27001"/>
    </owl:NamedIndividual>
    


    <!-- http://www.semanticweb.org/IG/Governance#Data_Quality_Management_1 -->

    <owl:NamedIndividual rdf:about="&Governance;Data_Quality_Management_1">
        <rdf:type rdf:resource="&Governance;Data_Quality_Management"/>
        <Governance:involvesArticle rdf:resource="&Governance;Article_32"/>
        <Governance:involvesArticle rdf:resource="&Governance;Article_5"/>
        <Governance:practicesDefinedInIso rdf:resource="&Governance;ISO_15489"/>
        <Governance:practicesDefinedInIso rdf:resource="&Governance;ISO_15939"/>
        <Governance:practicesDefinedInIso rdf:resource="&Governance;ISO_23081"/>
    </owl:NamedIndividual>
    


    <!-- http://www.semanticweb.org/IG/Governance#Data_Retention_And_Erasure -->

    <owl:NamedIndividual rdf:about="&Governance;Data_Retention_And_Erasure">
        <rdf:type rdf:resource="&Governance;IG_Capability"/>
    </owl:NamedIndividual>
    


    <!-- http://www.semanticweb.org/IG/Governance#Data_Retention_Policy_Dummy -->

    <owl:NamedIndividual rdf:about="&Governance;Data_Retention_Policy_Dummy">
        <rdf:type rdf:resource="&Governance;Data_Retention_Policy"/>
        <Governance:involvesArticle rdf:resource="&Governance;Article_17"/>
        <Governance:involvesArticle rdf:resource="&Governance;Article_25"/>
        <Governance:involvesArticle rdf:resource="&Governance;Article_30"/>
        <Governance:involvesArticle rdf:resource="&Governance;Article_5"/>
        <Governance:involvesArticle rdf:resource="&Governance;Article_6"/>
        <Governance:practicesDefinedInIso rdf:resource="&Governance;ISO_15489"/>
        <Governance:practicesDefinedInIso rdf:resource="&Governance;ISO_15939"/>
        <Governance:practicesDefinedInIso rdf:resource="&Governance;ISO_17000"/>
        <Governance:practicesDefinedInIso rdf:resource="&Governance;ISO_27001"/>
    </owl:NamedIndividual>
    


    <!-- http://www.semanticweb.org/IG/Governance#Data_Security_And_Privacy_Controls -->

    <owl:NamedIndividual rdf:about="&Governance;Data_Security_And_Privacy_Controls">
        <rdf:type rdf:resource="&Governance;IG_Capability"/>
    </owl:NamedIndividual>
    


    <!-- http://www.semanticweb.org/IG/Governance#Data_Sharing_Protocols_1 -->

    <owl:NamedIndividual rdf:about="&Governance;Data_Sharing_Protocols_1">
        <rdf:type rdf:resource="&Governance;Data_Sharing_Protocols"/>
        <Governance:involvesArticle rdf:resource="&Governance;Article_5"/>
        <Governance:involvesArticle rdf:resource="&Governance;Article_6"/>
        <Governance:involvesArticle rdf:resource="&Governance;Article_9"/>
        <Governance:practicesDefinedInIso rdf:resource="&Governance;ISO_15489"/>
    </owl:NamedIndividual>
    


    <!-- http://www.semanticweb.org/IG/Governance#Data_Storage_1 -->

    <owl:NamedIndividual rdf:about="&Governance;Data_Storage_1">
        <rdf:type rdf:resource="&Governance;Data_Storage"/>
        <Governance:involvesArticle rdf:resource="&Governance;Article_32"/>
        <Governance:involvesArticle rdf:resource="&Governance;Article_5"/>
        <Governance:practicesDefinedInIso rdf:resource="&Governance;ISO_15489"/>
        <Governance:practicesDefinedInIso rdf:resource="&Governance;ISO_27000"/>
    </owl:NamedIndividual>
    


    <!-- http://www.semanticweb.org/IG/Governance#Data_Subject_Rights -->

    <owl:NamedIndividual rdf:about="&Governance;Data_Subject_Rights">
        <rdf:type rdf:resource="&Governance;IG_Capability"/>
    </owl:NamedIndividual>
    


    <!-- http://www.semanticweb.org/IG/Governance#Database_Management_System_1 -->

    <owl:NamedIndividual rdf:about="&Governance;Database_Management_System_1">
        <rdf:type rdf:resource="&Governance;Database_Management_System"/>
        <Governance:involvedInRiskAndCompliance rdf:resource="&Governance;Article_5"/>
        <Governance:involvedInRiskAndCompliance rdf:resource="&Governance;Article_6"/>
        <Governance:uses rdf:resource="&Governance;Data_Mapping_And_Classification_System_1"/>
        <Governance:uses rdf:resource="&Governance;Data_Storage_1"/>
        <Governance:canBeInvolvedWith rdf:resource="&Governance;Disposition_Policies_And_Procedures_1"/>
        <Governance:practicesDefinedInIso rdf:resource="&Governance;ISO_15489"/>
    </owl:NamedIndividual>
    <owl:Axiom>
        <rdfs:comment>The Database Management System subcategory within the Records Management department uses &quot;Data Storage&quot; to manage and store structured data within databases. This involves employing database systems and technologies to organize and maintain data, ensuring data availability, consistency, and access controls. The focus is on efficiently storing and retrieving data as required for business processes and compliance purposes.</rdfs:comment>
        <owl:annotatedTarget rdf:resource="&Governance;Data_Storage_1"/>
        <owl:annotatedSource rdf:resource="&Governance;Database_Management_System_1"/>
        <owl:annotatedProperty rdf:resource="&Governance;uses"/>
    </owl:Axiom>
    <owl:Axiom>
        <rdfs:comment>The Database Management System subdivision within the Records Management department uses the &quot;Data Mapping And Classification System&quot; to ensure structured and orderly management of data in the databases. This helps identify data fields, their meaning, and relationship to each other, which in turn improves data integrity and efficient access.</rdfs:comment>
        <owl:annotatedTarget rdf:resource="&Governance;Data_Mapping_And_Classification_System_1"/>
        <owl:annotatedSource rdf:resource="&Governance;Database_Management_System_1"/>
        <owl:annotatedProperty rdf:resource="&Governance;uses"/>
    </owl:Axiom>
    <owl:Axiom>
        <rdfs:comment>The Database Management System subcategory within the Records Management department might also be involved in implementing &quot;Disposition Policies and Procedures&quot; for structured data stored in databases. Proper data disposition is essential to ensure that data is retained, archived, or deleted according to defined policies, maintaining data accuracy, compliance, and optimizing database resources.</rdfs:comment>
        <owl:annotatedSource rdf:resource="&Governance;Database_Management_System_1"/>
        <owl:annotatedTarget rdf:resource="&Governance;Disposition_Policies_And_Procedures_1"/>
        <owl:annotatedProperty rdf:resource="&Governance;canBeInvolvedWith"/>
    </owl:Axiom>
    


    <!-- http://www.semanticweb.org/IG/Governance#Deadline_Tracking_1 -->

    <owl:NamedIndividual rdf:about="&Governance;Deadline_Tracking_1">
        <rdf:type rdf:resource="&Governance;Deadline_Tracking"/>
        <Governance:involvesArticle rdf:resource="&Governance;Article_6"/>
        <Governance:practicesDefinedInIso rdf:resource="&Governance;ISO_17000"/>
    </owl:NamedIndividual>
    


    <!-- http://www.semanticweb.org/IG/Governance#Designation_Interface_1 -->

    <owl:NamedIndividual rdf:about="&Governance;Designation_Interface_1">
        <rdf:type rdf:resource="&Governance;Designation_Interface"/>
        <Governance:involvesArticle rdf:resource="&Governance;Article_32"/>
        <Governance:practicesDefinedInIso rdf:resource="&Governance;ISO_23081"/>
    </owl:NamedIndividual>
    


    <!-- http://www.semanticweb.org/IG/Governance#Development_1 -->

    <owl:NamedIndividual rdf:about="&Governance;Development_1">
        <rdf:type rdf:resource="&Governance;Development"/>
        <Governance:responsibleFor rdf:resource="&Governance;Collaboration_Tools_1"/>
        <Governance:responsibleFor rdf:resource="&Governance;Data_Mapping_And_Classification_System_1"/>
        <Governance:responsibleFor rdf:resource="&Governance;Data_Quality_Assurance_Framework_1"/>
        <Governance:responsibleFor rdf:resource="&Governance;Data_Quality_Management_1"/>
        <Governance:responsibleFor rdf:resource="&Governance;Data_Storage_1"/>
        <Governance:responsibleFor rdf:resource="&Governance;Digital_Signatures_And_Timestamps_1"/>
        <Governance:responsibleFor rdf:resource="&Governance;Document_Management_System_1"/>
        <Governance:responsibleFor rdf:resource="&Governance;Metadata_Framework_1"/>
        <Governance:responsibleFor rdf:resource="&Governance;Reporting_And_Analysis_System_1"/>
        <Governance:responsibleFor rdf:resource="&Governance;Search_And_Retrieval_System_1"/>
        <Governance:responsibleFor rdf:resource="&Governance;Workflow_Tools_1"/>
    </owl:NamedIndividual>
    <owl:Axiom>
        <rdfs:comment>The Development department is responsible for designing and implementing the mechanisms for &quot;Digital Signatures &amp; Timestamps.&quot; This includes incorporating cryptographic technologies to create digital signatures that verify the authenticity and integrity of electronic documents, as well as adding timestamps to record the time of signing. Development ensures the secure implementation of these features to enhance data security and non-repudiation.</rdfs:comment>
        <owl:annotatedSource rdf:resource="&Governance;Development_1"/>
        <owl:annotatedTarget rdf:resource="&Governance;Digital_Signatures_And_Timestamps_1"/>
        <owl:annotatedProperty rdf:resource="&Governance;responsibleFor"/>
    </owl:Axiom>
    <owl:Axiom>
        <rdfs:comment>The Development department is responsible for designing and implementing the &quot;Reporting and Analysis System.&quot; This system involves creating software-based tools, dashboards, or platforms that allow users to gather, analyze, and visualize data for reporting and decision-making purposes. Development ensures that the system is user-friendly, capable of handling data from various sources, and provides meaningful insights.</rdfs:comment>
        <owl:annotatedSource rdf:resource="&Governance;Development_1"/>
        <owl:annotatedTarget rdf:resource="&Governance;Reporting_And_Analysis_System_1"/>
        <owl:annotatedProperty rdf:resource="&Governance;responsibleFor"/>
    </owl:Axiom>
    <owl:Axiom>
        <rdfs:comment>The Development department is responsible for designing and implementing &quot;Workflow Tools.&quot; These tools are software-based solutions that automate and streamline business processes, enabling efficient task management, collaboration, and workflow automation.</rdfs:comment>
        <owl:annotatedSource rdf:resource="&Governance;Development_1"/>
        <owl:annotatedTarget rdf:resource="&Governance;Workflow_Tools_1"/>
        <owl:annotatedProperty rdf:resource="&Governance;responsibleFor"/>
    </owl:Axiom>
    <owl:Axiom>
        <rdfs:comment>The Development department is responsible for designing and implementing the &quot;Data Quality Assurance Framework.&quot; This framework establishes the processes, methodologies, and standards to ensure the quality and accuracy of data across the organization. Development ensures that the framework is tailored to the organization&apos;s needs and integrated effectively into existing data management practices.</rdfs:comment>
        <owl:annotatedTarget rdf:resource="&Governance;Data_Quality_Assurance_Framework_1"/>
        <owl:annotatedSource rdf:resource="&Governance;Development_1"/>
        <owl:annotatedProperty rdf:resource="&Governance;responsibleFor"/>
    </owl:Axiom>
    <owl:Axiom>
        <rdfs:comment>The Development department is responsible for designing and implementing the infrastructure and systems for &quot;Data Storage.&quot; This includes establishing storage solutions, architectures, and technologies that enable efficient and secure storage of organizational data. Development ensures that data storage meets performance, scalability, and data integrity requirements.</rdfs:comment>
        <owl:annotatedTarget rdf:resource="&Governance;Data_Storage_1"/>
        <owl:annotatedSource rdf:resource="&Governance;Development_1"/>
        <owl:annotatedProperty rdf:resource="&Governance;responsibleFor"/>
    </owl:Axiom>
    <owl:Axiom>
        <rdfs:comment>The Development department is responsible for designing and implementing the &quot;Data Quality Management&quot; processes and methodologies. These processes focus on maintaining and improving the overall quality of data throughout its lifecycle, including data validation, cleansing, and enrichment. Development ensures that data quality standards are integrated into the organization&apos;s systems and processes.</rdfs:comment>
        <owl:annotatedTarget rdf:resource="&Governance;Data_Quality_Management_1"/>
        <owl:annotatedSource rdf:resource="&Governance;Development_1"/>
        <owl:annotatedProperty rdf:resource="&Governance;responsibleFor"/>
    </owl:Axiom>
    <owl:Axiom>
        <rdfs:comment>The Development department is responsible for designing and implementing the &quot;Search and Retrieval System.&quot; This system involves creating software-based tools or platforms that enable users to efficiently search for and retrieve specific information, documents, or data within an organization&apos;s repositories. Development ensures the system&apos;s user interface, search algorithms, and integration capabilities are optimized for seamless retrieval.</rdfs:comment>
        <owl:annotatedSource rdf:resource="&Governance;Development_1"/>
        <owl:annotatedTarget rdf:resource="&Governance;Search_And_Retrieval_System_1"/>
        <owl:annotatedProperty rdf:resource="&Governance;responsibleFor"/>
    </owl:Axiom>
    <owl:Axiom>
        <rdfs:comment>The development department is responsible for the design and implementation of the &quot;Data Mapping And Classification System&quot;. This system helps to identify and classify data and understand its structure or relationships. The development ensures that the system meets the requirements of the organization and is effectively integrated into the existing infrastructure.</rdfs:comment>
        <owl:annotatedTarget rdf:resource="&Governance;Data_Mapping_And_Classification_System_1"/>
        <owl:annotatedSource rdf:resource="&Governance;Development_1"/>
        <owl:annotatedProperty rdf:resource="&Governance;responsibleFor"/>
    </owl:Axiom>
    <owl:Axiom>
        <rdfs:comment>The Development department is responsible for the design and implementation of collaboration tools. This includes creating software platforms or applications that allow employees to collaborate seamlessly, share files, and exchange information in real-time. The development ensures the technical implementation and adaptation to the requirements of the organization.</rdfs:comment>
        <owl:annotatedTarget rdf:resource="&Governance;Collaboration_Tools_1"/>
        <owl:annotatedSource rdf:resource="&Governance;Development_1"/>
        <owl:annotatedProperty rdf:resource="&Governance;responsibleFor"/>
    </owl:Axiom>
    <owl:Axiom>
        <rdfs:comment>The Development department is responsible for designing and implementing the &quot;Metadata Framework.&quot; This framework defines the structure, standards, and guidelines for capturing and managing metadata across the organization. Development ensures that metadata attributes, relationships, and definitions are well-defined and integrated into systems and applications.</rdfs:comment>
        <owl:annotatedSource rdf:resource="&Governance;Development_1"/>
        <owl:annotatedTarget rdf:resource="&Governance;Metadata_Framework_1"/>
        <owl:annotatedProperty rdf:resource="&Governance;responsibleFor"/>
    </owl:Axiom>
    <owl:Axiom>
        <rdfs:comment>The Development department is responsible for designing and implementing the &quot;Document Management System.&quot; This involves creating a software-based system that facilitates the organization, storage, retrieval, and management of electronic documents. Development ensures that the system&apos;s architecture, functionalities, and user interfaces meet the organization&apos;s document management needs.</rdfs:comment>
        <owl:annotatedSource rdf:resource="&Governance;Development_1"/>
        <owl:annotatedTarget rdf:resource="&Governance;Document_Management_System_1"/>
        <owl:annotatedProperty rdf:resource="&Governance;responsibleFor"/>
    </owl:Axiom>
    


    <!-- http://www.semanticweb.org/IG/Governance#Digital_Signatures_And_Timestamps_1 -->

    <owl:NamedIndividual rdf:about="&Governance;Digital_Signatures_And_Timestamps_1">
        <rdf:type rdf:resource="&Governance;Digital_Signatures_And_Timestamps"/>
        <Governance:practicesDefinedInIso rdf:resource="&Governance;Article_30"/>
        <Governance:involvesArticle rdf:resource="&Governance;Article_32"/>
        <Governance:involvesArticle rdf:resource="&Governance;Article_5"/>
        <Governance:practicesDefinedInIso rdf:resource="&Governance;Article_5"/>
        <Governance:practicesDefinedInIso rdf:resource="&Governance;ISO_14271"/>
        <Governance:practicesDefinedInIso rdf:resource="&Governance;ISO_17000"/>
        <Governance:practicesDefinedInIso rdf:resource="&Governance;ISO_23081"/>
        <Governance:practicesDefinedInIso rdf:resource="&Governance;ISO_27000"/>
        <Governance:practicesDefinedInIso rdf:resource="&Governance;ISO_27001"/>
    </owl:NamedIndividual>
    


    <!-- http://www.semanticweb.org/IG/Governance#Disposition_Policies_And_Procedures_1 -->

    <owl:NamedIndividual rdf:about="&Governance;Disposition_Policies_And_Procedures_1">
        <rdf:type rdf:resource="&Governance;Disposition_Policies_And_Procedures"/>
        <Governance:involvesArticle rdf:resource="&Governance;Article_24"/>
        <Governance:involvesArticle rdf:resource="&Governance;Article_25"/>
        <Governance:involvesArticle rdf:resource="&Governance;Article_32"/>
        <Governance:involvesArticle rdf:resource="&Governance;Article_5"/>
        <Governance:practicesDefinedInIso rdf:resource="&Governance;ISO_15489"/>
        <Governance:practicesDefinedInIso rdf:resource="&Governance;ISO_15939"/>
        <Governance:practicesDefinedInIso rdf:resource="&Governance;ISO_27001"/>
    </owl:NamedIndividual>
    


    <!-- http://www.semanticweb.org/IG/Governance#Document_Management_System_1 -->

    <owl:NamedIndividual rdf:about="&Governance;Document_Management_System_1">
        <rdf:type rdf:resource="&Governance;Document_Management_System"/>
        <Governance:involvesArticle rdf:resource="&Governance;Article_17"/>
        <Governance:involvesArticle rdf:resource="&Governance;Article_32"/>
        <Governance:involvesArticle rdf:resource="&Governance;Article_5"/>
        <Governance:involvesArticle rdf:resource="&Governance;Article_6"/>
        <Governance:involvesArticle rdf:resource="&Governance;Article_9"/>
        <Governance:practicesDefinedInIso rdf:resource="&Governance;ISO_15489"/>
        <Governance:practicesDefinedInIso rdf:resource="&Governance;ISO_17000"/>
        <Governance:practicesDefinedInIso rdf:resource="&Governance;ISO_23081"/>
    </owl:NamedIndividual>
    


    <!-- http://www.semanticweb.org/IG/Governance#ERM_1 -->

    <owl:NamedIndividual rdf:about="&Governance;ERM_1">
        <rdf:type rdf:resource="&Governance;Electronic_Records_Management"/>
        <Governance:involvesArticle rdf:resource="&Governance;Article_30"/>
        <Governance:involvesArticle rdf:resource="&Governance;Article_5"/>
        <Governance:uses rdf:resource="&Governance;Chain_Of_Custody_Tracking_1"/>
        <Governance:uses rdf:resource="&Governance;Data_Quality_Management_1"/>
        <Governance:defines rdf:resource="&Governance;Data_Retention_Policy_Dummy"/>
        <Governance:uses rdf:resource="&Governance;Disposition_Policies_And_Procedures_1"/>
        <Governance:uses rdf:resource="&Governance;Document_Management_System_1"/>
        <Governance:practicesDefinedInIso rdf:resource="&Governance;ISO_15489"/>
        <Governance:practicesDefinedInIso rdf:resource="&Governance;ISO_23081"/>
        <Governance:practicesDefinedInIso rdf:resource="&Governance;ISO_27001"/>
        <Governance:uses rdf:resource="&Governance;Metadata_Framework_1"/>
        <Governance:uses rdf:resource="&Governance;Records_Retention_Schedule_1"/>
        <Governance:uses rdf:resource="&Governance;Review_Cyles_1"/>
        <Governance:uses rdf:resource="&Governance;Search_And_Retrieval_System_1"/>
    </owl:NamedIndividual>
    <owl:Axiom>
        <rdfs:comment>The Electronic Records Management subcategory within the Records Management department may use the system to enhance the retrieval of electronic records, ensuring efficient access and compliance with retention policies.</rdfs:comment>
        <owl:annotatedSource rdf:resource="&Governance;ERM_1"/>
        <owl:annotatedTarget rdf:resource="&Governance;Search_And_Retrieval_System_1"/>
        <owl:annotatedProperty rdf:resource="&Governance;uses"/>
    </owl:Axiom>
    <owl:Axiom>
        <rdfs:comment>The Electronic Records Management subcategory within the Records Management department is highly likely to be involved in using the &quot;Records Retention Schedule.&quot; This schedule provides guidelines for retaining electronic records, ensuring compliance with retention policies, and facilitating proper management of electronic information.</rdfs:comment>
        <owl:annotatedSource rdf:resource="&Governance;ERM_1"/>
        <owl:annotatedTarget rdf:resource="&Governance;Records_Retention_Schedule_1"/>
        <owl:annotatedProperty rdf:resource="&Governance;uses"/>
    </owl:Axiom>
    <owl:Axiom>
        <rdfs:comment>The Electronic Records Management subcategory within the Records Management department is highly likely to be involved in using &quot;Review Cycles.&quot; They ensure that electronic records are periodically reviewed and maintained to meet business and compliance requirements.</rdfs:comment>
        <owl:annotatedSource rdf:resource="&Governance;ERM_1"/>
        <owl:annotatedTarget rdf:resource="&Governance;Review_Cyles_1"/>
        <owl:annotatedProperty rdf:resource="&Governance;uses"/>
    </owl:Axiom>
    <owl:Axiom>
        <rdfs:comment>The Electronic Records Management subcategory within the Records Management department uses &quot;Data Quality Management&quot; practices to ensure the accuracy and reliability of electronic records. This involves applying data quality checks, validations, and corrections to electronic records, ensuring their integrity and compliance with relevant regulations and policies.</rdfs:comment>
        <owl:annotatedTarget rdf:resource="&Governance;Data_Quality_Management_1"/>
        <owl:annotatedSource rdf:resource="&Governance;ERM_1"/>
        <owl:annotatedProperty rdf:resource="&Governance;uses"/>
    </owl:Axiom>
    <owl:Axiom>
        <rdfs:comment>The Electronic Records Management subcategory within the Records Management department exclusively uses the &quot;Document Management System&quot; to manage electronic records. This system allows for the organized storage, categorization, version control, and secure access to electronic documents throughout their lifecycle. It ensures proper records management practices and helps maintain compliance with records retention policies.</rdfs:comment>
        <owl:annotatedTarget rdf:resource="&Governance;Document_Management_System_1"/>
        <owl:annotatedSource rdf:resource="&Governance;ERM_1"/>
        <owl:annotatedProperty rdf:resource="&Governance;uses"/>
    </owl:Axiom>
    <owl:Axiom>
        <rdfs:comment>The Electronic Records Management subdivision within the Records Management department uses &quot;Chain of Custody Tracking&quot; to track the access history of electronic records and documents. This helps to ensure that the data is properly managed and that any changes or accesses are recorded to ensure the trustworthiness and usability of the electronic records.</rdfs:comment>
        <owl:annotatedTarget rdf:resource="&Governance;Chain_Of_Custody_Tracking_1"/>
        <owl:annotatedSource rdf:resource="&Governance;ERM_1"/>
        <owl:annotatedProperty rdf:resource="&Governance;uses"/>
    </owl:Axiom>
    <owl:Axiom>
        <rdfs:comment>The Electronic Records Management subcategory within the Records Management department exclusively uses the &quot;Metadata Framework.&quot; This framework is crucial for managing and describing electronic records, ensuring accurate categorization, classification, and retrieval of records. Metadata enhances the organization and accessibility of records, contributing to effective records management and compliance.</rdfs:comment>
        <owl:annotatedSource rdf:resource="&Governance;ERM_1"/>
        <owl:annotatedTarget rdf:resource="&Governance;Metadata_Framework_1"/>
        <owl:annotatedProperty rdf:resource="&Governance;uses"/>
    </owl:Axiom>
    <owl:Axiom>
        <rdfs:comment>The Electronic Records Management subcategory within the Records Management department uses &quot;Disposition Policies and Procedures&quot; to manage the lifecycle of electronic records. These policies define how electronic records are retained, archived, and eventually disposed of. The focus is on ensuring that electronic records are managed and retained according to established policies, contributing to compliance and efficient information governance.</rdfs:comment>
        <owl:annotatedTarget rdf:resource="&Governance;Disposition_Policies_And_Procedures_1"/>
        <owl:annotatedSource rdf:resource="&Governance;ERM_1"/>
        <owl:annotatedProperty rdf:resource="&Governance;uses"/>
    </owl:Axiom>
    


    <!-- http://www.semanticweb.org/IG/Governance#Early_Case_Assessment_1 -->

    <owl:NamedIndividual rdf:about="&Governance;Early_Case_Assessment_1">
        <rdf:type rdf:resource="&Governance;Early_Case_Assessment"/>
        <Governance:involvesArticle rdf:resource="&Governance;Article_5"/>
    </owl:NamedIndividual>
    


    <!-- http://www.semanticweb.org/IG/Governance#Employee_Engagement_Platforms_1 -->

    <owl:NamedIndividual rdf:about="&Governance;Employee_Engagement_Platforms_1">
        <rdf:type rdf:resource="&Governance;Employee_Engagement_Platforms"/>
        <Governance:involvesArticle rdf:resource="&Governance;Article_39"/>
        <Governance:practicesDefinedInIso rdf:resource="&Governance;ISO_14271"/>
    </owl:NamedIndividual>
    


    <!-- http://www.semanticweb.org/IG/Governance#Employee_Interviews_1 -->

    <owl:NamedIndividual rdf:about="&Governance;Employee_Interviews_1">
        <rdf:type rdf:resource="&Governance;Employee_Interviews"/>
        <Governance:involvesArticle rdf:resource="&Governance;Article_25"/>
        <Governance:involvesArticle rdf:resource="&Governance;Article_5"/>
        <Governance:involvesArticle rdf:resource="&Governance;Article_6"/>
        <Governance:practicesDefinedInIso rdf:resource="&Governance;ISO_15489"/>
        <Governance:practicesDefinedInIso rdf:resource="&Governance;ISO_15939"/>
        <Governance:practicesDefinedInIso rdf:resource="&Governance;ISO_27001"/>
    </owl:NamedIndividual>
    


    <!-- http://www.semanticweb.org/IG/Governance#Employee_Self_Service_Portal_1 -->

    <owl:NamedIndividual rdf:about="&Governance;Employee_Self_Service_Portal_1">
        <rdf:type rdf:resource="&Governance;Employee_Self_Service_Portal"/>
        <Governance:involvesArticle rdf:resource="&Governance;Article_12"/>
        <Governance:involvesArticle rdf:resource="&Governance;Article_5"/>
        <Governance:involvesArticle rdf:resource="&Governance;Article_6"/>
        <Governance:practicesDefinedInIso rdf:resource="&Governance;ISO_15000"/>
    </owl:NamedIndividual>
    


    <!-- http://www.semanticweb.org/IG/Governance#Encryption_1 -->

    <owl:NamedIndividual rdf:about="&Governance;Encryption_1">
        <rdf:type rdf:resource="&Governance;Encryption"/>
        <Governance:involvesArticle rdf:resource="&Governance;Article_32"/>
        <Governance:practicesDefinedInIso rdf:resource="&Governance;ISO_27001"/>
    </owl:NamedIndividual>
    


    <!-- http://www.semanticweb.org/IG/Governance#Enterprise_Risk_Management_1 -->

    <owl:NamedIndividual rdf:about="&Governance;Enterprise_Risk_Management_1">
        <rdf:type rdf:resource="&Governance;Enterprise_Risk_Management"/>
        <Governance:uses rdf:resource="&Governance;Data_Quality_Assurance_Framework_1"/>
        <Governance:canBeInvolvedWith rdf:resource="&Governance;Disposition_Policies_And_Procedures_1"/>
        <Governance:canBeInvolvedWith rdf:resource="&Governance;Document_Management_System_1"/>
    </owl:NamedIndividual>
    <owl:Axiom>
        <rdfs:comment>The Enterprise Risk Management subcategory within the Risk and Compliance department utilizes the &quot;Data Quality Assurance Framework&quot; to assess and manage data-related risks. The framework helps in identifying, measuring, and mitigating risks associated with data quality issues, contributing to the organization&apos;s overall risk management strategy.</rdfs:comment>
        <owl:annotatedTarget rdf:resource="&Governance;Data_Quality_Assurance_Framework_1"/>
        <owl:annotatedSource rdf:resource="&Governance;Enterprise_Risk_Management_1"/>
        <owl:annotatedProperty rdf:resource="&Governance;uses"/>
    </owl:Axiom>
    <owl:Axiom>
        <rdfs:comment>The Enterprise Risk Management subcategory could use the system to manage risk-related documentation, risk assessments, and mitigation plans. Proper document management supports risk assessment processes and ensures historical records for risk management decisions.</rdfs:comment>
        <owl:annotatedTarget rdf:resource="&Governance;Document_Management_System_1"/>
        <owl:annotatedSource rdf:resource="&Governance;Enterprise_Risk_Management_1"/>
        <owl:annotatedProperty rdf:resource="&Governance;canBeInvolvedWith"/>
    </owl:Axiom>
    <owl:Axiom>
        <rdfs:comment>The Enterprise Risk Management subcategory within the Risk and Compliance department is likely involved to assess and mitigate risks associated with data disposition. Inaccurate or improper disposition can lead to legal and compliance risks, data breaches, and unauthorized access. Implementing effective disposition policies and procedures helps manage these risks and ensures proper data handling.</rdfs:comment>
        <owl:annotatedTarget rdf:resource="&Governance;Disposition_Policies_And_Procedures_1"/>
        <owl:annotatedSource rdf:resource="&Governance;Enterprise_Risk_Management_1"/>
        <owl:annotatedProperty rdf:resource="&Governance;canBeInvolvedWith"/>
    </owl:Axiom>
    


    <!-- http://www.semanticweb.org/IG/Governance#Exception_Handling_System_1 -->

    <owl:NamedIndividual rdf:about="&Governance;Exception_Handling_System_1">
        <rdf:type rdf:resource="&Governance;Exception_Handling_System"/>
        <Governance:involvesArticle rdf:resource="&Governance;Article_25"/>
        <Governance:practicesDefinedInIso rdf:resource="&Governance;ISO_17000"/>
    </owl:NamedIndividual>
    


    <!-- http://www.semanticweb.org/IG/Governance#Give_Every_Capability_And_Their_Requirements -->

    <owl:NamedIndividual rdf:about="&Governance;Give_Every_Capability_And_Their_Requirements">
        <rdf:type rdf:resource="&Governance;Query"/>
        <rdfs:comment>Returns every capability, their requirements and what ISOs and GDPR articles are involved.



PREFIX rdf: &lt;http://www.w3.org/1999/02/22-rdf-syntax-ns#&gt;
PREFIX owl: &lt;http://www.w3.org/2002/07/owl#&gt;
PREFIX xsd: &lt;http://www.w3.org/2001/XMLSchema#&gt;
PREFIX rdfs: &lt;http://www.w3.org/2000/01/rdf-schema#&gt;
PREFIX igonto: &lt;http://www.semanticweb.org/IG/Governance#&gt;

SELECT ?maturityLevel ?capability ?description 
       (GROUP_CONCAT(DISTINCT REPLACE(STR(?objectType), &quot;http://www.semanticweb.org/IG/Governance#&quot;, &quot;&quot;) ; SEPARATOR=&quot;, &quot;) AS ?technicalRequirement)
       (GROUP_CONCAT(DISTINCT REPLACE(STR(?ISO), &quot;http://www.semanticweb.org/IG/Governance#&quot;, &quot;&quot;) ; SEPARATOR=&quot;, &quot;) AS ?ISOs)
       (GROUP_CONCAT(DISTINCT REPLACE(STR(?articles), &quot;http://www.semanticweb.org/IG/Governance#&quot;, &quot;&quot;) ; SEPARATOR=&quot;, &quot;) AS ?GDPR_Articles)
       ?framework ?process 
       ?comment
WHERE {
  ?annotation rdf:type owl:Axiom;
              owl:annotatedSource ?capability;
              owl:annotatedProperty igonto:needsTechnicalRequirement ;
              owl:annotatedTarget ?object;
              rdfs:comment ?comment.
  OPTIONAL { ?capability igonto:hasGoal ?goal }.
  ?capability igonto:linkedToFramework ?framework.
  OPTIONAL { ?capability igonto:linkedToProcess ?process }.
  ?capability igonto:capabilityDescription ?description.
  ?capability igonto:inMaturityLevel ?maturityLevel.
  OPTIONAL { ?object a ?objectType }.
  OPTIONAL { ?object igonto:involvesArticle ?articles }.
  OPTIONAL { ?object igonto:practicesDefinedInIso ?ISO }.
  FILTER (?objectType != owl:NamedIndividual)
}
GROUP BY ?maturityLevel ?capability ?framework ?process ?description ?comment</rdfs:comment>
    </owl:NamedIndividual>
    


    <!-- http://www.semanticweb.org/IG/Governance#Hold_Enforcement_Automation_System_1 -->

    <owl:NamedIndividual rdf:about="&Governance;Hold_Enforcement_Automation_System_1">
        <rdf:type rdf:resource="&Governance;Hold_Enforcement_Automation_System"/>
        <Governance:involvesArticle rdf:resource="&Governance;Article_32"/>
        <Governance:practicesDefinedInIso rdf:resource="&Governance;ISO_27001"/>
    </owl:NamedIndividual>
    


    <!-- http://www.semanticweb.org/IG/Governance#IG_Leadership_1 -->

    <owl:NamedIndividual rdf:about="&Governance;IG_Leadership_1">
        <rdf:type rdf:resource="&Governance;IG_Leadership"/>
        <Governance:involvesArticle rdf:resource="&Governance;Article_24"/>
        <Governance:practicesDefinedInIso rdf:resource="&Governance;ISO_15489"/>
    </owl:NamedIndividual>
    


    <!-- http://www.semanticweb.org/IG/Governance#IG_Policy_1 -->

    <owl:NamedIndividual rdf:about="&Governance;IG_Policy_1">
        <rdf:type rdf:resource="&Governance;IG_Policy"/>
        <Governance:involvesArticle rdf:resource="&Governance;Article_12"/>
        <Governance:involvesArticle rdf:resource="&Governance;Article_24"/>
        <Governance:involvesArticle rdf:resource="&Governance;Article_25"/>
        <Governance:involvesArticle rdf:resource="&Governance;Article_30"/>
        <Governance:involvesArticle rdf:resource="&Governance;Article_5"/>
        <Governance:involvesArticle rdf:resource="&Governance;Article_6"/>
        <Governance:practicesDefinedInIso rdf:resource="&Governance;ISO_15489"/>
        <Governance:practicesDefinedInIso rdf:resource="&Governance;ISO_23081"/>
        <Governance:practicesDefinedInIso rdf:resource="&Governance;ISO_27000"/>
        <Governance:practicesDefinedInIso rdf:resource="&Governance;ISO_27001"/>
    </owl:NamedIndividual>
    


    <!-- http://www.semanticweb.org/IG/Governance#IG_Programm_1 -->

    <owl:NamedIndividual rdf:about="&Governance;IG_Programm_1">
        <rdf:type rdf:resource="&Governance;IG_Programm"/>
        <Governance:involvesArticle rdf:resource="&Governance;Article_12"/>
        <Governance:involvesArticle rdf:resource="&Governance;Article_15"/>
        <Governance:involvesArticle rdf:resource="&Governance;Article_24"/>
        <Governance:involvesArticle rdf:resource="&Governance;Article_5"/>
        <Governance:practicesDefinedInIso rdf:resource="&Governance;ISO_15489"/>
        <Governance:practicesDefinedInIso rdf:resource="&Governance;ISO_23081"/>
        <Governance:practicesDefinedInIso rdf:resource="&Governance;ISO_27000"/>
    </owl:NamedIndividual>
    


    <!-- http://www.semanticweb.org/IG/Governance#IG_Strategic_Plan_1 -->

    <owl:NamedIndividual rdf:about="&Governance;IG_Strategic_Plan_1">
        <rdf:type rdf:resource="&Governance;IG_Strategic_Plan"/>
        <Governance:involvesArticle rdf:resource="&Governance;Article_24"/>
        <Governance:involvesArticle rdf:resource="&Governance;Article_5"/>
        <Governance:practicesDefinedInIso rdf:resource="&Governance;ISO_15000"/>
        <Governance:practicesDefinedInIso rdf:resource="&Governance;ISO_15489"/>
        <Governance:practicesDefinedInIso rdf:resource="&Governance;ISO_15939"/>
    </owl:NamedIndividual>
    


    <!-- http://www.semanticweb.org/IG/Governance#INT_1_1_3 -->

    <owl:NamedIndividual rdf:about="&Governance;INT_1_1_3">
        <rdf:type rdf:resource="&Governance;IG_Capability"/>
        <Governance:capabilityDescription>The organization has a formal process to ensure that the required level of authenticity and chain of custody can be applied to its systems and processes.</Governance:capabilityDescription>
        <Governance:inMaturityLevel rdf:resource="&Governance;3_Essential"/>
        <Governance:linkedToFramework rdf:resource="&Governance;ARMA_00"/>
        <Governance:needsTechnicalRequirement rdf:resource="&Governance;AccessControl_1"/>
        <Governance:involvesArticle rdf:resource="&Governance;Article_17"/>
        <Governance:involvesArticle rdf:resource="&Governance;Article_32"/>
        <Governance:involvesArticle rdf:resource="&Governance;Article_5"/>
        <Governance:needsTechnicalRequirement rdf:resource="&Governance;Digital_Signatures_And_Timestamps_1"/>
        <Governance:needsTechnicalRequirement rdf:resource="&Governance;Document_Management_System_1"/>
        <Governance:practicesDefinedInIso rdf:resource="&Governance;ISO_14271"/>
        <Governance:practicesDefinedInIso rdf:resource="&Governance;ISO_15489"/>
        <Governance:practicesDefinedInIso rdf:resource="&Governance;ISO_17000"/>
        <Governance:practicesDefinedInIso rdf:resource="&Governance;ISO_23081"/>
        <Governance:practicesDefinedInIso rdf:resource="&Governance;ISO_27000"/>
        <Governance:practicesDefinedInIso rdf:resource="&Governance;ISO_27001"/>
        <Governance:hasGoal rdf:resource="&Governance;Integrity"/>
    </owl:NamedIndividual>
    <owl:Axiom>
        <rdfs:comment>Implementing strict access controls and maintaining comprehensive logs helps ensure the traceability of who accessed what information and when. This is crucial for maintaining the chain of custody.</rdfs:comment>
        <owl:annotatedTarget rdf:resource="&Governance;AccessControl_1"/>
        <owl:annotatedSource rdf:resource="&Governance;INT_1_1_3"/>
        <owl:annotatedProperty rdf:resource="&Governance;needsTechnicalRequirement"/>
    </owl:Axiom>
    <owl:Axiom>
        <rdfs:comment>A robust DMS helps in maintaining a structured approach to document storage, access, version control, and retention. This supports the chain of custody by ensuring proper handling of documents throughout their lifecycle.</rdfs:comment>
        <owl:annotatedTarget rdf:resource="&Governance;Document_Management_System_1"/>
        <owl:annotatedSource rdf:resource="&Governance;INT_1_1_3"/>
        <owl:annotatedProperty rdf:resource="&Governance;needsTechnicalRequirement"/>
    </owl:Axiom>
    <owl:Axiom>
        <rdfs:comment>Digital signatures and timestamps play a crucial role in ensuring the authenticity and integrity of digital records and transactions. They provide evidence of the origin, identity, and time of creation or modification of digital data.</rdfs:comment>
        <owl:annotatedTarget rdf:resource="&Governance;Digital_Signatures_And_Timestamps_1"/>
        <owl:annotatedSource rdf:resource="&Governance;INT_1_1_3"/>
        <owl:annotatedProperty rdf:resource="&Governance;needsTechnicalRequirement"/>
    </owl:Axiom>
    


    <!-- http://www.semanticweb.org/IG/Governance#INT_1_1_4 -->

    <owl:NamedIndividual rdf:about="&Governance;INT_1_1_4">
        <rdf:type rdf:resource="&Governance;IG_Capability"/>
        <Governance:capabilityDescription>There is a clear definition of metadata requirements for all systems, business applications, and paper records that are needed to ensure the authenticity of records.</Governance:capabilityDescription>
        <Governance:inMaturityLevel rdf:resource="&Governance;4_Proactive"/>
        <Governance:linkedToFramework rdf:resource="&Governance;ARMA_00"/>
        <Governance:involvesArticle rdf:resource="&Governance;Article_30"/>
        <Governance:involvesArticle rdf:resource="&Governance;Article_5"/>
        <Governance:needsTechnicalRequirement rdf:resource="&Governance;Data_Mapping_And_Classification_System_1"/>
        <Governance:practicesDefinedInIso rdf:resource="&Governance;ISO_15489"/>
        <Governance:practicesDefinedInIso rdf:resource="&Governance;ISO_15939"/>
        <Governance:practicesDefinedInIso rdf:resource="&Governance;ISO_17000"/>
        <Governance:practicesDefinedInIso rdf:resource="&Governance;ISO_23081"/>
        <Governance:hasGoal rdf:resource="&Governance;Integrity"/>
        <Governance:needsTechnicalRequirement rdf:resource="&Governance;Metadata_Framework_1"/>
    </owl:NamedIndividual>
    <owl:Axiom>
        <rdfs:comment>Implementing a metadata framework ensures consistent and standardized metadata attributes are defined and associated with all records. Metadata provides context, provenance, and authenticity information essential for ensuring the integrity of records.</rdfs:comment>
        <owl:annotatedSource rdf:resource="&Governance;INT_1_1_4"/>
        <owl:annotatedTarget rdf:resource="&Governance;Metadata_Framework_1"/>
        <owl:annotatedProperty rdf:resource="&Governance;needsTechnicalRequirement"/>
    </owl:Axiom>
    <owl:Axiom>
        <rdfs:comment>Classifying records aids in tracking and authenticating records throughout their lifecycle. This enhances their traceability and ensures their authenticity.
Mapping data elements and cross-referencing records between systems and applications helps maintain the integrity and authenticity of records across different contexts.</rdfs:comment>
        <owl:annotatedTarget rdf:resource="&Governance;Data_Mapping_And_Classification_System_1"/>
        <owl:annotatedSource rdf:resource="&Governance;INT_1_1_4"/>
        <owl:annotatedProperty rdf:resource="&Governance;needsTechnicalRequirement"/>
    </owl:Axiom>
    


    <!-- http://www.semanticweb.org/IG/Governance#INT_1_1_5 -->

    <owl:NamedIndividual rdf:about="&Governance;INT_1_1_5">
        <rdf:type rdf:resource="&Governance;IG_Capability"/>
        <Governance:capabilityDescription>There is a formal, defined process for introducing new record-generating systems and the capture of their metadata and other authenticity requirements, including chain of custody.</Governance:capabilityDescription>
        <Governance:inMaturityLevel rdf:resource="&Governance;5_Transformational"/>
        <Governance:linkedToFramework rdf:resource="&Governance;ARMA_00"/>
        <Governance:involvesArticle rdf:resource="&Governance;Article_30"/>
        <Governance:involvesArticle rdf:resource="&Governance;Article_5"/>
        <Governance:needsTechnicalRequirement rdf:resource="&Governance;Chain_Of_Custody_Tracking_1"/>
        <Governance:needsTechnicalRequirement rdf:resource="&Governance;Data_Quality_Assurance_Framework_1"/>
        <Governance:practicesDefinedInIso rdf:resource="&Governance;ISO_15489"/>
        <Governance:practicesDefinedInIso rdf:resource="&Governance;ISO_17000"/>
        <Governance:practicesDefinedInIso rdf:resource="&Governance;ISO_23081"/>
        <Governance:hasGoal rdf:resource="&Governance;Integrity"/>
    </owl:NamedIndividual>
    <owl:Axiom>
        <rdfs:comment>Implement a mechanism for capturing and tracking the chain of custody information as records move through different stages and systems. This ensures the ability to demonstrate the authenticity and integrity of records throughout their lifecycle.</rdfs:comment>
        <owl:annotatedTarget rdf:resource="&Governance;Chain_Of_Custody_Tracking_1"/>
        <owl:annotatedSource rdf:resource="&Governance;INT_1_1_5"/>
        <owl:annotatedProperty rdf:resource="&Governance;needsTechnicalRequirement"/>
    </owl:Axiom>
    <owl:Axiom>
        <rdfs:comment>Implement processes for validating and ensuring the quality of captured metadata, including authenticity attributes. Metadata must remain accurate and consistent to support the authenticity of records.</rdfs:comment>
        <owl:annotatedTarget rdf:resource="&Governance;Data_Quality_Assurance_Framework_1"/>
        <owl:annotatedSource rdf:resource="&Governance;INT_1_1_5"/>
        <owl:annotatedProperty rdf:resource="&Governance;needsTechnicalRequirement"/>
    </owl:Axiom>
    


    <!-- http://www.semanticweb.org/IG/Governance#INT_1_2_3 -->

    <owl:NamedIndividual rdf:about="&Governance;INT_1_2_3">
        <rdf:type rdf:resource="&Governance;IG_Capability"/>
        <Governance:capabilityDescription>Appropriate data elements to demonstrate compliance with the policy are captured.</Governance:capabilityDescription>
        <Governance:inMaturityLevel rdf:resource="&Governance;3_Essential"/>
        <Governance:linkedToFramework rdf:resource="&Governance;ARMA_00"/>
        <Governance:involvesArticle rdf:resource="&Governance;Article_24"/>
        <Governance:involvesArticle rdf:resource="&Governance;Article_5"/>
        <Governance:needsTechnicalRequirement rdf:resource="&Governance;Data_Mapping_And_Classification_System_1"/>
        <Governance:practicesDefinedInIso rdf:resource="&Governance;ISO_15489"/>
        <Governance:practicesDefinedInIso rdf:resource="&Governance;ISO_15939"/>
        <Governance:practicesDefinedInIso rdf:resource="&Governance;ISO_17000"/>
        <Governance:practicesDefinedInIso rdf:resource="&Governance;ISO_23081"/>
        <Governance:hasGoal rdf:resource="&Governance;Integrity"/>
        <Governance:needsTechnicalRequirement rdf:resource="&Governance;Metadata_Framework_1"/>
    </owl:NamedIndividual>
    <owl:Axiom>
        <rdfs:comment>Properly classifying and mapping data elements according to their sensitivity and purpose aids in demonstrating compliance with data handling policies and GDPR principles.</rdfs:comment>
        <owl:annotatedTarget rdf:resource="&Governance;Data_Mapping_And_Classification_System_1"/>
        <owl:annotatedSource rdf:resource="&Governance;INT_1_2_3"/>
        <owl:annotatedProperty rdf:resource="&Governance;needsTechnicalRequirement"/>
    </owl:Axiom>
    <owl:Axiom>
        <rdfs:comment>A comprehensive metadata framework is crucial for capturing and managing relevant data elements that demonstrate compliance. Metadata provides context to data, enabling proper classification, searchability, and tracking of data in line with organizational policies.</rdfs:comment>
        <owl:annotatedSource rdf:resource="&Governance;INT_1_2_3"/>
        <owl:annotatedTarget rdf:resource="&Governance;Metadata_Framework_1"/>
        <owl:annotatedProperty rdf:resource="&Governance;needsTechnicalRequirement"/>
    </owl:Axiom>
    


    <!-- http://www.semanticweb.org/IG/Governance#INT_1_2_4 -->

    <owl:NamedIndividual rdf:about="&Governance;INT_1_2_4">
        <rdf:type rdf:resource="&Governance;IG_Capability"/>
        <Governance:capabilityDescription>Metadata requirements include security and signature requirements and chain of custody as needed to demonstrate authenticity.</Governance:capabilityDescription>
        <Governance:inMaturityLevel rdf:resource="&Governance;4_Proactive"/>
        <Governance:linkedToFramework rdf:resource="&Governance;ARMA_00"/>
        <Governance:involvesArticle rdf:resource="&Governance;Article_30"/>
        <Governance:involvesArticle rdf:resource="&Governance;Article_32"/>
        <Governance:involvesArticle rdf:resource="&Governance;Article_5"/>
        <Governance:needsTechnicalRequirement rdf:resource="&Governance;Chain_Of_Custody_Tracking_1"/>
        <Governance:needsTechnicalRequirement rdf:resource="&Governance;Digital_Signatures_And_Timestamps_1"/>
        <Governance:practicesDefinedInIso rdf:resource="&Governance;ISO_14271"/>
        <Governance:practicesDefinedInIso rdf:resource="&Governance;ISO_15489"/>
        <Governance:practicesDefinedInIso rdf:resource="&Governance;ISO_15939"/>
        <Governance:practicesDefinedInIso rdf:resource="&Governance;ISO_23081"/>
        <Governance:practicesDefinedInIso rdf:resource="&Governance;ISO_27000"/>
        <Governance:practicesDefinedInIso rdf:resource="&Governance;ISO_27001"/>
        <Governance:hasGoal rdf:resource="&Governance;Integrity"/>
    </owl:NamedIndividual>
    <owl:Axiom>
        <rdfs:comment>Integrating digital signatures within metadata supports the ability to verify the authenticity and integrity of records over time. Digital signatures provide a strong mechanism for ensuring the validity of records.</rdfs:comment>
        <owl:annotatedTarget rdf:resource="&Governance;Digital_Signatures_And_Timestamps_1"/>
        <owl:annotatedSource rdf:resource="&Governance;INT_1_2_4"/>
        <owl:annotatedProperty rdf:resource="&Governance;needsTechnicalRequirement"/>
    </owl:Axiom>
    <owl:Axiom>
        <rdfs:comment>Implementing a mechanism for tracking the chain of custody ensures that the record&apos;s journey from creation to storage is documented and verifiable. This is crucial for demonstrating authenticity and maintaining data integrity.</rdfs:comment>
        <owl:annotatedTarget rdf:resource="&Governance;Chain_Of_Custody_Tracking_1"/>
        <owl:annotatedSource rdf:resource="&Governance;INT_1_2_4"/>
        <owl:annotatedProperty rdf:resource="&Governance;needsTechnicalRequirement"/>
    </owl:Axiom>
    


    <!-- http://www.semanticweb.org/IG/Governance#INT_1_2_5 -->

    <owl:NamedIndividual rdf:about="&Governance;INT_1_2_5">
        <rdf:type rdf:resource="&Governance;IG_Capability"/>
        <Governance:capabilityDescription>This level is easily and regularly audited.</Governance:capabilityDescription>
        <Governance:inMaturityLevel rdf:resource="&Governance;5_Transformational"/>
        <Governance:linkedToFramework rdf:resource="&Governance;ARMA_00"/>
        <Governance:needsTechnicalRequirement rdf:resource="&Governance;AccessControl_1"/>
        <Governance:involvesArticle rdf:resource="&Governance;Article_30"/>
        <Governance:involvesArticle rdf:resource="&Governance;Article_32"/>
        <Governance:involvesArticle rdf:resource="&Governance;Article_5"/>
        <Governance:needsTechnicalRequirement rdf:resource="&Governance;Audit_1"/>
        <Governance:practicesDefinedInIso rdf:resource="&Governance;ISO_15489"/>
        <Governance:practicesDefinedInIso rdf:resource="&Governance;ISO_15939"/>
        <Governance:practicesDefinedInIso rdf:resource="&Governance;ISO_27000"/>
        <Governance:practicesDefinedInIso rdf:resource="&Governance;ISO_27001"/>
        <Governance:hasGoal rdf:resource="&Governance;Integrity"/>
    </owl:NamedIndividual>
    <owl:Axiom>
        <rdfs:comment> Implement an audit trail mechanism that captures relevant activities, changes, and access to records and their metadata. This enables easy monitoring and tracking of actions related to records, supporting transparency, accountability, and auditability.</rdfs:comment>
        <owl:annotatedTarget rdf:resource="&Governance;Audit_1"/>
        <owl:annotatedSource rdf:resource="&Governance;INT_1_2_5"/>
        <owl:annotatedProperty rdf:resource="&Governance;needsTechnicalRequirement"/>
    </owl:Axiom>
    <owl:Axiom>
        <rdfs:comment>Implement access controls and authorization mechanisms to ensure that only authorized individuals have access to records and their metadata. This safeguards the integrity of records and supports auditability.</rdfs:comment>
        <owl:annotatedTarget rdf:resource="&Governance;AccessControl_1"/>
        <owl:annotatedSource rdf:resource="&Governance;INT_1_2_5"/>
        <owl:annotatedProperty rdf:resource="&Governance;needsTechnicalRequirement"/>
    </owl:Axiom>
    


    <!-- http://www.semanticweb.org/IG/Governance#INT_1_3_3 -->

    <owl:NamedIndividual rdf:about="&Governance;INT_1_3_3">
        <rdf:type rdf:resource="&Governance;IG_Capability"/>
        <Governance:capabilityDescription>The organization has defined specific goals related to integrity.</Governance:capabilityDescription>
        <Governance:inMaturityLevel rdf:resource="&Governance;3_Essential"/>
        <Governance:linkedToFramework rdf:resource="&Governance;ARMA_00"/>
        <Governance:needsTechnicalRequirement rdf:resource="&Governance;AccessControl_1"/>
        <Governance:involvesArticle rdf:resource="&Governance;Article_24"/>
        <Governance:involvesArticle rdf:resource="&Governance;Article_5"/>
        <Governance:needsTechnicalRequirement rdf:resource="&Governance;Audit_1"/>
        <Governance:needsTechnicalRequirement rdf:resource="&Governance;Data_Quality_Management_1"/>
        <Governance:practicesDefinedInIso rdf:resource="&Governance;ISO_14271"/>
        <Governance:practicesDefinedInIso rdf:resource="&Governance;ISO_15489"/>
        <Governance:practicesDefinedInIso rdf:resource="&Governance;ISO_15939"/>
        <Governance:practicesDefinedInIso rdf:resource="&Governance;ISO_17000"/>
        <Governance:practicesDefinedInIso rdf:resource="&Governance;ISO_23081"/>
        <Governance:practicesDefinedInIso rdf:resource="&Governance;ISO_27000"/>
        <Governance:practicesDefinedInIso rdf:resource="&Governance;ISO_27001"/>
        <Governance:hasGoal rdf:resource="&Governance;Integrity"/>
        <Governance:needsTechnicalRequirement rdf:resource="&Governance;Monitoring_1"/>
    </owl:NamedIndividual>
    <owl:Axiom>
        <rdfs:comment>Implementing access controls ensures that the organization&apos;s data remains accurate, consistent, and unaltered. These controls prevent unauthorized changes, corruption, or tampering of data, supporting the achievement of specific integrity goals.</rdfs:comment>
        <owl:annotatedTarget rdf:resource="&Governance;AccessControl_1"/>
        <owl:annotatedSource rdf:resource="&Governance;INT_1_3_3"/>
        <owl:annotatedProperty rdf:resource="&Governance;needsTechnicalRequirement"/>
    </owl:Axiom>
    <owl:Axiom>
        <rdfs:comment>Proper data quality management processes ensure that data is accurate, reliable, and fit for its intended purpose. Defining integrity goals requires consistent data quality assessments, validations, and cleansing.</rdfs:comment>
        <owl:annotatedTarget rdf:resource="&Governance;Data_Quality_Management_1"/>
        <owl:annotatedSource rdf:resource="&Governance;INT_1_3_3"/>
        <owl:annotatedProperty rdf:resource="&Governance;needsTechnicalRequirement"/>
    </owl:Axiom>
    <owl:Axiom>
        <rdfs:comment>Regular monitoring of data processes and systems are essential to ensure that integrity goals are met and maintained over time. It provides visibility into data handling practices and identifies any deviations from established integrity standards.</rdfs:comment>
        <owl:annotatedSource rdf:resource="&Governance;INT_1_3_3"/>
        <owl:annotatedTarget rdf:resource="&Governance;Monitoring_1"/>
        <owl:annotatedProperty rdf:resource="&Governance;needsTechnicalRequirement"/>
    </owl:Axiom>
    <owl:Axiom>
        <rdfs:comment>Regular auditing of data processes and systems are essential to ensure that integrity goals are met and maintained over time. It provides visibility into data handling practices and identifies any deviations from established integrity standards.</rdfs:comment>
        <owl:annotatedTarget rdf:resource="&Governance;Audit_1"/>
        <owl:annotatedSource rdf:resource="&Governance;INT_1_3_3"/>
        <owl:annotatedProperty rdf:resource="&Governance;needsTechnicalRequirement"/>
    </owl:Axiom>
    


    <!-- http://www.semanticweb.org/IG/Governance#INT_1_3_4 -->

    <owl:NamedIndividual rdf:about="&Governance;INT_1_3_4">
        <rdf:type rdf:resource="&Governance;IG_Capability"/>
        <Governance:capabilityDescription>The metadata definition process is an integral part of the records management practice in the organization.</Governance:capabilityDescription>
        <Governance:inMaturityLevel rdf:resource="&Governance;4_Proactive"/>
        <Governance:linkedToFramework rdf:resource="&Governance;ARMA_00"/>
        <Governance:involvesArticle rdf:resource="&Governance;Article_30"/>
        <Governance:involvesArticle rdf:resource="&Governance;Article_5"/>
        <Governance:practicesDefinedInIso rdf:resource="&Governance;ISO_15489"/>
        <Governance:practicesDefinedInIso rdf:resource="&Governance;ISO_15939"/>
        <Governance:practicesDefinedInIso rdf:resource="&Governance;ISO_17000"/>
        <Governance:practicesDefinedInIso rdf:resource="&Governance;ISO_23081"/>
        <Governance:hasGoal rdf:resource="&Governance;Integrity"/>
        <Governance:needsTechnicalRequirement rdf:resource="&Governance;Metadata_1"/>
        <Governance:needsTechnicalRequirement rdf:resource="&Governance;Records_Information_Management_1"/>
    </owl:NamedIndividual>
    <owl:Axiom>
        <rdfs:comment>Integrating the metadata schema with the organization&apos;s records management system ensures that metadata is consistently captured, updated, and accessible throughout the records&apos; lifecycle. This integration enhances records management practices and supports compliance with GDPR&apos;s requirements for data minimization and accurate records.</rdfs:comment>
        <owl:annotatedSource rdf:resource="&Governance;INT_1_3_4"/>
        <owl:annotatedTarget rdf:resource="&Governance;Records_Information_Management_1"/>
        <owl:annotatedProperty rdf:resource="&Governance;needsTechnicalRequirement"/>
    </owl:Axiom>
    <owl:Axiom>
        <rdfs:comment>Developing a comprehensive metadata schema that includes attributes relevant to records management ensures that essential information is captured and associated with records. This metadata schema provides the context, classification, and management details required for effective records management.</rdfs:comment>
        <owl:annotatedSource rdf:resource="&Governance;INT_1_3_4"/>
        <owl:annotatedTarget rdf:resource="&Governance;Metadata_1"/>
        <owl:annotatedProperty rdf:resource="&Governance;needsTechnicalRequirement"/>
    </owl:Axiom>
    


    <!-- http://www.semanticweb.org/IG/Governance#INT_1_3_5 -->

    <owl:NamedIndividual rdf:about="&Governance;INT_1_3_5">
        <rdf:type rdf:resource="&Governance;IG_Capability"/>
        <Governance:capabilityDescription>The organization’s stated goals related to integrity have been met. The organization can consistently and confidently demonstrate the accuracy and authenticity of its records.</Governance:capabilityDescription>
        <Governance:inMaturityLevel rdf:resource="&Governance;5_Transformational"/>
        <Governance:linkedToFramework rdf:resource="&Governance;ARMA_00"/>
        <Governance:involvesArticle rdf:resource="&Governance;Article_32"/>
        <Governance:involvesArticle rdf:resource="&Governance;Article_5"/>
        <Governance:needsTechnicalRequirement rdf:resource="&Governance;Data_Quality_Assurance_Framework_1"/>
        <Governance:needsTechnicalRequirement rdf:resource="&Governance;Digital_Signatures_And_Timestamps_1"/>
        <Governance:practicesDefinedInIso rdf:resource="&Governance;ISO_14271"/>
        <Governance:practicesDefinedInIso rdf:resource="&Governance;ISO_27000"/>
        <Governance:practicesDefinedInIso rdf:resource="&Governance;ISO_27001"/>
        <Governance:hasGoal rdf:resource="&Governance;Integrity"/>
    </owl:NamedIndividual>
    <owl:Axiom>
        <rdfs:comment> Integrate digital signatures within record systems to provide an additional layer of authenticity and tamper-evident protection. This enhances confidence in the accuracy and authenticity of records.</rdfs:comment>
        <owl:annotatedTarget rdf:resource="&Governance;Digital_Signatures_And_Timestamps_1"/>
        <owl:annotatedSource rdf:resource="&Governance;INT_1_3_5"/>
        <owl:annotatedProperty rdf:resource="&Governance;needsTechnicalRequirement"/>
    </owl:Axiom>
    <owl:Axiom>
        <rdfs:comment>Implement automated data validation mechanisms to ensure the accuracy and integrity of records. This involves real-time or batch validation of data against predefined rules or standards, minimizing the risk of errors and ensuring compliance with stated integrity goals.</rdfs:comment>
        <owl:annotatedTarget rdf:resource="&Governance;Data_Quality_Assurance_Framework_1"/>
        <owl:annotatedSource rdf:resource="&Governance;INT_1_3_5"/>
        <owl:annotatedProperty rdf:resource="&Governance;needsTechnicalRequirement"/>
    </owl:Axiom>
    


    <!-- http://www.semanticweb.org/IG/Governance#ISACA_COBIT -->

    <owl:NamedIndividual rdf:about="&Governance;ISACA_COBIT">
        <rdf:type rdf:resource="&Governance;Framework"/>
    </owl:NamedIndividual>
    


    <!-- http://www.semanticweb.org/IG/Governance#ISO_14271 -->

    <owl:NamedIndividual rdf:about="&Governance;ISO_14271">
        <rdf:type rdf:resource="&Governance;ISO"/>
    </owl:NamedIndividual>
    


    <!-- http://www.semanticweb.org/IG/Governance#ISO_15000 -->

    <owl:NamedIndividual rdf:about="&Governance;ISO_15000">
        <rdf:type rdf:resource="&Governance;ISO"/>
    </owl:NamedIndividual>
    


    <!-- http://www.semanticweb.org/IG/Governance#ISO_15489 -->

    <owl:NamedIndividual rdf:about="&Governance;ISO_15489">
        <rdf:type rdf:resource="&Governance;ISO"/>
    </owl:NamedIndividual>
    


    <!-- http://www.semanticweb.org/IG/Governance#ISO_15926 -->

    <owl:NamedIndividual rdf:about="&Governance;ISO_15926">
        <rdf:type rdf:resource="&Governance;ISO"/>
    </owl:NamedIndividual>
    


    <!-- http://www.semanticweb.org/IG/Governance#ISO_15939 -->

    <owl:NamedIndividual rdf:about="&Governance;ISO_15939">
        <rdf:type rdf:resource="&Governance;ISO"/>
    </owl:NamedIndividual>
    


    <!-- http://www.semanticweb.org/IG/Governance#ISO_17000 -->

    <owl:NamedIndividual rdf:about="&Governance;ISO_17000">
        <rdf:type rdf:resource="&Governance;ISO"/>
    </owl:NamedIndividual>
    


    <!-- http://www.semanticweb.org/IG/Governance#ISO_22301 -->

    <owl:NamedIndividual rdf:about="&Governance;ISO_22301">
        <rdf:type rdf:resource="&Governance;ISO"/>
    </owl:NamedIndividual>
    


    <!-- http://www.semanticweb.org/IG/Governance#ISO_23081 -->

    <owl:NamedIndividual rdf:about="&Governance;ISO_23081">
        <rdf:type rdf:resource="&Governance;ISO"/>
    </owl:NamedIndividual>
    


    <!-- http://www.semanticweb.org/IG/Governance#ISO_27000 -->

    <owl:NamedIndividual rdf:about="&Governance;ISO_27000">
        <rdf:type rdf:resource="&Governance;ISO"/>
    </owl:NamedIndividual>
    


    <!-- http://www.semanticweb.org/IG/Governance#ISO_27001 -->

    <owl:NamedIndividual rdf:about="&Governance;ISO_27001">
        <rdf:type rdf:resource="&Governance;ISO"/>
    </owl:NamedIndividual>
    


    <!-- http://www.semanticweb.org/IG/Governance#ISO_27002 -->

    <owl:NamedIndividual rdf:about="&Governance;ISO_27002">
        <rdf:type rdf:resource="&Governance;ISO"/>
    </owl:NamedIndividual>
    


    <!-- http://www.semanticweb.org/IG/Governance#ISO_27010 -->

    <owl:NamedIndividual rdf:about="&Governance;ISO_27010">
        <rdf:type rdf:resource="&Governance;ISO"/>
    </owl:NamedIndividual>
    


    <!-- http://www.semanticweb.org/IG/Governance#ISO_27017 -->

    <owl:NamedIndividual rdf:about="&Governance;ISO_27017">
        <rdf:type rdf:resource="&Governance;ISO"/>
    </owl:NamedIndividual>
    


    <!-- http://www.semanticweb.org/IG/Governance#ISO_27050 -->

    <owl:NamedIndividual rdf:about="&Governance;ISO_27050">
        <rdf:type rdf:resource="&Governance;ISO"/>
    </owl:NamedIndividual>
    


    <!-- http://www.semanticweb.org/IG/Governance#ISO_8000 -->

    <owl:NamedIndividual rdf:about="&Governance;ISO_8000">
        <rdf:type rdf:resource="&Governance;ISO"/>
    </owl:NamedIndividual>
    


    <!-- http://www.semanticweb.org/IG/Governance#IT_P1_3 -->

    <owl:NamedIndividual rdf:about="&Governance;IT_P1_3">
        <rdf:type rdf:resource="&Governance;IG_Capability"/>
        <Governance:capabilityDescription>IT maintains an asset database for ist use; IT manually enters legal holds, business liaison and retention rules for each asset/ system. Legal maintains its own data map for eDiscovery purposes.</Governance:capabilityDescription>
        <Governance:inMaturityLevel rdf:resource="&Governance;3_Essential"/>
        <Governance:involvesArticle rdf:resource="&Governance;Article_30"/>
        <Governance:involvesArticle rdf:resource="&Governance;Article_32"/>
        <Governance:involvesArticle rdf:resource="&Governance;Article_5"/>
        <Governance:needsTechnicalRequirement rdf:resource="&Governance;Asset_Database_1"/>
        <Governance:linkedToFramework rdf:resource="&Governance;CGOC_02"/>
        <Governance:needsTechnicalRequirement rdf:resource="&Governance;Data_Mapping_And_Classification_System_1"/>
        <Governance:practicesDefinedInIso rdf:resource="&Governance;ISO_15926"/>
        <Governance:practicesDefinedInIso rdf:resource="&Governance;ISO_27001"/>
        <Governance:practicesDefinedInIso rdf:resource="&Governance;ISO_27050"/>
        <Governance:needsTechnicalRequirement rdf:resource="&Governance;Legal_Hold_Management_1"/>
        <Governance:linkedToProcess rdf:resource="&Governance;Process_Data_Source_Catalog_And_Stewardship_1"/>
        <Governance:needsTechnicalRequirement rdf:resource="&Governance;Retention_Rule_Management_System_1"/>
        <Governance:needsTechnicalRequirement rdf:resource="&Governance;eDiscovery_Integration_1"/>
    </owl:NamedIndividual>
    <owl:Axiom>
        <rdfs:comment>Establish an integrated asset database that includes all relevant information about IT assets and systems. This database should serve as a central repository for asset-related data.</rdfs:comment>
        <owl:annotatedTarget rdf:resource="&Governance;Asset_Database_1"/>
        <owl:annotatedSource rdf:resource="&Governance;IT_P1_3"/>
        <owl:annotatedProperty rdf:resource="&Governance;needsTechnicalRequirement"/>
    </owl:Axiom>
    <owl:Axiom>
        <rdfs:comment>Implement a retention rule management system that allows for the definition and enforcement of data retention rules for each asset and system.</rdfs:comment>
        <owl:annotatedSource rdf:resource="&Governance;IT_P1_3"/>
        <owl:annotatedTarget rdf:resource="&Governance;Retention_Rule_Management_System_1"/>
        <owl:annotatedProperty rdf:resource="&Governance;needsTechnicalRequirement"/>
    </owl:Axiom>
    <owl:Axiom>
        <rdfs:comment>Integrate the data map and asset database with eDiscovery tools and processes to facilitate legal discovery and compliance with legal requirements.</rdfs:comment>
        <owl:annotatedSource rdf:resource="&Governance;IT_P1_3"/>
        <owl:annotatedTarget rdf:resource="&Governance;eDiscovery_Integration_1"/>
        <owl:annotatedProperty rdf:resource="&Governance;needsTechnicalRequirement"/>
    </owl:Axiom>
    <owl:Axiom>
        <rdfs:comment>Develop a data mapping and classification system that categorizes data based on its sensitivity and importance. This system is essential for understanding and managing data.</rdfs:comment>
        <owl:annotatedTarget rdf:resource="&Governance;Data_Mapping_And_Classification_System_1"/>
        <owl:annotatedSource rdf:resource="&Governance;IT_P1_3"/>
        <owl:annotatedProperty rdf:resource="&Governance;needsTechnicalRequirement"/>
    </owl:Axiom>
    <owl:Axiom>
        <rdfs:comment> Implement an automated legal hold system that can manage and enforce legal holds on IT assets and systems. This system should ensure that assets are preserved when required for legal purposes.</rdfs:comment>
        <owl:annotatedSource rdf:resource="&Governance;IT_P1_3"/>
        <owl:annotatedTarget rdf:resource="&Governance;Legal_Hold_Management_1"/>
        <owl:annotatedProperty rdf:resource="&Governance;needsTechnicalRequirement"/>
    </owl:Axiom>
    


    <!-- http://www.semanticweb.org/IG/Governance#IT_P1_4 -->

    <owl:NamedIndividual rdf:about="&Governance;IT_P1_4">
        <rdf:type rdf:resource="&Governance;IG_Capability"/>
        <Governance:capabilityDescription>Shared data source catalog across IT, legal, records and business stakeholders which is used to express information assets and relevant business needs and legal obligations. Catalog as source of truth for provisioning and back up retention/ disposition requirements and all back up, archiving and provisioning procedures and decisions are transparent in the catalog. Common definitions are used to describe duties, needs, stewards, employees, laws and lawsuits across ILM&amp;G stakeholders.</Governance:capabilityDescription>
        <Governance:inMaturityLevel rdf:resource="&Governance;4_Proactive"/>
        <Governance:involvesArticle rdf:resource="&Governance;Article_30"/>
        <Governance:involvesArticle rdf:resource="&Governance;Article_32"/>
        <Governance:involvesArticle rdf:resource="&Governance;Article_5"/>
        <Governance:linkedToFramework rdf:resource="&Governance;CGOC_02"/>
        <Governance:needsTechnicalRequirement rdf:resource="&Governance;Centralized_Data_Source_Catalog_1"/>
        <Governance:practicesDefinedInIso rdf:resource="&Governance;ISO_15489"/>
        <Governance:practicesDefinedInIso rdf:resource="&Governance;ISO_23081"/>
        <Governance:needsTechnicalRequirement rdf:resource="&Governance;Metadata_Framework_1"/>
        <Governance:linkedToProcess rdf:resource="&Governance;Process_Data_Source_Catalog_And_Stewardship_1"/>
    </owl:NamedIndividual>
    <owl:Axiom>
        <rdfs:comment> Establishing common definitions for terms related to data governance, such as roles, responsibilities, and legal requirements, promotes clear communication and a shared understanding among stakeholders.</rdfs:comment>
        <owl:annotatedSource rdf:resource="&Governance;IT_P1_4"/>
        <owl:annotatedTarget rdf:resource="&Governance;Metadata_Framework_1"/>
        <owl:annotatedProperty rdf:resource="&Governance;needsTechnicalRequirement"/>
    </owl:Axiom>
    <owl:Axiom>
        <rdfs:comment>A centralized data source catalog is crucial for maintaining a comprehensive inventory of data assets, including their location, structure, and ownership. It provides a single point of reference for stakeholders to access accurate information about data resources.</rdfs:comment>
        <owl:annotatedTarget rdf:resource="&Governance;Centralized_Data_Source_Catalog_1"/>
        <owl:annotatedSource rdf:resource="&Governance;IT_P1_4"/>
        <owl:annotatedProperty rdf:resource="&Governance;needsTechnicalRequirement"/>
    </owl:Axiom>
    


    <!-- http://www.semanticweb.org/IG/Governance#IT_P2_3 -->

    <owl:NamedIndividual rdf:about="&Governance;IT_P2_3">
        <rdf:type rdf:resource="&Governance;IG_Capability"/>
        <Governance:capabilityDescription>Some systems are configured to retain, dispose, preserve and collect data but schedules and instructions are manually applied and configured. Instructions from legal, records and the business on duties and values are communicated in disparate tools and techniques and must be reconciled within IT.</Governance:capabilityDescription>
        <Governance:inMaturityLevel rdf:resource="&Governance;3_Essential"/>
        <Governance:involvesArticle rdf:resource="&Governance;Article_25"/>
        <Governance:involvesArticle rdf:resource="&Governance;Article_5"/>
        <Governance:needsTechnicalRequirement rdf:resource="&Governance;Automated_Data_Retention_And_Disposa_1"/>
        <Governance:linkedToFramework rdf:resource="&Governance;CGOC_02"/>
        <Governance:needsTechnicalRequirement rdf:resource="&Governance;Centralized_Instructions_Repository_1"/>
        <Governance:practicesDefinedInIso rdf:resource="&Governance;ISO_15489"/>
        <Governance:practicesDefinedInIso rdf:resource="&Governance;ISO_23081"/>
        <Governance:practicesDefinedInIso rdf:resource="&Governance;ISO_27001"/>
        <Governance:needsTechnicalRequirement rdf:resource="&Governance;Legal_Hold_Management_1"/>
        <Governance:linkedToProcess rdf:resource="&Governance;Process_System_Provisioning_1"/>
    </owl:NamedIndividual>
    <owl:Axiom>
        <rdfs:comment>Automated data retention and disposal capabilities are essential for systematically managing data throughout its lifecycle, ensuring compliance with data retention policies, and reducing the risk of retaining data longer than necessary.</rdfs:comment>
        <owl:annotatedTarget rdf:resource="&Governance;Automated_Data_Retention_And_Disposa_1"/>
        <owl:annotatedSource rdf:resource="&Governance;IT_P2_3"/>
        <owl:annotatedProperty rdf:resource="&Governance;needsTechnicalRequirement"/>
    </owl:Axiom>
    <owl:Axiom>
        <rdfs:comment>A centralized repository for legal, records, and business instructions is crucial for ensuring that duties and values related to data retention and disposal are effectively communicated, reconciled, and applied across IT systems.</rdfs:comment>
        <owl:annotatedTarget rdf:resource="&Governance;Centralized_Instructions_Repository_1"/>
        <owl:annotatedSource rdf:resource="&Governance;IT_P2_3"/>
        <owl:annotatedProperty rdf:resource="&Governance;needsTechnicalRequirement"/>
    </owl:Axiom>
    <owl:Axiom>
        <rdfs:comment>Integration with legal and records management systems allows for seamless communication and alignment of instructions and requirements with IT provisioning processes.</rdfs:comment>
        <owl:annotatedSource rdf:resource="&Governance;IT_P2_3"/>
        <owl:annotatedTarget rdf:resource="&Governance;Legal_Hold_Management_1"/>
        <owl:annotatedProperty rdf:resource="&Governance;needsTechnicalRequirement"/>
    </owl:Axiom>
    


    <!-- http://www.semanticweb.org/IG/Governance#IT_P2_4 -->

    <owl:NamedIndividual rdf:about="&Governance;IT_P2_4">
        <rdf:type rdf:resource="&Governance;IG_Capability"/>
        <Governance:capabilityDescription>Systems are provisioned with protocol and technical capability to retain/dispose and hold/collect, including a properly authorized retention schedule and business value inventory. Systems are provisioned with the capability to archive data to lower cost storage at the earliest point in time, archive procedures are well defined and archives execute retention/ disposition of approved schedules. Back up is used for disaster recovery only and does not function as long term archive. Retention schedules, legal holds and collection requests are systematically propagated from their respective initiators; data source catalog is updated to reflect the provisioning, archiving and back up mechanism.</Governance:capabilityDescription>
        <Governance:inMaturityLevel rdf:resource="&Governance;4_Proactive"/>
        <Governance:involvesArticle rdf:resource="&Governance;Article_25"/>
        <Governance:involvesArticle rdf:resource="&Governance;Article_30"/>
        <Governance:involvesArticle rdf:resource="&Governance;Article_5"/>
        <Governance:needsTechnicalRequirement rdf:resource="&Governance;Automated_Data_Retention_And_Disposa_1"/>
        <Governance:needsTechnicalRequirement rdf:resource="&Governance;Backup_1"/>
        <Governance:linkedToFramework rdf:resource="&Governance;CGOC_02"/>
        <Governance:needsTechnicalRequirement rdf:resource="&Governance;Centralized_Data_Source_Catalog_1"/>
        <Governance:practicesDefinedInIso rdf:resource="&Governance;ISO_15489"/>
        <Governance:practicesDefinedInIso rdf:resource="&Governance;ISO_22301"/>
        <Governance:practicesDefinedInIso rdf:resource="&Governance;ISO_23081"/>
        <Governance:practicesDefinedInIso rdf:resource="&Governance;ISO_8000"/>
        <Governance:linkedToProcess rdf:resource="&Governance;Process_System_Provisioning_1"/>
        <Governance:needsTechnicalRequirement rdf:resource="&Governance;Records_Retention_Schedule_1"/>
    </owl:NamedIndividual>
    <owl:Axiom>
        <rdfs:comment>Maintain an updated data source catalog to accurately inventory data sources and their attributes.</rdfs:comment>
        <owl:annotatedTarget rdf:resource="&Governance;Centralized_Data_Source_Catalog_1"/>
        <owl:annotatedSource rdf:resource="&Governance;IT_P2_4"/>
        <owl:annotatedProperty rdf:resource="&Governance;needsTechnicalRequirement"/>
    </owl:Axiom>
    <owl:Axiom>
        <rdfs:comment> Implement backup systems for disaster recovery and business continuity to ensure data availability.</rdfs:comment>
        <owl:annotatedTarget rdf:resource="&Governance;Backup_1"/>
        <owl:annotatedSource rdf:resource="&Governance;IT_P2_4"/>
        <owl:annotatedProperty rdf:resource="&Governance;needsTechnicalRequirement"/>
    </owl:Axiom>
    <owl:Axiom>
        <rdfs:comment> Ensure the systematic propagation of retention schedules and legal holds for consistent data management.</rdfs:comment>
        <owl:annotatedSource rdf:resource="&Governance;IT_P2_4"/>
        <owl:annotatedTarget rdf:resource="&Governance;Records_Retention_Schedule_1"/>
        <owl:annotatedProperty rdf:resource="&Governance;needsTechnicalRequirement"/>
    </owl:Axiom>
    <owl:Axiom>
        <rdfs:comment>Implement a comprehensive data retention and disposal capability to manage data throughout its lifecycle.</rdfs:comment>
        <owl:annotatedTarget rdf:resource="&Governance;Automated_Data_Retention_And_Disposa_1"/>
        <owl:annotatedSource rdf:resource="&Governance;IT_P2_4"/>
        <owl:annotatedProperty rdf:resource="&Governance;needsTechnicalRequirement"/>
    </owl:Axiom>
    


    <!-- http://www.semanticweb.org/IG/Governance#IT_P3_3 -->

    <owl:NamedIndividual rdf:about="&Governance;IT_P3_3">
        <rdf:type rdf:resource="&Governance;IG_Capability"/>
        <Governance:capabilityDescription>Current Service Level Agreeements (SLAs) with cloud service providers have been reviewed for those with a standards based cloud environment and a security program that meet regulatory policies and procedures. Detailed SLAs addressing specific requirements for encryption, application design, monitoring, incident response and disaster recovery have been created for future contracts.</Governance:capabilityDescription>
        <Governance:inMaturityLevel rdf:resource="&Governance;3_Essential"/>
        <Governance:involvesArticle rdf:resource="&Governance;Article_28"/>
        <Governance:involvesArticle rdf:resource="&Governance;Article_32"/>
        <Governance:linkedToFramework rdf:resource="&Governance;CGOC_02"/>
        <Governance:needsTechnicalRequirement rdf:resource="&Governance;Collaboration_Tools_1"/>
        <Governance:practicesDefinedInIso rdf:resource="&Governance;ISO_27000"/>
        <Governance:practicesDefinedInIso rdf:resource="&Governance;ISO_27001"/>
        <Governance:needsTechnicalRequirement rdf:resource="&Governance;Monitoring_1"/>
        <Governance:linkedToProcess rdf:resource="&Governance;Process_Cloud_Computing_1"/>
        <Governance:needsTechnicalRequirement rdf:resource="&Governance;Review_Cyles_1"/>
        <Governance:needsTechnicalRequirement rdf:resource="&Governance;SLA_1"/>
        <Governance:needsTechnicalRequirement rdf:resource="&Governance;Security_Assessment_Framework_1"/>
    </owl:NamedIndividual>
    <owl:Axiom>
        <rdfs:comment>Review cycles are necessary to ensure that cloud service providers align with the organization&apos;s security and regulatory requirements. It involves assessing SLAs to determine compliance with standards and regulatory policies.</rdfs:comment>
        <owl:annotatedSource rdf:resource="&Governance;IT_P3_3"/>
        <owl:annotatedTarget rdf:resource="&Governance;Review_Cyles_1"/>
        <owl:annotatedProperty rdf:resource="&Governance;needsTechnicalRequirement"/>
    </owl:Axiom>
    <owl:Axiom>
        <rdfs:comment>The security assessment framework facilitates assessments of cloud service providers and includes criteria and metrics for evaluating compliance with standards and regulatory policies.</rdfs:comment>
        <owl:annotatedSource rdf:resource="&Governance;IT_P3_3"/>
        <owl:annotatedTarget rdf:resource="&Governance;Security_Assessment_Framework_1"/>
        <owl:annotatedProperty rdf:resource="&Governance;needsTechnicalRequirement"/>
    </owl:Axiom>
    <owl:Axiom>
        <rdfs:comment>Detailed SLAs are crucial for defining specific security and compliance requirements, such as encryption, application design, monitoring, incident response, and disaster recovery.</rdfs:comment>
        <owl:annotatedSource rdf:resource="&Governance;IT_P3_3"/>
        <owl:annotatedTarget rdf:resource="&Governance;SLA_1"/>
        <owl:annotatedProperty rdf:resource="&Governance;needsTechnicalRequirement"/>
    </owl:Axiom>
    <owl:Axiom>
        <rdfs:comment>These tools facilitate collaboration between IT, Legal, Security, and other relevant teams involved in reviewing, validating, and creating SLAs.</rdfs:comment>
        <owl:annotatedTarget rdf:resource="&Governance;Collaboration_Tools_1"/>
        <owl:annotatedSource rdf:resource="&Governance;IT_P3_3"/>
        <owl:annotatedProperty rdf:resource="&Governance;needsTechnicalRequirement"/>
    </owl:Axiom>
    <owl:Axiom>
        <rdfs:comment>Continuously monitoring of cloud services for compliance with SLAs and regulatory requirements, generating reports and alerts for non-compliance are important.</rdfs:comment>
        <owl:annotatedSource rdf:resource="&Governance;IT_P3_3"/>
        <owl:annotatedTarget rdf:resource="&Governance;Monitoring_1"/>
        <owl:annotatedProperty rdf:resource="&Governance;needsTechnicalRequirement"/>
    </owl:Axiom>
    


    <!-- http://www.semanticweb.org/IG/Governance#IT_P3_4 -->

    <owl:NamedIndividual rdf:about="&Governance;IT_P3_4">
        <rdf:type rdf:resource="&Governance;IG_Capability"/>
        <Governance:capabilityDescription>Regular compliance audits are performed to verify cloud service providers’ security policies, practices and procedures. Audits show whether all of the applicable regulatory requirements are met and compliance is properly documented.</Governance:capabilityDescription>
        <Governance:inMaturityLevel rdf:resource="&Governance;4_Proactive"/>
        <Governance:involvesArticle rdf:resource="&Governance;Article_28"/>
        <Governance:involvesArticle rdf:resource="&Governance;Article_32"/>
        <Governance:needsTechnicalRequirement rdf:resource="&Governance;Audit_1"/>
        <Governance:linkedToFramework rdf:resource="&Governance;CGOC_02"/>
        <Governance:practicesDefinedInIso rdf:resource="&Governance;ISO_27001"/>
        <Governance:practicesDefinedInIso rdf:resource="&Governance;ISO_27017"/>
        <Governance:linkedToProcess rdf:resource="&Governance;Process_Cloud_Computing_1"/>
        <Governance:needsTechnicalRequirement rdf:resource="&Governance;SLA_1"/>
    </owl:NamedIndividual>
    <owl:Axiom>
        <rdfs:comment>Creating detailed SLAs for cloud service contracts is essential for specifying requirements related to encryption, application design, monitoring, incident response, and disaster recovery. These SLAs ensure that cloud service providers meet the organization&apos;s security and compliance needs.</rdfs:comment>
        <owl:annotatedSource rdf:resource="&Governance;IT_P3_4"/>
        <owl:annotatedTarget rdf:resource="&Governance;SLA_1"/>
        <owl:annotatedProperty rdf:resource="&Governance;needsTechnicalRequirement"/>
    </owl:Axiom>
    <owl:Axiom>
        <rdfs:comment>Regular compliance audits of cloud service providers are crucial to ensuring that the security policies, practices, and procedures of these providers align with the organization&apos;s requirements and applicable regulatory standards. Audits help verify compliance and document it appropriately.</rdfs:comment>
        <owl:annotatedTarget rdf:resource="&Governance;Audit_1"/>
        <owl:annotatedSource rdf:resource="&Governance;IT_P3_4"/>
        <owl:annotatedProperty rdf:resource="&Governance;needsTechnicalRequirement"/>
    </owl:Axiom>
    


    <!-- http://www.semanticweb.org/IG/Governance#IT_P4_3 -->

    <owl:NamedIndividual rdf:about="&Governance;IT_P4_3">
        <rdf:type rdf:resource="&Governance;IG_Capability"/>
        <Governance:capabilityDescription>Some archiving is performed to batch off aging data and provide business users with faster access to more frequently used data. Archive approach varies by data source and business unit. Policies for retention, privacy and security are manually applied, if at all.</Governance:capabilityDescription>
        <Governance:inMaturityLevel rdf:resource="&Governance;3_Essential"/>
        <Governance:practicesDefinedInIso rdf:resource="&Governance;Archieving_1"/>
        <Governance:involvesArticle rdf:resource="&Governance;Article_25"/>
        <Governance:involvesArticle rdf:resource="&Governance;Article_5"/>
        <Governance:involvesArticle rdf:resource="&Governance;Article_6"/>
        <Governance:linkedToFramework rdf:resource="&Governance;CGOC_02"/>
        <Governance:practicesDefinedInIso rdf:resource="&Governance;IG_Policy_1"/>
        <Governance:practicesDefinedInIso rdf:resource="&Governance;ISO_15489"/>
        <Governance:practicesDefinedInIso rdf:resource="&Governance;ISO_27001"/>
        <Governance:linkedToProcess rdf:resource="&Governance;Process_Active_Data_Management_1"/>
    </owl:NamedIndividual>
    <owl:Axiom>
        <rdfs:comment> Develop and implement a comprehensive data archiving strategy to address aging data and improve data accessibility.</rdfs:comment>
        <owl:annotatedTarget rdf:resource="&Governance;Archieving_1"/>
        <owl:annotatedSource rdf:resource="&Governance;IT_P4_3"/>
        <owl:annotatedProperty rdf:resource="&Governance;practicesDefinedInIso"/>
    </owl:Axiom>
    <owl:Axiom>
        <rdfs:comment> Establish clear policies for data retention, privacy, and security to govern the management of archived data.</rdfs:comment>
        <owl:annotatedTarget rdf:resource="&Governance;IG_Policy_1"/>
        <owl:annotatedSource rdf:resource="&Governance;IT_P4_3"/>
        <owl:annotatedProperty rdf:resource="&Governance;practicesDefinedInIso"/>
    </owl:Axiom>
    


    <!-- http://www.semanticweb.org/IG/Governance#IT_P4_4 -->

    <owl:NamedIndividual rdf:about="&Governance;IT_P4_4">
        <rdf:type rdf:resource="&Governance;IG_Capability"/>
        <Governance:inMaturityLevel rdf:resource="&Governance;4_Proactive"/>
        <Governance:needsTechnicalRequirement rdf:resource="&Governance;Archieving_1"/>
        <Governance:involvesArticle rdf:resource="&Governance;Article_17"/>
        <Governance:involvesArticle rdf:resource="&Governance;Article_25"/>
        <Governance:involvesArticle rdf:resource="&Governance;Article_32"/>
        <Governance:involvesArticle rdf:resource="&Governance;Article_5"/>
        <Governance:involvesArticle rdf:resource="&Governance;Article_6"/>
        <Governance:needsTechnicalRequirement rdf:resource="&Governance;Backup_1"/>
        <Governance:linkedToFramework rdf:resource="&Governance;CGOC_02"/>
        <Governance:needsTechnicalRequirement rdf:resource="&Governance;Data_Mapping_And_Classification_System_1"/>
        <Governance:needsTechnicalRequirement rdf:resource="&Governance;Data_Privacy_Masking_1"/>
        <Governance:needsTechnicalRequirement rdf:resource="&Governance;Data_Retention_Policy_Dummy"/>
        <Governance:practicesDefinedInIso rdf:resource="&Governance;ISO_15489"/>
        <Governance:practicesDefinedInIso rdf:resource="&Governance;ISO_15939"/>
        <Governance:practicesDefinedInIso rdf:resource="&Governance;ISO_27001"/>
        <Governance:linkedToProcess rdf:resource="&Governance;Process_Active_Data_Management_1"/>
    </owl:NamedIndividual>
    <owl:Axiom>
        <rdfs:comment>Establish security measures and retention policies based on the business value of data, securing and retaining it accordingly.</rdfs:comment>
        <owl:annotatedTarget rdf:resource="&Governance;Data_Retention_Policy_Dummy"/>
        <owl:annotatedSource rdf:resource="&Governance;IT_P4_4"/>
        <owl:annotatedProperty rdf:resource="&Governance;needsTechnicalRequirement"/>
    </owl:Axiom>
    <owl:Axiom>
        <rdfs:comment>Develop a strategy to differentiate high-value actively used data from aging data with declining value and implement solutions to provide business users with easy access to high-value data, reducing the time spent searching for it.</rdfs:comment>
        <owl:annotatedTarget rdf:resource="&Governance;Data_Mapping_And_Classification_System_1"/>
        <owl:annotatedSource rdf:resource="&Governance;IT_P4_4"/>
        <owl:annotatedProperty rdf:resource="&Governance;needsTechnicalRequirement"/>
    </owl:Axiom>
    <owl:Axiom>
        <rdfs:comment>Apply data privacy masking based on policy to protect sensitive data.</rdfs:comment>
        <owl:annotatedTarget rdf:resource="&Governance;Data_Privacy_Masking_1"/>
        <owl:annotatedSource rdf:resource="&Governance;IT_P4_4"/>
        <owl:annotatedProperty rdf:resource="&Governance;needsTechnicalRequirement"/>
    </owl:Axiom>
    <owl:Axiom>
        <rdfs:comment>Implement processes for archiving aging data and disposing of unnecessary data to optimize storage usage.</rdfs:comment>
        <owl:annotatedTarget rdf:resource="&Governance;Archieving_1"/>
        <owl:annotatedSource rdf:resource="&Governance;IT_P4_4"/>
        <owl:annotatedProperty rdf:resource="&Governance;needsTechnicalRequirement"/>
    </owl:Axiom>
    <owl:Axiom>
        <rdfs:comment>Ensure that backup data complies with the retention schedule and is not used as a long-term archive alternative.</rdfs:comment>
        <owl:annotatedTarget rdf:resource="&Governance;Backup_1"/>
        <owl:annotatedSource rdf:resource="&Governance;IT_P4_4"/>
        <owl:annotatedProperty rdf:resource="&Governance;needsTechnicalRequirement"/>
    </owl:Axiom>
    


    <!-- http://www.semanticweb.org/IG/Governance#IT_P5_3 -->

    <owl:NamedIndividual rdf:about="&Governance;IT_P5_3">
        <rdf:type rdf:resource="&Governance;IG_Capability"/>
        <Governance:capabilityDescription>IT de-duplicates files and disposes of log files under its control. IT responds to business requests to decommission applications and works with legal on a manual review process to determine if any open legal matters may apply before decommissioning.</Governance:capabilityDescription>
        <Governance:inMaturityLevel rdf:resource="&Governance;3_Essential"/>
        <Governance:involvesArticle rdf:resource="&Governance;Article_25"/>
        <Governance:involvesArticle rdf:resource="&Governance;Article_5"/>
        <Governance:linkedToFramework rdf:resource="&Governance;CGOC_02"/>
        <Governance:needsTechnicalRequirement rdf:resource="&Governance;Disposition_Policies_And_Procedures_1"/>
        <Governance:practicesDefinedInIso rdf:resource="&Governance;ISO_27001"/>
        <Governance:linkedToProcess rdf:resource="&Governance;Process_Disposal_And_Decomissioning_1"/>
        <Governance:needsTechnicalRequirement rdf:resource="&Governance;Review_Cyles_1"/>
    </owl:NamedIndividual>
    <owl:Axiom>
        <rdfs:comment>Collaborate with legal for a manual review process to ensure that ongoing legal matters are not affected by decommissioning.</rdfs:comment>
        <owl:annotatedSource rdf:resource="&Governance;IT_P5_3"/>
        <owl:annotatedTarget rdf:resource="&Governance;Review_Cyles_1"/>
        <owl:annotatedProperty rdf:resource="&Governance;needsTechnicalRequirement"/>
    </owl:Axiom>
    <owl:Axiom>
        <rdfs:comment>Implement a data deduplication system to identify and eliminate duplicate data, reducing storage costs and enhancing data retrieval efficiency. Log file disposal is essential to eliminate unnecessary log data, reducing security and compliance risks. Establish procedures for decommissioning outdated or unused applications. </rdfs:comment>
        <owl:annotatedTarget rdf:resource="&Governance;Disposition_Policies_And_Procedures_1"/>
        <owl:annotatedSource rdf:resource="&Governance;IT_P5_3"/>
        <owl:annotatedProperty rdf:resource="&Governance;needsTechnicalRequirement"/>
    </owl:Axiom>
    


    <!-- http://www.semanticweb.org/IG/Governance#IT_P5_4 -->

    <owl:NamedIndividual rdf:about="&Governance;IT_P5_4">
        <rdf:type rdf:resource="&Governance;IG_Capability"/>
        <Governance:capabilityDescription>Data is automatically deleted at the end of its retention period when no legal hold has been specified; back up data is routinely and systematically overwritten.IT routinely analyzes the data source catalog to identify systems with low business value to proactively determine savings opportunities; IT can easily determine duplicative systems from the business value and taxonomy map for instance consolidation. IT performs routine disposal with transparent, reliable facts on preservation and retention obligations; looks up any asset or employee to determine value, current legal requirements.</Governance:capabilityDescription>
        <Governance:inMaturityLevel rdf:resource="&Governance;4_Proactive"/>
        <Governance:involvesArticle rdf:resource="&Governance;Article_25"/>
        <Governance:involvesArticle rdf:resource="&Governance;Article_5"/>
        <Governance:needsTechnicalRequirement rdf:resource="&Governance;Automated_Data_Retention_And_Disposa_1"/>
        <Governance:linkedToFramework rdf:resource="&Governance;CGOC_02"/>
        <Governance:needsTechnicalRequirement rdf:resource="&Governance;Centralized_Data_Source_Catalog_1"/>
        <Governance:needsTechnicalRequirement rdf:resource="&Governance;Disposition_Policies_And_Procedures_1"/>
        <Governance:practicesDefinedInIso rdf:resource="&Governance;ISO_15489"/>
        <Governance:practicesDefinedInIso rdf:resource="&Governance;ISO_27001"/>
        <Governance:linkedToProcess rdf:resource="&Governance;Process_Disposal_And_Decomissioning_1"/>
    </owl:NamedIndividual>
    <owl:Axiom>
        <rdfs:comment> Establish transparent disposal processes that provide reliable information on preservation and retention obligations. Ensure that disposal decisions are made based on clear facts related to asset value and current legal requirements.</rdfs:comment>
        <owl:annotatedTarget rdf:resource="&Governance;Disposition_Policies_And_Procedures_1"/>
        <owl:annotatedSource rdf:resource="&Governance;IT_P5_4"/>
        <owl:annotatedProperty rdf:resource="&Governance;needsTechnicalRequirement"/>
    </owl:Axiom>
    <owl:Axiom>
        <rdfs:comment>Routinely analyze the data source catalog to identify systems with low business value. Proactively determine cost-saving opportunities by identifying duplicative systems and consolidation possibilities.</rdfs:comment>
        <owl:annotatedTarget rdf:resource="&Governance;Centralized_Data_Source_Catalog_1"/>
        <owl:annotatedSource rdf:resource="&Governance;IT_P5_4"/>
        <owl:annotatedProperty rdf:resource="&Governance;needsTechnicalRequirement"/>
    </owl:Axiom>
    <owl:Axiom>
        <rdfs:comment>Implement automated data deletion procedures to ensure that data is deleted at the end of its retention period when no legal hold has been specified. Back-up data should be routinely and systematically overwritten to prevent unnecessary data accumulation.</rdfs:comment>
        <owl:annotatedTarget rdf:resource="&Governance;Automated_Data_Retention_And_Disposa_1"/>
        <owl:annotatedSource rdf:resource="&Governance;IT_P5_4"/>
        <owl:annotatedProperty rdf:resource="&Governance;needsTechnicalRequirement"/>
    </owl:Axiom>
    


    <!-- http://www.semanticweb.org/IG/Governance#IT_P6_3 -->

    <owl:NamedIndividual rdf:about="&Governance;IT_P6_3">
        <rdf:type rdf:resource="&Governance;IG_Capability"/>
        <Governance:capabilityDescription>IT initiates a process with legal to “reverse engineer” legacy data holds to dispose of unstructured data or back up data.</Governance:capabilityDescription>
        <Governance:inMaturityLevel rdf:resource="&Governance;3_Essential"/>
        <Governance:involvesArticle rdf:resource="&Governance;Article_5"/>
        <Governance:linkedToFramework rdf:resource="&Governance;CGOC_02"/>
        <Governance:needsTechnicalRequirement rdf:resource="&Governance;Disposition_Policies_And_Procedures_1"/>
        <Governance:practicesDefinedInIso rdf:resource="&Governance;ISO_15489"/>
        <Governance:linkedToProcess rdf:resource="&Governance;Process_Legacy_Data_Management_1"/>
    </owl:NamedIndividual>
    <owl:Axiom>
        <rdfs:comment>Implement a process for reverse engineering legacy data holds to identify and dispose of unstructured data or backup data that is no longer needed. This process helps streamline data management and reduces the storage of unnecessary data.</rdfs:comment>
        <owl:annotatedTarget rdf:resource="&Governance;Disposition_Policies_And_Procedures_1"/>
        <owl:annotatedSource rdf:resource="&Governance;IT_P6_3"/>
        <owl:annotatedProperty rdf:resource="&Governance;needsTechnicalRequirement"/>
    </owl:Axiom>
    


    <!-- http://www.semanticweb.org/IG/Governance#IT_P6_4 -->

    <owl:NamedIndividual rdf:about="&Governance;IT_P6_4">
        <rdf:type rdf:resource="&Governance;IG_Capability"/>
        <Governance:capabilityDescription>Legacy data on disk and tape is dispositioned using legal hold inventory enriched with custodian and data sets subject to hold. Data subject to ongoing regulatory or legal requirement is isolated and “surrounding” data is disposed. Additional legacy data is not accumulated.
</Governance:capabilityDescription>
        <Governance:inMaturityLevel rdf:resource="&Governance;4_Proactive"/>
        <Governance:involvesArticle rdf:resource="&Governance;Article_25"/>
        <Governance:involvesArticle rdf:resource="&Governance;Article_32"/>
        <Governance:involvesArticle rdf:resource="&Governance;Article_5"/>
        <Governance:linkedToFramework rdf:resource="&Governance;CGOC_02"/>
        <Governance:needsTechnicalRequirement rdf:resource="&Governance;Disposition_Policies_And_Procedures_1"/>
        <Governance:practicesDefinedInIso rdf:resource="&Governance;ISO_15489"/>
        <Governance:practicesDefinedInIso rdf:resource="&Governance;ISO_27001"/>
        <Governance:needsTechnicalRequirement rdf:resource="&Governance;Legal_Hold_Inventory_1"/>
        <Governance:linkedToProcess rdf:resource="&Governance;Process_Legacy_Data_Management_1"/>
    </owl:NamedIndividual>
    <owl:Axiom>
        <rdfs:comment> Develop a system that maintains a legal hold inventory, enriched with information about custodians and data sets subject to legal holds. This system ensures that data subject to ongoing regulatory or legal requirements is isolated and that surrounding data can be disposed of safely.</rdfs:comment>
        <owl:annotatedSource rdf:resource="&Governance;IT_P6_4"/>
        <owl:annotatedTarget rdf:resource="&Governance;Legal_Hold_Inventory_1"/>
        <owl:annotatedProperty rdf:resource="&Governance;needsTechnicalRequirement"/>
    </owl:Axiom>
    <owl:Axiom>
        <rdfs:comment>Implement a data disposition mechanism capable of safely disposing of legacy data that is no longer required. This mechanism should be able to identify data subject to legal holds and exclude it from disposal.</rdfs:comment>
        <owl:annotatedTarget rdf:resource="&Governance;Disposition_Policies_And_Procedures_1"/>
        <owl:annotatedSource rdf:resource="&Governance;IT_P6_4"/>
        <owl:annotatedProperty rdf:resource="&Governance;needsTechnicalRequirement"/>
    </owl:Axiom>
    


    <!-- http://www.semanticweb.org/IG/Governance#IT_P7_3 -->

    <owl:NamedIndividual rdf:about="&Governance;IT_P7_3">
        <rdf:type rdf:resource="&Governance;IG_Capability"/>
        <Governance:capabilityDescription>Automated storage utilization reporting and charge back mechanism and transparency to refresh cycles across the inventory. Charge back reporting by tier and organization is reliable and fact based.</Governance:capabilityDescription>
        <Governance:inMaturityLevel rdf:resource="&Governance;3_Essential"/>
        <Governance:involvesArticle rdf:resource="&Governance;Article_25"/>
        <Governance:involvesArticle rdf:resource="&Governance;Article_32"/>
        <Governance:involvesArticle rdf:resource="&Governance;Article_5"/>
        <Governance:needsTechnicalRequirement rdf:resource="&Governance;Automated_Storage_Utilization_Reporting_1"/>
        <Governance:linkedToFramework rdf:resource="&Governance;CGOC_02"/>
        <Governance:needsTechnicalRequirement rdf:resource="&Governance;Cost_Calculations_1"/>
        <Governance:practicesDefinedInIso rdf:resource="&Governance;ISO_15000"/>
        <Governance:practicesDefinedInIso rdf:resource="&Governance;ISO_15489"/>
        <Governance:linkedToProcess rdf:resource="&Governance;Process_Storage_Alignment_1"/>
    </owl:NamedIndividual>
    <owl:Axiom>
        <rdfs:comment>Implement an automated system for storage utilization reporting that tracks and reports on storage usage across the organization. This system ensures transparency regarding the allocation of storage resources and helps in optimizing storage capacity.</rdfs:comment>
        <owl:annotatedTarget rdf:resource="&Governance;Automated_Storage_Utilization_Reporting_1"/>
        <owl:annotatedSource rdf:resource="&Governance;IT_P7_3"/>
        <owl:annotatedProperty rdf:resource="&Governance;needsTechnicalRequirement"/>
    </owl:Axiom>
    <owl:Axiom>
        <rdfs:comment>Establish a chargeback mechanism that transparently calculates and assigns storage costs to different tiers and organizational units. This ensures that storage costs are distributed accurately and fairly based on actual usage.</rdfs:comment>
        <owl:annotatedTarget rdf:resource="&Governance;Cost_Calculations_1"/>
        <owl:annotatedSource rdf:resource="&Governance;IT_P7_3"/>
        <owl:annotatedProperty rdf:resource="&Governance;needsTechnicalRequirement"/>
    </owl:Axiom>
    


    <!-- http://www.semanticweb.org/IG/Governance#IT_P7_4 -->

    <owl:NamedIndividual rdf:about="&Governance;IT_P7_4">
        <rdf:type rdf:resource="&Governance;IG_Capability"/>
        <Governance:capabilityDescription>Storage is provisioned for new systems commensurate with retention schedules and archive protocols; refresh accounts for capacity availability from continuous deletion and decommissioning activity. Storage cost is weighed in retention schedule approval process and archive decision-making; unit cost is available in data source catalog. Current and forecasted storage capacity and costs are transparent and align to business value and data retention schedules. Optimization practice captures benefit of deletion and decomm to avoid continuous capacity addition. Accurate charge back reporting by business unit and source and gap analysis to retention schedule, business value and information cost to inform business decision-making on the costs/benefits of storing data over time.</Governance:capabilityDescription>
        <Governance:inMaturityLevel rdf:resource="&Governance;4_Proactive"/>
        <Governance:needsTechnicalRequirement rdf:resource="&Governance;Analytics_1"/>
        <Governance:involvesArticle rdf:resource="&Governance;Article_5"/>
        <Governance:linkedToFramework rdf:resource="&Governance;CGOC_02"/>
        <Governance:needsTechnicalRequirement rdf:resource="&Governance;Cost_Calculations_1"/>
        <Governance:needsTechnicalRequirement rdf:resource="&Governance;Data_Storage_1"/>
        <Governance:practicesDefinedInIso rdf:resource="&Governance;ISO_15000"/>
        <Governance:practicesDefinedInIso rdf:resource="&Governance;ISO_15489"/>
        <Governance:practicesDefinedInIso rdf:resource="&Governance;ISO_15939"/>
        <Governance:practicesDefinedInIso rdf:resource="&Governance;ISO_17000"/>
        <Governance:linkedToProcess rdf:resource="&Governance;Process_Storage_Alignment_1"/>
    </owl:NamedIndividual>
    <owl:Axiom>
        <rdfs:comment>Conduct gap analyses to compare storage utilization against retention schedules, business value, and information cost. This information informs business decision-making regarding data storage.
Regularly analyze storage utilization to identify opportunities for reclaiming and reallocating storage resources.</rdfs:comment>
        <owl:annotatedTarget rdf:resource="&Governance;Analytics_1"/>
        <owl:annotatedSource rdf:resource="&Governance;IT_P7_4"/>
        <owl:annotatedProperty rdf:resource="&Governance;needsTechnicalRequirement"/>
    </owl:Axiom>
    <owl:Axiom>
        <rdfs:comment>Include storage costs as a consideration in the approval process for retention schedules and archive decision-making. Maintain a data source catalog that provides unit costs for storage. Ensure transparency regarding current and forecasted storage capacity and costs.
Implement accurate chargeback reporting mechanisms that allocate storage costs by business unit and data source.</rdfs:comment>
        <owl:annotatedTarget rdf:resource="&Governance;Cost_Calculations_1"/>
        <owl:annotatedSource rdf:resource="&Governance;IT_P7_4"/>
        <owl:annotatedProperty rdf:resource="&Governance;needsTechnicalRequirement"/>
    </owl:Axiom>
    <owl:Axiom>
        <rdfs:comment>Provision storage resources for new systems based on established retention schedules and archive protocols. This ensures that storage is aligned with data retention requirements and minimizes the risk of data being retained longer than necessary.</rdfs:comment>
        <owl:annotatedTarget rdf:resource="&Governance;Data_Storage_1"/>
        <owl:annotatedSource rdf:resource="&Governance;IT_P7_4"/>
        <owl:annotatedProperty rdf:resource="&Governance;needsTechnicalRequirement"/>
    </owl:Axiom>
    


    <!-- http://www.semanticweb.org/IG/Governance#IT_P8_3 -->

    <owl:NamedIndividual rdf:about="&Governance;IT_P8_3">
        <rdf:type rdf:resource="&Governance;IG_Capability"/>
        <Governance:capabilityDescription>Audits publication of records, privacy, disaster recovery, application lifecycle and legal hold policies. Does not test execution of the policy.</Governance:capabilityDescription>
        <Governance:inMaturityLevel rdf:resource="&Governance;3_Essential"/>
        <Governance:involvesArticle rdf:resource="&Governance;Article_5"/>
        <Governance:needsTechnicalRequirement rdf:resource="&Governance;Audit_1"/>
        <Governance:linkedToFramework rdf:resource="&Governance;CGOC_02"/>
        <Governance:practicesDefinedInIso rdf:resource="&Governance;ISO_15489"/>
        <Governance:practicesDefinedInIso rdf:resource="&Governance;ISO_27000"/>
        <Governance:linkedToProcess rdf:resource="&Governance;Process_Audit_1"/>
    </owl:NamedIndividual>
    <owl:Axiom>
        <rdfs:comment>Publish records management, privacy, disaster recovery, application lifecycle, and legal hold policies. Ensure that these policies are accessible to relevant stakeholders within the organization.
Implement a system for auditing the execution of policies related to records management, privacy, disaster recovery, application lifecycle, and legal holds. The audit should assess whether these policies are being followed effectively.
Ensure that the auditing process complies with relevant ISO standards, including ISO 14271, ISO 15000, ISO 15489, ISO 15939, ISO 17000, ISO 23081, and ISO 27000, as applicable. These standards provide best practices and guidelines for various aspects of information governance.</rdfs:comment>
        <owl:annotatedTarget rdf:resource="&Governance;Audit_1"/>
        <owl:annotatedSource rdf:resource="&Governance;IT_P8_3"/>
        <owl:annotatedProperty rdf:resource="&Governance;needsTechnicalRequirement"/>
    </owl:Axiom>
    


    <!-- http://www.semanticweb.org/IG/Governance#IT_P8_4 -->

    <owl:NamedIndividual rdf:about="&Governance;IT_P8_4">
        <rdf:type rdf:resource="&Governance;IG_Capability"/>
        <Governance:capabilityDescription>Establishes and conducts testing procedures for records management, business value inventories, data sources, privacy requirements and legal holds such that information assets are properly defined and retained until their value expires and it is timely disposed when there is no longer a business need or legal duty. Sample tests of organizations and record class for retention and timely disposition. Establishes and conducts testing procedures for legal matters to ensure preservation duties are properly communicated and executed and holds are timely released. Tests data source catalog, back up data and system provisioning to ensure ability to comply and actual policy adherence. Audits storage rovisioning and procurement against retention / disposition / decom schedules.</Governance:capabilityDescription>
        <Governance:inMaturityLevel rdf:resource="&Governance;4_Proactive"/>
        <Governance:involvesArticle rdf:resource="&Governance;Article_5"/>
        <Governance:involvesArticle rdf:resource="&Governance;Article_6"/>
        <Governance:involvesArticle rdf:resource="&Governance;Article_9"/>
        <Governance:linkedToFramework rdf:resource="&Governance;CGOC_02"/>
        <Governance:practicesDefinedInIso rdf:resource="&Governance;ISO_15489"/>
        <Governance:needsTechnicalRequirement rdf:resource="&Governance;Legal_Matters_Testing_1"/>
        <Governance:linkedToProcess rdf:resource="&Governance;Process_Audit_1"/>
        <Governance:needsTechnicalRequirement rdf:resource="&Governance;Testing_1"/>
    </owl:NamedIndividual>
    <owl:Axiom>
        <rdfs:comment>Establish and conduct testing procedures for records management, business value inventories, data sources, privacy requirements, and legal holds. Ensure that these procedures are robust, comprehensive, and capable of evaluating the effectiveness of information management processes.</rdfs:comment>
        <owl:annotatedSource rdf:resource="&Governance;IT_P8_4"/>
        <owl:annotatedTarget rdf:resource="&Governance;Testing_1"/>
        <owl:annotatedProperty rdf:resource="&Governance;needsTechnicalRequirement"/>
    </owl:Axiom>
    <owl:Axiom>
        <rdfs:comment>Establish and conduct testing procedures for legal matters to ensure that preservation duties are properly communicated and executed, and legal holds are timely released. This involves verifying that the organization can effectively respond to legal obligations related to data preservation.</rdfs:comment>
        <owl:annotatedSource rdf:resource="&Governance;IT_P8_4"/>
        <owl:annotatedTarget rdf:resource="&Governance;Legal_Matters_Testing_1"/>
        <owl:annotatedProperty rdf:resource="&Governance;needsTechnicalRequirement"/>
    </owl:Axiom>
    


    <!-- http://www.semanticweb.org/IG/Governance#IT_Planning_And_Strategy_Framework_1 -->

    <owl:NamedIndividual rdf:about="&Governance;IT_Planning_And_Strategy_Framework_1">
        <rdf:type rdf:resource="&Governance;IT_Planning_And_Strategy_Framework"/>
        <Governance:involvesArticle rdf:resource="&Governance;Article_25"/>
        <Governance:involvesArticle rdf:resource="&Governance;Article_5"/>
        <Governance:practicesDefinedInIso rdf:resource="&Governance;ISO_15489"/>
    </owl:NamedIndividual>
    


    <!-- http://www.semanticweb.org/IG/Governance#Incident_Response_And_Remediation_Protocol_1 -->

    <owl:NamedIndividual rdf:about="&Governance;Incident_Response_And_Remediation_Protocol_1">
        <rdf:type rdf:resource="&Governance;Incident_Response_And_Remediation_Protocol"/>
        <Governance:involvesArticle rdf:resource="&Governance;Article_32"/>
        <Governance:involvesArticle rdf:resource="&Governance;Article_33"/>
        <Governance:involvesArticle rdf:resource="&Governance;Article_34"/>
        <Governance:practicesDefinedInIso rdf:resource="&Governance;ISO_27001"/>
    </owl:NamedIndividual>
    


    <!-- http://www.semanticweb.org/IG/Governance#Information_Risk_Management_1 -->

    <owl:NamedIndividual rdf:about="&Governance;Information_Risk_Management_1">
        <rdf:type rdf:resource="&Governance;Information_Risk_Management"/>
        <Governance:uses rdf:resource="&Governance;Incident_Response_And_Remediation_Protocol_1"/>
    </owl:NamedIndividual>
    <owl:Axiom>
        <rdfs:comment>The Information Risk Management subcategory within the Risk and Compliance department exclusively uses the &quot;Incident Response and Remediation Protocol.&quot; This protocol guides the department in managing and responding to information security incidents to minimize risks, protect sensitive data, and maintain regulatory compliance.</rdfs:comment>
        <owl:annotatedTarget rdf:resource="&Governance;Incident_Response_And_Remediation_Protocol_1"/>
        <owl:annotatedSource rdf:resource="&Governance;Information_Risk_Management_1"/>
        <owl:annotatedProperty rdf:resource="&Governance;uses"/>
    </owl:Axiom>
    


    <!-- http://www.semanticweb.org/IG/Governance#Integrity -->

    <owl:NamedIndividual rdf:about="&Governance;Integrity">
        <rdf:type rdf:resource="&Governance;Goal"/>
    </owl:NamedIndividual>
    


    <!-- http://www.semanticweb.org/IG/Governance#Inventory_Of_Evidence -->

    <owl:NamedIndividual rdf:about="&Governance;Inventory_Of_Evidence">
        <rdf:type rdf:resource="&Governance;Inventory_Of_Evidence"/>
        <Governance:involvesArticle rdf:resource="&Governance;Article_32"/>
        <Governance:involvesArticle rdf:resource="&Governance;Article_5"/>
        <Governance:practicesDefinedInIso rdf:resource="&Governance;ISO_15489"/>
        <Governance:practicesDefinedInIso rdf:resource="&Governance;ISO_27001"/>
    </owl:NamedIndividual>
    


    <!-- http://www.semanticweb.org/IG/Governance#Lawful_Basis_For_Processing -->

    <owl:NamedIndividual rdf:about="&Governance;Lawful_Basis_For_Processing">
        <rdf:type rdf:resource="&Governance;IG_Capability"/>
    </owl:NamedIndividual>
    


    <!-- http://www.semanticweb.org/IG/Governance#Laws_Mapping_And_Compliance_Tracking_1 -->

    <owl:NamedIndividual rdf:about="&Governance;Laws_Mapping_And_Compliance_Tracking_1">
        <rdf:type rdf:resource="&Governance;Laws_Mapping_And_Compliance_Tracking"/>
        <Governance:involvesArticle rdf:resource="&Governance;Article_32"/>
        <Governance:involvesArticle rdf:resource="&Governance;Article_5"/>
        <Governance:practicesDefinedInIso rdf:resource="&Governance;ISO_17000"/>
    </owl:NamedIndividual>
    


    <!-- http://www.semanticweb.org/IG/Governance#Legal_1 -->

    <owl:NamedIndividual rdf:about="&Governance;Legal_1">
        <rdf:type rdf:resource="&Governance;Legal"/>
        <Governance:responsibleFor rdf:resource="&Governance;Chain_Of_Custody_Tracking_1"/>
        <Governance:responsibleFor rdf:resource="&Governance;Data_Retention_Policy_Dummy"/>
        <Governance:responsibleFor rdf:resource="&Governance;Disposition_Policies_And_Procedures_1"/>
        <Governance:canBeInvolvedWith rdf:resource="&Governance;Document_Management_System_1"/>
        <Governance:uses rdf:resource="&Governance;Records_Retention_Schedule_1"/>
        <Governance:uses rdf:resource="&Governance;Review_Cyles_1"/>
    </owl:NamedIndividual>
    <owl:Axiom>
        <rdfs:comment>The Legal department could use the &quot;Document Management System&quot; to manage legal documents, contracts, and agreements. The system ensures proper document retention, versioning, and access controls, helping legal teams maintain accurate and up-to-date records for legal matters.</rdfs:comment>
        <owl:annotatedTarget rdf:resource="&Governance;Document_Management_System_1"/>
        <owl:annotatedSource rdf:resource="&Governance;Legal_1"/>
        <owl:annotatedProperty rdf:resource="&Governance;canBeInvolvedWith"/>
    </owl:Axiom>
    <owl:Axiom>
        <rdfs:comment>The Legal department primarily uses &quot;Review Cycles&quot; to ensure that legal documents, contracts, and agreements are reviewed and updated as needed. The cycles help track expiration dates, renegotiations, and compliance with legal obligations.</rdfs:comment>
        <owl:annotatedSource rdf:resource="&Governance;Legal_1"/>
        <owl:annotatedTarget rdf:resource="&Governance;Review_Cyles_1"/>
        <owl:annotatedProperty rdf:resource="&Governance;uses"/>
    </owl:Axiom>
    <owl:Axiom>
        <rdfs:comment>The Legal department is responsible for designing and establishing the &quot;Disposition Policies and Procedures.&quot; These policies outline the guidelines and steps for the proper disposition (retention, archiving, deletion, etc.) of organizational records and data in compliance with legal and regulatory requirements. Legal ensures that the policies align with relevant laws and support the organization&apos;s legal obligations.</rdfs:comment>
        <owl:annotatedTarget rdf:resource="&Governance;Disposition_Policies_And_Procedures_1"/>
        <owl:annotatedSource rdf:resource="&Governance;Legal_1"/>
        <owl:annotatedProperty rdf:resource="&Governance;responsibleFor"/>
    </owl:Axiom>
    <owl:Axiom>
        <rdfs:comment>The legal department is responsible for the design and implementation of &quot;Chain of Custody Tracking&quot;. This includes the definition of procedures and protocols for the complete documentation of the ownership and access history of data or documents, especially in a legal context. This is to ensure the integrity and authenticity of evidence.</rdfs:comment>
        <owl:annotatedTarget rdf:resource="&Governance;Chain_Of_Custody_Tracking_1"/>
        <owl:annotatedSource rdf:resource="&Governance;Legal_1"/>
        <owl:annotatedProperty rdf:resource="&Governance;responsibleFor"/>
    </owl:Axiom>
    <owl:Axiom>
        <rdfs:comment>The Legal department is responsible for designing and implementing the &quot;Data Retention Policy.&quot; This policy outlines the rules and guidelines for retaining and disposing of organizational data in compliance with legal and regulatory requirements. Legal ensures that data retention periods are established, documented, and aligned with applicable laws.</rdfs:comment>
        <owl:annotatedTarget rdf:resource="&Governance;Data_Retention_Policy_Dummy"/>
        <owl:annotatedSource rdf:resource="&Governance;Legal_1"/>
        <owl:annotatedProperty rdf:resource="&Governance;responsibleFor"/>
    </owl:Axiom>
    <owl:Axiom>
        <rdfs:comment>The Legal department exclusively uses the &quot;Records Retention Schedule&quot; to ensure that records are retained and disposed of in compliance with legal and regulatory obligations. The schedule provides a framework for managing records related to legal matters, contracts, and agreements, helping to mitigate legal risks and support legal processes.</rdfs:comment>
        <owl:annotatedSource rdf:resource="&Governance;Legal_1"/>
        <owl:annotatedTarget rdf:resource="&Governance;Records_Retention_Schedule_1"/>
        <owl:annotatedProperty rdf:resource="&Governance;uses"/>
    </owl:Axiom>
    


    <!-- http://www.semanticweb.org/IG/Governance#Legal_Hold_Inventory_1 -->

    <owl:NamedIndividual rdf:about="&Governance;Legal_Hold_Inventory_1">
        <rdf:type rdf:resource="&Governance;Legal_Hold_Inventory"/>
        <Governance:involvesArticle rdf:resource="&Governance;Article_25"/>
        <Governance:involvesArticle rdf:resource="&Governance;Article_32"/>
        <Governance:involvesArticle rdf:resource="&Governance;Article_5"/>
        <Governance:practicesDefinedInIso rdf:resource="&Governance;ISO_15489"/>
    </owl:NamedIndividual>
    


    <!-- http://www.semanticweb.org/IG/Governance#Legal_Hold_Management_1 -->

    <owl:NamedIndividual rdf:about="&Governance;Legal_Hold_Management_1">
        <rdf:type rdf:resource="&Governance;Legal_Hold_Management"/>
        <Governance:involvesArticle rdf:resource="&Governance;Article_32"/>
        <Governance:involvesArticle rdf:resource="&Governance;Article_5"/>
        <Governance:practicesDefinedInIso rdf:resource="&Governance;ISO_15489"/>
        <Governance:practicesDefinedInIso rdf:resource="&Governance;ISO_27001"/>
    </owl:NamedIndividual>
    


    <!-- http://www.semanticweb.org/IG/Governance#Legal_Matters_Testing_1 -->

    <owl:NamedIndividual rdf:about="&Governance;Legal_Matters_Testing_1">
        <rdf:type rdf:resource="&Governance;Legal_Matters_Testing"/>
        <Governance:involvesArticle rdf:resource="&Governance;Article_6"/>
        <Governance:involvesArticle rdf:resource="&Governance;Article_9"/>
        <Governance:practicesDefinedInIso rdf:resource="&Governance;ISO_15489"/>
    </owl:NamedIndividual>
    


    <!-- http://www.semanticweb.org/IG/Governance#Legal_P1_3 -->

    <owl:NamedIndividual rdf:about="&Governance;Legal_P1_3">
        <rdf:type rdf:resource="&Governance;IG_Capability"/>
        <Governance:capabilityDescription>Systematic scope and selection by organization, people from current and
historical organization data. Systematically track all custodians in all holds including multiple holds per custodian. Scope terminated/transferred employees involved. Interviews are systematically done, responses compiled and responses are automatically flagged and escalated as appropriate.</Governance:capabilityDescription>
        <Governance:inMaturityLevel rdf:resource="&Governance;3_Essential"/>
        <Governance:involvesArticle rdf:resource="&Governance;Article_25"/>
        <Governance:involvesArticle rdf:resource="&Governance;Article_32"/>
        <Governance:involvesArticle rdf:resource="&Governance;Article_5"/>
        <Governance:involvesArticle rdf:resource="&Governance;Article_6"/>
        <Governance:involvesArticle rdf:resource="&Governance;Article_9"/>
        <Governance:linkedToFramework rdf:resource="&Governance;CGOC_02"/>
        <Governance:needsTechnicalRequirement rdf:resource="&Governance;Chain_Of_Custody_Tracking_1"/>
        <Governance:needsTechnicalRequirement rdf:resource="&Governance;Data_Mapping_And_Classification_System_1"/>
        <Governance:needsTechnicalRequirement rdf:resource="&Governance;Employee_Interviews_1"/>
        <Governance:practicesDefinedInIso rdf:resource="&Governance;ISO_15489"/>
        <Governance:practicesDefinedInIso rdf:resource="&Governance;ISO_27000"/>
        <Governance:practicesDefinedInIso rdf:resource="&Governance;ISO_27001"/>
        <Governance:linkedToProcess rdf:resource="&Governance;Process_Employees_On_Hold_1"/>
        <Governance:needsTechnicalRequirement rdf:resource="&Governance;Workflow_Tools_1"/>
    </owl:NamedIndividual>
    <owl:Axiom>
        <rdfs:comment>Ensuring that custodians are tracked, and responses are escalated helps manage and resolve legal and compliance issues promptly.</rdfs:comment>
        <owl:annotatedTarget rdf:resource="&Governance;Chain_Of_Custody_Tracking_1"/>
        <owl:annotatedSource rdf:resource="&Governance;Legal_P1_3"/>
        <owl:annotatedProperty rdf:resource="&Governance;needsTechnicalRequirement"/>
    </owl:Axiom>
    <owl:Axiom>
        <rdfs:comment> Structured interviews and response compilation ensure comprehensive data identification and proper documentation.</rdfs:comment>
        <owl:annotatedTarget rdf:resource="&Governance;Employee_Interviews_1"/>
        <owl:annotatedSource rdf:resource="&Governance;Legal_P1_3"/>
        <owl:annotatedProperty rdf:resource="&Governance;needsTechnicalRequirement"/>
    </owl:Axiom>
    <owl:Axiom>
        <rdfs:comment>Understanding where personal data resides and how it&apos;s used is crucial for effective data management, risk assessment, and compliance.</rdfs:comment>
        <owl:annotatedTarget rdf:resource="&Governance;Data_Mapping_And_Classification_System_1"/>
        <owl:annotatedSource rdf:resource="&Governance;Legal_P1_3"/>
        <owl:annotatedProperty rdf:resource="&Governance;needsTechnicalRequirement"/>
    </owl:Axiom>
    <owl:Axiom>
        <rdfs:comment>Automating flagging and escalation enhances efficiency and ensures compliance with response deadlines.</rdfs:comment>
        <owl:annotatedSource rdf:resource="&Governance;Legal_P1_3"/>
        <owl:annotatedTarget rdf:resource="&Governance;Workflow_Tools_1"/>
        <owl:annotatedProperty rdf:resource="&Governance;needsTechnicalRequirement"/>
    </owl:Axiom>
    


    <!-- http://www.semanticweb.org/IG/Governance#Legal_P1_4 -->

    <owl:NamedIndividual rdf:about="&Governance;Legal_P1_4">
        <rdf:type rdf:resource="&Governance;IG_Capability"/>
        <Governance:capabilityDescription>Real-time update of custodian roles, transitions, responsibilities, automatic employee transition/transition alerts by attorney and matter; copy or cross reference custodian lists across similar matters. Scope is revisited and refined at least quarterly to release or include custodians. Individual responses to interview questions are propagated to hold scope and interview results shared with outside counsel to interview by exception.</Governance:capabilityDescription>
        <Governance:inMaturityLevel rdf:resource="&Governance;4_Proactive"/>
        <Governance:involvesArticle rdf:resource="&Governance;Article_25"/>
        <Governance:involvesArticle rdf:resource="&Governance;Article_32"/>
        <Governance:involvesArticle rdf:resource="&Governance;Article_5"/>
        <Governance:involvesArticle rdf:resource="&Governance;Article_6"/>
        <Governance:involvesArticle rdf:resource="&Governance;Article_9"/>
        <Governance:linkedToFramework rdf:resource="&Governance;CGOC_02"/>
        <Governance:needsTechnicalRequirement rdf:resource="&Governance;Collaboration_Tools_1"/>
        <Governance:needsTechnicalRequirement rdf:resource="&Governance;Data_Sharing_Protocols_1"/>
        <Governance:needsTechnicalRequirement rdf:resource="&Governance;Data_Storage_1"/>
        <Governance:needsTechnicalRequirement rdf:resource="&Governance;Digital_Signatures_And_Timestamps_1"/>
        <Governance:needsTechnicalRequirement rdf:resource="&Governance;Document_Management_System_1"/>
        <Governance:practicesDefinedInIso rdf:resource="&Governance;ISO_15489"/>
        <Governance:practicesDefinedInIso rdf:resource="&Governance;ISO_15939"/>
        <Governance:practicesDefinedInIso rdf:resource="&Governance;ISO_23081"/>
        <Governance:practicesDefinedInIso rdf:resource="&Governance;ISO_27000"/>
        <Governance:needsTechnicalRequirement rdf:resource="&Governance;Incident_Response_And_Remediation_Protocol_1"/>
        <Governance:linkedToProcess rdf:resource="&Governance;Process_Employees_On_Hold_1"/>
        <Governance:needsTechnicalRequirement rdf:resource="&Governance;Revisitation_And_Refinement_1"/>
        <Governance:needsTechnicalRequirement rdf:resource="&Governance;Workflow_Tools_1"/>
    </owl:NamedIndividual>
    <owl:Axiom>
        <rdfs:comment>Sharing interview results ensures that all parties are informed, supporting effective collaboration and informed decision-making.

This aligns with &quot;Collaboration Tools&quot;  (to share results efficiently), &quot;Document Management System&quot; (to store and manage interview data) and &quot;Data Sharing Protocols&quot; (to ensure lawful sharing). Sharing interview results requires effective collaboration tools and proper document management and data sharing protocols.</rdfs:comment>
        <owl:annotatedTarget rdf:resource="&Governance;Data_Sharing_Protocols_1"/>
        <owl:annotatedSource rdf:resource="&Governance;Legal_P1_4"/>
        <owl:annotatedProperty rdf:resource="&Governance;needsTechnicalRequirement"/>
    </owl:Axiom>
    <owl:Axiom>
        <rdfs:comment>Automated alerts during employee transitions ensure that relevant personnel are aware of changes, facilitating data management and legal compliance.

This aligns with &quot;Incident Response and Remediation Protocol&quot;  (to address alerts efficiently) and &quot;Workflow Tools&quot; (to automate the alert process). Automation facilitates timely alerts and responses to employee transitions, resembling incident response mechanisms and workflow tools.</rdfs:comment>
        <owl:annotatedSource rdf:resource="&Governance;Legal_P1_4"/>
        <owl:annotatedTarget rdf:resource="&Governance;Workflow_Tools_1"/>
        <owl:annotatedProperty rdf:resource="&Governance;needsTechnicalRequirement"/>
    </owl:Axiom>
    <owl:Axiom>
        <rdfs:comment>Sharing interview results ensures that all parties are informed, supporting effective collaboration and informed decision-making.

This aligns with &quot;Collaboration Tools&quot;  (to share results efficiently), &quot;Document Management System&quot; (to store and manage interview data) and &quot;Data Sharing Protocols&quot; (to ensure lawful sharing). Sharing interview results requires effective collaboration tools and proper document management and data sharing protocols.</rdfs:comment>
        <owl:annotatedTarget rdf:resource="&Governance;Collaboration_Tools_1"/>
        <owl:annotatedSource rdf:resource="&Governance;Legal_P1_4"/>
        <owl:annotatedProperty rdf:resource="&Governance;needsTechnicalRequirement"/>
    </owl:Axiom>
    <owl:Axiom>
        <rdfs:comment>Sharing interview results ensures that all parties are informed, supporting effective collaboration and informed decision-making.

This aligns with &quot;Collaboration Tools&quot;  (to share results efficiently), &quot;Document Management System&quot; (to store and manage interview data) and &quot;Data Sharing Protocols&quot; (to ensure lawful sharing). Sharing interview results requires effective collaboration tools and proper document management and data sharing protocols.</rdfs:comment>
        <owl:annotatedTarget rdf:resource="&Governance;Document_Management_System_1"/>
        <owl:annotatedSource rdf:resource="&Governance;Legal_P1_4"/>
        <owl:annotatedProperty rdf:resource="&Governance;needsTechnicalRequirement"/>
    </owl:Axiom>
    <owl:Axiom>
        <rdfs:comment>Timely updates enable accurate identification of custodians, crucial for effective data management and legal holds.

This aligns with &quot;Data Storage&quot; (to ensure custodian data is current) and &quot;Data Signatures and Timestamps&quot; (to track custodian data changes over time). Real-time updates involve storing data and adding timestamps for accurate tracking.</rdfs:comment>
        <owl:annotatedTarget rdf:resource="&Governance;Digital_Signatures_And_Timestamps_1"/>
        <owl:annotatedSource rdf:resource="&Governance;Legal_P1_4"/>
        <owl:annotatedProperty rdf:resource="&Governance;needsTechnicalRequirement"/>
    </owl:Axiom>
    <owl:Axiom>
        <rdfs:comment>Timely updates enable accurate identification of custodians, crucial for effective data management and legal holds.

This aligns with &quot;Data Storage&quot; (to ensure custodian data is current) and &quot;Data Signatures and Timestamps&quot; (to track custodian data changes over time). Real-time updates involve storing data and adding timestamps for accurate tracking.</rdfs:comment>
        <owl:annotatedTarget rdf:resource="&Governance;Data_Storage_1"/>
        <owl:annotatedSource rdf:resource="&Governance;Legal_P1_4"/>
        <owl:annotatedProperty rdf:resource="&Governance;needsTechnicalRequirement"/>
    </owl:Axiom>
    <owl:Axiom>
        <rdfs:comment>Regularly revisiting and refining the scope ensures that only relevant custodians are included, minimizing data overreach and enhancing efficiency.</rdfs:comment>
        <owl:annotatedSource rdf:resource="&Governance;Legal_P1_4"/>
        <owl:annotatedTarget rdf:resource="&Governance;Revisitation_And_Refinement_1"/>
        <owl:annotatedProperty rdf:resource="&Governance;needsTechnicalRequirement"/>
    </owl:Axiom>
    <owl:Axiom>
        <rdfs:comment>Automated alerts during employee transitions ensure that relevant personnel are aware of changes, facilitating data management and legal compliance.

This aligns with &quot;Incident Response and Remediation Protocol&quot;  (to address alerts efficiently) and &quot;Workflow Tools&quot; (to automate the alert process). Automation facilitates timely alerts and responses to employee transitions, resembling incident response mechanisms and workflow tools.</rdfs:comment>
        <owl:annotatedTarget rdf:resource="&Governance;Incident_Response_And_Remediation_Protocol_1"/>
        <owl:annotatedSource rdf:resource="&Governance;Legal_P1_4"/>
        <owl:annotatedProperty rdf:resource="&Governance;needsTechnicalRequirement"/>
    </owl:Axiom>
    


    <!-- http://www.semanticweb.org/IG/Governance#Legal_P2_3 -->

    <owl:NamedIndividual rdf:about="&Governance;Legal_P2_3">
        <rdf:type rdf:resource="&Governance;IG_Capability"/>
        <Governance:capabilityDescription>Have linked legacy tapes and data sources to organizations and open holds/ collections.</Governance:capabilityDescription>
        <Governance:inMaturityLevel rdf:resource="&Governance;3_Essential"/>
        <Governance:involvesArticle rdf:resource="&Governance;Article_17"/>
        <Governance:involvesArticle rdf:resource="&Governance;Article_30"/>
        <Governance:involvesArticle rdf:resource="&Governance;Article_5"/>
        <Governance:linkedToFramework rdf:resource="&Governance;CGOC_02"/>
        <Governance:needsTechnicalRequirement rdf:resource="&Governance;Data_Mapping_And_Classification_System_1"/>
        <Governance:needsTechnicalRequirement rdf:resource="&Governance;Data_Quality_Assurance_Framework_1"/>
        <Governance:needsTechnicalRequirement rdf:resource="&Governance;Data_Retention_Policy_Dummy"/>
        <Governance:practicesDefinedInIso rdf:resource="&Governance;ISO_15489"/>
        <Governance:practicesDefinedInIso rdf:resource="&Governance;ISO_15939"/>
        <Governance:linkedToBusinessUnit rdf:resource="&Governance;Legal_1"/>
        <Governance:linkedToProcess rdf:resource="&Governance;Process_Data_On_Legal_Hold_1"/>
    </owl:NamedIndividual>
    <owl:Axiom>
        <rdfs:comment>Defining retention policies helps identify relevant data sources and legacy tapes for legal holds.</rdfs:comment>
        <owl:annotatedTarget rdf:resource="&Governance;Data_Retention_Policy_Dummy"/>
        <owl:annotatedSource rdf:resource="&Governance;Legal_P2_3"/>
        <owl:annotatedProperty rdf:resource="&Governance;needsTechnicalRequirement"/>
    </owl:Axiom>
    <owl:Axiom>
        <rdfs:comment>Understanding the organization&apos;s data landscape is vital to identify legacy tapes and data sources.</rdfs:comment>
        <owl:annotatedTarget rdf:resource="&Governance;Data_Mapping_And_Classification_System_1"/>
        <owl:annotatedSource rdf:resource="&Governance;Legal_P2_3"/>
        <owl:annotatedProperty rdf:resource="&Governance;needsTechnicalRequirement"/>
    </owl:Axiom>
    <owl:Axiom>
        <rdfs:comment>Ensuring data accuracy and quality is essential for linking relevant legacy tapes and data sources.</rdfs:comment>
        <owl:annotatedTarget rdf:resource="&Governance;Data_Quality_Assurance_Framework_1"/>
        <owl:annotatedSource rdf:resource="&Governance;Legal_P2_3"/>
        <owl:annotatedProperty rdf:resource="&Governance;needsTechnicalRequirement"/>
    </owl:Axiom>
    


    <!-- http://www.semanticweb.org/IG/Governance#Legal_P2_4 -->

    <owl:NamedIndividual rdf:about="&Governance;Legal_P2_4">
        <rdf:type rdf:resource="&Governance;IG_Capability"/>
        <Governance:capabilityDescription>Automatically scope people, systems, production and backup data, information and records in holds; scope terminated employee data and legacy data/tapes where applicable. Scope is revisited and refined at least quarterly to release or include data. Can scope directly from a data source catalog shared with business liaisons, IT, Info Sec and other data quality stakeholders with reliability. IT interviews are done both periodically and in matter context and responses are aggregated for individual matters and across the legal team.</Governance:capabilityDescription>
        <Governance:involvesArticle rdf:resource="&Governance;Article_30"/>
        <Governance:involvesArticle rdf:resource="&Governance;Article_32"/>
        <Governance:involvesArticle rdf:resource="&Governance;Article_5"/>
        <Governance:linkedToFramework rdf:resource="&Governance;CGOC_02"/>
        <Governance:needsTechnicalRequirement rdf:resource="&Governance;Collaboration_Tools_1"/>
        <Governance:needsTechnicalRequirement rdf:resource="&Governance;Data_Mapping_And_Classification_System_1"/>
        <Governance:needsTechnicalRequirement rdf:resource="&Governance;Data_Quality_Assurance_Framework_1"/>
        <Governance:needsTechnicalRequirement rdf:resource="&Governance;Data_Retention_Policy_Dummy"/>
        <Governance:practicesDefinedInIso rdf:resource="&Governance;ISO_15000"/>
        <Governance:practicesDefinedInIso rdf:resource="&Governance;ISO_15489"/>
        <Governance:practicesDefinedInIso rdf:resource="&Governance;ISO_15939"/>
        <Governance:practicesDefinedInIso rdf:resource="&Governance;ISO_23081"/>
        <Governance:linkedToBusinessUnit rdf:resource="&Governance;Legal_1"/>
        <Governance:needsTechnicalRequirement rdf:resource="&Governance;Metadata_Framework_1"/>
        <Governance:linkedToProcess rdf:resource="&Governance;Process_Data_On_Legal_Hold_1"/>
    </owl:NamedIndividual>
    <owl:Axiom>
        <rdfs:comment> A metadata framework aids in cataloging data sources and ensuring consistent scoping and revisitation processes.</rdfs:comment>
        <owl:annotatedSource rdf:resource="&Governance;Legal_P2_4"/>
        <owl:annotatedTarget rdf:resource="&Governance;Metadata_Framework_1"/>
        <owl:annotatedProperty rdf:resource="&Governance;needsTechnicalRequirement"/>
    </owl:Axiom>
    <owl:Axiom>
        <rdfs:comment>Data retention policies guide scoping, revisitation, and data inclusion/exclusion decisions.</rdfs:comment>
        <owl:annotatedTarget rdf:resource="&Governance;Data_Retention_Policy_Dummy"/>
        <owl:annotatedSource rdf:resource="&Governance;Legal_P2_4"/>
        <owl:annotatedProperty rdf:resource="&Governance;needsTechnicalRequirement"/>
    </owl:Axiom>
    <owl:Axiom>
        <rdfs:comment> Collaboration tools facilitate communication between Legal, IT, Info Sec, and other stakeholders involved in scoping and revisitation.</rdfs:comment>
        <owl:annotatedTarget rdf:resource="&Governance;Collaboration_Tools_1"/>
        <owl:annotatedSource rdf:resource="&Governance;Legal_P2_4"/>
        <owl:annotatedProperty rdf:resource="&Governance;needsTechnicalRequirement"/>
    </owl:Axiom>
    <owl:Axiom>
        <rdfs:comment> A robust data mapping system is crucial for automatically scoping and revisiting data sources, ensuring comprehensive coverage.</rdfs:comment>
        <owl:annotatedTarget rdf:resource="&Governance;Data_Mapping_And_Classification_System_1"/>
        <owl:annotatedSource rdf:resource="&Governance;Legal_P2_4"/>
        <owl:annotatedProperty rdf:resource="&Governance;needsTechnicalRequirement"/>
    </owl:Axiom>
    <owl:Axiom>
        <rdfs:comment>Data quality assurance ensures accuracy and reliability when scoping data sources and revisiting them.</rdfs:comment>
        <owl:annotatedTarget rdf:resource="&Governance;Data_Quality_Assurance_Framework_1"/>
        <owl:annotatedSource rdf:resource="&Governance;Legal_P2_4"/>
        <owl:annotatedProperty rdf:resource="&Governance;needsTechnicalRequirement"/>
    </owl:Axiom>
    


    <!-- http://www.semanticweb.org/IG/Governance#Legal_P3_3 -->

    <owl:NamedIndividual rdf:about="&Governance;Legal_P3_3">
        <rdf:type rdf:resource="&Governance;IG_Capability"/>
        <Governance:capabilityDescription>Systematically send notices and reminders, require and track confirmations, ability to manage exceptions, employees can look up their holds at any time. Communications tailored to recipient role (IT, RIM, employee).</Governance:capabilityDescription>
        <Governance:inMaturityLevel rdf:resource="&Governance;3_Essential"/>
        <Governance:involvesArticle rdf:resource="&Governance;Article_12"/>
        <Governance:involvesArticle rdf:resource="&Governance;Article_25"/>
        <Governance:involvesArticle rdf:resource="&Governance;Article_30"/>
        <Governance:linkedToFramework rdf:resource="&Governance;CGOC_02"/>
        <Governance:needsTechnicalRequirement rdf:resource="&Governance;Communication_Platforms_1"/>
        <Governance:needsTechnicalRequirement rdf:resource="&Governance;Confirmation_Tracking_Mechanism_1"/>
        <Governance:needsTechnicalRequirement rdf:resource="&Governance;Employee_Self_Service_Portal_1"/>
        <Governance:needsTechnicalRequirement rdf:resource="&Governance;Exception_Handling_System_1"/>
        <Governance:practicesDefinedInIso rdf:resource="&Governance;ISO_14271"/>
        <Governance:practicesDefinedInIso rdf:resource="&Governance;ISO_15000"/>
        <Governance:practicesDefinedInIso rdf:resource="&Governance;ISO_15489"/>
        <Governance:practicesDefinedInIso rdf:resource="&Governance;ISO_17000"/>
        <Governance:linkedToBusinessUnit rdf:resource="&Governance;Legal_1"/>
        <Governance:linkedToProcess rdf:resource="&Governance;Process_Hold_Publication_1"/>
    </owl:NamedIndividual>
    <owl:Axiom>
        <rdfs:comment>An exception handling system is necessary to manage cases that deviate from standard hold communications.</rdfs:comment>
        <owl:annotatedTarget rdf:resource="&Governance;Exception_Handling_System_1"/>
        <owl:annotatedSource rdf:resource="&Governance;Legal_P3_3"/>
        <owl:annotatedProperty rdf:resource="&Governance;needsTechnicalRequirement"/>
    </owl:Axiom>
    <owl:Axiom>
        <rdfs:comment>Providing employees with the ability to look up their holds promotes transparency and empowers individuals to exercise their data rights.</rdfs:comment>
        <owl:annotatedTarget rdf:resource="&Governance;Employee_Self_Service_Portal_1"/>
        <owl:annotatedSource rdf:resource="&Governance;Legal_P3_3"/>
        <owl:annotatedProperty rdf:resource="&Governance;needsTechnicalRequirement"/>
    </owl:Axiom>
    <owl:Axiom>
        <rdfs:comment>A robust communication platform is essential for systematically sending notices, reminders, and tracking confirmations.</rdfs:comment>
        <owl:annotatedTarget rdf:resource="&Governance;Communication_Platforms_1"/>
        <owl:annotatedSource rdf:resource="&Governance;Legal_P3_3"/>
        <owl:annotatedProperty rdf:resource="&Governance;needsTechnicalRequirement"/>
    </owl:Axiom>
    <owl:Axiom>
        <rdfs:comment>The ability to track confirmations ensures accountability and compliance with hold requirements.</rdfs:comment>
        <owl:annotatedTarget rdf:resource="&Governance;Confirmation_Tracking_Mechanism_1"/>
        <owl:annotatedSource rdf:resource="&Governance;Legal_P3_3"/>
        <owl:annotatedProperty rdf:resource="&Governance;needsTechnicalRequirement"/>
    </owl:Axiom>
    


    <!-- http://www.semanticweb.org/IG/Governance#Legal_P3_4 -->

    <owl:NamedIndividual rdf:about="&Governance;Legal_P3_4">
        <rdf:type rdf:resource="&Governance;IG_Capability"/>
        <Governance:capabilityDescription>Publish to system, propagate hold, automate hold enforcement. IT Staff have continuous visibility to current discovery duties, holds during routine data management activities; automatically flag records in appropriate systems. Holds are timely released and release syndication is done with same rigor as hold syndication.</Governance:capabilityDescription>
        <Governance:inMaturityLevel rdf:resource="&Governance;4_Proactive"/>
        <Governance:involvesArticle rdf:resource="&Governance;Article_25"/>
        <Governance:involvesArticle rdf:resource="&Governance;Article_32"/>
        <Governance:involvesArticle rdf:resource="&Governance;Article_5"/>
        <Governance:needsTechnicalRequirement rdf:resource="&Governance;Automated_Record_Flagging_System_1"/>
        <Governance:linkedToFramework rdf:resource="&Governance;CGOC_02"/>
        <Governance:needsTechnicalRequirement rdf:resource="&Governance;Continous_Visibility_And_Monitoring_System_1"/>
        <Governance:needsTechnicalRequirement rdf:resource="&Governance;Hold_Enforcement_Automation_System_1"/>
        <Governance:practicesDefinedInIso rdf:resource="&Governance;ISO_15000"/>
        <Governance:practicesDefinedInIso rdf:resource="&Governance;ISO_15489"/>
        <Governance:practicesDefinedInIso rdf:resource="&Governance;ISO_15939"/>
        <Governance:practicesDefinedInIso rdf:resource="&Governance;ISO_27001"/>
        <Governance:linkedToBusinessUnit rdf:resource="&Governance;Legal_1"/>
        <Governance:linkedToProcess rdf:resource="&Governance;Process_Hold_Publication_1"/>
        <Governance:needsTechnicalRequirement rdf:resource="&Governance;Syndication_System_For_Hold_Release_1"/>
    </owl:NamedIndividual>
    <owl:Axiom>
        <rdfs:comment>Automation of record flagging in appropriate systems helps identify and categorize records that are subject to legal holds, making it easier to enforce and manage holds.</rdfs:comment>
        <owl:annotatedTarget rdf:resource="&Governance;Automated_Record_Flagging_System_1"/>
        <owl:annotatedSource rdf:resource="&Governance;Legal_P3_4"/>
        <owl:annotatedProperty rdf:resource="&Governance;needsTechnicalRequirement"/>
    </owl:Axiom>
    <owl:Axiom>
        <rdfs:comment>Rigorous hold release syndication ensures that legal holds are accurately communicated to relevant parties, allowing for timely and compliant release of held data.</rdfs:comment>
        <owl:annotatedSource rdf:resource="&Governance;Legal_P3_4"/>
        <owl:annotatedTarget rdf:resource="&Governance;Syndication_System_For_Hold_Release_1"/>
        <owl:annotatedProperty rdf:resource="&Governance;needsTechnicalRequirement"/>
    </owl:Axiom>
    <owl:Axiom>
        <rdfs:comment>Automation of hold enforcement ensures that legal holds are consistently and accurately applied to relevant data sources and records, reducing the risk of non-compliance and data breaches.</rdfs:comment>
        <owl:annotatedTarget rdf:resource="&Governance;Hold_Enforcement_Automation_System_1"/>
        <owl:annotatedSource rdf:resource="&Governance;Legal_P3_4"/>
        <owl:annotatedProperty rdf:resource="&Governance;needsTechnicalRequirement"/>
    </owl:Axiom>
    <owl:Axiom>
        <rdfs:comment>Continuous visibility allows IT staff to monitor and track discovery duties and legal holds during routine data management activities, ensuring that holds are effectively enforced and managed.</rdfs:comment>
        <owl:annotatedTarget rdf:resource="&Governance;Continous_Visibility_And_Monitoring_System_1"/>
        <owl:annotatedSource rdf:resource="&Governance;Legal_P3_4"/>
        <owl:annotatedProperty rdf:resource="&Governance;needsTechnicalRequirement"/>
    </owl:Axiom>
    


    <!-- http://www.semanticweb.org/IG/Governance#Legal_P4_3 -->

    <owl:NamedIndividual rdf:about="&Governance;Legal_P4_3">
        <rdf:type rdf:resource="&Governance;IG_Capability"/>
        <Governance:capabilityDescription>System log of collection requests by matter, issuer and collector. Collection logging is done by discovery staff in a shared system. An inventory of evidence is well managed and not overlooked in scoping other matters. Interview results and insights are used to inform the collection activity.</Governance:capabilityDescription>
        <Governance:inMaturityLevel rdf:resource="&Governance;3_Essential"/>
        <Governance:involvesArticle rdf:resource="&Governance;Article_32"/>
        <Governance:involvesArticle rdf:resource="&Governance;Article_39"/>
        <Governance:involvesArticle rdf:resource="&Governance;Article_5"/>
        <Governance:involvesArticle rdf:resource="&Governance;Article_6"/>
        <Governance:linkedToFramework rdf:resource="&Governance;CGOC_02"/>
        <Governance:needsTechnicalRequirement rdf:resource="&Governance;Employee_Interviews_1"/>
        <Governance:practicesDefinedInIso rdf:resource="&Governance;ISO_15489"/>
        <Governance:practicesDefinedInIso rdf:resource="&Governance;ISO_15939"/>
        <Governance:practicesDefinedInIso rdf:resource="&Governance;ISO_17000"/>
        <Governance:practicesDefinedInIso rdf:resource="&Governance;ISO_27001"/>
        <Governance:needsTechnicalRequirement rdf:resource="&Governance;Inventory_Of_Evidence"/>
        <Governance:linkedToBusinessUnit rdf:resource="&Governance;Legal_1"/>
        <Governance:linkedToProcess rdf:resource="&Governance;Process_Evidence_Collection_1"/>
        <Governance:needsTechnicalRequirement rdf:resource="&Governance;System_Log_1"/>
        <Governance:needsTechnicalRequirement rdf:resource="&Governance;Training_1"/>
    </owl:NamedIndividual>
    <owl:Axiom>
        <rdfs:comment>Properly trained discovery staff ensure that evidence collection is conducted accurately, ethically, and in compliance with GDPR.</rdfs:comment>
        <owl:annotatedSource rdf:resource="&Governance;Legal_P4_3"/>
        <owl:annotatedTarget rdf:resource="&Governance;Training_1"/>
        <owl:annotatedProperty rdf:resource="&Governance;needsTechnicalRequirement"/>
    </owl:Axiom>
    <owl:Axiom>
        <rdfs:comment>Using interview results and insights enhances the effectiveness of evidence collection, ensuring relevant information is gathered and documented.</rdfs:comment>
        <owl:annotatedTarget rdf:resource="&Governance;Employee_Interviews_1"/>
        <owl:annotatedSource rdf:resource="&Governance;Legal_P4_3"/>
        <owl:annotatedProperty rdf:resource="&Governance;needsTechnicalRequirement"/>
    </owl:Axiom>
    <owl:Axiom>
        <rdfs:comment>Proper management of evidence inventories prevents overlooking potential evidence in scoping other matters and helps maintain accuracy and completeness.</rdfs:comment>
        <owl:annotatedTarget rdf:resource="&Governance;Inventory_Of_Evidence"/>
        <owl:annotatedSource rdf:resource="&Governance;Legal_P4_3"/>
        <owl:annotatedProperty rdf:resource="&Governance;needsTechnicalRequirement"/>
    </owl:Axiom>
    <owl:Axiom>
        <rdfs:comment>A system log is crucial for tracking collection requests, issuers, and collectors. It provides an audit trail of evidence collection activities, ensuring transparency and accountability.</rdfs:comment>
        <owl:annotatedSource rdf:resource="&Governance;Legal_P4_3"/>
        <owl:annotatedTarget rdf:resource="&Governance;System_Log_1"/>
        <owl:annotatedProperty rdf:resource="&Governance;needsTechnicalRequirement"/>
    </owl:Axiom>
    


    <!-- http://www.semanticweb.org/IG/Governance#Legal_P4_4 -->

    <owl:NamedIndividual rdf:about="&Governance;Legal_P4_4">
        <rdf:type rdf:resource="&Governance;IG_Capability"/>
        <Governance:capabilityDescription>Interview results are automatically incorporated into custodian or data source specific collection instructions without rekeying. IT or collection staff can efficiently and automatically collect by custodian and content without re- logging the request or recollecting the same data. Collection data and chain of custody is automatically logged. IT and legal share complete transparency on collections, and legal can monitor progress and process while IT can process work by custodian or data source efficiently. Evidence is not duplicated in multiple locations and it is timely disposed.</Governance:capabilityDescription>
        <Governance:inMaturityLevel rdf:resource="&Governance;4_Proactive"/>
        <Governance:involvesArticle rdf:resource="&Governance;Article_32"/>
        <Governance:involvesArticle rdf:resource="&Governance;Article_5"/>
        <Governance:involvesArticle rdf:resource="&Governance;Article_6"/>
        <Governance:needsTechnicalRequirement rdf:resource="&Governance;Automated_Chain_Of_Custody_Logging_1"/>
        <Governance:needsTechnicalRequirement rdf:resource="&Governance;Automated_Data_Collection"/>
        <Governance:needsTechnicalRequirement rdf:resource="&Governance;Automated_Integration"/>
        <Governance:linkedToFramework rdf:resource="&Governance;CGOC_02"/>
        <Governance:needsTechnicalRequirement rdf:resource="&Governance;Disposition_Policies_And_Procedures_1"/>
        <Governance:practicesDefinedInIso rdf:resource="&Governance;ISO_14271"/>
        <Governance:practicesDefinedInIso rdf:resource="&Governance;ISO_15000"/>
        <Governance:practicesDefinedInIso rdf:resource="&Governance;ISO_15489"/>
        <Governance:practicesDefinedInIso rdf:resource="&Governance;ISO_15939"/>
        <Governance:practicesDefinedInIso rdf:resource="&Governance;ISO_27000"/>
        <Governance:linkedToBusinessUnit rdf:resource="&Governance;Legal_1"/>
        <Governance:needsTechnicalRequirement rdf:resource="&Governance;Monitoring_1"/>
        <Governance:linkedToProcess rdf:resource="&Governance;Process_Evidence_Collection_1"/>
    </owl:NamedIndividual>
    <owl:Axiom>
        <rdfs:comment> Implementing a system that provides transparency to both IT and legal teams regarding collections, progress, and processes is important. Legal should be able to monitor progress, and IT should be able to process work efficiently by custodian or data source.</rdfs:comment>
        <owl:annotatedSource rdf:resource="&Governance;Legal_P4_4"/>
        <owl:annotatedTarget rdf:resource="&Governance;Monitoring_1"/>
        <owl:annotatedProperty rdf:resource="&Governance;needsTechnicalRequirement"/>
    </owl:Axiom>
    <owl:Axiom>
        <rdfs:comment>Implementing an automated chain of custody logging mechanism is essential. It ensures that the entire process of evidence collection is well-documented and traceable, maintaining the integrity and authenticity of collected data.</rdfs:comment>
        <owl:annotatedTarget rdf:resource="&Governance;Automated_Chain_Of_Custody_Logging_1"/>
        <owl:annotatedSource rdf:resource="&Governance;Legal_P4_4"/>
        <owl:annotatedProperty rdf:resource="&Governance;needsTechnicalRequirement"/>
    </owl:Axiom>
    <owl:Axiom>
        <rdfs:comment>A technical requirement is an automated integration mechanism that allows interview results to be seamlessly incorporated into custodian or data source-specific collection instructions without manual rekeying. This ensures that the insights gained from employee interviews are directly translated into actionable instructions for data collection.</rdfs:comment>
        <owl:annotatedTarget rdf:resource="&Governance;Automated_Integration"/>
        <owl:annotatedSource rdf:resource="&Governance;Legal_P4_4"/>
        <owl:annotatedProperty rdf:resource="&Governance;needsTechnicalRequirement"/>
    </owl:Axiom>
    <owl:Axiom>
        <rdfs:comment>A technical requirement involves the implementation of an automated data collection system that allows IT or collection staff to efficiently and automatically collect data by custodian and content without the need for manual re-logging or duplicate collection efforts.</rdfs:comment>
        <owl:annotatedTarget rdf:resource="&Governance;Automated_Data_Collection"/>
        <owl:annotatedSource rdf:resource="&Governance;Legal_P4_4"/>
        <owl:annotatedProperty rdf:resource="&Governance;needsTechnicalRequirement"/>
    </owl:Axiom>
    <owl:Axiom>
        <rdfs:comment> Implementing mechanisms for timely and proper data disposition is crucial. Unnecessary data should be disposed of properly to avoid data duplication and to comply with data retention policies.</rdfs:comment>
        <owl:annotatedTarget rdf:resource="&Governance;Disposition_Policies_And_Procedures_1"/>
        <owl:annotatedSource rdf:resource="&Governance;Legal_P4_4"/>
        <owl:annotatedProperty rdf:resource="&Governance;needsTechnicalRequirement"/>
    </owl:Axiom>
    


    <!-- http://www.semanticweb.org/IG/Governance#Legal_P5_3 -->

    <owl:NamedIndividual rdf:about="&Governance;Legal_P5_3">
        <rdf:type rdf:resource="&Governance;IG_Capability"/>
        <Governance:capabilityDescription>Quantity of data reviewed from tightly scoped custodians, leveraging prior scoping histories. Consistent &amp; enforced culling performed by preferred vendors utilizing objective criteria such as keywords, date ranges, file types, domain names &amp; data sources. Discovery cost forecasts available as the hold is scoped, costs are calculated continuously.</Governance:capabilityDescription>
        <Governance:inMaturityLevel rdf:resource="&Governance;3_Essential"/>
        <Governance:involvesArticle rdf:resource="&Governance;Article_25"/>
        <Governance:involvesArticle rdf:resource="&Governance;Article_5"/>
        <Governance:needsTechnicalRequirement rdf:resource="&Governance;Automated_Data_Culling_And_Scoping_1"/>
        <Governance:linkedToFramework rdf:resource="&Governance;CGOC_02"/>
        <Governance:needsTechnicalRequirement rdf:resource="&Governance;Cost_Calculations_1"/>
        <Governance:practicesDefinedInIso rdf:resource="&Governance;ISO_15489"/>
        <Governance:practicesDefinedInIso rdf:resource="&Governance;ISO_15939"/>
        <Governance:practicesDefinedInIso rdf:resource="&Governance;ISO_27001"/>
        <Governance:linkedToProcess rdf:resource="&Governance;Process_Evidence_Analysis_And_Cost_Controls_1"/>
    </owl:NamedIndividual>
    <owl:Axiom>
        <rdfs:comment>Efficiently reviewing a large quantity of data is crucial to reduce costs and ensure relevant information is identified. Automation of data culling and scoping helps to focus on specific custodians and data sources.
Also having objective criteria for data culling (e.g., keywords, date ranges, file types) ensures that the process is consistent and defensible.</rdfs:comment>
        <owl:annotatedTarget rdf:resource="&Governance;Automated_Data_Culling_And_Scoping_1"/>
        <owl:annotatedSource rdf:resource="&Governance;Legal_P5_3"/>
        <owl:annotatedProperty rdf:resource="&Governance;needsTechnicalRequirement"/>
    </owl:Axiom>
    <owl:Axiom>
        <rdfs:comment>Accurate cost forecasting helps in budget planning for legal matters and ensures transparency in financial aspects.</rdfs:comment>
        <owl:annotatedTarget rdf:resource="&Governance;Cost_Calculations_1"/>
        <owl:annotatedSource rdf:resource="&Governance;Legal_P5_3"/>
        <owl:annotatedProperty rdf:resource="&Governance;needsTechnicalRequirement"/>
    </owl:Axiom>
    


    <!-- http://www.semanticweb.org/IG/Governance#Legal_P5_4 -->

    <owl:NamedIndividual rdf:about="&Governance;Legal_P5_4">
        <rdf:type rdf:resource="&Governance;IG_Capability"/>
        <Governance:capabilityDescription>Consistently limit scope of collection and review; early case assessment performed before collection for earliest/optimized matter resolution, advanced culling techniques employed leveraging visual analytics; defined &amp; repeatable process for providing outside counsel early case assessment before processing, manage cost at portfolio level.</Governance:capabilityDescription>
        <Governance:inMaturityLevel rdf:resource="&Governance;4_Proactive"/>
        <Governance:involvesArticle rdf:resource="&Governance;Article_5"/>
        <Governance:needsTechnicalRequirement rdf:resource="&Governance;Automated_Data_Culling_And_Scoping_1"/>
        <Governance:linkedToFramework rdf:resource="&Governance;CGOC_02"/>
        <Governance:needsTechnicalRequirement rdf:resource="&Governance;Collaboration_Tools_1"/>
        <Governance:needsTechnicalRequirement rdf:resource="&Governance;Cost_Calculations_1"/>
        <Governance:needsTechnicalRequirement rdf:resource="&Governance;Early_Case_Assessment_1"/>
        <Governance:practicesDefinedInIso rdf:resource="&Governance;ISO_15939"/>
        <Governance:practicesDefinedInIso rdf:resource="&Governance;ISO_17000"/>
        <Governance:linkedToProcess rdf:resource="&Governance;Process_Evidence_Analysis_And_Cost_Controls_1"/>
    </owl:NamedIndividual>
    <owl:Axiom>
        <rdfs:comment>Automate the process of early case assessment before data collection. Utilize algorithms and machine learning to analyze case details and available data sources to determine potential case merits. This automation speeds up the assessment process and ensures that only relevant data is collected.</rdfs:comment>
        <owl:annotatedTarget rdf:resource="&Governance;Early_Case_Assessment_1"/>
        <owl:annotatedSource rdf:resource="&Governance;Legal_P5_4"/>
        <owl:annotatedProperty rdf:resource="&Governance;needsTechnicalRequirement"/>
    </owl:Axiom>
    <owl:Axiom>
        <rdfs:comment>Develop a centralized system to track and manage costs related to data collection and review across multiple matters. This system provides insights into cost trends, allowing for effective budget allocation.</rdfs:comment>
        <owl:annotatedTarget rdf:resource="&Governance;Cost_Calculations_1"/>
        <owl:annotatedSource rdf:resource="&Governance;Legal_P5_4"/>
        <owl:annotatedProperty rdf:resource="&Governance;needsTechnicalRequirement"/>
    </owl:Axiom>
    <owl:Axiom>
        <rdfs:comment>Establish an online platform for collaborative assessment by outside counsel. Legal teams and outside counsel can review and assess data sources together, identifying key evidence and potential strategies for data collection.</rdfs:comment>
        <owl:annotatedTarget rdf:resource="&Governance;Collaboration_Tools_1"/>
        <owl:annotatedSource rdf:resource="&Governance;Legal_P5_4"/>
        <owl:annotatedProperty rdf:resource="&Governance;needsTechnicalRequirement"/>
    </owl:Axiom>
    <owl:Axiom>
        <rdfs:comment>Implement visual analytics tools to perform advanced culling of data. These tools help legal professionals visually identify patterns and relevant data points, aiding in narrowing down the data volume for collection and review.</rdfs:comment>
        <owl:annotatedTarget rdf:resource="&Governance;Automated_Data_Culling_And_Scoping_1"/>
        <owl:annotatedSource rdf:resource="&Governance;Legal_P5_4"/>
        <owl:annotatedProperty rdf:resource="&Governance;needsTechnicalRequirement"/>
    </owl:Axiom>
    


    <!-- http://www.semanticweb.org/IG/Governance#Legal_P6_3 -->

    <owl:NamedIndividual rdf:about="&Governance;Legal_P6_3">
        <rdf:type rdf:resource="&Governance;IG_Capability"/>
        <Governance:capabilityDescription>Automated reminders and escalations, online audit trail, management reporting on discovery status, visibility within legal department across custodians, collected inventory and matters.</Governance:capabilityDescription>
        <Governance:inMaturityLevel rdf:resource="&Governance;3_Essential"/>
        <Governance:inMaturityLevel rdf:resource="&Governance;4_Proactive"/>
        <Governance:involvesArticle rdf:resource="&Governance;Article_5"/>
        <Governance:involvesArticle rdf:resource="&Governance;Article_6"/>
        <Governance:needsTechnicalRequirement rdf:resource="&Governance;Automated_Notification_System_1"/>
        <Governance:linkedToFramework rdf:resource="&Governance;CGOC_02"/>
        <Governance:needsTechnicalRequirement rdf:resource="&Governance;Deadline_Tracking_1"/>
        <Governance:practicesDefinedInIso rdf:resource="&Governance;ISO_17000"/>
        <Governance:practicesDefinedInIso rdf:resource="&Governance;ISO_23081"/>
        <Governance:practicesDefinedInIso rdf:resource="&Governance;ISO_27001"/>
        <Governance:linkedToProcess rdf:resource="&Governance;Process_Legal_Records_1"/>
        <Governance:needsTechnicalRequirement rdf:resource="&Governance;Workflow_Tools_1"/>
    </owl:NamedIndividual>
    <owl:Axiom>
        <rdfs:comment>Implementing an automated notification system is crucial to ensure that all relevant parties are promptly informed about their responsibilities and deadlines. This minimizes the risk of errors, oversight, and non-compliance.</rdfs:comment>
        <owl:annotatedTarget rdf:resource="&Governance;Automated_Notification_System_1"/>
        <owl:annotatedSource rdf:resource="&Governance;Legal_P6_3"/>
        <owl:annotatedProperty rdf:resource="&Governance;needsTechnicalRequirement"/>
    </owl:Axiom>
    <owl:Axiom>
        <rdfs:comment> Integrating the automated notification system with the workflow of the legal department ensures that notifications are triggered at appropriate stages of the legal records lifecycle, enhancing communication efficiency.</rdfs:comment>
        <owl:annotatedSource rdf:resource="&Governance;Legal_P6_3"/>
        <owl:annotatedTarget rdf:resource="&Governance;Workflow_Tools_1"/>
        <owl:annotatedProperty rdf:resource="&Governance;needsTechnicalRequirement"/>
    </owl:Axiom>
    <owl:Axiom>
        <rdfs:comment>Integrating a tracking mechanism for deadlines and escalations ensures that tasks are completed promptly within specified timeframes, reducing delays and non-compliance risks.</rdfs:comment>
        <owl:annotatedTarget rdf:resource="&Governance;Deadline_Tracking_1"/>
        <owl:annotatedSource rdf:resource="&Governance;Legal_P6_3"/>
        <owl:annotatedProperty rdf:resource="&Governance;needsTechnicalRequirement"/>
    </owl:Axiom>
    


    <!-- http://www.semanticweb.org/IG/Governance#Legal_P6_4 -->

    <owl:NamedIndividual rdf:about="&Governance;Legal_P6_4">
        <rdf:type rdf:resource="&Governance;IG_Capability"/>
        <Governance:capabilityDescription>Appropriate visibility across IT, Legal and Business; self- service dashboards for legal obligations, tasks, risk and cost reduction opportunities.</Governance:capabilityDescription>
        <Governance:inMaturityLevel rdf:resource="&Governance;4_Proactive"/>
        <Governance:needsTechnicalRequirement rdf:resource="&Governance;AccessControl_1"/>
        <Governance:involvesArticle rdf:resource="&Governance;Article_32"/>
        <Governance:involvesArticle rdf:resource="&Governance;Article_5"/>
        <Governance:involvesArticle rdf:resource="&Governance;Article_6"/>
        <Governance:linkedToFramework rdf:resource="&Governance;CGOC_02"/>
        <Governance:needsTechnicalRequirement rdf:resource="&Governance;Centralized_Data_Repository_1"/>
        <Governance:needsTechnicalRequirement rdf:resource="&Governance;Employee_Self_Service_Portal_1"/>
        <Governance:practicesDefinedInIso rdf:resource="&Governance;ISO_15000"/>
        <Governance:practicesDefinedInIso rdf:resource="&Governance;ISO_15489"/>
        <Governance:practicesDefinedInIso rdf:resource="&Governance;ISO_27001"/>
        <Governance:linkedToProcess rdf:resource="&Governance;Process_Legal_Records_1"/>
    </owl:NamedIndividual>
    <owl:Axiom>
        <rdfs:comment>Implement user access controls to ensure that only authorized individuals can access specific information based on their roles and responsibilities. Role-based access controls should be in place to enforce proper data access and prevent unauthorized disclosure.</rdfs:comment>
        <owl:annotatedTarget rdf:resource="&Governance;AccessControl_1"/>
        <owl:annotatedSource rdf:resource="&Governance;Legal_P6_4"/>
        <owl:annotatedProperty rdf:resource="&Governance;needsTechnicalRequirement"/>
    </owl:Axiom>
    <owl:Axiom>
        <rdfs:comment>Implement a centralized data repository that consolidates information related to legal obligations, tasks, risks, and cost reduction opportunities. This repository serves as a single source of truth for relevant data, ensuring accuracy and consistency in information dissemination.</rdfs:comment>
        <owl:annotatedTarget rdf:resource="&Governance;Centralized_Data_Repository_1"/>
        <owl:annotatedSource rdf:resource="&Governance;Legal_P6_4"/>
        <owl:annotatedProperty rdf:resource="&Governance;needsTechnicalRequirement"/>
    </owl:Axiom>
    <owl:Axiom>
        <rdfs:comment>Develop a user-friendly self-service dashboard interface that provides relevant stakeholders with personalized views of legal obligations, tasks, risks, and opportunities. The dashboard should offer intuitive navigation and customization options.</rdfs:comment>
        <owl:annotatedTarget rdf:resource="&Governance;Employee_Self_Service_Portal_1"/>
        <owl:annotatedSource rdf:resource="&Governance;Legal_P6_4"/>
        <owl:annotatedProperty rdf:resource="&Governance;needsTechnicalRequirement"/>
    </owl:Axiom>
    


    <!-- http://www.semanticweb.org/IG/Governance#Metadata_1 -->

    <owl:NamedIndividual rdf:about="&Governance;Metadata_1">
        <rdf:type rdf:resource="&Governance;Metadata"/>
        <Governance:involvesArticle rdf:resource="&Governance;Article_30"/>
        <Governance:involvesArticle rdf:resource="&Governance;Article_5"/>
        <Governance:practicesDefinedInIso rdf:resource="&Governance;ISO_15489"/>
        <Governance:practicesDefinedInIso rdf:resource="&Governance;ISO_15939"/>
        <Governance:practicesDefinedInIso rdf:resource="&Governance;ISO_23081"/>
    </owl:NamedIndividual>
    


    <!-- http://www.semanticweb.org/IG/Governance#Metadata_Framework_1 -->

    <owl:NamedIndividual rdf:about="&Governance;Metadata_Framework_1">
        <rdf:type rdf:resource="&Governance;Metadata_Framework"/>
        <Governance:involvesArticle rdf:resource="&Governance;Article_30"/>
        <Governance:involvesArticle rdf:resource="&Governance;Article_5"/>
        <Governance:involvesArticle rdf:resource="&Governance;Article_6"/>
        <Governance:practicesDefinedInIso rdf:resource="&Governance;ISO_15489"/>
        <Governance:practicesDefinedInIso rdf:resource="&Governance;ISO_17000"/>
        <Governance:practicesDefinedInIso rdf:resource="&Governance;ISO_23081"/>
    </owl:NamedIndividual>
    


    <!-- http://www.semanticweb.org/IG/Governance#Metrics_1 -->

    <owl:NamedIndividual rdf:about="&Governance;Metrics_1">
        <rdf:type rdf:resource="&Governance;Metrics"/>
        <Governance:involvesArticle rdf:resource="&Governance;Article_24"/>
        <Governance:practicesDefinedInIso rdf:resource="&Governance;ISO_14271"/>
        <Governance:practicesDefinedInIso rdf:resource="&Governance;ISO_15939"/>
        <Governance:practicesDefinedInIso rdf:resource="&Governance;ISO_23081"/>
    </owl:NamedIndividual>
    


    <!-- http://www.semanticweb.org/IG/Governance#Monitoring_1 -->

    <owl:NamedIndividual rdf:about="&Governance;Monitoring_1">
        <rdf:type rdf:resource="&Governance;Monitoring"/>
        <Governance:involvesArticle rdf:resource="&Governance;Article_24"/>
        <Governance:involvesArticle rdf:resource="&Governance;Article_25"/>
        <Governance:involvesArticle rdf:resource="&Governance;Article_32"/>
        <Governance:involvesArticle rdf:resource="&Governance;Article_35"/>
        <Governance:involvesArticle rdf:resource="&Governance;Article_5"/>
        <Governance:involvesArticle rdf:resource="&Governance;Article_6"/>
        <Governance:practicesDefinedInIso rdf:resource="&Governance;ISO_15000"/>
        <Governance:practicesDefinedInIso rdf:resource="&Governance;ISO_15489"/>
        <Governance:practicesDefinedInIso rdf:resource="&Governance;ISO_15939"/>
        <Governance:practicesDefinedInIso rdf:resource="&Governance;ISO_17000"/>
        <Governance:practicesDefinedInIso rdf:resource="&Governance;ISO_27000"/>
        <Governance:practicesDefinedInIso rdf:resource="&Governance;ISO_27001"/>
        <Governance:responsibleFor rdf:resource="&Governance;Incident_Response_And_Remediation_Protocol_1"/>
    </owl:NamedIndividual>
    <owl:Axiom>
        <rdfs:comment>The Monitoring subcategory is responsible for detecting and monitoring security incidents in real-time. They actively watch for signs of unauthorized access, unusual activities, or potential threats within the organization&apos;s systems and networks. When an incident is detected, the Monitoring team initiates the incident response process, including alerting relevant stakeholders, analyzing the incident, and coordinating the appropriate actions for remediation and recovery.</rdfs:comment>
        <owl:annotatedTarget rdf:resource="&Governance;Incident_Response_And_Remediation_Protocol_1"/>
        <owl:annotatedSource rdf:resource="&Governance;Monitoring_1"/>
        <owl:annotatedProperty rdf:resource="&Governance;responsibleFor"/>
    </owl:Axiom>
    


    <!-- http://www.semanticweb.org/IG/Governance#Organizational_Communication -->

    <owl:NamedIndividual rdf:about="&Governance;Organizational_Communication">
        <rdf:type rdf:resource="&Governance;Goal"/>
    </owl:NamedIndividual>
    


    <!-- http://www.semanticweb.org/IG/Governance#PO_1_3 -->

    <owl:NamedIndividual rdf:about="&Governance;PO_1_3">
        <rdf:type rdf:resource="&Governance;IG_Capability"/>
        <Governance:capabilityDescription>The organization consistently defines strategic IT plans that align with business objectives and takes steps to review and adjust these plans periodically.</Governance:capabilityDescription>
        <Governance:inMaturityLevel rdf:resource="&Governance;3_Essential"/>
        <Governance:involvesArticle rdf:resource="&Governance;Article_25"/>
        <Governance:involvesArticle rdf:resource="&Governance;Article_30"/>
        <Governance:involvesArticle rdf:resource="&Governance;Article_5"/>
        <Governance:needsTechnicalRequirement rdf:resource="&Governance;Data_Mapping_And_Classification_System_1"/>
        <Governance:linkedToFramework rdf:resource="&Governance;ISACA_COBIT"/>
        <Governance:practicesDefinedInIso rdf:resource="&Governance;ISO_15939"/>
        <Governance:practicesDefinedInIso rdf:resource="&Governance;ISO_17000"/>
        <Governance:practicesDefinedInIso rdf:resource="&Governance;ISO_23081"/>
        <Governance:needsTechnicalRequirement rdf:resource="&Governance;IT_Planning_And_Strategy_Framework_1"/>
        <Governance:linkedToProcess rdf:resource="&Governance;Process_Plan_And_Organize_Foundational"/>
        <Governance:needsTechnicalRequirement rdf:resource="&Governance;Review_Cyles_1"/>
    </owl:NamedIndividual>
    <owl:Axiom>
        <rdfs:comment> Periodic reviews of IT plans allow for alignment adjustments and ensure that they remain effective in achieving business goals.</rdfs:comment>
        <owl:annotatedSource rdf:resource="&Governance;PO_1_3"/>
        <owl:annotatedTarget rdf:resource="&Governance;Review_Cyles_1"/>
        <owl:annotatedProperty rdf:resource="&Governance;needsTechnicalRequirement"/>
    </owl:Axiom>
    <owl:Axiom>
        <rdfs:comment> Understanding where personal data resides within IT plans is crucial for ensuring compliance with data protection regulations and assessing data-related risks.</rdfs:comment>
        <owl:annotatedTarget rdf:resource="&Governance;Data_Mapping_And_Classification_System_1"/>
        <owl:annotatedSource rdf:resource="&Governance;PO_1_3"/>
        <owl:annotatedProperty rdf:resource="&Governance;needsTechnicalRequirement"/>
    </owl:Axiom>
    <owl:Axiom>
        <rdfs:comment>A robust IT planning and strategy framework is essential for aligning IT initiatives with overall business objectives, ensuring efficient resource allocation, and fostering adaptability to changing market conditions.</rdfs:comment>
        <owl:annotatedTarget rdf:resource="&Governance;IT_Planning_And_Strategy_Framework_1"/>
        <owl:annotatedSource rdf:resource="&Governance;PO_1_3"/>
        <owl:annotatedProperty rdf:resource="&Governance;needsTechnicalRequirement"/>
    </owl:Axiom>
    


    <!-- http://www.semanticweb.org/IG/Governance#PO_1_4 -->

    <owl:NamedIndividual rdf:about="&Governance;PO_1_4">
        <rdf:type rdf:resource="&Governance;IG_Capability"/>
        <Governance:capabilityDescription>The organization establishes a formalized process for developing and maintaining strategic IT plans. These plans are documented, shared, and aligned with overall business strategies.</Governance:capabilityDescription>
        <Governance:inMaturityLevel rdf:resource="&Governance;4_Proactive"/>
        <Governance:involvesArticle rdf:resource="&Governance;Article_25"/>
        <Governance:involvesArticle rdf:resource="&Governance;Article_30"/>
        <Governance:involvesArticle rdf:resource="&Governance;Article_32"/>
        <Governance:involvesArticle rdf:resource="&Governance;Article_35"/>
        <Governance:involvesArticle rdf:resource="&Governance;Article_6"/>
        <Governance:technicalRequirementFor rdf:resource="&Governance;Collaboration_Tools_1"/>
        <Governance:technicalRequirementFor rdf:resource="&Governance;Data_Mapping_And_Classification_System_1"/>
        <Governance:technicalRequirementFor rdf:resource="&Governance;Document_Management_System_1"/>
        <Governance:linkedToFramework rdf:resource="&Governance;ISACA_COBIT"/>
        <Governance:practicesDefinedInIso rdf:resource="&Governance;ISO_15489"/>
        <Governance:practicesDefinedInIso rdf:resource="&Governance;ISO_15939"/>
        <Governance:practicesDefinedInIso rdf:resource="&Governance;ISO_17000"/>
        <Governance:practicesDefinedInIso rdf:resource="&Governance;ISO_23081"/>
        <Governance:practicesDefinedInIso rdf:resource="&Governance;ISO_27001"/>
        <Governance:technicalRequirementFor rdf:resource="&Governance;IT_Planning_And_Strategy_Framework_1"/>
        <Governance:technicalRequirementFor rdf:resource="&Governance;Privacy_Impact_Assessment_Tools_1"/>
        <Governance:linkedToProcess rdf:resource="&Governance;Process_Plan_And_Organize_Foundational"/>
    </owl:NamedIndividual>
    <owl:Axiom>
        <rdfs:comment>PIA tools help assess the impact of IT plans on data protection and privacy.</rdfs:comment>
        <owl:annotatedSource rdf:resource="&Governance;PO_1_4"/>
        <owl:annotatedTarget rdf:resource="&Governance;Privacy_Impact_Assessment_Tools_1"/>
        <owl:annotatedProperty rdf:resource="&Governance;technicalRequirementFor"/>
    </owl:Axiom>
    <owl:Axiom>
        <rdfs:comment> A robust DMS helps organize, store, and share IT plans while ensuring version control and accessibility.</rdfs:comment>
        <owl:annotatedTarget rdf:resource="&Governance;Document_Management_System_1"/>
        <owl:annotatedSource rdf:resource="&Governance;PO_1_4"/>
        <owl:annotatedProperty rdf:resource="&Governance;technicalRequirementFor"/>
    </owl:Axiom>
    <owl:Axiom>
        <rdfs:comment> Collaboration tools facilitate cross-functional team involvement in developing and sharing IT plans, ensuring alignment and stakeholder engagement.</rdfs:comment>
        <owl:annotatedTarget rdf:resource="&Governance;Collaboration_Tools_1"/>
        <owl:annotatedSource rdf:resource="&Governance;PO_1_4"/>
        <owl:annotatedProperty rdf:resource="&Governance;technicalRequirementFor"/>
    </owl:Axiom>
    <owl:Axiom>
        <rdfs:comment>Data mapping and classification tools assist in identifying personal data within IT plans, ensuring compliance with GDPR principles.</rdfs:comment>
        <owl:annotatedTarget rdf:resource="&Governance;Data_Mapping_And_Classification_System_1"/>
        <owl:annotatedSource rdf:resource="&Governance;PO_1_4"/>
        <owl:annotatedProperty rdf:resource="&Governance;technicalRequirementFor"/>
    </owl:Axiom>
    <owl:Axiom>
        <rdfs:comment>Specialized IT Planning and Strategy software assists in creating, documenting, and visualizing strategic IT plans, enhancing collaboration and alignment with business goals.</rdfs:comment>
        <owl:annotatedTarget rdf:resource="&Governance;IT_Planning_And_Strategy_Framework_1"/>
        <owl:annotatedSource rdf:resource="&Governance;PO_1_4"/>
        <owl:annotatedProperty rdf:resource="&Governance;technicalRequirementFor"/>
    </owl:Axiom>
    


    <!-- http://www.semanticweb.org/IG/Governance#PO_1_5 -->

    <owl:NamedIndividual rdf:about="&Governance;PO_1_5">
        <rdf:type rdf:resource="&Governance;IG_Capability"/>
        <Governance:capabilityDescription>The organization continuously monitors and improves its strategic IT planning process. It actively seeks feedback from stakeholders, adapts plans to changing circumstances, and demonstrates the agility to respond to emerging technologies and market shifts.</Governance:capabilityDescription>
        <Governance:inMaturityLevel rdf:resource="&Governance;5_Transformational"/>
        <Governance:involvesArticle rdf:resource="&Governance;Article_25"/>
        <Governance:involvesArticle rdf:resource="&Governance;Article_32"/>
        <Governance:involvesArticle rdf:resource="&Governance;Article_5"/>
        <Governance:involvesArticle rdf:resource="&Governance;Article_6"/>
        <Governance:needsTechnicalRequirement rdf:resource="&Governance;Change_Management_1"/>
        <Governance:needsTechnicalRequirement rdf:resource="&Governance;Collaboration_Tools_1"/>
        <Governance:linkedToFramework rdf:resource="&Governance;ISACA_COBIT"/>
        <Governance:practicesDefinedInIso rdf:resource="&Governance;ISO_14271"/>
        <Governance:practicesDefinedInIso rdf:resource="&Governance;ISO_15000"/>
        <Governance:practicesDefinedInIso rdf:resource="&Governance;ISO_15939"/>
        <Governance:practicesDefinedInIso rdf:resource="&Governance;ISO_17000"/>
        <Governance:needsTechnicalRequirement rdf:resource="&Governance;Monitoring_1"/>
        <Governance:linkedToProcess rdf:resource="&Governance;Process_Plan_And_Organize_Foundational"/>
        <Governance:needsTechnicalRequirement rdf:resource="&Governance;Review_Cyles_1"/>
    </owl:NamedIndividual>
    <owl:Axiom>
        <rdfs:comment>A structured change management system allows for controlled adjustments to IT plans based on changing circumstances.</rdfs:comment>
        <owl:annotatedTarget rdf:resource="&Governance;Change_Management_1"/>
        <owl:annotatedSource rdf:resource="&Governance;PO_1_5"/>
        <owl:annotatedProperty rdf:resource="&Governance;needsTechnicalRequirement"/>
    </owl:Axiom>
    <owl:Axiom>
        <rdfs:comment>Having mechanisms for gathering feedback from stakeholders ensures that the IT planning process remains aligned with business needs and is adaptable to changes. 

Also regurlar reviews can identify emerging technologies and help the organization to adapt IT plans and to embrace innovation while managing risks.</rdfs:comment>
        <owl:annotatedSource rdf:resource="&Governance;PO_1_5"/>
        <owl:annotatedTarget rdf:resource="&Governance;Review_Cyles_1"/>
        <owl:annotatedProperty rdf:resource="&Governance;needsTechnicalRequirement"/>
    </owl:Axiom>
    <owl:Axiom>
        <rdfs:comment>Tools for monitoring the progress and performance of IT plans help identify areas for improvement and adaptation.</rdfs:comment>
        <owl:annotatedTarget rdf:resource="&Governance;Monitoring_1"/>
        <owl:annotatedSource rdf:resource="&Governance;PO_1_5"/>
        <owl:annotatedProperty rdf:resource="&Governance;needsTechnicalRequirement"/>
    </owl:Axiom>
    <owl:Axiom>
        <rdfs:comment>Collaboration tools enable ongoing communication with stakeholders, ensuring that IT plans reflect their evolving needs.</rdfs:comment>
        <owl:annotatedTarget rdf:resource="&Governance;Collaboration_Tools_1"/>
        <owl:annotatedSource rdf:resource="&Governance;PO_1_5"/>
        <owl:annotatedProperty rdf:resource="&Governance;needsTechnicalRequirement"/>
    </owl:Axiom>
    


    <!-- http://www.semanticweb.org/IG/Governance#Privacy_1 -->

    <owl:NamedIndividual rdf:about="&Governance;Privacy_1">
        <rdf:type rdf:resource="&Governance;Privacy"/>
        <Governance:uses rdf:resource="&Governance;Data_Retention_Policy_Dummy"/>
        <Governance:responsibleFor rdf:resource="&Governance;Data_Sharing_Protocols_1"/>
        <Governance:canBeInvolvedWith rdf:resource="&Governance;Disposition_Policies_And_Procedures_1"/>
        <Governance:canBeInvolvedWith rdf:resource="&Governance;Document_Management_System_1"/>
    </owl:NamedIndividual>
    <owl:Axiom>
        <rdfs:comment>The Privacy department may use the system to manage privacy-related documents, data protection policies, and compliance documentation. The system helps maintain proper data handling practices and supports privacy regulation compliance.</rdfs:comment>
        <owl:annotatedTarget rdf:resource="&Governance;Document_Management_System_1"/>
        <owl:annotatedSource rdf:resource="&Governance;Privacy_1"/>
        <owl:annotatedProperty rdf:resource="&Governance;canBeInvolvedWith"/>
    </owl:Axiom>
    <owl:Axiom>
        <rdfs:comment>The Privacy department is responsible for designing and implementing &quot;Data Sharing Protocols.&quot; These protocols establish guidelines and procedures for sharing sensitive data both within and outside the organization. They ensure that data sharing practices align with privacy regulations, consent requirements, and data protection principles.</rdfs:comment>
        <owl:annotatedTarget rdf:resource="&Governance;Data_Sharing_Protocols_1"/>
        <owl:annotatedSource rdf:resource="&Governance;Privacy_1"/>
        <owl:annotatedProperty rdf:resource="&Governance;responsibleFor"/>
    </owl:Axiom>
    <owl:Axiom>
        <rdfs:comment>The Privacy department is concerned with the proper handling and protection of sensitive data, including its disposition. Implementing well-defined disposition policies ensures that personal and sensitive information is disposed of securely and in compliance with privacy regulations, minimizing the risk of data exposure and unauthorized access.</rdfs:comment>
        <owl:annotatedTarget rdf:resource="&Governance;Disposition_Policies_And_Procedures_1"/>
        <owl:annotatedSource rdf:resource="&Governance;Privacy_1"/>
        <owl:annotatedProperty rdf:resource="&Governance;canBeInvolvedWith"/>
    </owl:Axiom>
    <owl:Axiom>
        <rdfs:comment>The Privacy department uses the &quot;Data Retention Policy&quot; to ensure that data is retained and managed according to privacy regulations and principles. This involves adhering to specified retention periods for different types of data, ensuring data is securely stored, and facilitating its timely disposal when no longer needed. The policy helps maintain data privacy and minimize data exposure risks.</rdfs:comment>
        <owl:annotatedTarget rdf:resource="&Governance;Data_Retention_Policy_Dummy"/>
        <owl:annotatedSource rdf:resource="&Governance;Privacy_1"/>
        <owl:annotatedProperty rdf:resource="&Governance;uses"/>
    </owl:Axiom>
    


    <!-- http://www.semanticweb.org/IG/Governance#Privacy_And_Security_P1_3 -->

    <owl:NamedIndividual rdf:about="&Governance;Privacy_And_Security_P1_3">
        <rdf:type rdf:resource="&Governance;IG_Capability"/>
        <Governance:capabilityDescription>An up-to-date and accurate catalog of privacy laws and policies by country is readily accessible to all relevant employees. Policy communications are routine and semi-automated. Privacy controls are included on any provisioned system. A comprehensive privacy zone schema is deployed.</Governance:capabilityDescription>
        <Governance:inMaturityLevel rdf:resource="&Governance;3_Essential"/>
        <Governance:involvesArticle rdf:resource="&Governance;Article_12"/>
        <Governance:involvesArticle rdf:resource="&Governance;Article_24"/>
        <Governance:involvesArticle rdf:resource="&Governance;Article_25"/>
        <Governance:involvesArticle rdf:resource="&Governance;Article_5"/>
        <Governance:needsTechnicalRequirement rdf:resource="&Governance;Automated_Integration"/>
        <Governance:needsTechnicalRequirement rdf:resource="&Governance;Automated_Notification_System_1"/>
        <Governance:linkedToFramework rdf:resource="&Governance;CGOC_02"/>
        <Governance:needsTechnicalRequirement rdf:resource="&Governance;Communication_Platforms_1"/>
        <Governance:needsTechnicalRequirement rdf:resource="&Governance;Data_Mapping_And_Classification_System_1"/>
        <Governance:practicesDefinedInIso rdf:resource="&Governance;ISO_15489"/>
        <Governance:practicesDefinedInIso rdf:resource="&Governance;ISO_15939"/>
        <Governance:practicesDefinedInIso rdf:resource="&Governance;ISO_17000"/>
        <Governance:practicesDefinedInIso rdf:resource="&Governance;ISO_23081"/>
        <Governance:practicesDefinedInIso rdf:resource="&Governance;ISO_27000"/>
        <Governance:needsTechnicalRequirement rdf:resource="&Governance;Privacy_Laws_And_Policies_Repository_1"/>
        <Governance:linkedToProcess rdf:resource="&Governance;Process_Privacy_And_data_Protection_Obligation_1"/>
        <Governance:needsTechnicalRequirement rdf:resource="&Governance;Review_Cyles_1"/>
    </owl:NamedIndividual>
    <owl:Axiom>
        <rdfs:comment>Establishing a mechanism for communicating privacy obligations to data subjects and third parties who process and control information is essential for compliance and transparency.</rdfs:comment>
        <owl:annotatedTarget rdf:resource="&Governance;Communication_Platforms_1"/>
        <owl:annotatedSource rdf:resource="&Governance;Privacy_And_Security_P1_3"/>
        <owl:annotatedProperty rdf:resource="&Governance;needsTechnicalRequirement"/>
    </owl:Axiom>
    <owl:Axiom>
        <rdfs:comment>A well-defined privacy zone schema helps categorize data based on sensitivity, enabling the organization to apply appropriate privacy safeguards and controls.</rdfs:comment>
        <owl:annotatedTarget rdf:resource="&Governance;Data_Mapping_And_Classification_System_1"/>
        <owl:annotatedSource rdf:resource="&Governance;Privacy_And_Security_P1_3"/>
        <owl:annotatedProperty rdf:resource="&Governance;needsTechnicalRequirement"/>
    </owl:Axiom>
    <owl:Axiom>
        <rdfs:comment>Privacy controls should be integrated into all provisioned systems to ensure that data protection measures are inherent in system design and operation.</rdfs:comment>
        <owl:annotatedTarget rdf:resource="&Governance;Automated_Integration"/>
        <owl:annotatedSource rdf:resource="&Governance;Privacy_And_Security_P1_3"/>
        <owl:annotatedProperty rdf:resource="&Governance;needsTechnicalRequirement"/>
    </owl:Axiom>
    <owl:Axiom>
        <rdfs:comment>An automated system for policy communication ensures that employees are regularly informed about privacy laws, policies, and updates. Automation reduces the risk of missed communications.</rdfs:comment>
        <owl:annotatedTarget rdf:resource="&Governance;Automated_Notification_System_1"/>
        <owl:annotatedSource rdf:resource="&Governance;Privacy_And_Security_P1_3"/>
        <owl:annotatedProperty rdf:resource="&Governance;needsTechnicalRequirement"/>
    </owl:Axiom>
    <owl:Axiom>
        <rdfs:comment> Regularly reviewing and updating the privacy laws, policies, and controls is essential to ensure ongoing compliance with changing regulations.</rdfs:comment>
        <owl:annotatedSource rdf:resource="&Governance;Privacy_And_Security_P1_3"/>
        <owl:annotatedTarget rdf:resource="&Governance;Review_Cyles_1"/>
        <owl:annotatedProperty rdf:resource="&Governance;needsTechnicalRequirement"/>
    </owl:Axiom>
    <owl:Axiom>
        <rdfs:comment>A centralized repository for privacy laws and policies is crucial for providing easy access to relevant information for employees. This repository should be regularly updated to ensure accuracy.</rdfs:comment>
        <owl:annotatedSource rdf:resource="&Governance;Privacy_And_Security_P1_3"/>
        <owl:annotatedTarget rdf:resource="&Governance;Privacy_Laws_And_Policies_Repository_1"/>
        <owl:annotatedProperty rdf:resource="&Governance;needsTechnicalRequirement"/>
    </owl:Axiom>
    


    <!-- http://www.semanticweb.org/IG/Governance#Privacy_And_Security_P1_4 -->

    <owl:NamedIndividual rdf:about="&Governance;Privacy_And_Security_P1_4">
        <rdf:type rdf:resource="&Governance;IG_Capability"/>
        <Governance:capabilityDescription>There is a process to continually monitor and update privacy obligations arising from changes to legislation, regulations, business practices and industry requirements. Privacy by Design is incorporated into design specifications and architecture of new systems and processes.</Governance:capabilityDescription>
        <Governance:inMaturityLevel rdf:resource="&Governance;4_Proactive"/>
        <Governance:involvesArticle rdf:resource="&Governance;Article_25"/>
        <Governance:involvesArticle rdf:resource="&Governance;Article_33"/>
        <Governance:involvesArticle rdf:resource="&Governance;Article_34"/>
        <Governance:involvesArticle rdf:resource="&Governance;Article_35"/>
        <Governance:involvesArticle rdf:resource="&Governance;Article_5"/>
        <Governance:needsTechnicalRequirement rdf:resource="&Governance;Automated_Integration"/>
        <Governance:needsTechnicalRequirement rdf:resource="&Governance;Automated_Notification_System_1"/>
        <Governance:linkedToFramework rdf:resource="&Governance;CGOC_02"/>
        <Governance:needsTechnicalRequirement rdf:resource="&Governance;Data_Mapping_And_Classification_System_1"/>
        <Governance:practicesDefinedInIso rdf:resource="&Governance;ISO_15489"/>
        <Governance:practicesDefinedInIso rdf:resource="&Governance;ISO_15939"/>
        <Governance:practicesDefinedInIso rdf:resource="&Governance;ISO_17000"/>
        <Governance:practicesDefinedInIso rdf:resource="&Governance;ISO_27001"/>
        <Governance:needsTechnicalRequirement rdf:resource="&Governance;Monitoring_1"/>
        <Governance:linkedToProcess rdf:resource="&Governance;Process_Privacy_And_data_Protection_Obligation_1"/>
    </owl:NamedIndividual>
    <owl:Axiom>
        <rdfs:comment>A system to continually monitor changes in legislation, regulations, business practices, and industry requirements is crucial. This ensures that the organization remains aware of evolving privacy obligations, facilitating compliance.</rdfs:comment>
        <owl:annotatedTarget rdf:resource="&Governance;Monitoring_1"/>
        <owl:annotatedSource rdf:resource="&Governance;Privacy_And_Security_P1_4"/>
        <owl:annotatedProperty rdf:resource="&Governance;needsTechnicalRequirement"/>
    </owl:Axiom>
    <owl:Axiom>
        <rdfs:comment>A data mapping and classification system is necessary to determine privacy obligations based on the type of data, data subjects, and data location. It helps in understanding which obligations apply to different data sets.</rdfs:comment>
        <owl:annotatedTarget rdf:resource="&Governance;Data_Mapping_And_Classification_System_1"/>
        <owl:annotatedSource rdf:resource="&Governance;Privacy_And_Security_P1_4"/>
        <owl:annotatedProperty rdf:resource="&Governance;needsTechnicalRequirement"/>
    </owl:Axiom>
    <owl:Axiom>
        <rdfs:comment>An automated system for alerting and notifying relevant stakeholders about changes in privacy obligations ensures timely action and compliance.</rdfs:comment>
        <owl:annotatedTarget rdf:resource="&Governance;Automated_Notification_System_1"/>
        <owl:annotatedSource rdf:resource="&Governance;Privacy_And_Security_P1_4"/>
        <owl:annotatedProperty rdf:resource="&Governance;needsTechnicalRequirement"/>
    </owl:Axiom>
    <owl:Axiom>
        <rdfs:comment>Integrating Privacy by Design into the design specifications and architecture of new systems and processes is vital to ensure that data protection is inherent from the start.</rdfs:comment>
        <owl:annotatedTarget rdf:resource="&Governance;Automated_Integration"/>
        <owl:annotatedSource rdf:resource="&Governance;Privacy_And_Security_P1_4"/>
        <owl:annotatedProperty rdf:resource="&Governance;needsTechnicalRequirement"/>
    </owl:Axiom>
    


    <!-- http://www.semanticweb.org/IG/Governance#Privacy_And_Security_P2_3 -->

    <owl:NamedIndividual rdf:about="&Governance;Privacy_And_Security_P2_3">
        <rdf:type rdf:resource="&Governance;IG_Capability"/>
        <Governance:capabilityDescription>Periodic cyber-risk audits or penetration testing are performed to identify areas of weakness and include “table-top” exercises, with participants from key areas that would be affected by an incident. There is dual factor authentication and encryption at rest of repositories. Sensitive and proprietary data is discovered, classified and segregated in repositories with strict access and security controls such as masking.</Governance:capabilityDescription>
        <Governance:inMaturityLevel rdf:resource="&Governance;3_Essential"/>
        <Governance:needsTechnicalRequirement rdf:resource="&Governance;AccessControl_1"/>
        <Governance:involvesArticle rdf:resource="&Governance;Article_32"/>
        <Governance:involvesArticle rdf:resource="&Governance;Article_5"/>
        <Governance:needsTechnicalRequirement rdf:resource="&Governance;Audit_1"/>
        <Governance:needsTechnicalRequirement rdf:resource="&Governance;Authentication_1"/>
        <Governance:linkedToFramework rdf:resource="&Governance;CGOC_02"/>
        <Governance:needsTechnicalRequirement rdf:resource="&Governance;Data_Mapping_And_Classification_System_1"/>
        <Governance:needsTechnicalRequirement rdf:resource="&Governance;Encryption_1"/>
        <Governance:practicesDefinedInIso rdf:resource="&Governance;ISO_15939"/>
        <Governance:practicesDefinedInIso rdf:resource="&Governance;ISO_22301"/>
        <Governance:practicesDefinedInIso rdf:resource="&Governance;ISO_27001"/>
        <Governance:linkedToProcess rdf:resource="&Governance;Process_External_Intrusion_1"/>
        <Governance:needsTechnicalRequirement rdf:resource="&Governance;Testing_1"/>
        <Governance:needsTechnicalRequirement rdf:resource="&Governance;Training_1"/>
    </owl:NamedIndividual>
    <owl:Axiom>
        <rdfs:comment>Table-top exercises simulate cybersecurity incidents, testing the organization&apos;s incident response plans and improving preparedness.</rdfs:comment>
        <owl:annotatedSource rdf:resource="&Governance;Privacy_And_Security_P2_3"/>
        <owl:annotatedTarget rdf:resource="&Governance;Training_1"/>
        <owl:annotatedProperty rdf:resource="&Governance;needsTechnicalRequirement"/>
    </owl:Axiom>
    <owl:Axiom>
        <rdfs:comment>Encrypting data at rest ensures that data stored on devices or repositories remains secure, even if physical access is compromised.</rdfs:comment>
        <owl:annotatedTarget rdf:resource="&Governance;Encryption_1"/>
        <owl:annotatedSource rdf:resource="&Governance;Privacy_And_Security_P2_3"/>
        <owl:annotatedProperty rdf:resource="&Governance;needsTechnicalRequirement"/>
    </owl:Axiom>
    <owl:Axiom>
        <rdfs:comment>Identifying and classifying sensitive and proprietary data is essential for applying appropriate security controls based on data sensitivity.</rdfs:comment>
        <owl:annotatedTarget rdf:resource="&Governance;Data_Mapping_And_Classification_System_1"/>
        <owl:annotatedSource rdf:resource="&Governance;Privacy_And_Security_P2_3"/>
        <owl:annotatedProperty rdf:resource="&Governance;needsTechnicalRequirement"/>
    </owl:Axiom>
    <owl:Axiom>
        <rdfs:comment>Segregating sensitive data and implementing strict access and security controls, including data masking, helps protect data from unauthorized access.</rdfs:comment>
        <owl:annotatedTarget rdf:resource="&Governance;AccessControl_1"/>
        <owl:annotatedSource rdf:resource="&Governance;Privacy_And_Security_P2_3"/>
        <owl:annotatedProperty rdf:resource="&Governance;needsTechnicalRequirement"/>
    </owl:Axiom>
    <owl:Axiom>
        <rdfs:comment>Penetration testing involves simulating cyberattacks to identify weaknesses in the organization&apos;s defenses, helping to proactively address vulnerabilities.</rdfs:comment>
        <owl:annotatedSource rdf:resource="&Governance;Privacy_And_Security_P2_3"/>
        <owl:annotatedTarget rdf:resource="&Governance;Testing_1"/>
        <owl:annotatedProperty rdf:resource="&Governance;needsTechnicalRequirement"/>
    </owl:Axiom>
    <owl:Axiom>
        <rdfs:comment>Regular cyber-risk audits help identify vulnerabilities and assess the overall security posture of the organization&apos;s information systems.</rdfs:comment>
        <owl:annotatedTarget rdf:resource="&Governance;Audit_1"/>
        <owl:annotatedSource rdf:resource="&Governance;Privacy_And_Security_P2_3"/>
        <owl:annotatedProperty rdf:resource="&Governance;needsTechnicalRequirement"/>
    </owl:Axiom>
    <owl:Axiom>
        <rdfs:comment> Implementing dual-factor authentication enhances security by requiring two forms of verification for access, reducing the risk of unauthorized entry.</rdfs:comment>
        <owl:annotatedTarget rdf:resource="&Governance;Authentication_1"/>
        <owl:annotatedSource rdf:resource="&Governance;Privacy_And_Security_P2_3"/>
        <owl:annotatedProperty rdf:resource="&Governance;needsTechnicalRequirement"/>
    </owl:Axiom>
    


    <!-- http://www.semanticweb.org/IG/Governance#Privacy_And_Security_P2_4 -->

    <owl:NamedIndividual rdf:about="&Governance;Privacy_And_Security_P2_4">
        <rdf:type rdf:resource="&Governance;IG_Capability"/>
        <Governance:capabilityDescription>Risk assessments and threat intelligence sharing are automated. There is an integrated view of log and event data, with network flow and packets.</Governance:capabilityDescription>
        <Governance:inMaturityLevel rdf:resource="&Governance;4_Proactive"/>
        <Governance:needsTechnicalRequirement rdf:resource="&Governance;Analytics_1"/>
        <Governance:involvesArticle rdf:resource="&Governance;Article_32"/>
        <Governance:needsTechnicalRequirement rdf:resource="&Governance;Automated_Integration"/>
        <Governance:needsTechnicalRequirement rdf:resource="&Governance;Automated_Risk_Assessment_System_1"/>
        <Governance:linkedToFramework rdf:resource="&Governance;CGOC_02"/>
        <Governance:needsTechnicalRequirement rdf:resource="&Governance;Collaboration_Tools_1"/>
        <Governance:practicesDefinedInIso rdf:resource="&Governance;ISO_27001"/>
        <Governance:practicesDefinedInIso rdf:resource="&Governance;ISO_27010"/>
        <Governance:linkedToProcess rdf:resource="&Governance;Process_External_Intrusion_1"/>
    </owl:NamedIndividual>
    <owl:Axiom>
        <rdfs:comment> Integration of log and event data from various sources provides a unified view of system activities, helping to detect and respond to security incidents effectively.</rdfs:comment>
        <owl:annotatedTarget rdf:resource="&Governance;Automated_Integration"/>
        <owl:annotatedSource rdf:resource="&Governance;Privacy_And_Security_P2_4"/>
        <owl:annotatedProperty rdf:resource="&Governance;needsTechnicalRequirement"/>
    </owl:Axiom>
    <owl:Axiom>
        <rdfs:comment>An automated risk assessment system is essential for continuously evaluating and identifying potential security risks, vulnerabilities, and threats to the organization&apos;s data and systems.</rdfs:comment>
        <owl:annotatedTarget rdf:resource="&Governance;Automated_Risk_Assessment_System_1"/>
        <owl:annotatedSource rdf:resource="&Governance;Privacy_And_Security_P2_4"/>
        <owl:annotatedProperty rdf:resource="&Governance;needsTechnicalRequirement"/>
    </owl:Axiom>
    <owl:Axiom>
        <rdfs:comment> Network flow and packet analysis systems enable the organization to inspect network traffic for abnormal patterns and potential intrusions, enhancing network security.</rdfs:comment>
        <owl:annotatedTarget rdf:resource="&Governance;Analytics_1"/>
        <owl:annotatedSource rdf:resource="&Governance;Privacy_And_Security_P2_4"/>
        <owl:annotatedProperty rdf:resource="&Governance;needsTechnicalRequirement"/>
    </owl:Axiom>
    <owl:Axiom>
        <rdfs:comment> A threat intelligence sharing platform facilitates collaboration and information exchange about emerging threats, enabling the organization to stay informed and take proactive security measures.</rdfs:comment>
        <owl:annotatedTarget rdf:resource="&Governance;Collaboration_Tools_1"/>
        <owl:annotatedSource rdf:resource="&Governance;Privacy_And_Security_P2_4"/>
        <owl:annotatedProperty rdf:resource="&Governance;needsTechnicalRequirement"/>
    </owl:Axiom>
    


    <!-- http://www.semanticweb.org/IG/Governance#Privacy_And_Security_P3_3 -->

    <owl:NamedIndividual rdf:about="&Governance;Privacy_And_Security_P3_3">
        <rdf:type rdf:resource="&Governance;IG_Capability"/>
        <Governance:capabilityDescription>Developing safeguards around classifying confidential information and preventing it from leaving via the network or employee devices.</Governance:capabilityDescription>
        <Governance:inMaturityLevel rdf:resource="&Governance;3_Essential"/>
        <Governance:needsTechnicalRequirement rdf:resource="&Governance;AccessControl_1"/>
        <Governance:involvesArticle rdf:resource="&Governance;Article_32"/>
        <Governance:involvesArticle rdf:resource="&Governance;Article_5"/>
        <Governance:needsTechnicalRequirement rdf:resource="&Governance;Backup_1"/>
        <Governance:linkedToFramework rdf:resource="&Governance;CGOC_02"/>
        <Governance:needsTechnicalRequirement rdf:resource="&Governance;Data_Mapping_And_Classification_System_1"/>
        <Governance:needsTechnicalRequirement rdf:resource="&Governance;Encryption_1"/>
        <Governance:practicesDefinedInIso rdf:resource="&Governance;ISO_27001"/>
        <Governance:linkedToProcess rdf:resource="&Governance;Process_Accidental_Data_Leakage_1"/>
        <Governance:needsTechnicalRequirement rdf:resource="&Governance;Remote_Wiping_1"/>
    </owl:NamedIndividual>
    <owl:Axiom>
        <rdfs:comment>A data classification system is crucial for allowing employees to designate sensitive or confidential information. It enables the organization to identify and categorize data based on its sensitivity, ensuring that appropriate security measures are applied.</rdfs:comment>
        <owl:annotatedTarget rdf:resource="&Governance;Data_Mapping_And_Classification_System_1"/>
        <owl:annotatedSource rdf:resource="&Governance;Privacy_And_Security_P3_3"/>
        <owl:annotatedProperty rdf:resource="&Governance;needsTechnicalRequirement"/>
    </owl:Axiom>
    <owl:Axiom>
        <rdfs:comment>Enforcing access controls across multiple channels, including mobile, social, and cloud, is vital to restrict unauthorized access to sensitive data and prevent data leakage.</rdfs:comment>
        <owl:annotatedTarget rdf:resource="&Governance;AccessControl_1"/>
        <owl:annotatedSource rdf:resource="&Governance;Privacy_And_Security_P3_3"/>
        <owl:annotatedProperty rdf:resource="&Governance;needsTechnicalRequirement"/>
    </owl:Axiom>
    <owl:Axiom>
        <rdfs:comment> Implementing endpoint data protection measures, including encryption, remote wiping, and backup, is essential to safeguard sensitive data on employee devices and prevent accidental data leakage.</rdfs:comment>
        <owl:annotatedSource rdf:resource="&Governance;Privacy_And_Security_P3_3"/>
        <owl:annotatedTarget rdf:resource="&Governance;Remote_Wiping_1"/>
        <owl:annotatedProperty rdf:resource="&Governance;needsTechnicalRequirement"/>
    </owl:Axiom>
    <owl:Axiom>
        <rdfs:comment> Implementing endpoint data protection measures, including encryption, remote wiping, and backup, is essential to safeguard sensitive data on employee devices and prevent accidental data leakage.</rdfs:comment>
        <owl:annotatedTarget rdf:resource="&Governance;Encryption_1"/>
        <owl:annotatedSource rdf:resource="&Governance;Privacy_And_Security_P3_3"/>
        <owl:annotatedProperty rdf:resource="&Governance;needsTechnicalRequirement"/>
    </owl:Axiom>
    <owl:Axiom>
        <rdfs:comment> Implementing endpoint data protection measures, including encryption, remote wiping, and backup, is essential to safeguard sensitive data on employee devices and prevent accidental data leakage.</rdfs:comment>
        <owl:annotatedTarget rdf:resource="&Governance;Backup_1"/>
        <owl:annotatedSource rdf:resource="&Governance;Privacy_And_Security_P3_3"/>
        <owl:annotatedProperty rdf:resource="&Governance;needsTechnicalRequirement"/>
    </owl:Axiom>
    


    <!-- http://www.semanticweb.org/IG/Governance#Privacy_And_Security_P3_4 -->

    <owl:NamedIndividual rdf:about="&Governance;Privacy_And_Security_P3_4">
        <rdf:type rdf:resource="&Governance;IG_Capability"/>
        <Governance:capabilityDescription>Messaging and other systems provide both automatic and easy-to-use manual designation of sensitive information.</Governance:capabilityDescription>
        <Governance:inMaturityLevel rdf:resource="&Governance;4_Proactive"/>
        <Governance:involvesArticle rdf:resource="&Governance;Article_32"/>
        <Governance:involvesArticle rdf:resource="&Governance;Article_5"/>
        <Governance:needsTechnicalRequirement rdf:resource="&Governance;Automated_Integration"/>
        <Governance:linkedToFramework rdf:resource="&Governance;CGOC_02"/>
        <Governance:needsTechnicalRequirement rdf:resource="&Governance;Data_Mapping_And_Classification_System_1"/>
        <Governance:needsTechnicalRequirement rdf:resource="&Governance;Designation_Interface_1"/>
        <Governance:practicesDefinedInIso rdf:resource="&Governance;ISO_15000"/>
        <Governance:practicesDefinedInIso rdf:resource="&Governance;ISO_15489"/>
        <Governance:practicesDefinedInIso rdf:resource="&Governance;ISO_23081"/>
        <Governance:linkedToProcess rdf:resource="&Governance;Process_Accidental_Data_Leakage_1"/>
    </owl:NamedIndividual>
    <owl:Axiom>
        <rdfs:comment> Integrating data classification with messaging and other systems ensures that sensitive information is properly tagged or encrypted, reducing the risk of accidental data leakage through these systems.</rdfs:comment>
        <owl:annotatedTarget rdf:resource="&Governance;Automated_Integration"/>
        <owl:annotatedSource rdf:resource="&Governance;Privacy_And_Security_P3_4"/>
        <owl:annotatedProperty rdf:resource="&Governance;needsTechnicalRequirement"/>
    </owl:Axiom>
    <owl:Axiom>
        <rdfs:comment> Implementing a data classification system is crucial for allowing both automatic and manual designation of sensitive information. It categorizes data based on its sensitivity, facilitating appropriate protection measures.</rdfs:comment>
        <owl:annotatedTarget rdf:resource="&Governance;Data_Mapping_And_Classification_System_1"/>
        <owl:annotatedSource rdf:resource="&Governance;Privacy_And_Security_P3_4"/>
        <owl:annotatedProperty rdf:resource="&Governance;needsTechnicalRequirement"/>
    </owl:Axiom>
    <owl:Axiom>
        <rdfs:comment>Providing easy-to-use manual designation interfaces empowers employees to label sensitive information, making the process efficient and reducing the likelihood of errors.</rdfs:comment>
        <owl:annotatedTarget rdf:resource="&Governance;Designation_Interface_1"/>
        <owl:annotatedSource rdf:resource="&Governance;Privacy_And_Security_P3_4"/>
        <owl:annotatedProperty rdf:resource="&Governance;needsTechnicalRequirement"/>
    </owl:Axiom>
    


    <!-- http://www.semanticweb.org/IG/Governance#Privacy_And_Security_P4_3 -->

    <owl:NamedIndividual rdf:about="&Governance;Privacy_And_Security_P4_3">
        <rdf:type rdf:resource="&Governance;IG_Capability"/>
        <Governance:capabilityDescription>Endpoint data protection including encryption, remote wiping and backup is implemented. Access controls enforced for users across multiple channels, including mobile, social and cloud.</Governance:capabilityDescription>
        <Governance:inMaturityLevel rdf:resource="&Governance;3_Essential"/>
        <Governance:needsTechnicalRequirement rdf:resource="&Governance;AccessControl_1"/>
        <Governance:involvesArticle rdf:resource="&Governance;Article_32"/>
        <Governance:involvesArticle rdf:resource="&Governance;Article_5"/>
        <Governance:needsTechnicalRequirement rdf:resource="&Governance;Backup_1"/>
        <Governance:linkedToFramework rdf:resource="&Governance;CGOC_02"/>
        <Governance:needsTechnicalRequirement rdf:resource="&Governance;Encryption_1"/>
        <Governance:practicesDefinedInIso rdf:resource="&Governance;ISO_27001"/>
        <Governance:linkedToProcess rdf:resource="&Governance;Process_Insider_Theft_Of_Data_1"/>
        <Governance:needsTechnicalRequirement rdf:resource="&Governance;Remote_Wiping_1"/>
    </owl:NamedIndividual>
    <owl:Axiom>
        <rdfs:comment> Implementing endpoint data protection measures, including encryption, remote wiping, and backup, is crucial for safeguarding sensitive data stored on endpoint devices such as laptops, smartphones, and tablets.</rdfs:comment>
        <owl:annotatedTarget rdf:resource="&Governance;Backup_1"/>
        <owl:annotatedSource rdf:resource="&Governance;Privacy_And_Security_P4_3"/>
        <owl:annotatedProperty rdf:resource="&Governance;needsTechnicalRequirement"/>
    </owl:Axiom>
    <owl:Axiom>
        <rdfs:comment>Enforcing access controls for users across multiple channels, including mobile, social, and cloud, helps prevent unauthorized access to sensitive data and mitigates the risk of insider theft.</rdfs:comment>
        <owl:annotatedTarget rdf:resource="&Governance;AccessControl_1"/>
        <owl:annotatedSource rdf:resource="&Governance;Privacy_And_Security_P4_3"/>
        <owl:annotatedProperty rdf:resource="&Governance;needsTechnicalRequirement"/>
    </owl:Axiom>
    <owl:Axiom>
        <rdfs:comment> Implementing endpoint data protection measures, including encryption, remote wiping, and backup, is crucial for safeguarding sensitive data stored on endpoint devices such as laptops, smartphones, and tablets.</rdfs:comment>
        <owl:annotatedTarget rdf:resource="&Governance;Encryption_1"/>
        <owl:annotatedSource rdf:resource="&Governance;Privacy_And_Security_P4_3"/>
        <owl:annotatedProperty rdf:resource="&Governance;needsTechnicalRequirement"/>
    </owl:Axiom>
    <owl:Axiom>
        <rdfs:comment> Implementing endpoint data protection measures, including encryption, remote wiping, and backup, is crucial for safeguarding sensitive data stored on endpoint devices such as laptops, smartphones, and tablets.</rdfs:comment>
        <owl:annotatedSource rdf:resource="&Governance;Privacy_And_Security_P4_3"/>
        <owl:annotatedTarget rdf:resource="&Governance;Remote_Wiping_1"/>
        <owl:annotatedProperty rdf:resource="&Governance;needsTechnicalRequirement"/>
    </owl:Axiom>
    


    <!-- http://www.semanticweb.org/IG/Governance#Privacy_And_Security_P4_4 -->

    <owl:NamedIndividual rdf:about="&Governance;Privacy_And_Security_P4_4">
        <rdf:type rdf:resource="&Governance;IG_Capability"/>
        <Governance:capabilityDescription>360-degree proactive monitoring of employee behavior including email, instant messages, documents accessed and software applications is available. Ability to capture and archive evidence of incidents for forensic analysis. Ability to perform behavioral analytics to perform threat analysis.</Governance:capabilityDescription>
        <Governance:inMaturityLevel rdf:resource="&Governance;4_Proactive"/>
        <Governance:needsTechnicalRequirement rdf:resource="&Governance;Analytics_1"/>
        <Governance:involvesArticle rdf:resource="&Governance;Article_32"/>
        <Governance:involvesArticle rdf:resource="&Governance;Article_33"/>
        <Governance:involvesArticle rdf:resource="&Governance;Article_34"/>
        <Governance:linkedToFramework rdf:resource="&Governance;CGOC_02"/>
        <Governance:practicesDefinedInIso rdf:resource="&Governance;ISO_27001"/>
        <Governance:practicesDefinedInIso rdf:resource="&Governance;ISO_27002"/>
        <Governance:needsTechnicalRequirement rdf:resource="&Governance;Incident_Response_And_Remediation_Protocol_1"/>
        <Governance:needsTechnicalRequirement rdf:resource="&Governance;Monitoring_1"/>
        <Governance:linkedToProcess rdf:resource="&Governance;Process_Insider_Theft_Of_Data_1"/>
    </owl:NamedIndividual>
    <owl:Axiom>
        <rdfs:comment>The ability to capture and archive evidence of incidents is critical for conducting forensic analysis and investigations in case of security incidents or insider threats.</rdfs:comment>
        <owl:annotatedTarget rdf:resource="&Governance;Incident_Response_And_Remediation_Protocol_1"/>
        <owl:annotatedSource rdf:resource="&Governance;Privacy_And_Security_P4_4"/>
        <owl:annotatedProperty rdf:resource="&Governance;needsTechnicalRequirement"/>
    </owl:Axiom>
    <owl:Axiom>
        <rdfs:comment>The capability to perform behavioral analytics is vital for identifying patterns, anomalies, or deviations in employee behavior that may indicate insider threats or security risks.</rdfs:comment>
        <owl:annotatedTarget rdf:resource="&Governance;Analytics_1"/>
        <owl:annotatedSource rdf:resource="&Governance;Privacy_And_Security_P4_4"/>
        <owl:annotatedProperty rdf:resource="&Governance;needsTechnicalRequirement"/>
    </owl:Axiom>
    <owl:Axiom>
        <rdfs:comment> Implementing a comprehensive system for monitoring employee behavior, including activities such as email communications, instant messages, document access, and software application usage, is essential for detecting suspicious or unauthorized actions.</rdfs:comment>
        <owl:annotatedTarget rdf:resource="&Governance;Monitoring_1"/>
        <owl:annotatedSource rdf:resource="&Governance;Privacy_And_Security_P4_4"/>
        <owl:annotatedProperty rdf:resource="&Governance;needsTechnicalRequirement"/>
    </owl:Axiom>
    


    <!-- http://www.semanticweb.org/IG/Governance#Privacy_Impact_Assesments -->

    <owl:NamedIndividual rdf:about="&Governance;Privacy_Impact_Assesments">
        <rdf:type rdf:resource="&Governance;IG_Capability"/>
    </owl:NamedIndividual>
    


    <!-- http://www.semanticweb.org/IG/Governance#Privacy_Impact_Assessment_Tools_1 -->

    <owl:NamedIndividual rdf:about="&Governance;Privacy_Impact_Assessment_Tools_1">
        <rdf:type rdf:resource="&Governance;Privacy_Impact_Assessment_Tools"/>
        <Governance:involvesArticle rdf:resource="&Governance;Article_35"/>
        <Governance:practicesDefinedInIso rdf:resource="&Governance;ISO_27001"/>
    </owl:NamedIndividual>
    


    <!-- http://www.semanticweb.org/IG/Governance#Privacy_Laws_And_Policies_Repository_1 -->

    <owl:NamedIndividual rdf:about="&Governance;Privacy_Laws_And_Policies_Repository_1">
        <rdf:type rdf:resource="&Governance;Privacy_Laws_And_Policies_Repository"/>
        <Governance:involvesArticle rdf:resource="&Governance;Article_12"/>
        <Governance:practicesDefinedInIso rdf:resource="&Governance;ISO_15489"/>
    </owl:NamedIndividual>
    


    <!-- http://www.semanticweb.org/IG/Governance#Process_Accidental_Data_Leakage_1 -->

    <owl:NamedIndividual rdf:about="&Governance;Process_Accidental_Data_Leakage_1">
        <rdf:type rdf:resource="&Governance;Process"/>
    </owl:NamedIndividual>
    


    <!-- http://www.semanticweb.org/IG/Governance#Process_Active_Data_Management_1 -->

    <owl:NamedIndividual rdf:about="&Governance;Process_Active_Data_Management_1">
        <rdf:type rdf:resource="&Governance;Process"/>
    </owl:NamedIndividual>
    


    <!-- http://www.semanticweb.org/IG/Governance#Process_Audit_1 -->

    <owl:NamedIndividual rdf:about="&Governance;Process_Audit_1">
        <rdf:type rdf:resource="&Governance;Process"/>
    </owl:NamedIndividual>
    


    <!-- http://www.semanticweb.org/IG/Governance#Process_Cloud_Computing_1 -->

    <owl:NamedIndividual rdf:about="&Governance;Process_Cloud_Computing_1">
        <rdf:type rdf:resource="&Governance;Process"/>
    </owl:NamedIndividual>
    


    <!-- http://www.semanticweb.org/IG/Governance#Process_Data_On_Legal_Hold_1 -->

    <owl:NamedIndividual rdf:about="&Governance;Process_Data_On_Legal_Hold_1">
        <rdf:type rdf:resource="&Governance;Process"/>
        <Governance:processDescription>Determining information, records and data sources that are potentially relevant to an actual or anticipated lawsuit or government investigation.</Governance:processDescription>
    </owl:NamedIndividual>
    


    <!-- http://www.semanticweb.org/IG/Governance#Process_Data_Quality_And_Data_Lineage_1 -->

    <owl:NamedIndividual rdf:about="&Governance;Process_Data_Quality_And_Data_Lineage_1">
        <rdf:type rdf:resource="&Governance;Process"/>
    </owl:NamedIndividual>
    


    <!-- http://www.semanticweb.org/IG/Governance#Process_Data_Source_Catalog_And_Stewardship_1 -->

    <owl:NamedIndividual rdf:about="&Governance;Process_Data_Source_Catalog_And_Stewardship_1">
        <rdf:type rdf:resource="&Governance;Process"/>
    </owl:NamedIndividual>
    


    <!-- http://www.semanticweb.org/IG/Governance#Process_Departmental_Information_Practice_1 -->

    <owl:NamedIndividual rdf:about="&Governance;Process_Departmental_Information_Practice_1">
        <rdf:type rdf:resource="&Governance;Process"/>
    </owl:NamedIndividual>
    


    <!-- http://www.semanticweb.org/IG/Governance#Process_Disposal_And_Decomissioning_1 -->

    <owl:NamedIndividual rdf:about="&Governance;Process_Disposal_And_Decomissioning_1">
        <rdf:type rdf:resource="&Governance;Process"/>
    </owl:NamedIndividual>
    


    <!-- http://www.semanticweb.org/IG/Governance#Process_Employees_On_Hold_1 -->

    <owl:NamedIndividual rdf:about="&Governance;Process_Employees_On_Hold_1">
        <rdf:type rdf:resource="&Governance;Process"/>
        <Governance:processDescription>Determining employees with information potentially relevant to an actual or anticipated lawsuit or government investigation.</Governance:processDescription>
    </owl:NamedIndividual>
    


    <!-- http://www.semanticweb.org/IG/Governance#Process_Evidence_Analysis_And_Cost_Controls_1 -->

    <owl:NamedIndividual rdf:about="&Governance;Process_Evidence_Analysis_And_Cost_Controls_1">
        <rdf:type rdf:resource="&Governance;Process"/>
        <Governance:processDescription>Assessing information to understand dispute and potential information sources and for determining, controlling and communicating the costs of outside review of relevant information.</Governance:processDescription>
    </owl:NamedIndividual>
    


    <!-- http://www.semanticweb.org/IG/Governance#Process_Evidence_Collection_1 -->

    <owl:NamedIndividual rdf:about="&Governance;Process_Evidence_Collection_1">
        <rdf:type rdf:resource="&Governance;Process"/>
        <Governance:processDescription>Fact finding and inquiry with employees with knowledge of a matter in dispute to determine potentially relevant information and its whereabouts and sources. Collecting potential evidence in response to an agreedupon request with an adversary or government agency.</Governance:processDescription>
    </owl:NamedIndividual>
    


    <!-- http://www.semanticweb.org/IG/Governance#Process_External_Intrusion_1 -->

    <owl:NamedIndividual rdf:about="&Governance;Process_External_Intrusion_1">
        <rdf:type rdf:resource="&Governance;Process"/>
    </owl:NamedIndividual>
    


    <!-- http://www.semanticweb.org/IG/Governance#Process_Hold_Publication_1 -->

    <owl:NamedIndividual rdf:about="&Governance;Process_Hold_Publication_1">
        <rdf:type rdf:resource="&Governance;Process"/>
    </owl:NamedIndividual>
    


    <!-- http://www.semanticweb.org/IG/Governance#Process_Information_Retention_And_Disposal_Obligation_1 -->

    <owl:NamedIndividual rdf:about="&Governance;Process_Information_Retention_And_Disposal_Obligation_1">
        <rdf:type rdf:resource="&Governance;Process"/>
    </owl:NamedIndividual>
    


    <!-- http://www.semanticweb.org/IG/Governance#Process_Insider_Theft_Of_Data_1 -->

    <owl:NamedIndividual rdf:about="&Governance;Process_Insider_Theft_Of_Data_1">
        <rdf:type rdf:resource="&Governance;Process"/>
    </owl:NamedIndividual>
    


    <!-- http://www.semanticweb.org/IG/Governance#Process_Legacy_Data_Management_1 -->

    <owl:NamedIndividual rdf:about="&Governance;Process_Legacy_Data_Management_1">
        <rdf:type rdf:resource="&Governance;Process"/>
    </owl:NamedIndividual>
    


    <!-- http://www.semanticweb.org/IG/Governance#Process_Legal_Records_1 -->

    <owl:NamedIndividual rdf:about="&Governance;Process_Legal_Records_1">
        <rdf:type rdf:resource="&Governance;Process"/>
        <Governance:processDescription>Documenting the custodians and data sources identified the legal hold and collection activities over multi-year matter lifecycle.</Governance:processDescription>
    </owl:NamedIndividual>
    


    <!-- http://www.semanticweb.org/IG/Governance#Process_Plan_And_Organize_Foundational -->

    <owl:NamedIndividual rdf:about="&Governance;Process_Plan_And_Organize_Foundational">
        <rdf:type rdf:resource="&Governance;Process"/>
    </owl:NamedIndividual>
    


    <!-- http://www.semanticweb.org/IG/Governance#Process_Privacy_And_data_Protection_Obligation_1 -->

    <owl:NamedIndividual rdf:about="&Governance;Process_Privacy_And_data_Protection_Obligation_1">
        <rdf:type rdf:resource="&Governance;Process"/>
    </owl:NamedIndividual>
    


    <!-- http://www.semanticweb.org/IG/Governance#Process_Realize_Information_Value_1 -->

    <owl:NamedIndividual rdf:about="&Governance;Process_Realize_Information_Value_1">
        <rdf:type rdf:resource="&Governance;Process"/>
    </owl:NamedIndividual>
    


    <!-- http://www.semanticweb.org/IG/Governance#Process_Storage_Alignment_1 -->

    <owl:NamedIndividual rdf:about="&Governance;Process_Storage_Alignment_1">
        <rdf:type rdf:resource="&Governance;Process"/>
    </owl:NamedIndividual>
    


    <!-- http://www.semanticweb.org/IG/Governance#Process_System_Provisioning_1 -->

    <owl:NamedIndividual rdf:about="&Governance;Process_System_Provisioning_1">
        <rdf:type rdf:resource="&Governance;Process"/>
    </owl:NamedIndividual>
    


    <!-- http://www.semanticweb.org/IG/Governance#Protection -->

    <owl:NamedIndividual rdf:about="&Governance;Protection">
        <rdf:type rdf:resource="&Governance;Goal"/>
    </owl:NamedIndividual>
    


    <!-- http://www.semanticweb.org/IG/Governance#RIM_P1_3 -->

    <owl:NamedIndividual rdf:about="&Governance;RIM_P1_3">
        <rdf:type rdf:resource="&Governance;IG_Capability"/>
        <Governance:capabilityDescription>Established retention period for regulated information. The specific or actual laws that dictate retention periods are known and clearly mapped to each record class so changes can be easily traced and decisions readily defended. Posted policy and schedules are role specific so that individuals can determine their obligations. Electronic and physical records are both retained and disposed against the schedule. Disaster recovery, retention, and preservation are all disentangled and severable in policy and practice.</Governance:capabilityDescription>
        <Governance:inMaturityLevel rdf:resource="&Governance;3_Essential"/>
        <Governance:involvesArticle rdf:resource="&Governance;Article_25"/>
        <Governance:involvesArticle rdf:resource="&Governance;Article_32"/>
        <Governance:involvesArticle rdf:resource="&Governance;Article_5"/>
        <Governance:linkedToFramework rdf:resource="&Governance;CGOC_02"/>
        <Governance:needsTechnicalRequirement rdf:resource="&Governance;Data_Mapping_And_Classification_System_1"/>
        <Governance:needsTechnicalRequirement rdf:resource="&Governance;ERM_1"/>
        <Governance:practicesDefinedInIso rdf:resource="&Governance;ISO_15489"/>
        <Governance:practicesDefinedInIso rdf:resource="&Governance;ISO_17000"/>
        <Governance:needsTechnicalRequirement rdf:resource="&Governance;Laws_Mapping_And_Compliance_Tracking_1"/>
        <Governance:linkedToProcess rdf:resource="&Governance;Process_Information_Retention_And_Disposal_Obligation_1"/>
        <Governance:needsTechnicalRequirement rdf:resource="&Governance;Records_Information_Management_1"/>
        <Governance:linkedToBusinessUnit rdf:resource="&Governance;Records_Information_Management_1"/>
    </owl:NamedIndividual>
    <owl:Axiom>
        <rdfs:comment> Developing an information classification schema is essential for categorizing and organizing data based on its significance and regulatory requirements. This enables effective retention management and ensures that each record class is aligned with relevant laws and obligations.</rdfs:comment>
        <owl:annotatedTarget rdf:resource="&Governance;Data_Mapping_And_Classification_System_1"/>
        <owl:annotatedSource rdf:resource="&Governance;RIM_P1_3"/>
        <owl:annotatedProperty rdf:resource="&Governance;needsTechnicalRequirement"/>
    </owl:Axiom>
    <owl:Axiom>
        <rdfs:comment>Mapping the laws that dictate retention periods to each record class is crucial for ensuring compliance with legal obligations. Tracking compliance allows organizations to adapt to changes in regulations while defending decisions related to record retention.</rdfs:comment>
        <owl:annotatedTarget rdf:resource="&Governance;Laws_Mapping_And_Compliance_Tracking_1"/>
        <owl:annotatedSource rdf:resource="&Governance;RIM_P1_3"/>
        <owl:annotatedProperty rdf:resource="&Governance;needsTechnicalRequirement"/>
    </owl:Axiom>
    <owl:Axiom>
        <rdfs:comment>Managing electronic records against established retention schedules ensures that all forms of data are retained and disposed of in compliance with regulatory requirements.</rdfs:comment>
        <owl:annotatedTarget rdf:resource="&Governance;ERM_1"/>
        <owl:annotatedSource rdf:resource="&Governance;RIM_P1_3"/>
        <owl:annotatedProperty rdf:resource="&Governance;needsTechnicalRequirement"/>
    </owl:Axiom>
    <owl:Axiom>
        <rdfs:comment>Managing physical records against established retention schedules ensures that all forms of data are retained and disposed of in compliance with regulatory requirements.</rdfs:comment>
        <owl:annotatedSource rdf:resource="&Governance;RIM_P1_3"/>
        <owl:annotatedTarget rdf:resource="&Governance;Records_Information_Management_1"/>
        <owl:annotatedProperty rdf:resource="&Governance;needsTechnicalRequirement"/>
    </owl:Axiom>
    


    <!-- http://www.semanticweb.org/IG/Governance#RIM_P1_4 -->

    <owl:NamedIndividual rdf:about="&Governance;RIM_P1_4">
        <rdf:type rdf:resource="&Governance;IG_Capability"/>
        <Governance:capabilityDescription>Retention schedules reflect regulatory, policy and business value and encompass all forms of information enabling them to be executed on records repositories, application and archived data, backup media and physical records. Legal holds can be applied by record class and suspend automated disposal. There is a shared library of country protocols for eDiscovery, privacy, and retention to form a comprehensive view. Schedules align with and are systematically used to dispose of production and back up data whether structured, unstructured, electronic, physical, record or business information.</Governance:capabilityDescription>
        <Governance:inMaturityLevel rdf:resource="&Governance;4_Proactive"/>
        <Governance:involvesArticle rdf:resource="&Governance;Article_32"/>
        <Governance:involvesArticle rdf:resource="&Governance;Article_5"/>
        <Governance:involvesArticle rdf:resource="&Governance;Article_50"/>
        <Governance:involvesArticle rdf:resource="&Governance;Article_6"/>
        <Governance:linkedToFramework rdf:resource="&Governance;CGOC_02"/>
        <Governance:practicesDefinedInIso rdf:resource="&Governance;ISO_15489"/>
        <Governance:needsTechnicalRequirement rdf:resource="&Governance;Legal_Hold_Management_1"/>
        <Governance:linkedToProcess rdf:resource="&Governance;Process_Information_Retention_And_Disposal_Obligation_1"/>
        <Governance:linkedToBusinessUnit rdf:resource="&Governance;Records_Information_Management_1"/>
        <Governance:needsTechnicalRequirement rdf:resource="&Governance;Records_Retention_Schedule_1"/>
        <Governance:needsTechnicalRequirement rdf:resource="&Governance;Shared_Library_Of_Country_Protocols_1"/>
    </owl:NamedIndividual>
    <owl:Axiom>
        <rdfs:comment>The capability to apply legal holds to specific record classes and suspend automated disposal is essential for ensuring the preservation of relevant data in legal or regulatory investigations or proceedings.</rdfs:comment>
        <owl:annotatedTarget rdf:resource="&Governance;Legal_Hold_Management_1"/>
        <owl:annotatedSource rdf:resource="&Governance;RIM_P1_4"/>
        <owl:annotatedProperty rdf:resource="&Governance;needsTechnicalRequirement"/>
    </owl:Axiom>
    <owl:Axiom>
        <rdfs:comment>Implementing a comprehensive retention schedule is crucial to ensure that all forms of information, whether electronic or physical, are properly managed and disposed of in alignment with regulatory, policy, and business requirements. This prevents unnecessary data accumulation and facilitates compliance.
Also integrating retention schedules with records repositories, applications, archived data, and physical records ensures that automated disposal processes are executed effectively and consistently.</rdfs:comment>
        <owl:annotatedSource rdf:resource="&Governance;RIM_P1_4"/>
        <owl:annotatedTarget rdf:resource="&Governance;Records_Retention_Schedule_1"/>
        <owl:annotatedProperty rdf:resource="&Governance;needsTechnicalRequirement"/>
    </owl:Axiom>
    <owl:Axiom>
        <rdfs:comment>Having a shared library of country-specific protocols for eDiscovery, privacy, and retention enables the organization to have a comprehensive view of obligations across different jurisdictions, ensuring compliance and consistent application of retention practices.</rdfs:comment>
        <owl:annotatedSource rdf:resource="&Governance;RIM_P1_4"/>
        <owl:annotatedTarget rdf:resource="&Governance;Shared_Library_Of_Country_Protocols_1"/>
        <owl:annotatedProperty rdf:resource="&Governance;needsTechnicalRequirement"/>
    </owl:Axiom>
    


    <!-- http://www.semanticweb.org/IG/Governance#RIM_P2_3 -->

    <owl:NamedIndividual rdf:about="&Governance;RIM_P2_3">
        <rdf:type rdf:resource="&Governance;IG_Capability"/>
        <Governance:capabilityDescription>Departmental liaisons work with their line of business to identify information of value, its duration of value and where it is managed; this informs more comprehensive retention schedules for all information (regulated, unregulated, electronic, physical). Business is able to request changes to master schedule and department/ country schedules at the rate of business change.</Governance:capabilityDescription>
        <Governance:inMaturityLevel rdf:resource="&Governance;3_Essential"/>
        <Governance:involvesArticle rdf:resource="&Governance;Article_30"/>
        <Governance:involvesArticle rdf:resource="&Governance;Article_5"/>
        <Governance:linkedToFramework rdf:resource="&Governance;CGOC_02"/>
        <Governance:needsTechnicalRequirement rdf:resource="&Governance;Collaboration_Tools_1"/>
        <Governance:practicesDefinedInIso rdf:resource="&Governance;ISO_14271"/>
        <Governance:practicesDefinedInIso rdf:resource="&Governance;ISO_15489"/>
        <Governance:practicesDefinedInIso rdf:resource="&Governance;ISO_15939"/>
        <Governance:practicesDefinedInIso rdf:resource="&Governance;ISO_17000"/>
        <Governance:practicesDefinedInIso rdf:resource="&Governance;ISO_23081"/>
        <Governance:linkedToProcess rdf:resource="&Governance;Process_Departmental_Information_Practice_1"/>
        <Governance:linkedToBusinessUnit rdf:resource="&Governance;Records_Information_Management_1"/>
        <Governance:needsTechnicalRequirement rdf:resource="&Governance;Records_Retention_Schedule_1"/>
        <Governance:needsTechnicalRequirement rdf:resource="&Governance;Request_Management_System_1"/>
    </owl:NamedIndividual>
    <owl:Axiom>
        <rdfs:comment> Utilizing collaboration tools enables effective communication between departmental liaisons and business units, facilitating the identification of valuable information and its proper management.</rdfs:comment>
        <owl:annotatedTarget rdf:resource="&Governance;Collaboration_Tools_1"/>
        <owl:annotatedSource rdf:resource="&Governance;RIM_P2_3"/>
        <owl:annotatedProperty rdf:resource="&Governance;needsTechnicalRequirement"/>
    </owl:Axiom>
    <owl:Axiom>
        <rdfs:comment>Developing comprehensive retention schedules that cover all types of information (regulated, unregulated, electronic, physical) helps ensure consistent and compliant information management practices.</rdfs:comment>
        <owl:annotatedSource rdf:resource="&Governance;RIM_P2_3"/>
        <owl:annotatedTarget rdf:resource="&Governance;Records_Retention_Schedule_1"/>
        <owl:annotatedProperty rdf:resource="&Governance;needsTechnicalRequirement"/>
    </owl:Axiom>
    <owl:Axiom>
        <rdfs:comment>Implementing a system that allows businesses to request changes to the master retention schedule and department/country-specific schedules facilitates agile adjustments to information management practices.</rdfs:comment>
        <owl:annotatedSource rdf:resource="&Governance;RIM_P2_3"/>
        <owl:annotatedTarget rdf:resource="&Governance;Request_Management_System_1"/>
        <owl:annotatedProperty rdf:resource="&Governance;needsTechnicalRequirement"/>
    </owl:Axiom>
    


    <!-- http://www.semanticweb.org/IG/Governance#RIM_P2_4 -->

    <owl:NamedIndividual rdf:about="&Governance;RIM_P2_4">
        <rdf:type rdf:resource="&Governance;IG_Capability"/>
        <Governance:capabilityDescription>Retention schedules are automatically executed across the information environment. Cost and benefit are weighed in determining retention periods and the enterprise impact is considered. Schedule changes are syndicated to IT and directly to systems for execution of both retention and disposition. When business objectives or laws change, schedules are updated and stakeholders notified. Legal and IT have transparency to what information each line of business has where and for how long to inform eDiscovery and data management.</Governance:capabilityDescription>
        <Governance:inMaturityLevel rdf:resource="&Governance;4_Proactive"/>
        <Governance:involvesArticle rdf:resource="&Governance;Article_17"/>
        <Governance:involvesArticle rdf:resource="&Governance;Article_25"/>
        <Governance:involvesArticle rdf:resource="&Governance;Article_32"/>
        <Governance:involvesArticle rdf:resource="&Governance;Article_35"/>
        <Governance:involvesArticle rdf:resource="&Governance;Article_5"/>
        <Governance:involvesArticle rdf:resource="&Governance;Article_6"/>
        <Governance:needsTechnicalRequirement rdf:resource="&Governance;Automated_Retention_Execution_1"/>
        <Governance:linkedToFramework rdf:resource="&Governance;CGOC_02"/>
        <Governance:needsTechnicalRequirement rdf:resource="&Governance;Cost_Calculations_1"/>
        <Governance:practicesDefinedInIso rdf:resource="&Governance;ISO_15489"/>
        <Governance:practicesDefinedInIso rdf:resource="&Governance;ISO_15939"/>
        <Governance:practicesDefinedInIso rdf:resource="&Governance;ISO_27001"/>
        <Governance:linkedToProcess rdf:resource="&Governance;Process_Departmental_Information_Practice_1"/>
        <Governance:linkedToBusinessUnit rdf:resource="&Governance;Records_Information_Management_1"/>
        <Governance:needsTechnicalRequirement rdf:resource="&Governance;Transparency"/>
    </owl:NamedIndividual>
    <owl:Axiom>
        <rdfs:comment>Weighing the costs and benefits of retention periods helps organizations make informed decisions about retaining or disposing of information, ensuring resource efficiency.</rdfs:comment>
        <owl:annotatedTarget rdf:resource="&Governance;Cost_Calculations_1"/>
        <owl:annotatedSource rdf:resource="&Governance;RIM_P2_4"/>
        <owl:annotatedProperty rdf:resource="&Governance;needsTechnicalRequirement"/>
    </owl:Axiom>
    <owl:Axiom>
        <rdfs:comment>The automated execution of retention schedules ensures consistent and timely management of information, reducing the risk of non-compliance and data clutter.</rdfs:comment>
        <owl:annotatedTarget rdf:resource="&Governance;Automated_Retention_Execution_1"/>
        <owl:annotatedSource rdf:resource="&Governance;RIM_P2_4"/>
        <owl:annotatedProperty rdf:resource="&Governance;needsTechnicalRequirement"/>
    </owl:Axiom>
    <owl:Axiom>
        <rdfs:comment>Providing transparency to legal and IT teams regarding information retention and location supports eDiscovery and data management efforts, ensuring compliance.</rdfs:comment>
        <owl:annotatedSource rdf:resource="&Governance;RIM_P2_4"/>
        <owl:annotatedTarget rdf:resource="&Governance;Transparency"/>
        <owl:annotatedProperty rdf:resource="&Governance;needsTechnicalRequirement"/>
    </owl:Axiom>
    


    <!-- http://www.semanticweb.org/IG/Governance#RIM_P3_3 -->

    <owl:NamedIndividual rdf:about="&Governance;RIM_P3_3">
        <rdf:type rdf:resource="&Governance;IG_Capability"/>
        <Governance:capabilityDescription>Application data and business process data cam be searched by departmental staff in the course of their work from within the system</Governance:capabilityDescription>
        <Governance:inMaturityLevel rdf:resource="&Governance;3_Essential"/>
        <Governance:needsTechnicalRequirement rdf:resource="&Governance;AccessControl_1"/>
        <Governance:involvesArticle rdf:resource="&Governance;Article_25"/>
        <Governance:involvesArticle rdf:resource="&Governance;Article_32"/>
        <Governance:involvesArticle rdf:resource="&Governance;Article_35"/>
        <Governance:involvesArticle rdf:resource="&Governance;Article_5"/>
        <Governance:involvesArticle rdf:resource="&Governance;Article_6"/>
        <Governance:linkedToFramework rdf:resource="&Governance;CGOC_02"/>
        <Governance:needsTechnicalRequirement rdf:resource="&Governance;Data_Quality_Management_1"/>
        <Governance:practicesDefinedInIso rdf:resource="&Governance;ISO_15489"/>
        <Governance:practicesDefinedInIso rdf:resource="&Governance;ISO_15939"/>
        <Governance:practicesDefinedInIso rdf:resource="&Governance;ISO_23081"/>
        <Governance:practicesDefinedInIso rdf:resource="&Governance;ISO_27001"/>
        <Governance:needsTechnicalRequirement rdf:resource="&Governance;Metadata_Framework_1"/>
        <Governance:linkedToProcess rdf:resource="&Governance;Process_Realize_Information_Value_1"/>
        <Governance:linkedToBusinessUnit rdf:resource="&Governance;Records_Information_Management_1"/>
        <Governance:needsTechnicalRequirement rdf:resource="&Governance;Search_And_Retrieval_System_1"/>
    </owl:NamedIndividual>
    <owl:Axiom>
        <rdfs:comment>Ensure the accuracy, completeness, and reliability of data by implementing data quality management practices. Clean, reliable data improves search results and decision-making.</rdfs:comment>
        <owl:annotatedTarget rdf:resource="&Governance;Data_Quality_Management_1"/>
        <owl:annotatedSource rdf:resource="&Governance;RIM_P3_3"/>
        <owl:annotatedProperty rdf:resource="&Governance;needsTechnicalRequirement"/>
    </owl:Axiom>
    <owl:Axiom>
        <rdfs:comment>Implement a robust searchable data indexing mechanism that allows departmental staff to search and retrieve relevant application and business process data within the system. This enhances efficiency and supports informed decision-making.</rdfs:comment>
        <owl:annotatedSource rdf:resource="&Governance;RIM_P3_3"/>
        <owl:annotatedTarget rdf:resource="&Governance;Search_And_Retrieval_System_1"/>
        <owl:annotatedProperty rdf:resource="&Governance;needsTechnicalRequirement"/>
    </owl:Axiom>
    <owl:Axiom>
        <rdfs:comment>Establish a comprehensive metadata framework that provides context and description for application and business process data, enhancing search accuracy and relevance.</rdfs:comment>
        <owl:annotatedTarget rdf:resource="&Governance;Metadata_Framework_1"/>
        <owl:annotatedSource rdf:resource="&Governance;RIM_P3_3"/>
        <owl:annotatedProperty rdf:resource="&Governance;needsTechnicalRequirement"/>
    </owl:Axiom>
    <owl:Axiom>
        <rdfs:comment>Implement strong access control and permissions mechanisms to ensure that departmental staff can access only the data that is relevant to their roles and responsibilities. This safeguards sensitive information and maintains data privacy.</rdfs:comment>
        <owl:annotatedTarget rdf:resource="&Governance;AccessControl_1"/>
        <owl:annotatedSource rdf:resource="&Governance;RIM_P3_3"/>
        <owl:annotatedProperty rdf:resource="&Governance;needsTechnicalRequirement"/>
    </owl:Axiom>
    


    <!-- http://www.semanticweb.org/IG/Governance#RIM_P3_4 -->

    <owl:NamedIndividual rdf:about="&Governance;RIM_P3_4">
        <rdf:type rdf:resource="&Governance;IG_Capability"/>
        <Governance:capabilityDescription>Search and analytics enable employees to realize value and to apply information to decisionmaking in real time even as context erodes across information sources and types; assertions on value and sources of information made in processes H, I and J are used to ensure accessibility and authenticity of information the business defined as valuable. The cost of information to the enterprise is consistent and appropriate over its lifecycle.</Governance:capabilityDescription>
        <Governance:inMaturityLevel rdf:resource="&Governance;4_Proactive"/>
        <Governance:needsTechnicalRequirement rdf:resource="&Governance;AccessControl_1"/>
        <Governance:involvesArticle rdf:resource="&Governance;Article_32"/>
        <Governance:involvesArticle rdf:resource="&Governance;Article_5"/>
        <Governance:involvesArticle rdf:resource="&Governance;Article_6"/>
        <Governance:linkedToFramework rdf:resource="&Governance;CGOC_02"/>
        <Governance:needsTechnicalRequirement rdf:resource="&Governance;Data_Mapping_And_Classification_System_1"/>
        <Governance:needsTechnicalRequirement rdf:resource="&Governance;Data_Quality_Assurance_Framework_1"/>
        <Governance:practicesDefinedInIso rdf:resource="&Governance;ISO_14271"/>
        <Governance:practicesDefinedInIso rdf:resource="&Governance;ISO_15489"/>
        <Governance:practicesDefinedInIso rdf:resource="&Governance;ISO_15939"/>
        <Governance:practicesDefinedInIso rdf:resource="&Governance;ISO_23081"/>
        <Governance:practicesDefinedInIso rdf:resource="&Governance;ISO_27001"/>
        <Governance:needsTechnicalRequirement rdf:resource="&Governance;Metadata_Framework_1"/>
        <Governance:linkedToProcess rdf:resource="&Governance;Process_Realize_Information_Value_1"/>
        <Governance:linkedToBusinessUnit rdf:resource="&Governance;Records_Information_Management_1"/>
        <Governance:needsTechnicalRequirement rdf:resource="&Governance;Search_And_Retrieval_System_1"/>
    </owl:NamedIndividual>
    <owl:Axiom>
        <rdfs:comment>A comprehensive data classification helps organize and categorize information, facilitating effective search and analytics by providing context and relevance.</rdfs:comment>
        <owl:annotatedTarget rdf:resource="&Governance;Data_Mapping_And_Classification_System_1"/>
        <owl:annotatedSource rdf:resource="&Governance;RIM_P3_4"/>
        <owl:annotatedProperty rdf:resource="&Governance;needsTechnicalRequirement"/>
    </owl:Axiom>
    <owl:Axiom>
        <rdfs:comment>A comprehensive metadata framework helps organize and categorize information, facilitating effective search and analytics by providing context and relevance.</rdfs:comment>
        <owl:annotatedTarget rdf:resource="&Governance;Metadata_Framework_1"/>
        <owl:annotatedSource rdf:resource="&Governance;RIM_P3_4"/>
        <owl:annotatedProperty rdf:resource="&Governance;needsTechnicalRequirement"/>
    </owl:Axiom>
    <owl:Axiom>
        <rdfs:comment> Implementing a robust search and analytics platform is essential for enabling employees to efficiently access and utilize information in real time for decision-making, despite potential erosion of context across various information sources and types.</rdfs:comment>
        <owl:annotatedSource rdf:resource="&Governance;RIM_P3_4"/>
        <owl:annotatedTarget rdf:resource="&Governance;Search_And_Retrieval_System_1"/>
        <owl:annotatedProperty rdf:resource="&Governance;needsTechnicalRequirement"/>
    </owl:Axiom>
    <owl:Axiom>
        <rdfs:comment>Maintaining data quality is crucial for accurate search results and reliable analytics. Data validation, cleansing, and enrichment processes contribute to the effectiveness of information utilization.</rdfs:comment>
        <owl:annotatedTarget rdf:resource="&Governance;Data_Quality_Assurance_Framework_1"/>
        <owl:annotatedSource rdf:resource="&Governance;RIM_P3_4"/>
        <owl:annotatedProperty rdf:resource="&Governance;needsTechnicalRequirement"/>
    </owl:Axiom>
    <owl:Axiom>
        <rdfs:comment> Implementing robust authentication and authorization mechanisms ensures that only authorized users can access specific information, maintaining data privacy and security.</rdfs:comment>
        <owl:annotatedTarget rdf:resource="&Governance;AccessControl_1"/>
        <owl:annotatedSource rdf:resource="&Governance;RIM_P3_4"/>
        <owl:annotatedProperty rdf:resource="&Governance;needsTechnicalRequirement"/>
    </owl:Axiom>
    


    <!-- http://www.semanticweb.org/IG/Governance#RIM_P4_3 -->

    <owl:NamedIndividual rdf:about="&Governance;RIM_P4_3">
        <rdf:type rdf:resource="&Governance;IG_Capability"/>
        <Governance:capabilityDescription>Data quality assessment conducted resulting in a management strategy tailored to its needs, and governance policies addressing specific data management requirements. Master datamap for 50% or more silos. A virtual data quality firewall is implemented to detect and quarantine bad data at the point of entry. ”Golden Sources” of key data elements identified, monitored and updated. Business intelligence solutions determine which data sets are most likely to be utilized and targeted for quality management and governance.</Governance:capabilityDescription>
        <Governance:inMaturityLevel rdf:resource="&Governance;3_Essential"/>
        <Governance:involvesArticle rdf:resource="&Governance;Article_32"/>
        <Governance:involvesArticle rdf:resource="&Governance;Article_5"/>
        <Governance:involvesArticle rdf:resource="&Governance;Article_6"/>
        <Governance:linkedToFramework rdf:resource="&Governance;CGOC_02"/>
        <Governance:needsTechnicalRequirement rdf:resource="&Governance;Data_Mapping_And_Classification_System_1"/>
        <Governance:needsTechnicalRequirement rdf:resource="&Governance;Data_Quality_Assurance_Framework_1"/>
        <Governance:practicesDefinedInIso rdf:resource="&Governance;ISO_14271"/>
        <Governance:practicesDefinedInIso rdf:resource="&Governance;ISO_15000"/>
        <Governance:practicesDefinedInIso rdf:resource="&Governance;ISO_15489"/>
        <Governance:practicesDefinedInIso rdf:resource="&Governance;ISO_15939"/>
        <Governance:practicesDefinedInIso rdf:resource="&Governance;ISO_23081"/>
        <Governance:practicesDefinedInIso rdf:resource="&Governance;ISO_27001"/>
        <Governance:needsTechnicalRequirement rdf:resource="&Governance;Monitoring_1"/>
        <Governance:linkedToProcess rdf:resource="&Governance;Process_Data_Quality_And_Data_Lineage_1"/>
        <Governance:linkedToBusinessUnit rdf:resource="&Governance;Records_Information_Management_1"/>
    </owl:NamedIndividual>
    <owl:Axiom>
        <rdfs:comment>Creating a master data map for various data silos ensures a clear understanding of data sources and their relationships. This is crucial for effective data quality assessment and governance.</rdfs:comment>
        <owl:annotatedTarget rdf:resource="&Governance;Data_Mapping_And_Classification_System_1"/>
        <owl:annotatedSource rdf:resource="&Governance;RIM_P4_3"/>
        <owl:annotatedProperty rdf:resource="&Governance;needsTechnicalRequirement"/>
    </owl:Axiom>
    <owl:Axiom>
        <rdfs:comment>Identifying and monitoring &quot;Golden Sources&quot; of key data elements ensures that reliable and authoritative data is used as a reference throughout the organization.</rdfs:comment>
        <owl:annotatedTarget rdf:resource="&Governance;Monitoring_1"/>
        <owl:annotatedSource rdf:resource="&Governance;RIM_P4_3"/>
        <owl:annotatedProperty rdf:resource="&Governance;needsTechnicalRequirement"/>
    </owl:Axiom>
    <owl:Axiom>
        <rdfs:comment>Conducting data quality assessments and establishing governance policies are crucial for maintaining accurate and reliable data across the organization. A well-defined strategy ensures that data is fit for its intended purpose and complies with data protection regulations.
Also implementing a virtual data quality firewall at the point of entry helps prevent the entry of bad or incorrect data into the system, ensuring the initial quality of data.</rdfs:comment>
        <owl:annotatedTarget rdf:resource="&Governance;Data_Quality_Assurance_Framework_1"/>
        <owl:annotatedSource rdf:resource="&Governance;RIM_P4_3"/>
        <owl:annotatedProperty rdf:resource="&Governance;needsTechnicalRequirement"/>
    </owl:Axiom>
    


    <!-- http://www.semanticweb.org/IG/Governance#RIM_P4_4 -->

    <owl:NamedIndividual rdf:about="&Governance;RIM_P4_4">
        <rdf:type rdf:resource="&Governance;IG_Capability"/>
        <Governance:capabilityDescription>Data quality management processes are fully automated with complete audit trails. Master datamap is fully integrated and ubiquitous. Astute data management processes can collect and move data to a repository for cleansing. Advanced analytics used to predict the use and misuse of data.</Governance:capabilityDescription>
        <Governance:inMaturityLevel rdf:resource="&Governance;4_Proactive"/>
        <Governance:needsTechnicalRequirement rdf:resource="&Governance;Analytics_1"/>
        <Governance:involvesArticle rdf:resource="&Governance;Article_5"/>
        <Governance:needsTechnicalRequirement rdf:resource="&Governance;Audit_1"/>
        <Governance:needsTechnicalRequirement rdf:resource="&Governance;Automated_Data_Collection"/>
        <Governance:needsTechnicalRequirement rdf:resource="&Governance;Automated_Integration"/>
        <Governance:linkedToFramework rdf:resource="&Governance;CGOC_02"/>
        <Governance:practicesDefinedInIso rdf:resource="&Governance;ISO_15489"/>
        <Governance:practicesDefinedInIso rdf:resource="&Governance;ISO_15939"/>
        <Governance:practicesDefinedInIso rdf:resource="&Governance;ISO_23081"/>
        <Governance:practicesDefinedInIso rdf:resource="&Governance;ISO_27000"/>
        <Governance:linkedToProcess rdf:resource="&Governance;Process_Data_Quality_And_Data_Lineage_1"/>
        <Governance:linkedToBusinessUnit rdf:resource="&Governance;Records_Information_Management_1"/>
    </owl:NamedIndividual>
    <owl:Axiom>
        <rdfs:comment>Automated data collection and movement to a repository for cleansing streamline the data quality improvement process. It ensures that data is cleansed, validated, and enriched in a timely manner.</rdfs:comment>
        <owl:annotatedTarget rdf:resource="&Governance;Automated_Data_Collection"/>
        <owl:annotatedSource rdf:resource="&Governance;RIM_P4_4"/>
        <owl:annotatedProperty rdf:resource="&Governance;needsTechnicalRequirement"/>
    </owl:Axiom>
    <owl:Axiom>
        <rdfs:comment>Automated data quality management processes with audit trails are essential to ensure that data is accurate, reliable, and fit for its intended purposes. Audit trails provide a transparent record of data quality activities, facilitating accountability and traceability.</rdfs:comment>
        <owl:annotatedTarget rdf:resource="&Governance;Audit_1"/>
        <owl:annotatedSource rdf:resource="&Governance;RIM_P4_4"/>
        <owl:annotatedProperty rdf:resource="&Governance;needsTechnicalRequirement"/>
    </owl:Axiom>
    <owl:Axiom>
        <rdfs:comment>Advanced analytics enable organizations to predict patterns of data usage and misuse, enhancing data quality management. This proactive approach helps address data quality issues before they impact business processes.</rdfs:comment>
        <owl:annotatedTarget rdf:resource="&Governance;Analytics_1"/>
        <owl:annotatedSource rdf:resource="&Governance;RIM_P4_4"/>
        <owl:annotatedProperty rdf:resource="&Governance;needsTechnicalRequirement"/>
    </owl:Axiom>
    <owl:Axiom>
        <rdfs:comment>Integrating a master datamap across the organization ensures consistency in data understanding and management. It allows for centralized control and governance of data assets.</rdfs:comment>
        <owl:annotatedTarget rdf:resource="&Governance;Automated_Integration"/>
        <owl:annotatedSource rdf:resource="&Governance;RIM_P4_4"/>
        <owl:annotatedProperty rdf:resource="&Governance;needsTechnicalRequirement"/>
    </owl:Axiom>
    


    <!-- http://www.semanticweb.org/IG/Governance#Records_Information_Management_1 -->

    <owl:NamedIndividual rdf:about="&Governance;Records_Information_Management_1">
        <rdf:type rdf:resource="&Governance;Records_And_Information_Management"/>
        <Governance:involvesArticle rdf:resource="&Governance;Article_30"/>
        <Governance:involvesArticle rdf:resource="&Governance;Article_5"/>
        <Governance:canBeInvolvedWith rdf:resource="&Governance;Disposition_Policies_And_Procedures_1"/>
        <Governance:canBeInvolvedWith rdf:resource="&Governance;Document_Management_System_1"/>
        <Governance:practicesDefinedInIso rdf:resource="&Governance;ISO_15489"/>
        <Governance:practicesDefinedInIso rdf:resource="&Governance;ISO_17000"/>
        <Governance:practicesDefinedInIso rdf:resource="&Governance;ISO_23081"/>
        <Governance:responsibleFor rdf:resource="&Governance;Records_Retention_Schedule_1"/>
        <Governance:responsibleFor rdf:resource="&Governance;Review_Cyles_1"/>
    </owl:NamedIndividual>
    <owl:Axiom>
        <rdfs:comment>The Records And Information Management subcategory within the Records Management department is responsible for designing and implementing &quot;Review Cycles.&quot; These cycles determine the frequency and process for reviewing and assessing the relevance, accuracy, and value of records and information within the organization. They ensure that records are periodically reviewed, updated, retained, or disposed of according to established policies.</rdfs:comment>
        <owl:annotatedSource rdf:resource="&Governance;Records_Information_Management_1"/>
        <owl:annotatedTarget rdf:resource="&Governance;Review_Cyles_1"/>
        <owl:annotatedProperty rdf:resource="&Governance;responsibleFor"/>
    </owl:Axiom>
    <owl:Axiom>
        <rdfs:comment>The Records And Information Management subcategory within the Records Management department focuses on proper records management practices. Implementing effective disposition policies and procedures ensures that records are managed throughout their lifecycle and disposed of appropriately, minimizing the risk of non-compliance and facilitating efficient records management.</rdfs:comment>
        <owl:annotatedTarget rdf:resource="&Governance;Disposition_Policies_And_Procedures_1"/>
        <owl:annotatedSource rdf:resource="&Governance;Records_Information_Management_1"/>
        <owl:annotatedProperty rdf:resource="&Governance;canBeInvolvedWith"/>
    </owl:Axiom>
    <owl:Axiom>
        <rdfs:comment>The Records And Information Management subcategory within the Records Management department is responsible for designing and implementing the &quot;Records Retention Schedule.&quot; This schedule outlines the specific timeframes and guidelines for retaining and disposing of records based on legal, regulatory, and business requirements. It ensures that records are managed and retained appropriately throughout their lifecycle.</rdfs:comment>
        <owl:annotatedSource rdf:resource="&Governance;Records_Information_Management_1"/>
        <owl:annotatedTarget rdf:resource="&Governance;Records_Retention_Schedule_1"/>
        <owl:annotatedProperty rdf:resource="&Governance;responsibleFor"/>
    </owl:Axiom>
    <owl:Axiom>
        <rdfs:comment>The Records And Information Management subcategory could use the system to manage official records, archives, and historical documents. The system supports records retention, archiving, and disposal processes.</rdfs:comment>
        <owl:annotatedTarget rdf:resource="&Governance;Document_Management_System_1"/>
        <owl:annotatedSource rdf:resource="&Governance;Records_Information_Management_1"/>
        <owl:annotatedProperty rdf:resource="&Governance;canBeInvolvedWith"/>
    </owl:Axiom>
    


    <!-- http://www.semanticweb.org/IG/Governance#Records_Retention_Schedule_1 -->

    <owl:NamedIndividual rdf:about="&Governance;Records_Retention_Schedule_1">
        <rdf:type rdf:resource="&Governance;Records_Retention_Schedule"/>
        <Governance:involvesArticle rdf:resource="&Governance;Article_25"/>
        <Governance:involvesArticle rdf:resource="&Governance;Article_30"/>
        <Governance:involvesArticle rdf:resource="&Governance;Article_5"/>
        <Governance:practicesDefinedInIso rdf:resource="&Governance;ISO_15489"/>
        <Governance:practicesDefinedInIso rdf:resource="&Governance;ISO_15939"/>
        <Governance:practicesDefinedInIso rdf:resource="&Governance;ISO_23081"/>
    </owl:NamedIndividual>
    


    <!-- http://www.semanticweb.org/IG/Governance#Remote_Wiping_1 -->

    <owl:NamedIndividual rdf:about="&Governance;Remote_Wiping_1">
        <rdf:type rdf:resource="&Governance;Remote_Wiping"/>
        <Governance:involvesArticle rdf:resource="&Governance;Article_32"/>
        <Governance:practicesDefinedInIso rdf:resource="&Governance;ISO_27001"/>
    </owl:NamedIndividual>
    


    <!-- http://www.semanticweb.org/IG/Governance#Reporting_And_Analysis_System_1 -->

    <owl:NamedIndividual rdf:about="&Governance;Reporting_And_Analysis_System_1">
        <rdf:type rdf:resource="&Governance;Reporting_And_Analysis_System"/>
        <Governance:involvesArticle rdf:resource="&Governance;Article_24"/>
        <Governance:involvesArticle rdf:resource="&Governance;Article_33"/>
        <Governance:involvesArticle rdf:resource="&Governance;Article_5"/>
        <Governance:practicesDefinedInIso rdf:resource="&Governance;ISO_15000"/>
        <Governance:practicesDefinedInIso rdf:resource="&Governance;ISO_15489"/>
        <Governance:practicesDefinedInIso rdf:resource="&Governance;ISO_15939"/>
    </owl:NamedIndividual>
    


    <!-- http://www.semanticweb.org/IG/Governance#Request_Management_System_1 -->

    <owl:NamedIndividual rdf:about="&Governance;Request_Management_System_1">
        <rdf:type rdf:resource="&Governance;Request_Management_System"/>
        <Governance:involvesArticle rdf:resource="&Governance;Article_30"/>
        <Governance:involvesArticle rdf:resource="&Governance;Article_5"/>
        <Governance:practicesDefinedInIso rdf:resource="&Governance;ISO_17000"/>
    </owl:NamedIndividual>
    


    <!-- http://www.semanticweb.org/IG/Governance#Retention_Rule_Management_System_1 -->

    <owl:NamedIndividual rdf:about="&Governance;Retention_Rule_Management_System_1">
        <rdf:type rdf:resource="&Governance;Retention_Rule_Management_System"/>
        <Governance:involvesArticle rdf:resource="&Governance;Article_5"/>
        <Governance:practicesDefinedInIso rdf:resource="&Governance;ISO_15489"/>
    </owl:NamedIndividual>
    


    <!-- http://www.semanticweb.org/IG/Governance#Review_Cyles_1 -->

    <owl:NamedIndividual rdf:about="&Governance;Review_Cyles_1">
        <rdf:type rdf:resource="&Governance;Review_Cycles"/>
        <Governance:involvesArticle rdf:resource="&Governance;Article_24"/>
        <Governance:involvesArticle rdf:resource="&Governance;Article_25"/>
        <Governance:involvesArticle rdf:resource="&Governance;Article_28"/>
        <Governance:involvesArticle rdf:resource="&Governance;Article_5"/>
        <Governance:practicesDefinedInIso rdf:resource="&Governance;ISO_14271"/>
        <Governance:practicesDefinedInIso rdf:resource="&Governance;ISO_15489"/>
        <Governance:practicesDefinedInIso rdf:resource="&Governance;ISO_15939"/>
        <Governance:practicesDefinedInIso rdf:resource="&Governance;ISO_17000"/>
        <Governance:practicesDefinedInIso rdf:resource="&Governance;ISO_27000"/>
        <Governance:practicesDefinedInIso rdf:resource="&Governance;ISO_27001"/>
    </owl:NamedIndividual>
    


    <!-- http://www.semanticweb.org/IG/Governance#Revisitation_And_Refinement_1 -->

    <owl:NamedIndividual rdf:about="&Governance;Revisitation_And_Refinement_1">
        <rdf:type rdf:resource="&Governance;Revisitation_And_Refinement"/>
        <Governance:involvesArticle rdf:resource="&Governance;Article_25"/>
        <Governance:involvesArticle rdf:resource="&Governance;Article_32"/>
        <Governance:involvesArticle rdf:resource="&Governance;Article_5"/>
        <Governance:involvesArticle rdf:resource="&Governance;Article_6"/>
        <Governance:involvesArticle rdf:resource="&Governance;Article_9"/>
        <Governance:needsTechnicalRequirement rdf:resource="&Governance;Collaboration_Tools_1"/>
        <Governance:needsTechnicalRequirement rdf:resource="&Governance;Data_Storage_1"/>
        <Governance:needsTechnicalRequirement rdf:resource="&Governance;Database_Management_System_1"/>
        <Governance:needsTechnicalRequirement rdf:resource="&Governance;Digital_Signatures_And_Timestamps_1"/>
        <Governance:needsTechnicalRequirement rdf:resource="&Governance;Incident_Response_And_Remediation_Protocol_1"/>
        <Governance:needsTechnicalRequirement rdf:resource="&Governance;Revisitation_And_Refinement_1"/>
        <Governance:needsTechnicalRequirement rdf:resource="&Governance;Workflow_Tools_1"/>
    </owl:NamedIndividual>
    <owl:Axiom>
        <rdfs:comment>Sharing interview results ensures that all parties are informed, supporting effective collaboration and informed decision-making.

This aligns with &quot;Collaboration Tools&quot; and &quot;Document Management System.&quot; Sharing interview results requires effective collaboration tools and proper document management.</rdfs:comment>
        <owl:annotatedTarget rdf:resource="&Governance;Database_Management_System_1"/>
        <owl:annotatedSource rdf:resource="&Governance;Revisitation_And_Refinement_1"/>
        <owl:annotatedProperty rdf:resource="&Governance;needsTechnicalRequirement"/>
    </owl:Axiom>
    <owl:Axiom>
        <rdfs:comment>Automated alerts during employee transitions ensure that relevant personnel are aware of changes, facilitating data management and legal compliance.

This aligns with &quot;Incident Response and Remediation Protocol&quot; and &quot;Workflow Tools.&quot; Automation facilitates timely alerts and responses to employee transitions, resembling incident response mechanisms and workflow tools.</rdfs:comment>
        <owl:annotatedSource rdf:resource="&Governance;Revisitation_And_Refinement_1"/>
        <owl:annotatedTarget rdf:resource="&Governance;Workflow_Tools_1"/>
        <owl:annotatedProperty rdf:resource="&Governance;needsTechnicalRequirement"/>
    </owl:Axiom>
    <owl:Axiom>
        <rdfs:comment>Timely updates enable accurate identification of custodians, crucial for effective data management and legal holds.

This aligns with &quot;Data Storage&quot; and &quot;Data Signatures and Timestamps.&quot; Real-time updates involve storing data and adding timestamps for accurate tracking.</rdfs:comment>
        <owl:annotatedTarget rdf:resource="&Governance;Digital_Signatures_And_Timestamps_1"/>
        <owl:annotatedSource rdf:resource="&Governance;Revisitation_And_Refinement_1"/>
        <owl:annotatedProperty rdf:resource="&Governance;needsTechnicalRequirement"/>
    </owl:Axiom>
    <owl:Axiom>
        <rdfs:comment>Automated alerts during employee transitions ensure that relevant personnel are aware of changes, facilitating data management and legal compliance.

This aligns with &quot;Incident Response and Remediation Protocol&quot; and &quot;Workflow Tools.&quot; Automation facilitates timely alerts and responses to employee transitions, resembling incident response mechanisms and workflow tools.</rdfs:comment>
        <owl:annotatedTarget rdf:resource="&Governance;Incident_Response_And_Remediation_Protocol_1"/>
        <owl:annotatedSource rdf:resource="&Governance;Revisitation_And_Refinement_1"/>
        <owl:annotatedProperty rdf:resource="&Governance;needsTechnicalRequirement"/>
    </owl:Axiom>
    <owl:Axiom>
        <rdfs:comment>Sharing interview results ensures that all parties are informed, supporting effective collaboration and informed decision-making.

This aligns with &quot;Collaboration Tools&quot; and &quot;Document Management System.&quot; Sharing interview results requires effective collaboration tools and proper document management.</rdfs:comment>
        <owl:annotatedTarget rdf:resource="&Governance;Collaboration_Tools_1"/>
        <owl:annotatedSource rdf:resource="&Governance;Revisitation_And_Refinement_1"/>
        <owl:annotatedProperty rdf:resource="&Governance;needsTechnicalRequirement"/>
    </owl:Axiom>
    <owl:Axiom>
        <rdfs:comment>Timely updates enable accurate identification of custodians, crucial for effective data management and legal holds.

This aligns with &quot;Data Storage&quot; and &quot;Data Signatures and Timestamps.&quot; Real-time updates involve storing data and adding timestamps for accurate tracking.</rdfs:comment>
        <owl:annotatedTarget rdf:resource="&Governance;Data_Storage_1"/>
        <owl:annotatedSource rdf:resource="&Governance;Revisitation_And_Refinement_1"/>
        <owl:annotatedProperty rdf:resource="&Governance;needsTechnicalRequirement"/>
    </owl:Axiom>
    <owl:Axiom>
        <rdfs:comment>Regularly revisiting and refining the scope ensures that only relevant custodians are included, minimizing data overreach and enhancing efficiency.</rdfs:comment>
        <owl:annotatedSource rdf:resource="&Governance;Revisitation_And_Refinement_1"/>
        <owl:annotatedTarget rdf:resource="&Governance;Revisitation_And_Refinement_1"/>
        <owl:annotatedProperty rdf:resource="&Governance;needsTechnicalRequirement"/>
    </owl:Axiom>
    


    <!-- http://www.semanticweb.org/IG/Governance#Risk_And_Compliance_1 -->

    <owl:NamedIndividual rdf:about="&Governance;Risk_And_Compliance_1">
        <rdf:type rdf:resource="&Governance;Risk_And_Compliance"/>
        <Governance:involvesArticle rdf:resource="&Governance;Article_24"/>
        <Governance:practicesDefinedInIso rdf:resource="&Governance;ISO_17000"/>
    </owl:NamedIndividual>
    


    <!-- http://www.semanticweb.org/IG/Governance#SLA_1 -->

    <owl:NamedIndividual rdf:about="&Governance;SLA_1">
        <rdf:type rdf:resource="&Governance;SLA"/>
        <Governance:involvesArticle rdf:resource="&Governance;Article_32"/>
        <Governance:practicesDefinedInIso rdf:resource="&Governance;ISO_27001"/>
    </owl:NamedIndividual>
    


    <!-- http://www.semanticweb.org/IG/Governance#Search_And_Retrieval_System_1 -->

    <owl:NamedIndividual rdf:about="&Governance;Search_And_Retrieval_System_1">
        <rdf:type rdf:resource="&Governance;Search_And_Retrieval_System"/>
        <Governance:involvesArticle rdf:resource="&Governance;Article_15"/>
        <Governance:involvesArticle rdf:resource="&Governance;Article_20"/>
        <Governance:involvesArticle rdf:resource="&Governance;Article_25"/>
        <Governance:involvesArticle rdf:resource="&Governance;Article_5"/>
        <Governance:involvesArticle rdf:resource="&Governance;Article_6"/>
        <Governance:practicesDefinedInIso rdf:resource="&Governance;ISO_15489"/>
        <Governance:practicesDefinedInIso rdf:resource="&Governance;ISO_23081"/>
    </owl:NamedIndividual>
    


    <!-- http://www.semanticweb.org/IG/Governance#Security_Assessment_Framework_1 -->

    <owl:NamedIndividual rdf:about="&Governance;Security_Assessment_Framework_1">
        <rdf:type rdf:resource="&Governance;Security_Assessment_Framework"/>
        <Governance:involvesArticle rdf:resource="&Governance;Article_32"/>
        <Governance:practicesDefinedInIso rdf:resource="&Governance;ISO_27001"/>
    </owl:NamedIndividual>
    


    <!-- http://www.semanticweb.org/IG/Governance#Senior_Records_Officer_1 -->

    <owl:NamedIndividual rdf:about="&Governance;Senior_Records_Officer_1">
        <rdf:type rdf:resource="&Governance;Senior_Records_Officer"/>
        <Governance:involvesArticle rdf:resource="&Governance;Article_39"/>
        <Governance:involvesArticle rdf:resource="&Governance;Article_5"/>
        <Governance:practicesDefinedInIso rdf:resource="&Governance;ISO_15489"/>
    </owl:NamedIndividual>
    


    <!-- http://www.semanticweb.org/IG/Governance#Shared_Library_Of_Country_Protocols_1 -->

    <owl:NamedIndividual rdf:about="&Governance;Shared_Library_Of_Country_Protocols_1">
        <rdf:type rdf:resource="&Governance;Shared_Library_Of_Country_Protocols"/>
        <Governance:involvesArticle rdf:resource="&Governance;Article_50"/>
        <Governance:involvesArticle rdf:resource="&Governance;Article_6"/>
        <Governance:practicesDefinedInIso rdf:resource="&Governance;ISO_15489"/>
    </owl:NamedIndividual>
    


    <!-- http://www.semanticweb.org/IG/Governance#Stakeholder_1 -->

    <owl:NamedIndividual rdf:about="&Governance;Stakeholder_1">
        <rdf:type rdf:resource="&Governance;Stakeholder"/>
        <Governance:involvesArticle rdf:resource="&Governance;Article_24"/>
        <Governance:involvesArticle rdf:resource="&Governance;Article_5"/>
        <Governance:practicesDefinedInIso rdf:resource="&Governance;ISO_15489"/>
        <Governance:practicesDefinedInIso rdf:resource="&Governance;ISO_23081"/>
    </owl:NamedIndividual>
    


    <!-- http://www.semanticweb.org/IG/Governance#Steering_Commitee_1 -->

    <owl:NamedIndividual rdf:about="&Governance;Steering_Commitee_1">
        <rdf:type rdf:resource="&Governance;Steering_Commitee"/>
        <Governance:involvesArticle rdf:resource="&Governance;Article_35"/>
        <Governance:practicesDefinedInIso rdf:resource="&Governance;ISO_15489"/>
        <Governance:practicesDefinedInIso rdf:resource="&Governance;ISO_23081"/>
    </owl:NamedIndividual>
    


    <!-- http://www.semanticweb.org/IG/Governance#Supervisor_Authority_1 -->

    <owl:NamedIndividual rdf:about="&Governance;Supervisor_Authority_1">
        <rdf:type rdf:resource="&Governance;Supervisor_Authority"/>
    </owl:NamedIndividual>
    


    <!-- http://www.semanticweb.org/IG/Governance#Syndication_System_For_Hold_Release_1 -->

    <owl:NamedIndividual rdf:about="&Governance;Syndication_System_For_Hold_Release_1">
        <rdf:type rdf:resource="&Governance;Syndication_System_For_Hold_Release"/>
        <Governance:involvesArticle rdf:resource="&Governance;Article_5"/>
        <Governance:practicesDefinedInIso rdf:resource="&Governance;ISO_15000"/>
    </owl:NamedIndividual>
    


    <!-- http://www.semanticweb.org/IG/Governance#System_Log_1 -->

    <owl:NamedIndividual rdf:about="&Governance;System_Log_1">
        <rdf:type rdf:resource="&Governance;System_Log"/>
        <Governance:involvesArticle rdf:resource="&Governance;Article_32"/>
        <Governance:involvesArticle rdf:resource="&Governance;Article_5"/>
        <Governance:practicesDefinedInIso rdf:resource="&Governance;ISO_15489"/>
        <Governance:practicesDefinedInIso rdf:resource="&Governance;ISO_27001"/>
    </owl:NamedIndividual>
    


    <!-- http://www.semanticweb.org/IG/Governance#TRA_1_1_3 -->

    <owl:NamedIndividual rdf:about="&Governance;TRA_1_1_3">
        <rdf:type rdf:resource="&Governance;IG_Capability"/>
        <Governance:capabilityDescription>Transparency in recordkeeping is taken seriously and information is readily and systematically available when needed.</Governance:capabilityDescription>
        <Governance:inMaturityLevel rdf:resource="&Governance;3_Essential"/>
        <Governance:linkedToFramework rdf:resource="&Governance;ARMA_00"/>
        <Governance:needsTechnicalRequirement rdf:resource="&Governance;AccessControl_1"/>
        <Governance:involvesArticle rdf:resource="&Governance;Article_15"/>
        <Governance:involvesArticle rdf:resource="&Governance;Article_20"/>
        <Governance:involvesArticle rdf:resource="&Governance;Article_30"/>
        <Governance:involvesArticle rdf:resource="&Governance;Article_32"/>
        <Governance:involvesArticle rdf:resource="&Governance;Article_5"/>
        <Governance:needsTechnicalRequirement rdf:resource="&Governance;Audit_1"/>
        <Governance:needsTechnicalRequirement rdf:resource="&Governance;Data_Storage_1"/>
        <Governance:practicesDefinedInIso rdf:resource="&Governance;ISO_15489"/>
        <Governance:practicesDefinedInIso rdf:resource="&Governance;ISO_15939"/>
        <Governance:practicesDefinedInIso rdf:resource="&Governance;ISO_23081"/>
        <Governance:practicesDefinedInIso rdf:resource="&Governance;ISO_27000"/>
        <Governance:needsTechnicalRequirement rdf:resource="&Governance;Records_Information_Management_1"/>
        <Governance:needsTechnicalRequirement rdf:resource="&Governance;Search_And_Retrieval_System_1"/>
        <Governance:hasGoal rdf:resource="&Governance;Transparency"/>
    </owl:NamedIndividual>
    <owl:Axiom>
        <rdfs:comment>Secure and scalable data storage ensures that records are stored in a manner that prevents unauthorized access, tampering, or loss. It also enables efficient retrieval of records when needed, enhancing transparency.</rdfs:comment>
        <owl:annotatedTarget rdf:resource="&Governance;Data_Storage_1"/>
        <owl:annotatedSource rdf:resource="&Governance;TRA_1_1_3"/>
        <owl:annotatedProperty rdf:resource="&Governance;needsTechnicalRequirement"/>
    </owl:Axiom>
    <owl:Axiom>
        <rdfs:comment>Robust metadata management is crucial for transparency in recordkeeping as it ensures that relevant information about records, including creation, modification, access, and retention, is accurately captured and organized. Proper metadata management enhances searchability and retrievability of records, facilitating transparency.  Metadata management is a core element of effective records management, ensuring accurate classification, retrieval, and preservation of records.</rdfs:comment>
        <owl:annotatedTarget rdf:resource="&Governance;Records_Information_Management_1"/>
        <owl:annotatedSource rdf:resource="&Governance;TRA_1_1_3"/>
        <owl:annotatedProperty rdf:resource="&Governance;needsTechnicalRequirement"/>
    </owl:Axiom>
    <owl:Axiom>
        <rdfs:comment>Effective search and retrieval mechanisms enable quick and accurate access to records, supporting transparency by providing the ability to locate relevant information promptly.</rdfs:comment>
        <owl:annotatedTarget rdf:resource="&Governance;Search_And_Retrieval_System_1"/>
        <owl:annotatedSource rdf:resource="&Governance;TRA_1_1_3"/>
        <owl:annotatedProperty rdf:resource="&Governance;needsTechnicalRequirement"/>
    </owl:Axiom>
    <owl:Axiom>
        <rdfs:comment>Audit trails provide an essential tool for monitoring and ensuring compliance with regulations.</rdfs:comment>
        <owl:annotatedTarget rdf:resource="&Governance;Audit_1"/>
        <owl:annotatedSource rdf:resource="&Governance;TRA_1_1_3"/>
        <owl:annotatedProperty rdf:resource="&Governance;needsTechnicalRequirement"/>
    </owl:Axiom>
    <owl:Axiom>
        <rdfs:comment>Logging and auditing contribute to identifying and addressing security breaches and incidents.</rdfs:comment>
        <owl:annotatedTarget rdf:resource="&Governance;AccessControl_1"/>
        <owl:annotatedSource rdf:resource="&Governance;TRA_1_1_3"/>
        <owl:annotatedProperty rdf:resource="&Governance;needsTechnicalRequirement"/>
    </owl:Axiom>
    


    <!-- http://www.semanticweb.org/IG/Governance#TRA_1_1_4 -->

    <owl:NamedIndividual rdf:about="&Governance;TRA_1_1_4">
        <rdf:type rdf:resource="&Governance;IG_Capability"/>
        <Governance:capabilityDescription>Transparency is an essential part of the corporate culture and is emphasized in training.</Governance:capabilityDescription>
        <Governance:inMaturityLevel rdf:resource="&Governance;4_Proactive"/>
        <Governance:linkedToFramework rdf:resource="&Governance;ARMA_00"/>
        <Governance:involvesArticle rdf:resource="&Governance;Article_25"/>
        <Governance:involvesArticle rdf:resource="&Governance;Article_39"/>
        <Governance:needsTechnicalRequirement rdf:resource="&Governance;Employee_Engagement_Platforms_1"/>
        <Governance:practicesDefinedInIso rdf:resource="&Governance;ISO_15939"/>
        <Governance:practicesDefinedInIso rdf:resource="&Governance;ISO_23081"/>
        <Governance:practicesDefinedInIso rdf:resource="&Governance;ISO_27001"/>
        <Governance:needsTechnicalRequirement rdf:resource="&Governance;Training_1"/>
        <Governance:hasGoal rdf:resource="&Governance;Transparency"/>
    </owl:NamedIndividual>
    <owl:Axiom>
        <rdfs:comment>An integrated communication platform ensures that transparency principles are effectively communicated to employees across the organization, embedding transparency into the corporate culture.</rdfs:comment>
        <owl:annotatedTarget rdf:resource="&Governance;Employee_Engagement_Platforms_1"/>
        <owl:annotatedSource rdf:resource="&Governance;TRA_1_1_4"/>
        <owl:annotatedProperty rdf:resource="&Governance;needsTechnicalRequirement"/>
    </owl:Axiom>
    <owl:Axiom>
        <rdfs:comment>Tailored training modules ensure that transparency concepts are customized to various roles and departments, making the training more relevant and impactful. 
Continuous learning and assessment ensure that transparency concepts are reinforced over time and that employees are regularly updated on evolving practices.</rdfs:comment>
        <owl:annotatedSource rdf:resource="&Governance;TRA_1_1_4"/>
        <owl:annotatedTarget rdf:resource="&Governance;Training_1"/>
        <owl:annotatedProperty rdf:resource="&Governance;needsTechnicalRequirement"/>
    </owl:Axiom>
    


    <!-- http://www.semanticweb.org/IG/Governance#TRA_1_1_5 -->

    <owl:NamedIndividual rdf:about="&Governance;TRA_1_1_5">
        <rdf:type rdf:resource="&Governance;IG_Capability"/>
        <Governance:capabilityDescription>The organization’s senior management considers transparency as a key component of information governance.</Governance:capabilityDescription>
        <Governance:inMaturityLevel rdf:resource="&Governance;5_Transformational"/>
        <Governance:linkedToFramework rdf:resource="&Governance;ARMA_00"/>
        <Governance:involvesArticle rdf:resource="&Governance;Article_24"/>
        <Governance:involvesArticle rdf:resource="&Governance;Article_5"/>
        <Governance:needsTechnicalRequirement rdf:resource="&Governance;IG_Policy_1"/>
        <Governance:practicesDefinedInIso rdf:resource="&Governance;ISO_15489"/>
        <Governance:practicesDefinedInIso rdf:resource="&Governance;ISO_15939"/>
        <Governance:practicesDefinedInIso rdf:resource="&Governance;ISO_27001"/>
        <Governance:needsTechnicalRequirement rdf:resource="&Governance;Reporting_And_Analysis_System_1"/>
        <Governance:needsTechnicalRequirement rdf:resource="&Governance;Review_Cyles_1"/>
        <Governance:hasGoal rdf:resource="&Governance;Transparency"/>
    </owl:NamedIndividual>
    <owl:Axiom>
        <rdfs:comment>Transparent information governance policies clearly outline the organization&apos;s commitment to transparency and the specific measures in place to achieve it. These policies guide senior management&apos;s understanding of their role in fostering transparency.</rdfs:comment>
        <owl:annotatedTarget rdf:resource="&Governance;IG_Policy_1"/>
        <owl:annotatedSource rdf:resource="&Governance;TRA_1_1_5"/>
        <owl:annotatedProperty rdf:resource="&Governance;needsTechnicalRequirement"/>
    </owl:Axiom>
    <owl:Axiom>
        <rdfs:comment>A compliance review framework ensures that transparency initiatives are regularly assessed against regulatory requirements and organizational objectives. This enables senior management to assess the effectiveness of transparency efforts.</rdfs:comment>
        <owl:annotatedTarget rdf:resource="&Governance;Review_Cyles_1"/>
        <owl:annotatedSource rdf:resource="&Governance;TRA_1_1_5"/>
        <owl:annotatedProperty rdf:resource="&Governance;needsTechnicalRequirement"/>
    </owl:Axiom>
    <owl:Axiom>
        <rdfs:comment>An executive dashboard and reporting system provides senior management with real-time insights into transparency initiatives and compliance efforts. It allows them to make informed decisions, allocate resources, and demonstrate commitment to transparency.</rdfs:comment>
        <owl:annotatedTarget rdf:resource="&Governance;Reporting_And_Analysis_System_1"/>
        <owl:annotatedSource rdf:resource="&Governance;TRA_1_1_5"/>
        <owl:annotatedProperty rdf:resource="&Governance;needsTechnicalRequirement"/>
    </owl:Axiom>
    


    <!-- http://www.semanticweb.org/IG/Governance#TRA_1_2_3 -->

    <owl:NamedIndividual rdf:about="&Governance;TRA_1_2_3">
        <rdf:type rdf:resource="&Governance;IG_Capability"/>
        <Governance:capabilityDescription>There is a written policy regarding transparency.</Governance:capabilityDescription>
        <Governance:inMaturityLevel rdf:resource="&Governance;3_Essential"/>
        <Governance:linkedToFramework rdf:resource="&Governance;ARMA_00"/>
        <Governance:involvesArticle rdf:resource="&Governance;Article_12"/>
        <Governance:involvesArticle rdf:resource="&Governance;Article_5"/>
        <Governance:needsTechnicalRequirement rdf:resource="&Governance;IG_Policy_1"/>
        <Governance:practicesDefinedInIso rdf:resource="&Governance;ISO_15489"/>
        <Governance:hasGoal rdf:resource="&Governance;Transparency"/>
    </owl:NamedIndividual>
    <owl:Axiom>
        <rdfs:comment>A documented policy framework provides clear guidance on transparency, ensuring that all stakeholders understand their roles and responsibilities in maintaining transparency, and fostering a culture of openness.</rdfs:comment>
        <owl:annotatedTarget rdf:resource="&Governance;IG_Policy_1"/>
        <owl:annotatedSource rdf:resource="&Governance;TRA_1_2_3"/>
        <owl:annotatedProperty rdf:resource="&Governance;needsTechnicalRequirement"/>
    </owl:Axiom>
    


    <!-- http://www.semanticweb.org/IG/Governance#TRA_1_2_4 -->

    <owl:NamedIndividual rdf:about="&Governance;TRA_1_2_4">
        <rdf:type rdf:resource="&Governance;IG_Capability"/>
        <Governance:capabilityDescription>The organization monitors compliance on a regular basis.</Governance:capabilityDescription>
        <Governance:inMaturityLevel rdf:resource="&Governance;4_Proactive"/>
        <Governance:linkedToFramework rdf:resource="&Governance;ARMA_00"/>
        <Governance:involvesArticle rdf:resource="&Governance;Article_24"/>
        <Governance:involvesArticle rdf:resource="&Governance;Article_30"/>
        <Governance:involvesArticle rdf:resource="&Governance;Article_33"/>
        <Governance:needsTechnicalRequirement rdf:resource="&Governance;Audit_1"/>
        <Governance:practicesDefinedInIso rdf:resource="&Governance;ISO_15489"/>
        <Governance:practicesDefinedInIso rdf:resource="&Governance;ISO_27000"/>
        <Governance:practicesDefinedInIso rdf:resource="&Governance;ISO_27001"/>
        <Governance:needsTechnicalRequirement rdf:resource="&Governance;Incident_Response_And_Remediation_Protocol_1"/>
        <Governance:needsTechnicalRequirement rdf:resource="&Governance;Monitoring_1"/>
        <Governance:hasGoal rdf:resource="&Governance;Transparency"/>
    </owl:NamedIndividual>
    <owl:Axiom>
        <rdfs:comment>An automated compliance monitoring system ensures that the organization can efficiently track adherence to transparency and data protection requirements, proactively identifying and addressing non-compliance.</rdfs:comment>
        <owl:annotatedTarget rdf:resource="&Governance;Monitoring_1"/>
        <owl:annotatedSource rdf:resource="&Governance;TRA_1_2_4"/>
        <owl:annotatedProperty rdf:resource="&Governance;needsTechnicalRequirement"/>
    </owl:Axiom>
    <owl:Axiom>
        <rdfs:comment>An incident response and remediation protocol ensures that any compliance breaches or data incidents are promptly identified, reported, and addressed, minimizing potential harm and demonstrating accountability.</rdfs:comment>
        <owl:annotatedTarget rdf:resource="&Governance;Incident_Response_And_Remediation_Protocol_1"/>
        <owl:annotatedSource rdf:resource="&Governance;TRA_1_2_4"/>
        <owl:annotatedProperty rdf:resource="&Governance;needsTechnicalRequirement"/>
    </owl:Axiom>
    <owl:Axiom>
        <rdfs:comment>Periodic data audits verify the accuracy, completeness, and transparency of data processing practices, ensuring that the organization adheres to established policies and regulations.</rdfs:comment>
        <owl:annotatedTarget rdf:resource="&Governance;Audit_1"/>
        <owl:annotatedSource rdf:resource="&Governance;TRA_1_2_4"/>
        <owl:annotatedProperty rdf:resource="&Governance;needsTechnicalRequirement"/>
    </owl:Axiom>
    


    <!-- http://www.semanticweb.org/IG/Governance#TRA_1_2_5 -->

    <owl:NamedIndividual rdf:about="&Governance;TRA_1_2_5">
        <rdf:type rdf:resource="&Governance;IG_Capability"/>
        <Governance:capabilityDescription>The organization’s stated goals related to transparency have been met.</Governance:capabilityDescription>
        <Governance:inMaturityLevel rdf:resource="&Governance;5_Transformational"/>
        <Governance:linkedToFramework rdf:resource="&Governance;ARMA_00"/>
        <Governance:involvesArticle rdf:resource="&Governance;Article_24"/>
        <Governance:involvesArticle rdf:resource="&Governance;Article_5"/>
        <Governance:needsTechnicalRequirement rdf:resource="&Governance;Data_Quality_Assurance_Framework_1"/>
        <Governance:practicesDefinedInIso rdf:resource="&Governance;ISO_14271"/>
        <Governance:practicesDefinedInIso rdf:resource="&Governance;ISO_15000"/>
        <Governance:practicesDefinedInIso rdf:resource="&Governance;ISO_15489"/>
        <Governance:practicesDefinedInIso rdf:resource="&Governance;ISO_15939"/>
        <Governance:practicesDefinedInIso rdf:resource="&Governance;ISO_23081"/>
        <Governance:needsTechnicalRequirement rdf:resource="&Governance;Metrics_1"/>
        <Governance:needsTechnicalRequirement rdf:resource="&Governance;Reporting_And_Analysis_System_1"/>
        <Governance:hasGoal rdf:resource="&Governance;Transparency"/>
    </owl:NamedIndividual>
    <owl:Axiom>
        <rdfs:comment>A data quality assurance framework ensures that the data used to measure transparency goals is accurate, complete, and reliable, enhancing the credibility of goal attainment.</rdfs:comment>
        <owl:annotatedTarget rdf:resource="&Governance;Data_Quality_Assurance_Framework_1"/>
        <owl:annotatedSource rdf:resource="&Governance;TRA_1_2_5"/>
        <owl:annotatedProperty rdf:resource="&Governance;needsTechnicalRequirement"/>
    </owl:Axiom>
    <owl:Axiom>
        <rdfs:comment>Transparent performance metrics clearly define how transparency goals are measured, providing a clear understanding of the criteria and standards for goal attainment.</rdfs:comment>
        <owl:annotatedTarget rdf:resource="&Governance;Metrics_1"/>
        <owl:annotatedSource rdf:resource="&Governance;TRA_1_2_5"/>
        <owl:annotatedProperty rdf:resource="&Governance;needsTechnicalRequirement"/>
    </owl:Axiom>
    <owl:Axiom>
        <rdfs:comment>An analysis and reporting system allows the organization to track progress towards its transparency goals, identify areas for improvement, and provide evidence of goal attainment.</rdfs:comment>
        <owl:annotatedTarget rdf:resource="&Governance;Reporting_And_Analysis_System_1"/>
        <owl:annotatedSource rdf:resource="&Governance;TRA_1_2_5"/>
        <owl:annotatedProperty rdf:resource="&Governance;needsTechnicalRequirement"/>
    </owl:Axiom>
    


    <!-- http://www.semanticweb.org/IG/Governance#TRA_1_3_3 -->

    <owl:NamedIndividual rdf:about="&Governance;TRA_1_3_3">
        <rdf:type rdf:resource="&Governance;IG_Capability"/>
        <Governance:capabilityDescription>Employees are educated on the importance of Transparency and the specifics of the organization’s commitment to transparency.</Governance:capabilityDescription>
        <Governance:inMaturityLevel rdf:resource="&Governance;3_Essential"/>
        <Governance:linkedToFramework rdf:resource="&Governance;ARMA_00"/>
        <Governance:involvesArticle rdf:resource="&Governance;Article_24"/>
        <Governance:involvesArticle rdf:resource="&Governance;Article_39"/>
        <Governance:involvesArticle rdf:resource="&Governance;Article_5"/>
        <Governance:needsTechnicalRequirement rdf:resource="&Governance;Employee_Engagement_Platforms_1"/>
        <Governance:practicesDefinedInIso rdf:resource="&Governance;ISO_14271"/>
        <Governance:practicesDefinedInIso rdf:resource="&Governance;ISO_27000"/>
        <Governance:practicesDefinedInIso rdf:resource="&Governance;ISO_27001"/>
        <Governance:needsTechnicalRequirement rdf:resource="&Governance;Training_1"/>
        <Governance:hasGoal rdf:resource="&Governance;Transparency"/>
    </owl:NamedIndividual>
    <owl:Axiom>
        <rdfs:comment>Employee engagement platforms facilitate communication and interaction, allowing employees to access resources, ask questions, and engage in discussions related to transparency and data protection.</rdfs:comment>
        <owl:annotatedTarget rdf:resource="&Governance;Employee_Engagement_Platforms_1"/>
        <owl:annotatedSource rdf:resource="&Governance;TRA_1_3_3"/>
        <owl:annotatedProperty rdf:resource="&Governance;needsTechnicalRequirement"/>
    </owl:Axiom>
    <owl:Axiom>
        <rdfs:comment>A comprehensive training and awareness program ensures that employees understand the significance of transparency, their roles in promoting it, and the organization&apos;s commitment. Well-informed employees contribute to a culture of transparency and responsible data handling.</rdfs:comment>
        <owl:annotatedSource rdf:resource="&Governance;TRA_1_3_3"/>
        <owl:annotatedTarget rdf:resource="&Governance;Training_1"/>
        <owl:annotatedProperty rdf:resource="&Governance;needsTechnicalRequirement"/>
    </owl:Axiom>
    


    <!-- http://www.semanticweb.org/IG/Governance#TRA_1_3_5 -->

    <owl:NamedIndividual rdf:about="&Governance;TRA_1_3_5">
        <rdf:type rdf:resource="&Governance;IG_Capability"/>
        <Governance:capabilityDescription>The organization # has implemented a continuous improvement process to ensure transparency is maintained over time.</Governance:capabilityDescription>
        <Governance:inMaturityLevel rdf:resource="&Governance;5_Transformational"/>
        <Governance:linkedToFramework rdf:resource="&Governance;ARMA_00"/>
        <Governance:involvesArticle rdf:resource="&Governance;Article_24"/>
        <Governance:involvesArticle rdf:resource="&Governance;Article_5"/>
        <Governance:needsTechnicalRequirement rdf:resource="&Governance;Change_Management_1"/>
        <Governance:needsTechnicalRequirement rdf:resource="&Governance;IG_Strategic_Plan_1"/>
        <Governance:practicesDefinedInIso rdf:resource="&Governance;ISO_15000"/>
        <Governance:practicesDefinedInIso rdf:resource="&Governance;ISO_15489"/>
        <Governance:practicesDefinedInIso rdf:resource="&Governance;ISO_15939"/>
        <Governance:practicesDefinedInIso rdf:resource="&Governance;ISO_17000"/>
        <Governance:needsTechnicalRequirement rdf:resource="&Governance;Risk_And_Compliance_1"/>
        <Governance:hasGoal rdf:resource="&Governance;Transparency"/>
    </owl:NamedIndividual>
    <owl:Axiom>
        <rdfs:comment> Regular risk assessments help identify potential gaps, vulnerabilities, and emerging risks that may impact transparency initiatives. Continuous monitoring of risks ensures that transparency efforts are adaptable and can be improved over time.</rdfs:comment>
        <owl:annotatedTarget rdf:resource="&Governance;Risk_And_Compliance_1"/>
        <owl:annotatedSource rdf:resource="&Governance;TRA_1_3_5"/>
        <owl:annotatedProperty rdf:resource="&Governance;needsTechnicalRequirement"/>
    </owl:Axiom>
    <owl:Axiom>
        <rdfs:comment>A robust strategic plan provides a structured approach to managing and improving data quality, integrity, and availability. This is essential for maintaining transparency over time as it ensures that data used for transparency initiatives remains accurate and reliable.</rdfs:comment>
        <owl:annotatedTarget rdf:resource="&Governance;IG_Strategic_Plan_1"/>
        <owl:annotatedSource rdf:resource="&Governance;TRA_1_3_5"/>
        <owl:annotatedProperty rdf:resource="&Governance;needsTechnicalRequirement"/>
    </owl:Axiom>
    <owl:Axiom>
        <rdfs:comment>A well-defined change management process ensures that updates, enhancements, or modifications to transparency initiatives are effectively planned, communicated, and implemented without disrupting existing processes.</rdfs:comment>
        <owl:annotatedTarget rdf:resource="&Governance;Change_Management_1"/>
        <owl:annotatedSource rdf:resource="&Governance;TRA_1_3_5"/>
        <owl:annotatedProperty rdf:resource="&Governance;needsTechnicalRequirement"/>
    </owl:Axiom>
    


    <!-- http://www.semanticweb.org/IG/Governance#TRA_1_4_3 -->

    <owl:NamedIndividual rdf:about="&Governance;TRA_1_4_3">
        <rdf:type rdf:resource="&Governance;IG_Capability"/>
        <Governance:capabilityDescription>The organization has defined specific goals related to Transparency.</Governance:capabilityDescription>
        <Governance:inMaturityLevel rdf:resource="&Governance;3_Essential"/>
        <Governance:linkedToFramework rdf:resource="&Governance;ARMA_00"/>
        <Governance:involvesArticle rdf:resource="&Governance;Article_24"/>
        <Governance:involvesArticle rdf:resource="&Governance;Article_33"/>
        <Governance:involvesArticle rdf:resource="&Governance;Article_5"/>
        <Governance:needsTechnicalRequirement rdf:resource="&Governance;IG_Strategic_Plan_1"/>
        <Governance:practicesDefinedInIso rdf:resource="&Governance;ISO_15000"/>
        <Governance:practicesDefinedInIso rdf:resource="&Governance;ISO_15489"/>
        <Governance:practicesDefinedInIso rdf:resource="&Governance;ISO_15939"/>
        <Governance:needsTechnicalRequirement rdf:resource="&Governance;Reporting_And_Analysis_System_1"/>
        <Governance:hasGoal rdf:resource="&Governance;Transparency"/>
    </owl:NamedIndividual>
    <owl:Axiom>
        <rdfs:comment>Data analytics and reporting tools facilitate the measurement and reporting of progress toward transparency goals, allowing the organization to track achievements and identify areas for improvement.</rdfs:comment>
        <owl:annotatedTarget rdf:resource="&Governance;Reporting_And_Analysis_System_1"/>
        <owl:annotatedSource rdf:resource="&Governance;TRA_1_4_3"/>
        <owl:annotatedProperty rdf:resource="&Governance;needsTechnicalRequirement"/>
    </owl:Axiom>
    <owl:Axiom>
        <rdfs:comment>Establishing specific goals related to transparency provides a clear direction for the organization&apos;s efforts, ensuring a focused and measurable approach to promoting transparency in data handling and governance.</rdfs:comment>
        <owl:annotatedTarget rdf:resource="&Governance;IG_Strategic_Plan_1"/>
        <owl:annotatedSource rdf:resource="&Governance;TRA_1_4_3"/>
        <owl:annotatedProperty rdf:resource="&Governance;needsTechnicalRequirement"/>
    </owl:Axiom>
    


    <!-- http://www.semanticweb.org/IG/Governance#TRA_1_4_5 -->

    <owl:NamedIndividual rdf:about="&Governance;TRA_1_4_5">
        <rdf:type rdf:resource="&Governance;IG_Capability"/>
        <Governance:capabilityDescription>Software tools that are in place assist in transparency.</Governance:capabilityDescription>
        <Governance:linkedToFramework rdf:resource="&Governance;ARMA_00"/>
        <Governance:needsTechnicalRequirement rdf:resource="&Governance;AccessControl_1"/>
        <Governance:involvesArticle rdf:resource="&Governance;Article_5"/>
        <Governance:needsTechnicalRequirement rdf:resource="&Governance;IG_Programm_1"/>
        <Governance:practicesDefinedInIso rdf:resource="&Governance;ISO_15489"/>
        <Governance:practicesDefinedInIso rdf:resource="&Governance;ISO_15939"/>
        <Governance:practicesDefinedInIso rdf:resource="&Governance;ISO_23081"/>
        <Governance:practicesDefinedInIso rdf:resource="&Governance;ISO_27001"/>
        <Governance:needsTechnicalRequirement rdf:resource="&Governance;Reporting_And_Analysis_System_1"/>
        <Governance:hasGoal rdf:resource="&Governance;Transparency"/>
    </owl:NamedIndividual>
    <owl:Axiom>
        <rdfs:comment>A well defined IG Programm with an Information Management System (IMS) provides a centralized platform for managing and organizing information assets, facilitating transparency by ensuring easy access, retrieval, and sharing of information.</rdfs:comment>
        <owl:annotatedTarget rdf:resource="&Governance;IG_Programm_1"/>
        <owl:annotatedSource rdf:resource="&Governance;TRA_1_4_5"/>
        <owl:annotatedProperty rdf:resource="&Governance;needsTechnicalRequirement"/>
    </owl:Axiom>
    <owl:Axiom>
        <rdfs:comment>Reporting and analysis tools enable organizations to analyze and visualize data related to transparency efforts, allowing for informed decision-making and identification of areas for improvement.</rdfs:comment>
        <owl:annotatedTarget rdf:resource="&Governance;Reporting_And_Analysis_System_1"/>
        <owl:annotatedSource rdf:resource="&Governance;TRA_1_4_5"/>
        <owl:annotatedProperty rdf:resource="&Governance;needsTechnicalRequirement"/>
    </owl:Axiom>
    <owl:Axiom>
        <rdfs:comment>Strong access control and authentication mechanisms ensure that only authorized personnel can access and utilize software tools, safeguarding sensitive information and maintaining transparency.</rdfs:comment>
        <owl:annotatedTarget rdf:resource="&Governance;AccessControl_1"/>
        <owl:annotatedSource rdf:resource="&Governance;TRA_1_4_5"/>
        <owl:annotatedProperty rdf:resource="&Governance;needsTechnicalRequirement"/>
    </owl:Axiom>
    


    <!-- http://www.semanticweb.org/IG/Governance#TRA_1_5_5 -->

    <owl:NamedIndividual rdf:about="&Governance;TRA_1_5_5">
        <rdf:type rdf:resource="&Governance;IG_Capability"/>
        <Governance:capabilityDescription>Requestors, courts, and other legitimately interested parties are consistently satisfied with the transparency of the processes and the response</Governance:capabilityDescription>
        <Governance:inMaturityLevel rdf:resource="&Governance;5_Transformational"/>
        <Governance:linkedToFramework rdf:resource="&Governance;ARMA_00"/>
        <Governance:needsTechnicalRequirement rdf:resource="&Governance;AccessControl_1"/>
        <Governance:involvesArticle rdf:resource="&Governance;Article_12"/>
        <Governance:involvesArticle rdf:resource="&Governance;Article_15"/>
        <Governance:involvesArticle rdf:resource="&Governance;Article_30"/>
        <Governance:involvesArticle rdf:resource="&Governance;Article_5"/>
        <Governance:needsTechnicalRequirement rdf:resource="&Governance;Audit_1"/>
        <Governance:needsTechnicalRequirement rdf:resource="&Governance;Data_Mapping_And_Classification_System_1"/>
        <Governance:practicesDefinedInIso rdf:resource="&Governance;ISO_15489"/>
        <Governance:practicesDefinedInIso rdf:resource="&Governance;ISO_27001"/>
        <Governance:needsTechnicalRequirement rdf:resource="&Governance;Monitoring_1"/>
        <Governance:hasGoal rdf:resource="&Governance;Transparency"/>
    </owl:NamedIndividual>
    <owl:Axiom>
        <rdfs:comment>A robust monitoring (with a good Case Management System) allows for systematic tracking, monitoring, and documentation of requests and inquiries from various parties. It ensures that processes are transparent and that responses are managed efficiently.</rdfs:comment>
        <owl:annotatedTarget rdf:resource="&Governance;Monitoring_1"/>
        <owl:annotatedSource rdf:resource="&Governance;TRA_1_5_5"/>
        <owl:annotatedProperty rdf:resource="&Governance;needsTechnicalRequirement"/>
    </owl:Axiom>
    <owl:Axiom>
        <rdfs:comment>Data classification ensures that requests and responses are handled according to their sensitivity.</rdfs:comment>
        <owl:annotatedTarget rdf:resource="&Governance;Data_Mapping_And_Classification_System_1"/>
        <owl:annotatedSource rdf:resource="&Governance;TRA_1_5_5"/>
        <owl:annotatedProperty rdf:resource="&Governance;needsTechnicalRequirement"/>
    </owl:Axiom>
    <owl:Axiom>
        <rdfs:comment>Access controls ensure that requests and responses are handled according to their sensitivity and that only authorized personnel can access and manage the information.</rdfs:comment>
        <owl:annotatedTarget rdf:resource="&Governance;AccessControl_1"/>
        <owl:annotatedSource rdf:resource="&Governance;TRA_1_5_5"/>
        <owl:annotatedProperty rdf:resource="&Governance;needsTechnicalRequirement"/>
    </owl:Axiom>
    <owl:Axiom>
        <rdfs:comment>An audit trail and logging mechanism captures and records activities related to requests, processes, and responses. This ensures transparency, accountability, and the ability to trace interactions.</rdfs:comment>
        <owl:annotatedTarget rdf:resource="&Governance;Audit_1"/>
        <owl:annotatedSource rdf:resource="&Governance;TRA_1_5_5"/>
        <owl:annotatedProperty rdf:resource="&Governance;needsTechnicalRequirement"/>
    </owl:Axiom>
    


    <!-- http://www.semanticweb.org/IG/Governance#Testing_1 -->

    <owl:NamedIndividual rdf:about="&Governance;Testing_1">
        <rdf:type rdf:resource="&Governance;Testing"/>
        <Governance:involvesArticle rdf:resource="&Governance;Article_32"/>
        <Governance:practicesDefinedInIso rdf:resource="&Governance;ISO_27001"/>
    </owl:NamedIndividual>
    


    <!-- http://www.semanticweb.org/IG/Governance#Training_1 -->

    <owl:NamedIndividual rdf:about="&Governance;Training_1">
        <rdf:type rdf:resource="&Governance;Training"/>
        <Governance:involvesArticle rdf:resource="&Governance;Article_24"/>
        <Governance:involvesArticle rdf:resource="&Governance;Article_25"/>
        <Governance:involvesArticle rdf:resource="&Governance;Article_32"/>
        <Governance:involvesArticle rdf:resource="&Governance;Article_39"/>
        <Governance:practicesDefinedInIso rdf:resource="&Governance;ISO_15489"/>
        <Governance:practicesDefinedInIso rdf:resource="&Governance;ISO_15939"/>
        <Governance:practicesDefinedInIso rdf:resource="&Governance;ISO_17000"/>
        <Governance:practicesDefinedInIso rdf:resource="&Governance;ISO_22301"/>
        <Governance:practicesDefinedInIso rdf:resource="&Governance;ISO_23081"/>
        <Governance:practicesDefinedInIso rdf:resource="&Governance;ISO_27000"/>
    </owl:NamedIndividual>
    


    <!-- http://www.semanticweb.org/IG/Governance#Transparency -->

    <owl:NamedIndividual rdf:about="&Governance;Transparency">
        <rdf:type rdf:resource="&Governance;Goal"/>
    </owl:NamedIndividual>
    


    <!-- http://www.semanticweb.org/IG/Governance#Vendor_Management -->

    <owl:NamedIndividual rdf:about="&Governance;Vendor_Management">
        <rdf:type rdf:resource="&Governance;IG_Capability"/>
    </owl:NamedIndividual>
    


    <!-- http://www.semanticweb.org/IG/Governance#Workflow_Tools_1 -->

    <owl:NamedIndividual rdf:about="&Governance;Workflow_Tools_1">
        <rdf:type rdf:resource="&Governance;Workflow_Tools"/>
        <Governance:involvesArticle rdf:resource="&Governance;Article_24"/>
        <Governance:involvesArticle rdf:resource="&Governance;Article_25"/>
        <Governance:involvesArticle rdf:resource="&Governance;Article_32"/>
        <Governance:involvesArticle rdf:resource="&Governance;Article_5"/>
        <Governance:involvesArticle rdf:resource="&Governance;Article_6"/>
        <Governance:practicesDefinedInIso rdf:resource="&Governance;ISO_14271"/>
        <Governance:practicesDefinedInIso rdf:resource="&Governance;ISO_15489"/>
        <Governance:practicesDefinedInIso rdf:resource="&Governance;ISO_23081"/>
        <Governance:practicesDefinedInIso rdf:resource="&Governance;ISO_27001"/>
    </owl:NamedIndividual>
    


    <!-- http://www.semanticweb.org/IG/Governance#eDiscovery_Integration_1 -->

    <owl:NamedIndividual rdf:about="&Governance;eDiscovery_Integration_1">
        <rdf:type rdf:resource="&Governance;eDiscovery_Integration"/>
        <Governance:involvesArticle rdf:resource="&Governance;Article_32"/>
        <Governance:practicesDefinedInIso rdf:resource="&Governance;ISO_27050"/>
    </owl:NamedIndividual>
    <rdf:Description>
        <rdfs:comment></rdfs:comment>
    </rdf:Description>
    


    <!-- 
    ///////////////////////////////////////////////////////////////////////////////////////
    //
    // General axioms
    //
    ///////////////////////////////////////////////////////////////////////////////////////
     -->

    <rdf:Description>
        <rdf:type rdf:resource="&owl;AllDisjointClasses"/>
        <owl:members rdf:parseType="Collection">
            <rdf:Description rdf:about="&Governance;Goal"/>
            <rdf:Description rdf:about="&Governance;Maturity"/>
            <rdf:Description rdf:about="&Governance;Organization"/>
            <rdf:Description rdf:about="&Governance;Role"/>
        </owl:members>
    </rdf:Description>
    <rdf:Description>
        <rdf:type rdf:resource="&owl;AllDisjointClasses"/>
        <owl:members rdf:parseType="Collection">
            <rdf:Description rdf:about="&Governance;Business_Unit"/>
            <rdf:Description rdf:about="&Governance;Change_Management"/>
            <rdf:Description rdf:about="&Governance;Development"/>
            <rdf:Description rdf:about="&Governance;Legal"/>
            <rdf:Description rdf:about="&Governance;Privacy"/>
            <rdf:Description rdf:about="&Governance;Records_Management"/>
            <rdf:Description rdf:about="&Governance;Risk_And_Compliance"/>
            <rdf:Description rdf:about="&Governance;Security"/>
        </owl:members>
    </rdf:Description>
    <rdf:Description>
        <rdf:type rdf:resource="&owl;AllDisjointClasses"/>
        <owl:members rdf:parseType="Collection">
            <rdf:Description rdf:about="&Governance;CCO"/>
            <rdf:Description rdf:about="&Governance;CSO"/>
            <rdf:Description rdf:about="&Governance;DPO"/>
            <rdf:Description rdf:about="&Governance;Data_Controller"/>
            <rdf:Description rdf:about="&Governance;Data_Processor"/>
            <rdf:Description rdf:about="&Governance;Data_Subject"/>
            <rdf:Description rdf:about="&Governance;Executive_Sponsor"/>
            <rdf:Description rdf:about="&Governance;IG_Leadership"/>
            <rdf:Description rdf:about="&Governance;Project_Manager"/>
            <rdf:Description rdf:about="&Governance;Stakeholder"/>
            <rdf:Description rdf:about="&Governance;Steering_Commitee"/>
        </owl:members>
    </rdf:Description>
</rdf:RDF>



<!-- Generated by the OWL API (version 3.4.2) http://owlapi.sourceforge.net -->

